<?xml version="1.0"?>


<!DOCTYPE rdf:RDF [
    <!ENTITY vocab "http://vocab.deri.ie/" >
    <!ENTITY terms "http://purl.org/dc/terms/" >
    <!ENTITY adms "http://www.w3.org/ns/adms#" >
    <!ENTITY foaf "http://xmlns.com/foaf/0.1/" >
    <!ENTITY scovo2 "http://purl.org/NET/scovo#" >
    <!ENTITY scovo "http://vocab.deri.ie/scovo#" >
    <!ENTITY vann "http://purl.org/vocab/vann/" >
    <!ENTITY time "http://www.w3.org/2006/time#" >
    <!ENTITY sf "http://www.opengis.net/ont/sf#" >
    <!ENTITY owl "http://www.w3.org/2002/07/owl#" >
    <!ENTITY gml "http://www.opengis.net/ont/gml#" >
    <!ENTITY dc "http://purl.org/dc/elements/1.1/" >
    <!ENTITY timezone "http://www.w3.org/2006/timezone#" >
    <!ENTITY xsd "http://www.w3.org/2001/XMLSchema#" >
    <!ENTITY ontology "http://geo.linkeddata.es/ontology/" >
    <!ENTITY skos "http://www.w3.org/2004/02/skos/core#" >
    <!ENTITY btn100 "ttp://geo.linkeddata.es/def/feature#" >
    <!ENTITY geosparql "http://www.opengis.net/ont/geosparql#" >
    <!ENTITY rdfs "http://www.w3.org/2000/01/rdf-schema#" >
    <!ENTITY wgs84_pos "http://www.w3.org/2003/01/geo/wgs84_pos#" >
    <!ENTITY geopolitical "http://aims.fao.org/aos/geopolitical.owl#" >
    <!ENTITY rdf "http://www.w3.org/1999/02/22-rdf-syntax-ns#" >
]>


<rdf:RDF xmlns="h&btn100;"
     xml:base="http://geo.linkeddata.es/def/feature"
     xmlns:dc="http://purl.org/dc/elements/1.1/"
     xmlns:wgs84_pos="http://www.w3.org/2003/01/geo/wgs84_pos#"
     xmlns:foaf="http://xmlns.com/foaf/0.1/"
     xmlns:terms="http://purl.org/dc/terms/"
     xmlns:vann="http://purl.org/vocab/vann/"
     xmlns:sf="http://www.opengis.net/ont/sf#"
     xmlns:ontology="http://geo.linkeddata.es/ontology/"
     xmlns:scovo2="http://purl.org/NET/scovo#"
     xmlns:adms="http://www.w3.org/ns/adms#"
     xmlns:geosparql="http://www.opengis.net/ont/geosparql#"
     xmlns:rdfs="http://www.w3.org/2000/01/rdf-schema#"
     xmlns:timezone="http://www.w3.org/2006/timezone#"
     xmlns:time="http://www.w3.org/2006/time#"
     xmlns:geopolitical="http://aims.fao.org/aos/geopolitical.owl#"
     xmlns:owl="http://www.w3.org/2002/07/owl#"
     xmlns:xsd="http://www.w3.org/2001/XMLSchema#"
     xmlns:scovo="&vocab;scovo#"
     xmlns:rdf="http://www.w3.org/1999/02/22-rdf-syntax-ns#"
     xmlns:gml="http://www.opengis.net/ont/gml#"
     xmlns:btn100="ttp://geo.linkeddata.es/def/feature#"
     xmlns:vocab="http://vocab.deri.ie/"
     xmlns:skos="http://www.w3.org/2004/02/skos/core#">
    <owl:Ontology rdf:about="http://geo.linkeddata.es/def/feature">
        <rdfs:label xml:lang="es">Ontología utilizada para modelar geo.linkeddata.es</rdfs:label>
        <rdfs:comment rdf:datatype="&xsd;string"> prior version : &quot; http://aims.fao.org/aos/geopolitical_v10.owl&quot;   </rdfs:comment>
        <terms:created rdf:datatype="&xsd;date">2010-01-26</terms:created>
        <terms:modified rdf:datatype="&xsd;string">2011-01-18</terms:modified>
        <dc:date rdf:datatype="&xsd;date">2012-04-30</dc:date>
        <terms:modified rdf:datatype="&xsd;date">2012-08-09</terms:modified>
        <dc:description rdf:datatype="&xsd;string">An RDF/OWL vocabulary for representing spatial information</dc:description>
        <rdfs:comment rdf:datatype="&xsd;string">FAO DISCLAIMER:  Information on the FAO Country Profiles portal is provided as and when available. The designations employed and the presentation of information do not imply the expression of any opinion whatsoever on the part of the Food and Agriculture Organization of the United Nations (FAO) concerning the legal status of any country, territory, city or area, or of its authorities, or concerning the delimitation of its frontiers or boundaries. FAO makes every effort to ensure, but does not guarantee, the accuracy or completeness of and declines responsibility for any loss, damage, liability or expense suffered which is claimed to result from its use. </rdfs:comment>
        <rdfs:comment rdf:datatype="&xsd;string">FAO&#39;s geopolitical ontology version 1.1 was populated with FAO, UN and internationally recognized data sources.    </rdfs:comment>
        <terms:creator rdf:datatype="&xsd;string">Luis Manuel Vilches-Blázquez</terms:creator>
        <dc:creator rdf:datatype="&xsd;string">Luis Manuel Vilches-Blázquez</dc:creator>
        <owl:versionInfo rdf:datatype="&xsd;string">OGC GeoSPARQL 1.0</owl:versionInfo>
        <dc:source rdf:datatype="&xsd;string">OGC GeoSPARQL – A Geographic Query Language for RDF Data OGC 11-052r5</dc:source>
        <dc:creator rdf:datatype="&xsd;string">Open Geospatial Consortium</dc:creator>
        <rdfs:comment rdf:datatype="&xsd;string">The use of the information presented on the FAO Country Profiles portal is governed by FAO&#39;s copyright reservation. Any queries regarding the content, sources or use, please contact FAO-country-profiles@fao.org or visit http://www.fao.org/countryprofiles. </rdfs:comment>
        <rdfs:comment rdf:datatype="&xsd;string">Version 1.1 of the ontology includes a structured description of sources (source creator, source identifier by language, and last updated date on source) . 
   </rdfs:comment>
        <terms:contributor rdf:datatype="&xsd;anyURI">http://delicias.dia.fi.upm.es/members/DGarijo/#me</terms:contributor>
        <dc:title rdf:datatype="&xsd;string">hydrOntology</dc:title>
        <owl:versionInfo rdf:datatype="&xsd;string">v0.1</owl:versionInfo>
        <owl:versionInfo rdf:datatype="&xsd;string">v0.2</owl:versionInfo>
        <terms:publisher>http://vocab.deri.ie/scovo#LiDRC</terms:publisher>
        <vann:preferredNamespacePrefix>geoes</vann:preferredNamespacePrefix>
        <terms:creator>Alistair Miles</terms:creator>
        <vann:preferredNamespacePrefix>scovo</vann:preferredNamespacePrefix>
        <terms:contributor>Nikki Rogers</terms:contributor>
        <vann:preferredNamespaceUri>http://purl.org/NET/scovo#</vann:preferredNamespaceUri>
        <terms:contributor>Participants in W3C&#39;s Semantic Web Deployment Working Group.</terms:contributor>
        <rdfs:comment>
      An OWL Ontology of Time (OWL-Time).
    </rdfs:comment>
        <terms:description>A vocabulary for representing statistical data on the Web.

&lt;div style=&quot;border: 2px solid red; padding: 0.4em 0.7em; background: #fcc&quot;&gt;Note: The SCOVO vocabulary is deprecated. We strongly advise to use the &lt;a href=&quot;http://www.w3.org/TR/vocab-data-cube/&quot;&gt;Data Cube Vocabulary&lt;/a&gt; instead.&lt;/div&gt;</terms:description>
        <terms:license>http://creativecommons.org/licenses/by-nc-sa/2.0/</terms:license>
        <rdfs:comment xml:lang="en"></rdfs:comment>
        <terms:description xml:lang="en">An RDF vocabulary for describing the basic structure and content of concept schemes such as thesauri, classification schemes, subject heading lists, taxonomies, &#39;folksonomies&#39;, other types of controlled vocabulary, and also concept schemes embedded in glossaries and terminologies.</terms:description>
        <terms:creator>Sean Bechhofer</terms:creator>
        <vann:preferredNamespaceUri>http://geo.linkeddata.es/ontology/</vann:preferredNamespaceUri>
        <terms:title>The Statistical Core Vocabulary (SCOVO)</terms:title>
        <terms:contributor>Dave Beckett</terms:contributor>
        <rdfs:comment xml:lang="en">Geo.linkeddata.es ontology network</rdfs:comment>
        <terms:publisher xml:lang="en">Ontology Engineering Group</terms:publisher>
        <dc:publisher xml:lang="en">Ontology Engineering Group</dc:publisher>
        <terms:title xml:lang="en">SKOS Vocabulary</terms:title>
        <owl:versionInfo xml:lang="en">version 1.1</owl:versionInfo>
        <dc:creator xml:lang="es">Ontology Engineering Group, Facultad de Informática, Universidad Politécnica de Madrid</dc:creator>
        <rdfs:comment xml:lang="es">Ontología global de dominio sobre fenómenos hidrográficos</rdfs:comment>
        <terms:title xml:lang="es">Red de ontologías geo.linkeddata.es</terms:title>
        <rdfs:comment xml:lang="es">Red de ontologías geo.linkeddata.es</rdfs:comment>
        <rdfs:comment xml:lang="es">Red de ontologías para modelar la información disponible en geo.linkeddata.es</rdfs:comment>
        <terms:partOf rdf:resource="http://vocab.deri.ie"/>
        <terms:type rdf:resource="http://purl.org/adms/assettype/Ontology"/>
        <terms:status rdf:resource="http://purl.org/adms/status/UnderDevelopment"/>
        <foaf:homepage rdf:resource="&vocab;scovo.html"/>
        <dc:creator rdf:resource="&vocab;scovo#Michael%20Hausenblas"/>
        <dc:creator rdf:resource="&vocab;scovo#dayers"/>
        <dc:creator rdf:resource="&vocab;scovo#lfeigenbaum"/>
        <dc:creator rdf:resource="&vocab;scovo#theath"/>
        <dc:creator rdf:resource="&vocab;scovo#whalb"/>
        <dc:creator rdf:resource="&vocab;scovo#yraimond"/>
        <rdfs:seeAlso rdf:resource="http://www.opengis.net/def/function/ogc-geosparql/1.0"/>
        <rdfs:seeAlso rdf:resource="http://www.opengis.net/def/rule/ogc-geosparql/1.0"/>
        <dc:source rdf:resource="http://www.opengis.net/doc/IS/geosparql/1.0"/>
        <rdfs:seeAlso rdf:resource="http://www.opengis.net/doc/IS/geosparql/1.0"/>
        <rdfs:seeAlso rdf:resource="http://www.w3.org/TR/owl-time"/>
        <rdfs:seeAlso rdf:resource="http://www.w3.org/TR/skos-reference/"/>
    </owl:Ontology>
    


    <!-- 
    ///////////////////////////////////////////////////////////////////////////////////////
    //
    // Annotation properties
    //
    ///////////////////////////////////////////////////////////////////////////////////////
     -->

    <owl:AnnotationProperty rdf:about="&skos;prefLabel">
        <rdfs:label xml:lang="en">preferred label</rdfs:label>
        <rdfs:comment xml:lang="en">A resource has no more than one value of skos:prefLabel per language tag, and no more than one value of skos:prefLabel without language tag.</rdfs:comment>
        <skos:definition xml:lang="en">The preferred lexical label for a resource, in a given language.</skos:definition>
        <rdfs:comment xml:lang="en">The range of skos:prefLabel is the class of RDF plain literals.</rdfs:comment>
        <rdfs:comment xml:lang="en">skos:prefLabel, skos:altLabel and skos:hiddenLabel are pairwise
      disjoint properties.</rdfs:comment>
        <rdfs:subPropertyOf rdf:resource="&rdfs;label"/>
        <rdfs:isDefinedBy rdf:resource="http://www.w3.org/2004/02/skos/core"/>
    </owl:AnnotationProperty>
    <owl:AnnotationProperty rdf:about="&terms;hasPart">
        <rdfs:label xml:lang="en">Has Part</rdfs:label>
        <terms:issued rdf:datatype="&xsd;date">2000-07-11</terms:issued>
        <terms:modified rdf:datatype="&xsd;date">2008-01-14</terms:modified>
        <rdfs:comment xml:lang="en">A related resource that is included either physically or logically in the described resource.</rdfs:comment>
        <skos:note xml:lang="en">This term is intended to be used with non-literal values as defined in the DCMI Abstract Model (http://dublincore.org/documents/abstract-model/).  As of December 2007, the DCMI Usage Board is seeking a way to express this intention with a formal range declaration.</skos:note>
        <terms:hasVersion rdf:resource="http://dublincore.org/usage/terms/history/#hasPart-003"/>
        <rdfs:subPropertyOf rdf:resource="&dc;relation"/>
        <rdfs:isDefinedBy rdf:resource="http://purl.org/dc/terms/"/>
        <rdfs:subPropertyOf rdf:resource="&terms;relation"/>
    </owl:AnnotationProperty>
    <owl:AnnotationProperty rdf:about="&terms;language">
        <rdfs:label xml:lang="en">Language</rdfs:label>
        <terms:modified rdf:datatype="&xsd;date">2008-01-14</terms:modified>
        <terms:issued rdf:datatype="&xsd;date">2008-01-14</terms:issued>
        <rdfs:comment xml:lang="en">A language of the resource.</rdfs:comment>
        <terms:description xml:lang="en">Recommended best practice is to use a controlled vocabulary such as RFC 4646 [RFC4646].</terms:description>
        <terms:hasVersion rdf:resource="http://dublincore.org/usage/terms/history/#languageT-001"/>
        <rdfs:subPropertyOf rdf:resource="&dc;language"/>
        <rdfs:isDefinedBy rdf:resource="http://purl.org/dc/terms/"/>
    </owl:AnnotationProperty>
    <owl:AnnotationProperty rdf:about="&dc;description">
        <rdfs:label xml:lang="en">Description</rdfs:label>
        <terms:issued rdf:datatype="&xsd;date">1999-07-02</terms:issued>
        <terms:modified rdf:datatype="&xsd;date">2008-01-14</terms:modified>
        <skos:note xml:lang="en">A second property with the same name as this property has been declared in the dcterms: namespace (http://purl.org/dc/terms/).  See the Introduction to the document &quot;DCMI Metadata Terms&quot; (http://dublincore.org/documents/dcmi-terms/) for an explanation.</skos:note>
        <rdfs:comment xml:lang="en">An account of the resource.</rdfs:comment>
        <terms:description xml:lang="en">Description may include but is not limited to: an abstract, a table of contents, a graphical representation, or a free-text account of the resource.</terms:description>
        <terms:hasVersion rdf:resource="http://dublincore.org/usage/terms/history/#description-006"/>
        <rdfs:isDefinedBy rdf:resource="http://purl.org/dc/elements/1.1/"/>
    </owl:AnnotationProperty>
    <owl:AnnotationProperty rdf:about="&skos;historyNote">
        <rdfs:label xml:lang="en">history note</rdfs:label>
        <skos:definition xml:lang="en">A note about the past state/use/meaning of a concept.</skos:definition>
        <rdfs:isDefinedBy rdf:resource="http://www.w3.org/2004/02/skos/core"/>
        <rdfs:subPropertyOf rdf:resource="&skos;note"/>
    </owl:AnnotationProperty>
    <owl:AnnotationProperty rdf:about="&terms;isVersionOf">
        <rdfs:label xml:lang="en">Is Version Of</rdfs:label>
        <terms:issued rdf:datatype="&xsd;date">2000-07-11</terms:issued>
        <terms:modified rdf:datatype="&xsd;date">2008-01-14</terms:modified>
        <rdfs:comment xml:lang="en">A related resource of which the described resource is a version, edition, or adaptation.</rdfs:comment>
        <terms:description xml:lang="en">Changes in version imply substantive changes in content rather than differences in format.</terms:description>
        <skos:note xml:lang="en">This term is intended to be used with non-literal values as defined in the DCMI Abstract Model (http://dublincore.org/documents/abstract-model/).  As of December 2007, the DCMI Usage Board is seeking a way to express this intention with a formal range declaration.</skos:note>
        <terms:hasVersion rdf:resource="http://dublincore.org/usage/terms/history/#isVersionOf-003"/>
        <rdfs:subPropertyOf rdf:resource="&dc;relation"/>
        <rdfs:isDefinedBy rdf:resource="http://purl.org/dc/terms/"/>
        <rdfs:subPropertyOf rdf:resource="&terms;relation"/>
    </owl:AnnotationProperty>
    <owl:AnnotationProperty rdf:about="&terms;isReplacedBy">
        <rdfs:label xml:lang="en">Is Replaced By</rdfs:label>
        <terms:issued rdf:datatype="&xsd;date">2000-07-11</terms:issued>
        <terms:modified rdf:datatype="&xsd;date">2008-01-14</terms:modified>
        <rdfs:comment xml:lang="en">A related resource that supplants, displaces, or supersedes the described resource.</rdfs:comment>
        <skos:note xml:lang="en">This term is intended to be used with non-literal values as defined in the DCMI Abstract Model (http://dublincore.org/documents/abstract-model/).  As of December 2007, the DCMI Usage Board is seeking a way to express this intention with a formal range declaration.</skos:note>
        <terms:hasVersion rdf:resource="http://dublincore.org/usage/terms/history/#isReplacedBy-003"/>
        <rdfs:subPropertyOf rdf:resource="&dc;relation"/>
        <rdfs:isDefinedBy rdf:resource="http://purl.org/dc/terms/"/>
        <rdfs:subPropertyOf rdf:resource="&terms;relation"/>
    </owl:AnnotationProperty>
    <owl:AnnotationProperty rdf:about="&terms;available">
        <rdfs:subPropertyOf rdf:resource="&dc;date"/>
        <rdfs:subPropertyOf rdf:resource="&terms;date"/>
    </owl:AnnotationProperty>
    <owl:AnnotationProperty rdf:about="&terms;dateSubmitted">
        <rdfs:subPropertyOf rdf:resource="&dc;date"/>
        <rdfs:subPropertyOf rdf:resource="&terms;date"/>
    </owl:AnnotationProperty>
    <owl:AnnotationProperty rdf:about="&terms;coverage">
        <rdfs:label xml:lang="en">Coverage</rdfs:label>
        <terms:issued rdf:datatype="&xsd;date">2008-01-14</terms:issued>
        <terms:modified rdf:datatype="&xsd;date">2008-01-14</terms:modified>
        <terms:description xml:lang="en">Spatial topic and spatial applicability may be a named place or a location specified by its geographic coordinates. Temporal topic may be a named period, date, or date range. A jurisdiction may be a named administrative entity or a geographic place to which the resource applies. Recommended best practice is to use a controlled vocabulary such as the Thesaurus of Geographic Names [TGN]. Where appropriate, named places or time periods can be used in preference to numeric identifiers such as sets of coordinates or date ranges.</terms:description>
        <rdfs:comment xml:lang="en">The spatial or temporal topic of the resource, the spatial applicability of the resource, or the jurisdiction under which the resource is relevant.</rdfs:comment>
        <terms:hasVersion rdf:resource="http://dublincore.org/usage/terms/history/#coverageT-001"/>
        <rdfs:subPropertyOf rdf:resource="&dc;coverage"/>
        <rdfs:isDefinedBy rdf:resource="http://purl.org/dc/terms/"/>
    </owl:AnnotationProperty>
    <owl:AnnotationProperty rdf:about="&terms;created">
        <rdfs:label xml:lang="en">Date Created</rdfs:label>
        <terms:issued rdf:datatype="&xsd;date">2000-07-11</terms:issued>
        <terms:modified rdf:datatype="&xsd;date">2008-01-14</terms:modified>
        <rdfs:comment xml:lang="en">Date of creation of the resource.</rdfs:comment>
        <terms:hasVersion rdf:resource="http://dublincore.org/usage/terms/history/#created-003"/>
        <rdfs:domain rdf:resource="h&btn100;ver"/>
        <rdfs:subPropertyOf rdf:resource="&dc;date"/>
        <rdfs:isDefinedBy rdf:resource="http://purl.org/dc/terms/"/>
        <rdfs:subPropertyOf rdf:resource="&terms;date"/>
        <rdfs:domain rdf:resource="&geosparql;Feature"/>
        <rdfs:domain rdf:resource="&btn100;Relieve"/>
    </owl:AnnotationProperty>
    <owl:AnnotationProperty rdf:about="&skos;editorialNote">
        <rdfs:label xml:lang="en">editorial note</rdfs:label>
        <skos:definition xml:lang="en">A note for an editor, translator or maintainer of the vocabulary.</skos:definition>
        <rdfs:isDefinedBy rdf:resource="http://www.w3.org/2004/02/skos/core"/>
        <rdfs:subPropertyOf rdf:resource="&skos;note"/>
    </owl:AnnotationProperty>
    <owl:AnnotationProperty rdf:about="&terms;isFormatOf">
        <rdfs:label xml:lang="en">Is Format Of</rdfs:label>
        <terms:issued rdf:datatype="&xsd;date">2000-07-11</terms:issued>
        <terms:modified rdf:datatype="&xsd;date">2008-01-14</terms:modified>
        <rdfs:comment xml:lang="en">A related resource that is substantially the same as the described resource, but in another format.</rdfs:comment>
        <skos:note xml:lang="en">This term is intended to be used with non-literal values as defined in the DCMI Abstract Model (http://dublincore.org/documents/abstract-model/).  As of December 2007, the DCMI Usage Board is seeking a way to express this intention with a formal range declaration.</skos:note>
        <terms:hasVersion rdf:resource="http://dublincore.org/usage/terms/history/#isFormatOf-003"/>
        <rdfs:subPropertyOf rdf:resource="&dc;relation"/>
        <rdfs:isDefinedBy rdf:resource="http://purl.org/dc/terms/"/>
        <rdfs:subPropertyOf rdf:resource="&terms;relation"/>
    </owl:AnnotationProperty>
    <owl:AnnotationProperty rdf:about="&terms;isRequiredBy">
        <rdfs:label xml:lang="en">Is Required By</rdfs:label>
        <terms:issued rdf:datatype="&xsd;date">2000-07-11</terms:issued>
        <terms:modified rdf:datatype="&xsd;date">2008-01-14</terms:modified>
        <rdfs:comment xml:lang="en">A related resource that requires the described resource to support its function, delivery, or coherence.</rdfs:comment>
        <skos:note xml:lang="en">This term is intended to be used with non-literal values as defined in the DCMI Abstract Model (http://dublincore.org/documents/abstract-model/).  As of December 2007, the DCMI Usage Board is seeking a way to express this intention with a formal range declaration.</skos:note>
        <terms:hasVersion rdf:resource="http://dublincore.org/usage/terms/history/#isRequiredBy-003"/>
        <rdfs:subPropertyOf rdf:resource="&dc;relation"/>
        <rdfs:isDefinedBy rdf:resource="http://purl.org/dc/terms/"/>
        <rdfs:subPropertyOf rdf:resource="&terms;relation"/>
    </owl:AnnotationProperty>
    <owl:AnnotationProperty rdf:about="&terms;conformsTo">
        <rdfs:label xml:lang="en">Conforms To</rdfs:label>
        <terms:issued rdf:datatype="&xsd;date">2001-05-21</terms:issued>
        <terms:modified rdf:datatype="&xsd;date">2008-01-14</terms:modified>
        <rdfs:comment xml:lang="en">An established standard to which the described resource conforms.</rdfs:comment>
        <terms:hasVersion rdf:resource="http://dublincore.org/usage/terms/history/#conformsTo-003"/>
        <rdfs:subPropertyOf rdf:resource="&dc;relation"/>
        <rdfs:isDefinedBy rdf:resource="http://purl.org/dc/terms/"/>
        <rdfs:subPropertyOf rdf:resource="&terms;relation"/>
    </owl:AnnotationProperty>
    <owl:AnnotationProperty rdf:about="&terms;abstract">
        <rdfs:label xml:lang="en">Abstract</rdfs:label>
        <terms:issued rdf:datatype="&xsd;date">2000-07-11</terms:issued>
        <terms:modified rdf:datatype="&xsd;date">2008-01-14</terms:modified>
        <rdfs:comment xml:lang="en">A summary of the resource.</rdfs:comment>
        <terms:hasVersion rdf:resource="http://dublincore.org/usage/terms/history/#abstract-003"/>
        <rdfs:subPropertyOf rdf:resource="&dc;description"/>
        <rdfs:isDefinedBy rdf:resource="http://purl.org/dc/terms/"/>
        <rdfs:subPropertyOf rdf:resource="&terms;description"/>
    </owl:AnnotationProperty>
    <owl:AnnotationProperty rdf:about="&dc;subject">
        <rdfs:label xml:lang="en">Subject</rdfs:label>
        <terms:issued rdf:datatype="&xsd;date">1999-07-02</terms:issued>
        <terms:modified rdf:datatype="&xsd;date">2012-06-14</terms:modified>
        <skos:note xml:lang="en">A second property with the same name as this property has been declared in the dcterms: namespace (http://purl.org/dc/terms/).  See the Introduction to the document &quot;DCMI Metadata Terms&quot; (http://dublincore.org/documents/dcmi-terms/) for an explanation.</skos:note>
        <rdfs:comment xml:lang="en">The topic of the resource.</rdfs:comment>
        <terms:description xml:lang="en">Typically, the subject will be represented using keywords, key phrases, or classification codes. Recommended best practice is to use a controlled vocabulary.</terms:description>
        <terms:hasVersion rdf:resource="http://dublincore.org/usage/terms/history/#subject-007"/>
        <rdfs:isDefinedBy rdf:resource="http://purl.org/dc/elements/1.1/"/>
    </owl:AnnotationProperty>
    <owl:AnnotationProperty rdf:about="&terms;bibliographicCitation">
        <rdfs:subPropertyOf rdf:resource="&dc;identifier"/>
        <rdfs:domain rdf:resource="&terms;BibliographicResource"/>
        <rdfs:subPropertyOf rdf:resource="&terms;identifier"/>
    </owl:AnnotationProperty>
    <owl:AnnotationProperty rdf:about="&wgs84_pos;lat">
        <rdfs:label>latitude</rdfs:label>
        <rdfs:comment>The WGS84 latitude of a SpatialThing (decimal degrees).</rdfs:comment>
        <rdfs:domain rdf:resource="&wgs84_pos;SpatialThing"/>
    </owl:AnnotationProperty>
    <owl:AnnotationProperty rdf:about="&scovo2;dataset"/>
    <owl:AnnotationProperty rdf:about="&foaf;member"/>
    <owl:AnnotationProperty rdf:about="&skos;scopeNote">
        <rdfs:label xml:lang="en">scope note</rdfs:label>
        <skos:definition xml:lang="en">A note that helps to clarify the meaning and/or the use of a concept.</skos:definition>
        <rdfs:isDefinedBy rdf:resource="http://www.w3.org/2004/02/skos/core"/>
        <rdfs:subPropertyOf rdf:resource="&skos;note"/>
    </owl:AnnotationProperty>
    <owl:AnnotationProperty rdf:about="&terms;license">
        <rdfs:label xml:lang="en">License</rdfs:label>
        <terms:issued rdf:datatype="&xsd;date">2004-06-14</terms:issued>
        <terms:modified rdf:datatype="&xsd;date">2008-01-14</terms:modified>
        <rdfs:comment xml:lang="en">A legal document giving official permission to do something with the resource.</rdfs:comment>
        <terms:hasVersion rdf:resource="http://dublincore.org/usage/terms/history/#license-002"/>
        <rdfs:subPropertyOf rdf:resource="&dc;rights"/>
        <rdfs:isDefinedBy rdf:resource="http://purl.org/dc/terms/"/>
        <rdfs:subPropertyOf rdf:resource="&terms;rights"/>
    </owl:AnnotationProperty>
    <owl:AnnotationProperty rdf:about="&terms;hasFormat">
        <rdfs:label xml:lang="en">Has Format</rdfs:label>
        <terms:issued rdf:datatype="&xsd;date">2000-07-11</terms:issued>
        <terms:modified rdf:datatype="&xsd;date">2008-01-14</terms:modified>
        <rdfs:comment xml:lang="en">A related resource that is substantially the same as the pre-existing described resource, but in another format.</rdfs:comment>
        <skos:note xml:lang="en">This term is intended to be used with non-literal values as defined in the DCMI Abstract Model (http://dublincore.org/documents/abstract-model/).  As of December 2007, the DCMI Usage Board is seeking a way to express this intention with a formal range declaration.</skos:note>
        <terms:hasVersion rdf:resource="http://dublincore.org/usage/terms/history/#hasFormat-003"/>
        <rdfs:subPropertyOf rdf:resource="&dc;relation"/>
        <rdfs:isDefinedBy rdf:resource="http://purl.org/dc/terms/"/>
        <rdfs:subPropertyOf rdf:resource="&terms;relation"/>
    </owl:AnnotationProperty>
    <owl:AnnotationProperty rdf:about="&geopolitical;sourceModified"/>
    <owl:AnnotationProperty rdf:about="&geopolitical;sourceIdentifier"/>
    <owl:AnnotationProperty rdf:about="&skos;definition">
        <rdfs:label xml:lang="en">definition</rdfs:label>
        <skos:definition xml:lang="en">A statement or formal explanation of the meaning of a concept.</skos:definition>
        <rdfs:isDefinedBy rdf:resource="http://www.w3.org/2004/02/skos/core"/>
        <rdfs:subPropertyOf rdf:resource="&skos;note"/>
    </owl:AnnotationProperty>
    <owl:AnnotationProperty rdf:about="&foaf;mbox"/>
    <owl:AnnotationProperty rdf:about="&terms;relation">
        <rdfs:label xml:lang="en">Relation</rdfs:label>
        <terms:modified rdf:datatype="&xsd;date">2008-01-14</terms:modified>
        <terms:issued rdf:datatype="&xsd;date">2008-01-14</terms:issued>
        <rdfs:comment xml:lang="en">A related resource.</rdfs:comment>
        <terms:description xml:lang="en">Recommended best practice is to identify the related resource by means of a string conforming to a formal identification system. </terms:description>
        <skos:note xml:lang="en">This term is intended to be used with non-literal values as defined in the DCMI Abstract Model (http://dublincore.org/documents/abstract-model/).  As of December 2007, the DCMI Usage Board is seeking a way to express this intention with a formal range declaration.</skos:note>
        <terms:hasVersion rdf:resource="http://dublincore.org/usage/terms/history/#relationT-001"/>
        <rdfs:subPropertyOf rdf:resource="&dc;relation"/>
        <rdfs:isDefinedBy rdf:resource="http://purl.org/dc/terms/"/>
    </owl:AnnotationProperty>
    <owl:AnnotationProperty rdf:about="&dc;title">
        <rdfs:label xml:lang="en">Title</rdfs:label>
        <terms:issued rdf:datatype="&xsd;date">1999-07-02</terms:issued>
        <terms:modified rdf:datatype="&xsd;date">2008-01-14</terms:modified>
        <rdfs:comment xml:lang="en">A name given to the resource.</rdfs:comment>
        <skos:note xml:lang="en">A second property with the same name as this property has been declared in the dcterms: namespace (http://purl.org/dc/terms/).  See the Introduction to the document &quot;DCMI Metadata Terms&quot; (http://dublincore.org/documents/dcmi-terms/) for an explanation.</skos:note>
        <terms:hasVersion rdf:resource="http://dublincore.org/usage/terms/history/#title-006"/>
        <rdfs:isDefinedBy rdf:resource="http://purl.org/dc/elements/1.1/"/>
    </owl:AnnotationProperty>
    <owl:AnnotationProperty rdf:about="&wgs84_pos;location">
        <rdfs:subPropertyOf rdf:resource="&foaf;based_near"/>
    </owl:AnnotationProperty>
    <owl:AnnotationProperty rdf:about="&terms;mediator">
        <rdfs:label xml:lang="en">Mediator</rdfs:label>
        <terms:issued rdf:datatype="&xsd;date">2001-05-21</terms:issued>
        <terms:modified rdf:datatype="&xsd;date">2008-01-14</terms:modified>
        <rdfs:comment xml:lang="en">An entity that mediates access to the resource and for whom the resource is intended or useful.</rdfs:comment>
        <terms:description xml:lang="en">In an educational context, a mediator might be a parent, teacher, teaching assistant, or care-giver.</terms:description>
        <terms:hasVersion rdf:resource="http://dublincore.org/usage/terms/history/#mediator-003"/>
        <rdfs:isDefinedBy rdf:resource="http://purl.org/dc/terms/"/>
        <rdfs:subPropertyOf rdf:resource="&terms;audience"/>
    </owl:AnnotationProperty>
    <owl:AnnotationProperty rdf:about="&dc;relation">
        <rdfs:label xml:lang="en">Relation</rdfs:label>
        <terms:issued rdf:datatype="&xsd;date">1999-07-02</terms:issued>
        <terms:modified rdf:datatype="&xsd;date">2008-01-14</terms:modified>
        <rdfs:comment xml:lang="en">A related resource.</rdfs:comment>
        <skos:note xml:lang="en">A second property with the same name as this property has been declared in the dcterms: namespace (http://purl.org/dc/terms/).  See the Introduction to the document &quot;DCMI Metadata Terms&quot; (http://dublincore.org/documents/dcmi-terms/) for an explanation.</skos:note>
        <terms:description xml:lang="en">Recommended best practice is to identify the related resource by means of a string conforming to a formal identification system. </terms:description>
        <terms:hasVersion rdf:resource="http://dublincore.org/usage/terms/history/#relation-006"/>
        <rdfs:isDefinedBy rdf:resource="http://purl.org/dc/elements/1.1/"/>
    </owl:AnnotationProperty>
    <owl:AnnotationProperty rdf:about="&scovo2;max">
        <rdfs:label>has a maximum range value</rdfs:label>
        <rdfs:domain rdf:resource="&scovo2;Dimension"/>
    </owl:AnnotationProperty>
    <owl:AnnotationProperty rdf:about="&scovo2;min">
        <rdfs:label>has a minimum range value</rdfs:label>
        <rdfs:domain rdf:resource="&scovo2;Dimension"/>
    </owl:AnnotationProperty>
    <owl:AnnotationProperty rdf:about="&foaf;homepage"/>
    <owl:AnnotationProperty rdf:about="&terms;accrualPolicy">
        <rdfs:label xml:lang="en">Accrual Policy</rdfs:label>
        <terms:issued rdf:datatype="&xsd;date">2005-06-13</terms:issued>
        <terms:modified rdf:datatype="&xsd;date">2010-10-11</terms:modified>
        <rdfs:comment xml:lang="en">The policy governing the addition of items to a collection.</rdfs:comment>
        <terms:hasVersion rdf:resource="http://dublincore.org/usage/terms/history/#accrualPolicy-003"/>
        <rdfs:domain rdf:resource="http://purl.org/dc/dcmitype/Collection"/>
        <rdfs:isDefinedBy rdf:resource="http://purl.org/dc/terms/"/>
    </owl:AnnotationProperty>
    <owl:AnnotationProperty rdf:about="&foaf;based_near"/>
    <owl:AnnotationProperty rdf:about="&wgs84_pos;alt">
        <rdfs:label>altitude</rdfs:label>
        <rdfs:comment>The WGS84 altitude of a SpatialThing (decimal meters 
above the local reference ellipsoid).</rdfs:comment>
        <rdfs:domain rdf:resource="&wgs84_pos;SpatialThing"/>
    </owl:AnnotationProperty>
    <owl:AnnotationProperty rdf:about="&terms;valid">
        <rdfs:subPropertyOf rdf:resource="&dc;date"/>
        <rdfs:subPropertyOf rdf:resource="&terms;date"/>
    </owl:AnnotationProperty>
    <owl:AnnotationProperty rdf:about="&geopolitical;sourceCreator"/>
    <owl:AnnotationProperty rdf:about="&terms;modified">
        <rdfs:subPropertyOf rdf:resource="&dc;date"/>
        <rdfs:subPropertyOf rdf:resource="&terms;date"/>
    </owl:AnnotationProperty>
    <owl:AnnotationProperty rdf:about="&dc;type">
        <rdfs:label xml:lang="en">Type</rdfs:label>
        <terms:issued rdf:datatype="&xsd;date">1999-07-02</terms:issued>
        <terms:modified rdf:datatype="&xsd;date">2008-01-14</terms:modified>
        <skos:note xml:lang="en">A second property with the same name as this property has been declared in the dcterms: namespace (http://purl.org/dc/terms/).  See the Introduction to the document &quot;DCMI Metadata Terms&quot; (http://dublincore.org/documents/dcmi-terms/) for an explanation.</skos:note>
        <terms:description xml:lang="en">Recommended best practice is to use a controlled vocabulary such as the DCMI Type Vocabulary [DCMITYPE]. To describe the file format, physical medium, or dimensions of the resource, use the Format element.</terms:description>
        <rdfs:comment xml:lang="en">The nature or genre of the resource.</rdfs:comment>
        <terms:hasVersion rdf:resource="http://dublincore.org/usage/terms/history/#type-006"/>
        <rdfs:isDefinedBy rdf:resource="http://purl.org/dc/elements/1.1/"/>
    </owl:AnnotationProperty>
    <owl:AnnotationProperty rdf:about="&terms;educationLevel">
        <rdfs:label xml:lang="en">Audience Education Level</rdfs:label>
        <terms:issued rdf:datatype="&xsd;date">2002-07-13</terms:issued>
        <terms:modified rdf:datatype="&xsd;date">2008-01-14</terms:modified>
        <rdfs:comment xml:lang="en">A class of entity, defined in terms of progression through an educational or training context, for which the described resource is intended.</rdfs:comment>
        <terms:hasVersion rdf:resource="http://dublincore.org/usage/terms/history/#educationLevel-002"/>
        <rdfs:isDefinedBy rdf:resource="http://purl.org/dc/terms/"/>
        <rdfs:subPropertyOf rdf:resource="&terms;audience"/>
    </owl:AnnotationProperty>
    <owl:AnnotationProperty rdf:about="&dc;source">
        <rdfs:label xml:lang="en">Source</rdfs:label>
        <terms:issued rdf:datatype="&xsd;date">1999-07-02</terms:issued>
        <terms:modified rdf:datatype="&xsd;date">2008-01-14</terms:modified>
        <rdfs:comment xml:lang="en">A related resource from which the described resource is derived.</rdfs:comment>
        <skos:note xml:lang="en">A second property with the same name as this property has been declared in the dcterms: namespace (http://purl.org/dc/terms/).  See the Introduction to the document &quot;DCMI Metadata Terms&quot; (http://dublincore.org/documents/dcmi-terms/) for an explanation.</skos:note>
        <terms:description xml:lang="en">The described resource may be derived from the related resource in whole or in part. Recommended best practice is to identify the related resource by means of a string conforming to a formal identification system.</terms:description>
        <terms:hasVersion rdf:resource="http://dublincore.org/usage/terms/history/#source-006"/>
        <rdfs:isDefinedBy rdf:resource="http://purl.org/dc/elements/1.1/"/>
    </owl:AnnotationProperty>
    <owl:AnnotationProperty rdf:about="&terms;accrualPeriodicity">
        <rdfs:label xml:lang="en">Accrual Periodicity</rdfs:label>
        <terms:issued rdf:datatype="&xsd;date">2005-06-13</terms:issued>
        <terms:modified rdf:datatype="&xsd;date">2010-10-11</terms:modified>
        <rdfs:comment xml:lang="en">The frequency with which items are added to a collection.</rdfs:comment>
        <terms:hasVersion rdf:resource="http://dublincore.org/usage/terms/history/#accrualPeriodicity-003"/>
        <rdfs:domain rdf:resource="http://purl.org/dc/dcmitype/Collection"/>
        <rdfs:isDefinedBy rdf:resource="http://purl.org/dc/terms/"/>
    </owl:AnnotationProperty>
    <owl:AnnotationProperty rdf:about="&terms;replaces">
        <rdfs:label xml:lang="en">Replaces</rdfs:label>
        <terms:issued rdf:datatype="&xsd;date">2000-07-11</terms:issued>
        <terms:modified rdf:datatype="&xsd;date">2008-01-14</terms:modified>
        <rdfs:comment xml:lang="en">A related resource that is supplanted, displaced, or superseded by the described resource.</rdfs:comment>
        <skos:note xml:lang="en">This term is intended to be used with non-literal values as defined in the DCMI Abstract Model (http://dublincore.org/documents/abstract-model/).  As of December 2007, the DCMI Usage Board is seeking a way to express this intention with a formal range declaration.</skos:note>
        <terms:hasVersion rdf:resource="http://dublincore.org/usage/terms/history/#replaces-003"/>
        <rdfs:subPropertyOf rdf:resource="&dc;relation"/>
        <rdfs:isDefinedBy rdf:resource="http://purl.org/dc/terms/"/>
        <rdfs:subPropertyOf rdf:resource="&terms;relation"/>
        <rdfs:domain rdf:resource="&geosparql;Feature"/>
    </owl:AnnotationProperty>
    <owl:AnnotationProperty rdf:about="&terms;spatial">
        <rdfs:label xml:lang="en">Spatial Coverage</rdfs:label>
        <terms:issued rdf:datatype="&xsd;date">2000-07-11</terms:issued>
        <terms:modified rdf:datatype="&xsd;date">2008-01-14</terms:modified>
        <rdfs:comment xml:lang="en">Spatial characteristics of the resource.</rdfs:comment>
        <terms:hasVersion rdf:resource="http://dublincore.org/usage/terms/history/#spatial-003"/>
        <rdfs:subPropertyOf rdf:resource="&dc;coverage"/>
        <rdfs:isDefinedBy rdf:resource="http://purl.org/dc/terms/"/>
        <rdfs:subPropertyOf rdf:resource="&terms;coverage"/>
    </owl:AnnotationProperty>
    <owl:AnnotationProperty rdf:about="&terms;subject">
        <rdfs:label xml:lang="en">Subject</rdfs:label>
        <terms:issued rdf:datatype="&xsd;date">2008-01-14</terms:issued>
        <terms:modified rdf:datatype="&xsd;date">2012-06-14</terms:modified>
        <rdfs:comment xml:lang="en">The topic of the resource.</rdfs:comment>
        <skos:note xml:lang="en">This term is intended to be used with non-literal values as defined in the DCMI Abstract Model (http://dublincore.org/documents/abstract-model/).  As of December 2007, the DCMI Usage Board is seeking a way to express this intention with a formal range declaration.</skos:note>
        <terms:description xml:lang="en">Typically, the subject will be represented using keywords, key phrases, or classification codes. Recommended best practice is to use a controlled vocabulary.</terms:description>
        <terms:hasVersion rdf:resource="http://dublincore.org/usage/terms/history/#subjectT-002"/>
        <rdfs:subPropertyOf rdf:resource="&dc;subject"/>
        <rdfs:isDefinedBy rdf:resource="http://purl.org/dc/terms/"/>
    </owl:AnnotationProperty>
    <owl:AnnotationProperty rdf:about="&terms;format">
        <rdfs:label xml:lang="en">Format</rdfs:label>
        <terms:issued rdf:datatype="&xsd;date">2008-01-14</terms:issued>
        <terms:modified rdf:datatype="&xsd;date">2008-01-14</terms:modified>
        <terms:description xml:lang="en">Examples of dimensions include size and duration. Recommended best practice is to use a controlled vocabulary such as the list of Internet Media Types [MIME].</terms:description>
        <rdfs:comment xml:lang="en">The file format, physical medium, or dimensions of the resource.</rdfs:comment>
        <terms:hasVersion rdf:resource="http://dublincore.org/usage/terms/history/#formatT-001"/>
        <rdfs:subPropertyOf rdf:resource="&dc;format"/>
        <rdfs:isDefinedBy rdf:resource="http://purl.org/dc/terms/"/>
    </owl:AnnotationProperty>
    <owl:AnnotationProperty rdf:about="&terms;identifier">
        <rdfs:label xml:lang="en">Identifier</rdfs:label>
        <terms:issued rdf:datatype="&xsd;date">2008-01-14</terms:issued>
        <terms:modified rdf:datatype="&xsd;date">2008-01-14</terms:modified>
        <rdfs:comment xml:lang="en">An unambiguous reference to the resource within a given context.</rdfs:comment>
        <terms:description xml:lang="en">Recommended best practice is to identify the resource by means of a string conforming to a formal identification system. </terms:description>
        <terms:hasVersion rdf:resource="http://dublincore.org/usage/terms/history/#identifierT-001"/>
        <rdfs:subPropertyOf rdf:resource="&dc;identifier"/>
        <rdfs:isDefinedBy rdf:resource="http://purl.org/dc/terms/"/>
        <rdfs:domain rdf:resource="&geosparql;Feature"/>
    </owl:AnnotationProperty>
    <owl:AnnotationProperty rdf:about="&terms;type">
        <rdfs:label xml:lang="en">Type</rdfs:label>
        <terms:modified rdf:datatype="&xsd;date">2008-01-14</terms:modified>
        <terms:issued rdf:datatype="&xsd;date">2008-01-14</terms:issued>
        <terms:description xml:lang="en">Recommended best practice is to use a controlled vocabulary such as the DCMI Type Vocabulary [DCMITYPE]. To describe the file format, physical medium, or dimensions of the resource, use the Format element.</terms:description>
        <rdfs:comment xml:lang="en">The nature or genre of the resource.</rdfs:comment>
        <terms:hasVersion rdf:resource="http://dublincore.org/usage/terms/history/#typeT-001"/>
        <rdfs:subPropertyOf rdf:resource="&dc;type"/>
        <rdfs:isDefinedBy rdf:resource="http://purl.org/dc/terms/"/>
    </owl:AnnotationProperty>
    <owl:AnnotationProperty rdf:about="&terms;requires">
        <rdfs:label xml:lang="en">Requires</rdfs:label>
        <terms:issued rdf:datatype="&xsd;date">2000-07-11</terms:issued>
        <terms:modified rdf:datatype="&xsd;date">2008-01-14</terms:modified>
        <rdfs:comment xml:lang="en">A related resource that is required by the described resource to support its function, delivery, or coherence.</rdfs:comment>
        <skos:note xml:lang="en">This term is intended to be used with non-literal values as defined in the DCMI Abstract Model (http://dublincore.org/documents/abstract-model/).  As of December 2007, the DCMI Usage Board is seeking a way to express this intention with a formal range declaration.</skos:note>
        <terms:hasVersion rdf:resource="http://dublincore.org/usage/terms/history/#requires-003"/>
        <rdfs:subPropertyOf rdf:resource="&dc;relation"/>
        <rdfs:isDefinedBy rdf:resource="http://purl.org/dc/terms/"/>
        <rdfs:subPropertyOf rdf:resource="&terms;relation"/>
    </owl:AnnotationProperty>
    <owl:AnnotationProperty rdf:about="&terms;extent">
        <rdfs:label xml:lang="en">Extent</rdfs:label>
        <terms:issued rdf:datatype="&xsd;date">2000-07-11</terms:issued>
        <terms:modified rdf:datatype="&xsd;date">2008-01-14</terms:modified>
        <rdfs:comment xml:lang="en">The size or duration of the resource.</rdfs:comment>
        <terms:hasVersion rdf:resource="http://dublincore.org/usage/terms/history/#extent-003"/>
        <rdfs:subPropertyOf rdf:resource="&dc;format"/>
        <rdfs:isDefinedBy rdf:resource="http://purl.org/dc/terms/"/>
        <rdfs:subPropertyOf rdf:resource="&terms;format"/>
    </owl:AnnotationProperty>
    <owl:AnnotationProperty rdf:about="&scovo2;dimension"/>
    <owl:AnnotationProperty rdf:about="&terms;rights">
        <rdfs:label xml:lang="en">Rights</rdfs:label>
        <terms:issued rdf:datatype="&xsd;date">2008-01-14</terms:issued>
        <terms:modified rdf:datatype="&xsd;date">2008-01-14</terms:modified>
        <rdfs:comment xml:lang="en">Information about rights held in and over the resource.</rdfs:comment>
        <terms:description xml:lang="en">Typically, rights information includes a statement about various property rights associated with the resource, including intellectual property rights.</terms:description>
        <terms:hasVersion rdf:resource="http://dublincore.org/usage/terms/history/#rightsT-001"/>
        <rdfs:subPropertyOf rdf:resource="&dc;rights"/>
        <rdfs:isDefinedBy rdf:resource="http://purl.org/dc/terms/"/>
    </owl:AnnotationProperty>
    <owl:AnnotationProperty rdf:about="&dc;format">
        <rdfs:label xml:lang="en">Format</rdfs:label>
        <terms:issued rdf:datatype="&xsd;date">1999-07-02</terms:issued>
        <terms:modified rdf:datatype="&xsd;date">2008-01-14</terms:modified>
        <skos:note xml:lang="en">A second property with the same name as this property has been declared in the dcterms: namespace (http://purl.org/dc/terms/).  See the Introduction to the document &quot;DCMI Metadata Terms&quot; (http://dublincore.org/documents/dcmi-terms/) for an explanation.</skos:note>
        <terms:description xml:lang="en">Examples of dimensions include size and duration. Recommended best practice is to use a controlled vocabulary such as the list of Internet Media Types [MIME].</terms:description>
        <rdfs:comment xml:lang="en">The file format, physical medium, or dimensions of the resource.</rdfs:comment>
        <terms:hasVersion rdf:resource="http://dublincore.org/usage/terms/history/#format-007"/>
        <rdfs:isDefinedBy rdf:resource="http://purl.org/dc/elements/1.1/"/>
    </owl:AnnotationProperty>
    <owl:AnnotationProperty rdf:about="&terms;isReferencedBy">
        <rdfs:label xml:lang="en">Is Referenced By</rdfs:label>
        <terms:issued rdf:datatype="&xsd;date">2000-07-11</terms:issued>
        <terms:modified rdf:datatype="&xsd;date">2008-01-14</terms:modified>
        <rdfs:comment xml:lang="en">A related resource that references, cites, or otherwise points to the described resource.</rdfs:comment>
        <skos:note xml:lang="en">This term is intended to be used with non-literal values as defined in the DCMI Abstract Model (http://dublincore.org/documents/abstract-model/).  As of December 2007, the DCMI Usage Board is seeking a way to express this intention with a formal range declaration.</skos:note>
        <terms:hasVersion rdf:resource="http://dublincore.org/usage/terms/history/#isReferencedBy-003"/>
        <rdfs:subPropertyOf rdf:resource="&dc;relation"/>
        <rdfs:isDefinedBy rdf:resource="http://purl.org/dc/terms/"/>
        <rdfs:subPropertyOf rdf:resource="&terms;relation"/>
    </owl:AnnotationProperty>
    <owl:AnnotationProperty rdf:about="&dc;rights">
        <rdfs:label xml:lang="en">Rights</rdfs:label>
        <terms:issued rdf:datatype="&xsd;date">1999-07-02</terms:issued>
        <terms:modified rdf:datatype="&xsd;date">2008-01-14</terms:modified>
        <skos:note xml:lang="en">A second property with the same name as this property has been declared in the dcterms: namespace (http://purl.org/dc/terms/).  See the Introduction to the document &quot;DCMI Metadata Terms&quot; (http://dublincore.org/documents/dcmi-terms/) for an explanation.</skos:note>
        <rdfs:comment xml:lang="en">Information about rights held in and over the resource.</rdfs:comment>
        <terms:description xml:lang="en">Typically, rights information includes a statement about various property rights associated with the resource, including intellectual property rights.</terms:description>
        <terms:hasVersion rdf:resource="http://dublincore.org/usage/terms/history/#rights-006"/>
        <rdfs:isDefinedBy rdf:resource="http://purl.org/dc/elements/1.1/"/>
    </owl:AnnotationProperty>
    <owl:AnnotationProperty rdf:about="&ontology;provenance"/>
    <owl:AnnotationProperty rdf:about="&skos;changeNote">
        <rdfs:label xml:lang="en">change note</rdfs:label>
        <skos:definition xml:lang="en">A note about a modification to a concept.</skos:definition>
        <rdfs:isDefinedBy rdf:resource="http://www.w3.org/2004/02/skos/core"/>
        <rdfs:subPropertyOf rdf:resource="&skos;note"/>
    </owl:AnnotationProperty>
    <owl:AnnotationProperty rdf:about="&dc;contributor">
        <rdfs:label xml:lang="en">Contributor</rdfs:label>
        <terms:issued rdf:datatype="&xsd;date">1999-07-02</terms:issued>
        <terms:modified rdf:datatype="&xsd;date">2008-01-14</terms:modified>
        <skos:note xml:lang="en">A second property with the same name as this property has been declared in the dcterms: namespace (http://purl.org/dc/terms/).  See the Introduction to the document &quot;DCMI Metadata Terms&quot; (http://dublincore.org/documents/dcmi-terms/) for an explanation.</skos:note>
        <rdfs:comment xml:lang="en">An entity responsible for making contributions to the resource.</rdfs:comment>
        <terms:description xml:lang="en">Examples of a Contributor include a person, an organization, or a service. Typically, the name of a Contributor should be used to indicate the entity.</terms:description>
        <terms:hasVersion rdf:resource="http://dublincore.org/usage/terms/history/#contributor-006"/>
        <rdfs:isDefinedBy rdf:resource="http://purl.org/dc/elements/1.1/"/>
    </owl:AnnotationProperty>
    <owl:AnnotationProperty rdf:about="&terms;source">
        <rdfs:label xml:lang="en">Source</rdfs:label>
        <terms:issued rdf:datatype="&xsd;date">2008-01-14</terms:issued>
        <terms:modified rdf:datatype="&xsd;date">2008-01-14</terms:modified>
        <rdfs:comment xml:lang="en">A related resource from which the described resource is derived.</rdfs:comment>
        <terms:description xml:lang="en">The described resource may be derived from the related resource in whole or in part. Recommended best practice is to identify the related resource by means of a string conforming to a formal identification system.</terms:description>
        <skos:note xml:lang="en">This term is intended to be used with non-literal values as defined in the DCMI Abstract Model (http://dublincore.org/documents/abstract-model/).  As of December 2007, the DCMI Usage Board is seeking a way to express this intention with a formal range declaration.</skos:note>
        <terms:hasVersion rdf:resource="http://dublincore.org/usage/terms/history/#sourceT-001"/>
        <rdfs:subPropertyOf rdf:resource="&dc;source"/>
        <rdfs:isDefinedBy rdf:resource="http://purl.org/dc/terms/"/>
        <rdfs:subPropertyOf rdf:resource="&terms;relation"/>
    </owl:AnnotationProperty>
    <owl:AnnotationProperty rdf:about="&terms;accrualMethod">
        <rdfs:label xml:lang="en">Accrual Method</rdfs:label>
        <terms:issued rdf:datatype="&xsd;date">2005-06-13</terms:issued>
        <terms:modified rdf:datatype="&xsd;date">2010-10-11</terms:modified>
        <rdfs:comment xml:lang="en">The method by which items are added to a collection.</rdfs:comment>
        <terms:hasVersion rdf:resource="http://dublincore.org/usage/terms/history/#accrualMethod-003"/>
        <rdfs:domain rdf:resource="http://purl.org/dc/dcmitype/Collection"/>
        <rdfs:isDefinedBy rdf:resource="http://purl.org/dc/terms/"/>
    </owl:AnnotationProperty>
    <owl:AnnotationProperty rdf:about="&terms;tableOfContents">
        <rdfs:label xml:lang="en">Table Of Contents</rdfs:label>
        <terms:issued rdf:datatype="&xsd;date">2000-07-11</terms:issued>
        <terms:modified rdf:datatype="&xsd;date">2008-01-14</terms:modified>
        <rdfs:comment xml:lang="en">A list of subunits of the resource.</rdfs:comment>
        <terms:hasVersion rdf:resource="http://dublincore.org/usage/terms/history/#tableOfContents-003"/>
        <rdfs:subPropertyOf rdf:resource="&dc;description"/>
        <rdfs:isDefinedBy rdf:resource="http://purl.org/dc/terms/"/>
        <rdfs:subPropertyOf rdf:resource="&terms;description"/>
    </owl:AnnotationProperty>
    <owl:AnnotationProperty rdf:about="&dc;creator">
        <rdfs:label xml:lang="en">Creator</rdfs:label>
        <terms:issued rdf:datatype="&xsd;date">1999-07-02</terms:issued>
        <terms:modified rdf:datatype="&xsd;date">2008-01-14</terms:modified>
        <skos:note xml:lang="en">A second property with the same name as this property has been declared in the dcterms: namespace (http://purl.org/dc/terms/).  See the Introduction to the document &quot;DCMI Metadata Terms&quot; (http://dublincore.org/documents/dcmi-terms/) for an explanation.</skos:note>
        <rdfs:comment xml:lang="en">An entity primarily responsible for making the resource.</rdfs:comment>
        <terms:description xml:lang="en">Examples of a Creator include a person, an organization, or a service. Typically, the name of a Creator should be used to indicate the entity.</terms:description>
        <terms:hasVersion rdf:resource="http://dublincore.org/usage/terms/history/#creator-006"/>
        <rdfs:isDefinedBy rdf:resource="http://purl.org/dc/elements/1.1/"/>
    </owl:AnnotationProperty>
    <owl:AnnotationProperty rdf:about="h&btn100;provenance"/>
    <owl:AnnotationProperty rdf:about="&terms;medium">
        <rdfs:label xml:lang="en">Medium</rdfs:label>
        <terms:issued rdf:datatype="&xsd;date">2000-07-11</terms:issued>
        <terms:modified rdf:datatype="&xsd;date">2008-01-14</terms:modified>
        <rdfs:comment xml:lang="en">The material or physical carrier of the resource.</rdfs:comment>
        <terms:hasVersion rdf:resource="http://dublincore.org/usage/terms/history/#medium-003"/>
        <rdfs:subPropertyOf rdf:resource="&dc;format"/>
        <rdfs:isDefinedBy rdf:resource="http://purl.org/dc/terms/"/>
        <rdfs:domain rdf:resource="&terms;PhysicalResource"/>
        <rdfs:subPropertyOf rdf:resource="&terms;format"/>
    </owl:AnnotationProperty>
    <owl:AnnotationProperty rdf:about="&skos;hiddenLabel">
        <rdfs:label xml:lang="en">hidden label</rdfs:label>
        <skos:definition xml:lang="en">A lexical label for a resource that should be hidden when generating visual displays of the resource, but should still be accessible to free text search operations.</skos:definition>
        <rdfs:comment xml:lang="en">The range of skos:hiddenLabel is the class of RDF plain literals.</rdfs:comment>
        <rdfs:comment xml:lang="en">skos:prefLabel, skos:altLabel and skos:hiddenLabel are pairwise disjoint properties.</rdfs:comment>
        <rdfs:subPropertyOf rdf:resource="&rdfs;label"/>
        <rdfs:isDefinedBy rdf:resource="http://www.w3.org/2004/02/skos/core"/>
    </owl:AnnotationProperty>
    <owl:AnnotationProperty rdf:about="&terms;dateAccepted">
        <rdfs:subPropertyOf rdf:resource="&dc;date"/>
        <rdfs:subPropertyOf rdf:resource="&terms;date"/>
    </owl:AnnotationProperty>
    <owl:AnnotationProperty rdf:about="&terms;temporal">
        <rdfs:label xml:lang="en">Temporal Coverage</rdfs:label>
        <terms:issued rdf:datatype="&xsd;date">2000-07-11</terms:issued>
        <terms:modified rdf:datatype="&xsd;date">2008-01-14</terms:modified>
        <rdfs:comment xml:lang="en">Temporal characteristics of the resource.</rdfs:comment>
        <terms:hasVersion rdf:resource="http://dublincore.org/usage/terms/history/#temporal-003"/>
        <rdfs:subPropertyOf rdf:resource="&dc;coverage"/>
        <rdfs:isDefinedBy rdf:resource="http://purl.org/dc/terms/"/>
        <rdfs:subPropertyOf rdf:resource="&terms;coverage"/>
    </owl:AnnotationProperty>
    <owl:AnnotationProperty rdf:about="&dc;identifier">
        <rdfs:label xml:lang="en">Identifier</rdfs:label>
        <terms:issued rdf:datatype="&xsd;date">1999-07-02</terms:issued>
        <terms:modified rdf:datatype="&xsd;date">2008-01-14</terms:modified>
        <skos:note xml:lang="en">A second property with the same name as this property has been declared in the dcterms: namespace (http://purl.org/dc/terms/).  See the Introduction to the document &quot;DCMI Metadata Terms&quot; (http://dublincore.org/documents/dcmi-terms/) for an explanation.</skos:note>
        <rdfs:comment xml:lang="en">An unambiguous reference to the resource within a given context.</rdfs:comment>
        <terms:description xml:lang="en">Recommended best practice is to identify the resource by means of a string conforming to a formal identification system. </terms:description>
        <terms:hasVersion rdf:resource="http://dublincore.org/usage/terms/history/#identifier-006"/>
        <rdfs:isDefinedBy rdf:resource="http://purl.org/dc/elements/1.1/"/>
    </owl:AnnotationProperty>
    <owl:AnnotationProperty rdf:about="&terms;issued">
        <rdfs:subPropertyOf rdf:resource="&dc;date"/>
        <rdfs:subPropertyOf rdf:resource="&terms;date"/>
    </owl:AnnotationProperty>
    <owl:AnnotationProperty rdf:about="&dc;date">
        <rdfs:label xml:lang="en">Date</rdfs:label>
        <terms:issued rdf:datatype="&xsd;date">1999-07-02</terms:issued>
        <terms:modified rdf:datatype="&xsd;date">2008-01-14</terms:modified>
        <rdfs:comment xml:lang="en">A point or period of time associated with an event in the lifecycle of the resource.</rdfs:comment>
        <skos:note xml:lang="en">A second property with the same name as this property has been declared in the dcterms: namespace (http://purl.org/dc/terms/).  See the Introduction to the document &quot;DCMI Metadata Terms&quot; (http://dublincore.org/documents/dcmi-terms/) for an explanation.</skos:note>
        <terms:description xml:lang="en">Date may be used to express temporal information at any level of granularity.  Recommended best practice is to use an encoding scheme, such as the W3CDTF profile of ISO 8601 [W3CDTF].</terms:description>
        <terms:hasVersion rdf:resource="http://dublincore.org/usage/terms/history/#date-006"/>
        <rdfs:isDefinedBy rdf:resource="http://purl.org/dc/elements/1.1/"/>
    </owl:AnnotationProperty>
    <owl:AnnotationProperty rdf:about="&terms;dateCopyrighted">
        <rdfs:subPropertyOf rdf:resource="&dc;date"/>
        <rdfs:subPropertyOf rdf:resource="&terms;date"/>
    </owl:AnnotationProperty>
    <owl:AnnotationProperty rdf:about="&skos;altLabel">
        <rdfs:label xml:lang="en">alternative label</rdfs:label>
        <skos:example xml:lang="en">Acronyms, abbreviations, spelling variants, and irregular plural/singular forms may be included among the alternative labels for a concept. Mis-spelled terms are normally included as hidden labels (see skos:hiddenLabel).</skos:example>
        <skos:definition xml:lang="en">An alternative lexical label for a resource.</skos:definition>
        <rdfs:comment xml:lang="en">The range of skos:altLabel is the class of RDF plain literals.</rdfs:comment>
        <rdfs:comment xml:lang="en">skos:prefLabel, skos:altLabel and skos:hiddenLabel are pairwise disjoint properties.</rdfs:comment>
        <rdfs:subPropertyOf rdf:resource="&rdfs;label"/>
        <rdfs:isDefinedBy rdf:resource="http://www.w3.org/2004/02/skos/core"/>
    </owl:AnnotationProperty>
    <owl:AnnotationProperty rdf:about="&scovo2;datasetOf"/>
    <owl:AnnotationProperty rdf:about="&terms;FileFormat"/>
    <owl:AnnotationProperty rdf:about="&terms;description">
        <rdfs:label xml:lang="en">Description</rdfs:label>
        <terms:issued rdf:datatype="&xsd;date">2008-01-14</terms:issued>
        <terms:modified rdf:datatype="&xsd;date">2008-01-14</terms:modified>
        <rdfs:comment xml:lang="en">An account of the resource.</rdfs:comment>
        <terms:description xml:lang="en">Description may include but is not limited to: an abstract, a table of contents, a graphical representation, or a free-text account of the resource.</terms:description>
        <terms:hasVersion rdf:resource="http://dublincore.org/usage/terms/history/#descriptionT-001"/>
        <rdfs:subPropertyOf rdf:resource="&dc;description"/>
        <rdfs:isDefinedBy rdf:resource="http://purl.org/dc/terms/"/>
    </owl:AnnotationProperty>
    <owl:AnnotationProperty rdf:about="&terms;hasVersion">
        <rdfs:label xml:lang="en">Has Version</rdfs:label>
        <terms:issued rdf:datatype="&xsd;date">2000-07-11</terms:issued>
        <terms:modified rdf:datatype="&xsd;date">2008-01-14</terms:modified>
        <rdfs:comment xml:lang="en">A related resource that is a version, edition, or adaptation of the described resource.</rdfs:comment>
        <skos:note xml:lang="en">This term is intended to be used with non-literal values as defined in the DCMI Abstract Model (http://dublincore.org/documents/abstract-model/).  As of December 2007, the DCMI Usage Board is seeking a way to express this intention with a formal range declaration.</skos:note>
        <terms:hasVersion rdf:resource="http://dublincore.org/usage/terms/history/#hasVersion-003"/>
        <rdfs:subPropertyOf rdf:resource="&dc;relation"/>
        <rdfs:isDefinedBy rdf:resource="http://purl.org/dc/terms/"/>
        <rdfs:subPropertyOf rdf:resource="&terms;relation"/>
    </owl:AnnotationProperty>
    <owl:AnnotationProperty rdf:about="&adms;accessURL"/>
    <owl:AnnotationProperty rdf:about="&terms;date">
        <rdfs:subPropertyOf rdf:resource="&dc;date"/>
    </owl:AnnotationProperty>
    <owl:AnnotationProperty rdf:about="&terms;publisher">
        <rdfs:label xml:lang="en">Publisher</rdfs:label>
        <terms:issued rdf:datatype="&xsd;date">2008-01-14</terms:issued>
        <terms:modified rdf:datatype="&xsd;date">2010-10-11</terms:modified>
        <rdfs:comment xml:lang="en">An entity responsible for making the resource available.</rdfs:comment>
        <terms:description xml:lang="en">Examples of a Publisher include a person, an organization, or a service.</terms:description>
        <terms:hasVersion rdf:resource="http://dublincore.org/usage/terms/history/#publisherT-001"/>
        <rdfs:subPropertyOf rdf:resource="&dc;publisher"/>
        <rdfs:isDefinedBy rdf:resource="http://purl.org/dc/terms/"/>
    </owl:AnnotationProperty>
    <owl:AnnotationProperty rdf:about="&terms;isPartOf">
        <rdfs:label xml:lang="en">Is Part Of</rdfs:label>
        <terms:issued rdf:datatype="&xsd;date">2000-07-11</terms:issued>
        <terms:modified rdf:datatype="&xsd;date">2008-01-14</terms:modified>
        <rdfs:comment xml:lang="en">A related resource in which the described resource is physically or logically included.</rdfs:comment>
        <skos:note xml:lang="en">This term is intended to be used with non-literal values as defined in the DCMI Abstract Model (http://dublincore.org/documents/abstract-model/).  As of December 2007, the DCMI Usage Board is seeking a way to express this intention with a formal range declaration.</skos:note>
        <terms:hasVersion rdf:resource="http://dublincore.org/usage/terms/history/#isPartOf-003"/>
        <rdfs:subPropertyOf rdf:resource="&dc;relation"/>
        <rdfs:isDefinedBy rdf:resource="http://purl.org/dc/terms/"/>
        <rdfs:subPropertyOf rdf:resource="&terms;relation"/>
    </owl:AnnotationProperty>
    <owl:AnnotationProperty rdf:about="&dc;language">
        <rdfs:label xml:lang="en">Language</rdfs:label>
        <terms:issued rdf:datatype="&xsd;date">1999-07-02</terms:issued>
        <terms:modified rdf:datatype="&xsd;date">2008-01-14</terms:modified>
        <rdfs:comment xml:lang="en">A language of the resource.</rdfs:comment>
        <skos:note xml:lang="en">A second property with the same name as this property has been declared in the dcterms: namespace (http://purl.org/dc/terms/).  See the Introduction to the document &quot;DCMI Metadata Terms&quot; (http://dublincore.org/documents/dcmi-terms/) for an explanation.</skos:note>
        <terms:description xml:lang="en">Recommended best practice is to use a controlled vocabulary such as RFC 4646 [RFC4646].</terms:description>
        <terms:hasVersion rdf:resource="http://dublincore.org/usage/terms/history/#language-007"/>
        <rdfs:isDefinedBy rdf:resource="http://purl.org/dc/elements/1.1/"/>
        <rdfs:seeAlso rdf:resource="http://www.ietf.org/rfc/rfc4646.txt"/>
    </owl:AnnotationProperty>
    <owl:AnnotationProperty rdf:about="&wgs84_pos;long">
        <rdfs:label>longitude</rdfs:label>
        <rdfs:comment>The WGS84 longitude of a SpatialThing (decimal degrees).</rdfs:comment>
        <rdfs:domain rdf:resource="&wgs84_pos;SpatialThing"/>
    </owl:AnnotationProperty>
    <owl:AnnotationProperty rdf:about="&terms;accessRights">
        <rdfs:label xml:lang="en">Access Rights</rdfs:label>
        <terms:issued rdf:datatype="&xsd;date">2003-02-15</terms:issued>
        <terms:modified rdf:datatype="&xsd;date">2008-01-14</terms:modified>
        <terms:description xml:lang="en">Access Rights may include information regarding access or restrictions based on privacy, security, or other policies.</terms:description>
        <rdfs:comment xml:lang="en">Information about who can access the resource or an indication of its security status.</rdfs:comment>
        <terms:hasVersion rdf:resource="http://dublincore.org/usage/terms/history/#accessRights-002"/>
        <rdfs:subPropertyOf rdf:resource="&dc;rights"/>
        <rdfs:isDefinedBy rdf:resource="http://purl.org/dc/terms/"/>
        <rdfs:subPropertyOf rdf:resource="&terms;rights"/>
    </owl:AnnotationProperty>
    <owl:AnnotationProperty rdf:about="&foaf;name"/>
    <owl:AnnotationProperty rdf:about="&skos;example">
        <rdfs:label xml:lang="en">example</rdfs:label>
        <skos:definition xml:lang="en">An example of the use of a concept.</skos:definition>
        <rdfs:isDefinedBy rdf:resource="http://www.w3.org/2004/02/skos/core"/>
        <rdfs:subPropertyOf rdf:resource="&skos;note"/>
    </owl:AnnotationProperty>
    <owl:AnnotationProperty rdf:about="&terms;contributor">
        <rdfs:label xml:lang="en">Contributor</rdfs:label>
        <terms:issued rdf:datatype="&xsd;date">2008-01-14</terms:issued>
        <terms:modified rdf:datatype="&xsd;date">2010-10-11</terms:modified>
        <rdfs:comment xml:lang="en">An entity responsible for making contributions to the resource.</rdfs:comment>
        <terms:description xml:lang="en">Examples of a Contributor include a person, an organization, or a service.</terms:description>
        <terms:hasVersion rdf:resource="http://dublincore.org/usage/terms/history/#contributorT-001"/>
        <rdfs:subPropertyOf rdf:resource="&dc;contributor"/>
        <rdfs:isDefinedBy rdf:resource="http://purl.org/dc/terms/"/>
    </owl:AnnotationProperty>
    <owl:AnnotationProperty rdf:about="&terms;title">
        <rdfs:label xml:lang="en">Title</rdfs:label>
        <terms:issued rdf:datatype="&xsd;date">2008-01-14</terms:issued>
        <terms:modified rdf:datatype="&xsd;date">2010-10-11</terms:modified>
        <rdfs:comment xml:lang="en">A name given to the resource.</rdfs:comment>
        <terms:hasVersion rdf:resource="http://dublincore.org/usage/terms/history/#titleT-002"/>
        <rdfs:domain rdf:resource="h&btn100;AccidenteMaritimo"/>
        <rdfs:domain rdf:resource="h&btn100;Alojamiento"/>
        <rdfs:domain rdf:resource="h&btn100;Autovia"/>
        <rdfs:domain rdf:resource="h&btn100;CauceArtificial"/>
        <rdfs:domain rdf:resource="h&btn100;Diseminado"/>
        <rdfs:domain rdf:resource="h&btn100;ExplotacionMinera"/>
        <rdfs:domain rdf:resource="h&btn100;InstalacionFerroviaria"/>
        <rdfs:domain rdf:resource="h&btn100;Isla"/>
        <rdfs:domain rdf:resource="h&btn100;Itinerario"/>
        <rdfs:domain rdf:resource="h&btn100;LugarDeInteres"/>
        <rdfs:domain rdf:resource="h&btn100;LugarDeOcio"/>
        <rdfs:domain rdf:resource="h&btn100;NucleoPoblacional"/>
        <rdfs:domain rdf:resource="h&btn100;Rio"/>
        <rdfs:domain rdf:resource="h&btn100;UnidadAdministrativa"/>
        <rdfs:domain rdf:resource="h&btn100;ViaDeFerrocarril"/>
        <rdfs:domain rdf:resource="h&btn100;ZonaDeUsoCaracteristico"/>
        <rdfs:domain rdf:resource="h&btn100;ZonaProtegida"/>
        <rdfs:domain rdf:resource="&ontology;Aeropuerto"/>
        <rdfs:domain rdf:resource="&ontology;Alberca"/>
        <rdfs:domain rdf:resource="&ontology;Autopista"/>
        <rdfs:domain rdf:resource="&ontology;Carretera"/>
        <rdfs:domain rdf:resource="&ontology;Embalse"/>
        <rdfs:domain rdf:resource="&ontology;Faro"/>
        <rdfs:domain rdf:resource="&ontology;Humedal"/>
        <rdfs:domain rdf:resource="&ontology;Laguna"/>
        <rdfs:domain rdf:resource="&ontology;Mar"/>
        <rdfs:domain rdf:resource="&ontology;Oceano"/>
        <rdfs:domain rdf:resource="&ontology;Pista"/>
        <rdfs:domain rdf:resource="&ontology;Puerto"/>
        <rdfs:domain rdf:resource="&ontology;Ria"/>
        <rdfs:subPropertyOf rdf:resource="&dc;title"/>
        <rdfs:isDefinedBy rdf:resource="http://purl.org/dc/terms/"/>
        <rdfs:domain rdf:resource="&btn100;Cerro"/>
        <rdfs:domain rdf:resource="&btn100;Collado"/>
        <rdfs:domain rdf:resource="&btn100;EntidadVirtualDeAccidenteOrografico"/>
        <rdfs:domain rdf:resource="&btn100;Pico"/>
        <rdfs:domain rdf:resource="&btn100;PuertoDeMontanna"/>
        <rdfs:domain rdf:resource="&btn100;Relieve"/>
    </owl:AnnotationProperty>
    <rdf:Description rdf:about="&terms;audience">
        <rdfs:label xml:lang="en">Audience</rdfs:label>
        <terms:issued rdf:datatype="&xsd;date">2001-05-21</terms:issued>
        <terms:modified rdf:datatype="&xsd;date">2008-01-14</terms:modified>
        <rdfs:comment xml:lang="en">A class of entity for whom the resource is intended or useful.</rdfs:comment>
        <terms:hasVersion rdf:resource="http://dublincore.org/usage/terms/history/#audience-003"/>
        <rdfs:isDefinedBy rdf:resource="http://purl.org/dc/terms/"/>
    </rdf:Description>
    <owl:AnnotationProperty rdf:about="&terms;creator">
        <rdfs:label xml:lang="en">Creator</rdfs:label>
        <terms:issued rdf:datatype="&xsd;date">2008-01-14</terms:issued>
        <terms:modified rdf:datatype="&xsd;date">2010-10-11</terms:modified>
        <rdfs:comment xml:lang="en">An entity primarily responsible for making the resource.</rdfs:comment>
        <terms:description xml:lang="en">Examples of a Creator include a person, an organization, or a service.</terms:description>
        <terms:hasVersion rdf:resource="http://dublincore.org/usage/terms/history/#creatorT-002"/>
        <rdfs:subPropertyOf rdf:resource="&dc;creator"/>
        <rdfs:isDefinedBy rdf:resource="http://purl.org/dc/terms/"/>
        <rdfs:subPropertyOf rdf:resource="&terms;contributor"/>
    </owl:AnnotationProperty>
    <owl:AnnotationProperty rdf:about="&dc;publisher">
        <rdfs:label xml:lang="en">Publisher</rdfs:label>
        <terms:issued rdf:datatype="&xsd;date">1999-07-02</terms:issued>
        <terms:modified rdf:datatype="&xsd;date">2008-01-14</terms:modified>
        <skos:note xml:lang="en">A second property with the same name as this property has been declared in the dcterms: namespace (http://purl.org/dc/terms/).  See the Introduction to the document &quot;DCMI Metadata Terms&quot; (http://dublincore.org/documents/dcmi-terms/) for an explanation.</skos:note>
        <rdfs:comment xml:lang="en">An entity responsible for making the resource available.</rdfs:comment>
        <terms:description xml:lang="en">Examples of a Publisher include a person, an organization, or a service. Typically, the name of a Publisher should be used to indicate the entity.</terms:description>
        <terms:hasVersion rdf:resource="http://dublincore.org/usage/terms/history/#publisher-006"/>
        <rdfs:isDefinedBy rdf:resource="http://purl.org/dc/elements/1.1/"/>
    </owl:AnnotationProperty>
    <owl:AnnotationProperty rdf:about="&terms;alternative">
        <rdfs:subPropertyOf rdf:resource="&dc;title"/>
        <rdfs:subPropertyOf rdf:resource="&terms;title"/>
    </owl:AnnotationProperty>
    <owl:AnnotationProperty rdf:about="&terms;references">
        <rdfs:label xml:lang="en">References</rdfs:label>
        <terms:issued rdf:datatype="&xsd;date">2000-07-11</terms:issued>
        <terms:modified rdf:datatype="&xsd;date">2008-01-14</terms:modified>
        <rdfs:comment xml:lang="en">A related resource that is referenced, cited, or otherwise pointed to by the described resource.</rdfs:comment>
        <skos:note xml:lang="en">This term is intended to be used with non-literal values as defined in the DCMI Abstract Model (http://dublincore.org/documents/abstract-model/).  As of December 2007, the DCMI Usage Board is seeking a way to express this intention with a formal range declaration.</skos:note>
        <terms:hasVersion rdf:resource="http://dublincore.org/usage/terms/history/#references-003"/>
        <rdfs:subPropertyOf rdf:resource="&dc;relation"/>
        <rdfs:isDefinedBy rdf:resource="http://purl.org/dc/terms/"/>
        <rdfs:subPropertyOf rdf:resource="&terms;relation"/>
    </owl:AnnotationProperty>
    <owl:AnnotationProperty rdf:about="&dc;coverage">
        <rdfs:label xml:lang="en">Coverage</rdfs:label>
        <terms:issued rdf:datatype="&xsd;date">1999-07-02</terms:issued>
        <terms:modified rdf:datatype="&xsd;date">2008-01-14</terms:modified>
        <skos:note xml:lang="en">A second property with the same name as this property has been declared in the dcterms: namespace (http://purl.org/dc/terms/).  See the Introduction to the document &quot;DCMI Metadata Terms&quot; (http://dublincore.org/documents/dcmi-terms/) for an explanation.</skos:note>
        <terms:description xml:lang="en">Spatial topic and spatial applicability may be a named place or a location specified by its geographic coordinates. Temporal topic may be a named period, date, or date range. A jurisdiction may be a named administrative entity or a geographic place to which the resource applies. Recommended best practice is to use a controlled vocabulary such as the Thesaurus of Geographic Names [TGN]. Where appropriate, named places or time periods can be used in preference to numeric identifiers such as sets of coordinates or date ranges.</terms:description>
        <rdfs:comment xml:lang="en">The spatial or temporal topic of the resource, the spatial applicability of the resource, or the jurisdiction under which the resource is relevant.</rdfs:comment>
        <terms:hasVersion rdf:resource="http://dublincore.org/usage/terms/history/#coverage-006"/>
        <rdfs:isDefinedBy rdf:resource="http://purl.org/dc/elements/1.1/"/>
    </owl:AnnotationProperty>
    <owl:AnnotationProperty rdf:about="&skos;note">
        <rdfs:label xml:lang="en">note</rdfs:label>
        <skos:definition xml:lang="en">A general note, for any purpose.</skos:definition>
        <skos:scopeNote xml:lang="en">This property may be used directly, or as a super-property for more specific note types.</skos:scopeNote>
        <rdfs:isDefinedBy rdf:resource="http://www.w3.org/2004/02/skos/core"/>
    </owl:AnnotationProperty>
    <owl:AnnotationProperty rdf:about="&adms;status"/>
    


    <!-- 
    ///////////////////////////////////////////////////////////////////////////////////////
    //
    // Datatypes
    //
    ///////////////////////////////////////////////////////////////////////////////////////
     -->

    


    <!-- http://purl.org/dc/terms/Box -->

    <rdfs:Datatype rdf:about="&terms;Box">
        <rdfs:label xml:lang="en">DCMI Box</rdfs:label>
        <terms:issued rdf:datatype="&xsd;date">2000-07-11</terms:issued>
        <terms:modified rdf:datatype="&xsd;date">2008-01-14</terms:modified>
        <rdfs:comment xml:lang="en">The set of regions in space defined by their geographic coordinates according to the DCMI Box Encoding Scheme.</rdfs:comment>
        <rdfs:seeAlso rdf:resource="http://dublincore.org/documents/dcmi-box/"/>
        <terms:hasVersion rdf:resource="http://dublincore.org/usage/terms/history/#Box-003"/>
        <rdfs:isDefinedBy rdf:resource="http://purl.org/dc/terms/"/>
    </rdfs:Datatype>
    


    <!-- http://purl.org/dc/terms/ISO3166 -->

    <rdfs:Datatype rdf:about="&terms;ISO3166">
        <rdfs:label xml:lang="en">ISO 3166</rdfs:label>
        <terms:issued rdf:datatype="&xsd;date">2000-07-11</terms:issued>
        <terms:modified rdf:datatype="&xsd;date">2008-01-14</terms:modified>
        <rdfs:comment xml:lang="en">The set of codes listed in ISO 3166-1 for the representation of names of countries.</rdfs:comment>
        <terms:hasVersion rdf:resource="http://dublincore.org/usage/terms/history/#ISO3166-004"/>
        <rdfs:isDefinedBy rdf:resource="http://purl.org/dc/terms/"/>
        <rdfs:seeAlso rdf:resource="http://www.iso.org/iso/en/prods-services/iso3166ma/02iso-3166-code-lists/list-en1.html"/>
    </rdfs:Datatype>
    


    <!-- http://purl.org/dc/terms/ISO639-2 -->

    <rdfs:Datatype rdf:about="&terms;ISO639-2">
        <rdfs:label xml:lang="en">ISO 639-2</rdfs:label>
        <terms:issued rdf:datatype="&xsd;date">2000-07-11</terms:issued>
        <terms:modified rdf:datatype="&xsd;date">2008-01-14</terms:modified>
        <rdfs:comment xml:lang="en">The three-letter alphabetic codes listed in ISO639-2 for the representation of names of languages.</rdfs:comment>
        <terms:hasVersion rdf:resource="http://dublincore.org/usage/terms/history/#ISO639-2-003"/>
        <rdfs:seeAlso rdf:resource="http://lcweb.loc.gov/standards/iso639-2/langhome.html"/>
        <rdfs:isDefinedBy rdf:resource="http://purl.org/dc/terms/"/>
    </rdfs:Datatype>
    


    <!-- http://purl.org/dc/terms/ISO639-3 -->

    <rdfs:Datatype rdf:about="&terms;ISO639-3">
        <rdfs:label xml:lang="en">ISO 639-3</rdfs:label>
        <terms:issued rdf:datatype="&xsd;date">2008-01-14</terms:issued>
        <rdfs:comment xml:lang="en">The set of three-letter codes listed in ISO 639-3 for the representation of names of languages.</rdfs:comment>
        <terms:hasVersion rdf:resource="http://dublincore.org/usage/terms/history/#ISO639-3-001"/>
        <rdfs:isDefinedBy rdf:resource="http://purl.org/dc/terms/"/>
        <rdfs:seeAlso rdf:resource="http://www.sil.org/iso639-3/"/>
    </rdfs:Datatype>
    


    <!-- http://purl.org/dc/terms/Period -->

    <rdfs:Datatype rdf:about="&terms;Period">
        <rdfs:label xml:lang="en">DCMI Period</rdfs:label>
        <terms:issued rdf:datatype="&xsd;date">2000-07-11</terms:issued>
        <terms:modified rdf:datatype="&xsd;date">2008-01-14</terms:modified>
        <rdfs:comment xml:lang="en">The set of time intervals defined by their limits according to the DCMI Period Encoding Scheme.</rdfs:comment>
        <rdfs:seeAlso rdf:resource="http://dublincore.org/documents/dcmi-period/"/>
        <terms:hasVersion rdf:resource="http://dublincore.org/usage/terms/history/#Period-003"/>
        <rdfs:isDefinedBy rdf:resource="http://purl.org/dc/terms/"/>
    </rdfs:Datatype>
    


    <!-- http://purl.org/dc/terms/Point -->

    <rdfs:Datatype rdf:about="&terms;Point">
        <rdfs:label xml:lang="en">DCMI Point</rdfs:label>
        <terms:issued rdf:datatype="&xsd;date">2000-07-11</terms:issued>
        <terms:modified rdf:datatype="&xsd;date">2008-01-14</terms:modified>
        <rdfs:comment xml:lang="en">The set of points in space defined by their geographic coordinates according to the DCMI Point Encoding Scheme.</rdfs:comment>
        <rdfs:seeAlso rdf:resource="http://dublincore.org/documents/dcmi-point/"/>
        <terms:hasVersion rdf:resource="http://dublincore.org/usage/terms/history/#Point-003"/>
        <rdfs:isDefinedBy rdf:resource="http://purl.org/dc/terms/"/>
    </rdfs:Datatype>
    


    <!-- http://purl.org/dc/terms/RFC1766 -->

    <rdfs:Datatype rdf:about="&terms;RFC1766">
        <rdfs:label xml:lang="en">RFC 1766</rdfs:label>
        <terms:issued rdf:datatype="&xsd;date">2000-07-11</terms:issued>
        <terms:modified rdf:datatype="&xsd;date">2008-01-14</terms:modified>
        <rdfs:comment xml:lang="en">The set of tags, constructed according to RFC 1766, for the identification of languages.</rdfs:comment>
        <terms:hasVersion rdf:resource="http://dublincore.org/usage/terms/history/#RFC1766-003"/>
        <rdfs:isDefinedBy rdf:resource="http://purl.org/dc/terms/"/>
        <rdfs:seeAlso rdf:resource="http://www.ietf.org/rfc/rfc1766.txt"/>
    </rdfs:Datatype>
    


    <!-- http://purl.org/dc/terms/RFC3066 -->

    <rdfs:Datatype rdf:about="&terms;RFC3066">
        <rdfs:label xml:lang="en">RFC 3066</rdfs:label>
        <terms:issued rdf:datatype="&xsd;date">2002-07-13</terms:issued>
        <terms:modified rdf:datatype="&xsd;date">2008-01-14</terms:modified>
        <terms:description xml:lang="en">RFC 3066 has been obsoleted by RFC 4646.</terms:description>
        <rdfs:comment xml:lang="en">The set of tags constructed according to RFC 3066 for the identification of languages.</rdfs:comment>
        <terms:hasVersion rdf:resource="http://dublincore.org/usage/terms/history/#RFC3066-002"/>
        <rdfs:isDefinedBy rdf:resource="http://purl.org/dc/terms/"/>
        <rdfs:seeAlso rdf:resource="http://www.ietf.org/rfc/rfc3066.txt"/>
    </rdfs:Datatype>
    


    <!-- http://purl.org/dc/terms/RFC4646 -->

    <rdfs:Datatype rdf:about="&terms;RFC4646">
        <rdfs:label xml:lang="en">RFC 4646</rdfs:label>
        <terms:issued rdf:datatype="&xsd;date">2008-01-14</terms:issued>
        <terms:description xml:lang="en">RFC 4646 obsoletes RFC 3066.</terms:description>
        <rdfs:comment xml:lang="en">The set of tags constructed according to RFC 4646 for the identification of languages.</rdfs:comment>
        <terms:hasVersion rdf:resource="http://dublincore.org/usage/terms/history/#RFC4646-001"/>
        <rdfs:isDefinedBy rdf:resource="http://purl.org/dc/terms/"/>
        <rdfs:seeAlso rdf:resource="http://www.ietf.org/rfc/rfc4646.txt"/>
    </rdfs:Datatype>
    


    <!-- http://purl.org/dc/terms/RFC5646 -->

    <rdfs:Datatype rdf:about="&terms;RFC5646">
        <rdfs:label xml:lang="en">RFC 5646</rdfs:label>
        <terms:issued rdf:datatype="&xsd;date">2010-10-11</terms:issued>
        <terms:description xml:lang="en">RFC 5646 obsoletes RFC 4646.</terms:description>
        <rdfs:comment xml:lang="en">The set of tags constructed according to RFC 5646 for the identification of languages.</rdfs:comment>
        <terms:hasVersion rdf:resource="http://dublincore.org/usage/terms/history/#RFC5646-001"/>
        <rdfs:isDefinedBy rdf:resource="http://purl.org/dc/terms/"/>
        <rdfs:seeAlso rdf:resource="http://www.ietf.org/rfc/rfc5646.txt"/>
    </rdfs:Datatype>
    


    <!-- http://purl.org/dc/terms/URI -->

    <rdfs:Datatype rdf:about="&terms;URI">
        <rdfs:label xml:lang="en">URI</rdfs:label>
        <terms:issued rdf:datatype="&xsd;date">2000-07-11</terms:issued>
        <terms:modified rdf:datatype="&xsd;date">2008-01-14</terms:modified>
        <rdfs:comment xml:lang="en">The set of identifiers constructed according to the generic syntax for Uniform Resource Identifiers as specified by the Internet Engineering Task Force.</rdfs:comment>
        <terms:hasVersion rdf:resource="http://dublincore.org/usage/terms/history/#URI-003"/>
        <rdfs:isDefinedBy rdf:resource="http://purl.org/dc/terms/"/>
        <rdfs:seeAlso rdf:resource="http://www.ietf.org/rfc/rfc3986.txt"/>
    </rdfs:Datatype>
    


    <!-- http://purl.org/dc/terms/W3CDTF -->

    <rdfs:Datatype rdf:about="&terms;W3CDTF">
        <rdfs:label xml:lang="en">W3C-DTF</rdfs:label>
        <terms:issued rdf:datatype="&xsd;date">2000-07-11</terms:issued>
        <terms:modified rdf:datatype="&xsd;date">2008-01-14</terms:modified>
        <rdfs:comment xml:lang="en">The set of dates and times constructed according to the W3C Date and Time Formats Specification.</rdfs:comment>
        <terms:hasVersion rdf:resource="http://dublincore.org/usage/terms/history/#W3CDTF-003"/>
        <rdfs:isDefinedBy rdf:resource="http://purl.org/dc/terms/"/>
        <rdfs:seeAlso rdf:resource="http://www.w3.org/TR/NOTE-datetime"/>
    </rdfs:Datatype>
    


    <!-- http://www.opengis.net/ont/geosparql#gmlLiteral -->

    <rdfs:Datatype rdf:about="&geosparql;gmlLiteral">
        <rdfs:label xml:lang="en">GML Literal</rdfs:label>
        <dc:date rdf:datatype="&xsd;date">2011-06-16</dc:date>
        <dc:creator>OGC GeoSPARQL 1.0 Standard Working Group</dc:creator>
        <dc:contributor>Matthew Perry</dc:contributor>
        <dc:description xml:lang="en">
      A GML serialization of a geometry object.
    </dc:description>
        <skos:definition xml:lang="en">
      A GML serialization of a geometry object.
    </skos:definition>
        <rdfs:comment xml:lang="en">
      A GML serialization of a geometry object.
    </rdfs:comment>
        <skos:prefLabel xml:lang="en">GML Literal</skos:prefLabel>
        <rdfs:isDefinedBy rdf:resource="http://www.opengis.net/ont/geosparql"/>
        <rdfs:isDefinedBy rdf:resource="http://www.opengis.net/spec/geosparql/1.0"/>
    </rdfs:Datatype>
    


    <!-- http://www.opengis.net/ont/geosparql#wktLiteral -->

    <rdfs:Datatype rdf:about="&geosparql;wktLiteral">
        <rdfs:label xml:lang="en">Well-known Text Literal</rdfs:label>
        <dc:date rdf:datatype="&xsd;date">2011-06-16</dc:date>
        <dc:description xml:lang="en">
      A Well-known Text serialization of a geometry object.
    </dc:description>
        <skos:definition xml:lang="en">
      A Well-known Text serialization of a geometry object.
    </skos:definition>
        <rdfs:comment xml:lang="en">
      A Well-known Text serialization of a geometry object.
    </rdfs:comment>
        <dc:creator>OGC GeoSPARQL 1.0 Standard Working Group</dc:creator>
        <dc:contributor>Matthew Perry</dc:contributor>
        <skos:prefLabel xml:lang="en">Well-known Text Literal</skos:prefLabel>
        <rdfs:isDefinedBy rdf:resource="http://www.opengis.net/ont/geosparql"/>
        <rdfs:isDefinedBy rdf:resource="http://www.opengis.net/spec/geosparql/1.0"/>
    </rdfs:Datatype>
    


    <!-- http://www.w3.org/2001/XMLSchema#date -->

    <rdfs:Datatype rdf:about="&xsd;date"/>
    


    <!-- http://www.w3.org/2001/XMLSchema#gDay -->

    <rdfs:Datatype rdf:about="&xsd;gDay"/>
    


    <!-- http://www.w3.org/2001/XMLSchema#gMonth -->

    <rdfs:Datatype rdf:about="&xsd;gMonth"/>
    


    <!-- http://www.w3.org/2001/XMLSchema#gYear -->

    <rdfs:Datatype rdf:about="&xsd;gYear"/>
    


    <!-- 
    ///////////////////////////////////////////////////////////////////////////////////////
    //
    // Object Properties
    //
    ///////////////////////////////////////////////////////////////////////////////////////
     -->

    


    <!-- http://geo.linkeddata.es/ontology/parte_de -->

    <owl:ObjectProperty rdf:about="&ontology;parte_de"/>
    


    <!-- http://www.opengis.net/ont/geosparql#defaultGeometry -->

    <owl:ObjectProperty rdf:about="&geosparql;defaultGeometry">
        <rdfs:label xml:lang="en">defaultGeometry</rdfs:label>
        <dc:date rdf:datatype="&xsd;date">2011-06-16</dc:date>
        <dc:contributor>Matthew Perry</dc:contributor>
        <dc:creator>OGC GeoSPARQL 1.0 Standard Working Group</dc:creator>
        <skos:definition xml:lang="en">
      The default geometry to be used in spatial calculations.
      It is Usually the most detailed geometry.
    </skos:definition>
        <rdfs:comment xml:lang="en">
      The default geometry to be used in spatial calculations.
      It is Usually the most detailed geometry.
    </rdfs:comment>
        <dc:description xml:lang="en">
      The default geometry to be used in spatial calculations.
      It is Usually the most detailed geometry.
    </dc:description>
        <skos:prefLabel xml:lang="en">defaultGeometry</skos:prefLabel>
        <rdfs:isDefinedBy rdf:resource="http://www.opengis.net/ont/geosparql"/>
        <rdfs:domain rdf:resource="&geosparql;Feature"/>
        <rdfs:range rdf:resource="&geosparql;Geometry"/>
        <rdfs:subPropertyOf rdf:resource="&geosparql;hasGeometry"/>
        <rdfs:isDefinedBy rdf:resource="http://www.opengis.net/spec/geosparql/1.0"/>
    </owl:ObjectProperty>
    


    <!-- http://www.opengis.net/ont/geosparql#hasGeometry -->

    <owl:ObjectProperty rdf:about="&geosparql;hasGeometry">
        <rdfs:label xml:lang="en">hasGeometry</rdfs:label>
        <dc:date rdf:datatype="&xsd;date">2011-06-16</dc:date>
        <dc:contributor>Matthew Perry</dc:contributor>
        <dc:creator>OGC GeoSPARQL 1.0 Standard Working Group</dc:creator>
        <dc:description xml:lang="en">
      A spatial representation for a given feature.
    </dc:description>
        <skos:definition xml:lang="en">
      A spatial representation for a given feature.
    </skos:definition>
        <rdfs:comment xml:lang="en">
      A spatial representation for a given feature.
    </rdfs:comment>
        <skos:prefLabel xml:lang="en">hasGeometry</skos:prefLabel>
        <rdfs:isDefinedBy rdf:resource="http://www.opengis.net/ont/geosparql"/>
        <rdfs:domain rdf:resource="&geosparql;Feature"/>
        <rdfs:range rdf:resource="&geosparql;Geometry"/>
        <rdfs:isDefinedBy rdf:resource="http://www.opengis.net/spec/geosparql/1.0"/>
    </owl:ObjectProperty>
    


    <!-- 
    ///////////////////////////////////////////////////////////////////////////////////////
    //
    // Data properties
    //
    ///////////////////////////////////////////////////////////////////////////////////////
     -->

    


    <!-- http://geo.linkeddata.es/def/feature#OWLDataProperty_7fe078a6_48e8_40c9_a50c_536e433fea96 -->

    <owl:DatatypeProperty rdf:about="h&btn100;OWLDataProperty_7fe078a6_48e8_40c9_a50c_536e433fea96">
        <rdfs:label xml:lang="es">cota</rdfs:label>
        <rdfs:comment xml:lang="es">Altitud expresada en metros</rdfs:comment>
        <rdfs:range rdf:resource="&xsd;int"/>
        <rdfs:domain rdf:resource="&btn100;CurvaDeNivel"/>
        <rdfs:domain rdf:resource="&btn100;PuntoAcotado"/>
    </owl:DatatypeProperty>
    


    <!-- http://geo.linkeddata.es/def/feature#UNCode -->

    <owl:DatatypeProperty rdf:about="h&btn100;UNCode">
        <rdfs:label xml:lang="es">UNCode</rdfs:label>
        <rdfs:comment xml:lang="es">Código de localización de Naciones Unidas (United
Nations / Location CODE – UN/LOCODE)</rdfs:comment>
        <rdfs:domain rdf:resource="&ontology;Puerto"/>
        <rdfs:range>
            <rdfs:Datatype>
                <owl:onDatatype rdf:resource="&xsd;string"/>
                <owl:withRestrictions rdf:parseType="Collection">
                    <rdf:Description>
                        <xsd:length rdf:datatype="&xsd;integer">3</xsd:length>
                    </rdf:Description>
                </owl:withRestrictions>
            </rdfs:Datatype>
        </rdfs:range>
    </owl:DatatypeProperty>
    


    <!-- http://geo.linkeddata.es/def/feature#acceso -->

    <owl:DatatypeProperty rdf:about="h&btn100;acceso">
        <rdfs:label xml:lang="es">acceso</rdfs:label>
        <rdfs:comment xml:lang="es">Indica si una autovia es de acceso libre o de peaje.</rdfs:comment>
        <rdfs:domain rdf:resource="&ontology;Autopista"/>
        <rdfs:range>
            <rdfs:Datatype>
                <owl:oneOf>
                    <rdf:Description>
                        <rdf:type rdf:resource="&rdf;List"/>
                        <rdf:first rdf:datatype="&xsd;string">de peaje</rdf:first>
                        <rdf:rest>
                            <rdf:Description>
                                <rdf:type rdf:resource="&rdf;List"/>
                                <rdf:first rdf:datatype="&xsd;string">libre</rdf:first>
                                <rdf:rest rdf:resource="&rdf;nil"/>
                            </rdf:Description>
                        </rdf:rest>
                    </rdf:Description>
                </owl:oneOf>
            </rdfs:Datatype>
        </rdfs:range>
    </owl:DatatypeProperty>
    


    <!-- http://geo.linkeddata.es/def/feature#altitud -->

    <owl:DatatypeProperty rdf:about="h&btn100;altitud">
        <rdfs:label xml:lang="es">altitud</rdfs:label>
        <rdfs:comment xml:lang="es">altitud en metros</rdfs:comment>
        <rdfs:domain rdf:resource="&ontology;Aeropuerto"/>
        <rdfs:range rdf:resource="&xsd;int"/>
    </owl:DatatypeProperty>
    


    <!-- http://geo.linkeddata.es/def/feature#anchoDeVia -->

    <owl:DatatypeProperty rdf:about="h&btn100;anchoDeVia">
        <rdfs:label xml:lang="es">anchoDeVia</rdfs:label>
        <rdfs:domain rdf:resource="h&btn100;ViaDeFerrocarrilConvencional"/>
        <rdfs:range>
            <rdfs:Datatype>
                <owl:oneOf>
                    <rdf:Description>
                        <rdf:type rdf:resource="&rdf;List"/>
                        <rdf:first rdf:datatype="&xsd;string">desconocido</rdf:first>
                        <rdf:rest>
                            <rdf:Description>
                                <rdf:type rdf:resource="&rdf;List"/>
                                <rdf:first rdf:datatype="&xsd;string">ibérico</rdf:first>
                                <rdf:rest>
                                    <rdf:Description>
                                        <rdf:type rdf:resource="&rdf;List"/>
                                        <rdf:first rdf:datatype="&xsd;string">internacional</rdf:first>
                                        <rdf:rest>
                                            <rdf:Description>
                                                <rdf:type rdf:resource="&rdf;List"/>
                                                <rdf:first rdf:datatype="&xsd;string">mixto</rdf:first>
                                                <rdf:rest>
                                                    <rdf:Description>
                                                        <rdf:type rdf:resource="&rdf;List"/>
                                                        <rdf:first rdf:datatype="&xsd;string">métrico</rdf:first>
                                                        <rdf:rest rdf:resource="&rdf;nil"/>
                                                    </rdf:Description>
                                                </rdf:rest>
                                            </rdf:Description>
                                        </rdf:rest>
                                    </rdf:Description>
                                </rdf:rest>
                            </rdf:Description>
                        </rdf:rest>
                    </rdf:Description>
                </owl:oneOf>
            </rdfs:Datatype>
        </rdfs:range>
    </owl:DatatypeProperty>
    


    <!-- http://geo.linkeddata.es/def/feature#codificacionOficial -->

    <owl:DatatypeProperty rdf:about="h&btn100;codificacionOficial">
        <rdfs:label xml:lang="es">codificacionOficial</rdfs:label>
        <rdfs:comment xml:lang="es">refleja el valor del código INE en los municipios, y códigos arbitrarios consensuados para el resto de entidades</rdfs:comment>
        <rdfs:domain rdf:resource="h&btn100;UnidadAdministrativa"/>
        <rdfs:range>
            <rdfs:Datatype>
                <owl:onDatatype rdf:resource="&xsd;string"/>
                <owl:withRestrictions rdf:parseType="Collection">
                    <rdf:Description>
                        <xsd:length rdf:datatype="&xsd;integer">11</xsd:length>
                    </rdf:Description>
                </owl:withRestrictions>
            </rdfs:Datatype>
        </rdfs:range>
    </owl:DatatypeProperty>
    


    <!-- http://geo.linkeddata.es/def/feature#codigoBIC -->

    <owl:DatatypeProperty rdf:about="h&btn100;codigoBIC">
        <rdfs:label xml:lang="es">codigoBIC</rdfs:label>
        <rdfs:comment xml:lang="es"> código de identificación bancaria</rdfs:comment>
        <rdfs:domain rdf:resource="h&btn100;LugarDeInteres"/>
        <rdfs:range rdf:resource="&xsd;string"/>
    </owl:DatatypeProperty>
    


    <!-- http://geo.linkeddata.es/def/feature#codigoDeEstacion -->

    <owl:DatatypeProperty rdf:about="h&btn100;codigoDeEstacion">
        <rdfs:label xml:lang="es">codigoDeEstacion</rdfs:label>
        <rdfs:comment xml:lang="es">Código de la estación segun el administrador de Infraestructuras Ferroviarias (ADIF).</rdfs:comment>
        <rdfs:domain rdf:resource="h&btn100;InstalacionFerroviaria"/>
        <rdfs:range>
            <rdfs:Datatype>
                <owl:onDatatype rdf:resource="&xsd;string"/>
                <owl:withRestrictions rdf:parseType="Collection">
                    <rdf:Description>
                        <xsd:length rdf:datatype="&xsd;integer">6</xsd:length>
                    </rdf:Description>
                </owl:withRestrictions>
            </rdfs:Datatype>
        </rdfs:range>
    </owl:DatatypeProperty>
    


    <!-- http://geo.linkeddata.es/def/feature#codigoDeRio -->

    <owl:DatatypeProperty rdf:about="h&btn100;codigoDeRio">
        <rdfs:label xml:lang="es">codigoDeRio</rdfs:label>
        <rdfs:comment xml:lang="es">Codificación única para cada río de otros organismos </rdfs:comment>
        <rdfs:domain rdf:resource="h&btn100;Rio"/>
        <rdfs:range rdf:resource="&rdfs;Literal"/>
    </owl:DatatypeProperty>
    


    <!-- http://geo.linkeddata.es/def/feature#codigoDeVia -->

    <owl:DatatypeProperty rdf:about="h&btn100;codigoDeVia">
        <rdfs:label xml:lang="es">codigoDeVia</rdfs:label>
        <rdfs:comment xml:lang="es">Código de la vía segun el administrador de Infraestructuras Ferroviarias (ADIF)</rdfs:comment>
        <rdfs:domain rdf:resource="h&btn100;ViaDeFerrocarrilConvencional"/>
        <rdfs:domain rdf:resource="h&btn100;ViaDeFerrocarrilDeAltaVelocidad"/>
        <rdfs:range>
            <rdfs:Datatype>
                <owl:onDatatype rdf:resource="&xsd;string"/>
                <owl:withRestrictions rdf:parseType="Collection">
                    <rdf:Description>
                        <xsd:length rdf:datatype="&xsd;integer">6</xsd:length>
                    </rdf:Description>
                </owl:withRestrictions>
            </rdfs:Datatype>
        </rdfs:range>
    </owl:DatatypeProperty>
    


    <!-- http://geo.linkeddata.es/def/feature#codigoIATA -->

    <owl:DatatypeProperty rdf:about="h&btn100;codigoIATA">
        <rdfs:label xml:lang="es">codigoIATA</rdfs:label>
        <rdfs:comment xml:lang="es">Se especificará el código IATA a partir del Listado de Aeropuertos de AENA.</rdfs:comment>
        <rdfs:domain rdf:resource="&ontology;Aeropuerto"/>
        <rdfs:range>
            <rdfs:Datatype>
                <owl:onDatatype rdf:resource="&xsd;string"/>
                <owl:withRestrictions rdf:parseType="Collection">
                    <rdf:Description>
                        <xsd:length rdf:datatype="&xsd;integer">3</xsd:length>
                    </rdf:Description>
                </owl:withRestrictions>
            </rdfs:Datatype>
        </rdfs:range>
    </owl:DatatypeProperty>
    


    <!-- http://geo.linkeddata.es/def/feature#codigoICAO -->

    <owl:DatatypeProperty rdf:about="h&btn100;codigoICAO">
        <rdfs:label xml:lang="es">codigoICAO</rdfs:label>
        <rdfs:comment xml:lang="es">Se especificará el código IACO a partir del Listado de Aeropuertos de AENA.</rdfs:comment>
        <rdfs:domain rdf:resource="&ontology;Aeropuerto"/>
        <rdfs:range>
            <rdfs:Datatype>
                <owl:onDatatype rdf:resource="&xsd;string"/>
                <owl:withRestrictions rdf:parseType="Collection">
                    <rdf:Description>
                        <xsd:length rdf:datatype="&xsd;integer">5</xsd:length>
                    </rdf:Description>
                </owl:withRestrictions>
            </rdfs:Datatype>
        </rdfs:range>
    </owl:DatatypeProperty>
    


    <!-- http://geo.linkeddata.es/def/feature#codigoINE -->

    <owl:DatatypeProperty rdf:about="h&btn100;codigoINE">
        <rdfs:label xml:lang="es">codigoINE</rdfs:label>
        <scovo2:max xml:lang="es">Codificación asignada por el Nomenclátor del Instituto Nacional de Estadística (INE) del Ministerio de Economía y Hacienda.</scovo2:max>
        <rdfs:domain rdf:resource="h&btn100;Diseminado"/>
        <rdfs:domain rdf:resource="h&btn100;NucleoPoblacional"/>
        <rdfs:range rdf:resource="&xsd;string"/>
    </owl:DatatypeProperty>
    


    <!-- http://geo.linkeddata.es/def/feature#competencia -->

    <owl:DatatypeProperty rdf:about="h&btn100;competencia">
        <rdfs:label xml:lang="es">competencia</rdfs:label>
        <rdfs:comment xml:lang="es">Se indicará la competencia de la vía o carretera.
ESTATAL. La competencia es del Estado
AUTONÓMICA. La competencia es de la administración de las CCAA
PROVINCIAL. La competencia es de la Diputación Provincial
LOCAL. La competencia es del Municipio</rdfs:comment>
        <rdfs:domain rdf:resource="h&btn100;Autovia"/>
        <rdfs:domain rdf:resource="h&btn100;CarreteraAutonomica"/>
        <rdfs:domain rdf:resource="&ontology;Autopista"/>
        <rdfs:range>
            <rdfs:Datatype>
                <owl:oneOf>
                    <rdf:Description>
                        <rdf:type rdf:resource="&rdf;List"/>
                        <rdf:first rdf:datatype="&xsd;string">autonómica</rdf:first>
                        <rdf:rest>
                            <rdf:Description>
                                <rdf:type rdf:resource="&rdf;List"/>
                                <rdf:first rdf:datatype="&xsd;string">estatal</rdf:first>
                                <rdf:rest>
                                    <rdf:Description>
                                        <rdf:type rdf:resource="&rdf;List"/>
                                        <rdf:first rdf:datatype="&xsd;string">municipal</rdf:first>
                                        <rdf:rest>
                                            <rdf:Description>
                                                <rdf:type rdf:resource="&rdf;List"/>
                                                <rdf:first rdf:datatype="&xsd;string">provincial</rdf:first>
                                                <rdf:rest rdf:resource="&rdf;nil"/>
                                            </rdf:Description>
                                        </rdf:rest>
                                    </rdf:Description>
                                </rdf:rest>
                            </rdf:Description>
                        </rdf:rest>
                    </rdf:Description>
                </owl:oneOf>
            </rdfs:Datatype>
        </rdfs:range>
    </owl:DatatypeProperty>
    


    <!-- http://geo.linkeddata.es/def/feature#competenciaAeroportuaria -->

    <owl:DatatypeProperty rdf:about="h&btn100;competenciaAeroportuaria">
        <rdfs:label xml:lang="es">competenciaAeroportuaria</rdfs:label>
        <rdfs:domain rdf:resource="&ontology;Aeropuerto"/>
        <rdfs:range>
            <rdfs:Datatype>
                <owl:oneOf>
                    <rdf:Description>
                        <rdf:type rdf:resource="&rdf;List"/>
                        <rdf:first rdf:datatype="&xsd;string">Aena</rdf:first>
                        <rdf:rest>
                            <rdf:Description>
                                <rdf:type rdf:resource="&rdf;List"/>
                                <rdf:first rdf:datatype="&xsd;string">Militar</rdf:first>
                                <rdf:rest>
                                    <rdf:Description>
                                        <rdf:type rdf:resource="&rdf;List"/>
                                        <rdf:first rdf:datatype="&xsd;string">Privado</rdf:first>
                                        <rdf:rest rdf:resource="&rdf;nil"/>
                                    </rdf:Description>
                                </rdf:rest>
                            </rdf:Description>
                        </rdf:rest>
                    </rdf:Description>
                </owl:oneOf>
            </rdfs:Datatype>
        </rdfs:range>
    </owl:DatatypeProperty>
    


    <!-- http://geo.linkeddata.es/def/feature#competenciaExplotacionPortuaria -->

    <owl:DatatypeProperty rdf:about="h&btn100;competenciaExplotacionPortuaria">
        <rdfs:label xml:lang="es">competenciaExplotacionPortuaria</rdfs:label>
        <rdfs:domain rdf:resource="&ontology;Puerto"/>
        <rdfs:range>
            <rdfs:Datatype>
                <owl:oneOf>
                    <rdf:Description>
                        <rdf:type rdf:resource="&rdf;List"/>
                        <rdf:first rdf:datatype="&xsd;string">otros</rdf:first>
                        <rdf:rest>
                            <rdf:Description>
                                <rdf:type rdf:resource="&rdf;List"/>
                                <rdf:first rdf:datatype="&xsd;string">puerto del estado</rdf:first>
                                <rdf:rest rdf:resource="&rdf;nil"/>
                            </rdf:Description>
                        </rdf:rest>
                    </rdf:Description>
                </owl:oneOf>
            </rdfs:Datatype>
        </rdfs:range>
    </owl:DatatypeProperty>
    


    <!-- http://geo.linkeddata.es/def/feature#componente -->

    <owl:DatatypeProperty rdf:about="h&btn100;componente">
        <rdfs:label xml:lang="es">componente</rdfs:label>
        <rdfs:domain rdf:resource="h&btn100;EstacionTelecomunicaciones"/>
        <rdfs:range>
            <rdfs:Datatype>
                <owl:oneOf>
                    <rdf:Description>
                        <rdf:type rdf:resource="&rdf;List"/>
                        <rdf:first rdf:datatype="&xsd;string">desconocido</rdf:first>
                        <rdf:rest>
                            <rdf:Description>
                                <rdf:type rdf:resource="&rdf;List"/>
                                <rdf:first rdf:datatype="&xsd;string">emisor</rdf:first>
                                <rdf:rest>
                                    <rdf:Description>
                                        <rdf:type rdf:resource="&rdf;List"/>
                                        <rdf:first rdf:datatype="&xsd;string">repetidor</rdf:first>
                                        <rdf:rest rdf:resource="&rdf;nil"/>
                                    </rdf:Description>
                                </rdf:rest>
                            </rdf:Description>
                        </rdf:rest>
                    </rdf:Description>
                </owl:oneOf>
            </rdfs:Datatype>
        </rdfs:range>
    </owl:DatatypeProperty>
    


    <!-- http://geo.linkeddata.es/def/feature#eje -->

    <owl:DatatypeProperty rdf:about="h&btn100;eje">
        <rdfs:label xml:lang="es">eje</rdfs:label>
        <rdfs:comment xml:lang="es">Define si el rio tiene un eje de cauce o un eje ficticio</rdfs:comment>
        <rdfs:domain rdf:resource="h&btn100;RioLineal"/>
        <rdfs:range>
            <rdfs:Datatype>
                <owl:oneOf>
                    <rdf:Description>
                        <rdf:type rdf:resource="&rdf;List"/>
                        <rdf:first rdf:datatype="&xsd;string">conexión (eje ficticio establecido para conexión en zonas hidrográficas
superficiales)</rdf:first>
                        <rdf:rest>
                            <rdf:Description>
                                <rdf:type rdf:resource="&rdf;List"/>
                                <rdf:first rdf:datatype="&xsd;string">eje de cauce)</rdf:first>
                                <rdf:rest rdf:resource="&rdf;nil"/>
                            </rdf:Description>
                        </rdf:rest>
                    </rdf:Description>
                </owl:oneOf>
            </rdfs:Datatype>
        </rdfs:range>
    </owl:DatatypeProperty>
    


    <!-- http://geo.linkeddata.es/def/feature#electrificacion -->

    <owl:DatatypeProperty rdf:about="h&btn100;electrificacion">
        <rdfs:label xml:lang="es">electrificacion</rdfs:label>
        <rdfs:comment xml:lang="es">Indica si la via esta o no electrificada.</rdfs:comment>
        <rdfs:domain rdf:resource="h&btn100;ViaDeFerrocarrilConvencional"/>
        <rdfs:range>
            <rdfs:Datatype>
                <owl:oneOf>
                    <rdf:Description>
                        <rdf:type rdf:resource="&rdf;List"/>
                        <rdf:first rdf:datatype="&xsd;string">desconocido</rdf:first>
                        <rdf:rest>
                            <rdf:Description>
                                <rdf:type rdf:resource="&rdf;List"/>
                                <rdf:first rdf:datatype="&xsd;string">electrificada</rdf:first>
                                <rdf:rest>
                                    <rdf:Description>
                                        <rdf:type rdf:resource="&rdf;List"/>
                                        <rdf:first rdf:datatype="&xsd;string">no electrificada</rdf:first>
                                        <rdf:rest rdf:resource="&rdf;nil"/>
                                    </rdf:Description>
                                </rdf:rest>
                            </rdf:Description>
                        </rdf:rest>
                    </rdf:Description>
                </owl:oneOf>
            </rdfs:Datatype>
        </rdfs:range>
    </owl:DatatypeProperty>
    


    <!-- http://geo.linkeddata.es/def/feature#estado -->

    <owl:DatatypeProperty rdf:about="h&btn100;estado">
        <rdfs:label xml:lang="es">estado</rdfs:label>
        <rdfs:domain rdf:resource="h&btn100;Autovia"/>
        <rdfs:domain rdf:resource="h&btn100;Enlace"/>
        <rdfs:domain rdf:resource="h&btn100;ExplotacionMinera"/>
        <rdfs:domain rdf:resource="h&btn100;ViaDeFerrocarrilConvencional"/>
        <rdfs:domain rdf:resource="h&btn100;ViaDeFerrocarrilDeAltaVelocidad"/>
        <rdfs:domain rdf:resource="&ontology;Autopista"/>
        <rdfs:domain rdf:resource="&ontology;Carretera"/>
        <rdfs:domain rdf:resource="&ontology;Puerto"/>
        <rdfs:range>
            <rdfs:Datatype>
                <owl:oneOf>
                    <rdf:Description>
                        <rdf:type rdf:resource="&rdf;List"/>
                        <rdf:first rdf:datatype="&xsd;string">abandonado</rdf:first>
                        <rdf:rest>
                            <rdf:Description>
                                <rdf:type rdf:resource="&rdf;List"/>
                                <rdf:first rdf:datatype="&xsd;string">en construcción</rdf:first>
                                <rdf:rest>
                                    <rdf:Description>
                                        <rdf:type rdf:resource="&rdf;List"/>
                                        <rdf:first rdf:datatype="&xsd;string">en uso</rdf:first>
                                        <rdf:rest rdf:resource="&rdf;nil"/>
                                    </rdf:Description>
                                </rdf:rest>
                            </rdf:Description>
                        </rdf:rest>
                    </rdf:Description>
                </owl:oneOf>
            </rdfs:Datatype>
        </rdfs:range>
    </owl:DatatypeProperty>
    


    <!-- http://geo.linkeddata.es/def/feature#grupoTematico -->

    <owl:DatatypeProperty rdf:about="h&btn100;grupoTematico">
        <rdfs:label xml:lang="es">grupoTematico</rdfs:label>
        <rdfs:domain rdf:resource="h&btn100;UnidadAdministrativa"/>
        <rdfs:domain rdf:resource="h&btn100;ZonaProtegida"/>
        <rdfs:range>
            <rdfs:Datatype>
                <owl:oneOf>
                    <rdf:Description>
                        <rdf:type rdf:resource="&rdf;List"/>
                        <rdf:first rdf:datatype="&xsd;string">Conducciones y energía</rdf:first>
                        <rdf:rest>
                            <rdf:Description>
                                <rdf:type rdf:resource="&rdf;List"/>
                                <rdf:first rdf:datatype="&xsd;string">Hidrografía</rdf:first>
                                <rdf:rest>
                                    <rdf:Description>
                                        <rdf:type rdf:resource="&rdf;List"/>
                                        <rdf:first rdf:datatype="&xsd;string">Poblaciones y construcciones</rdf:first>
                                        <rdf:rest>
                                            <rdf:Description>
                                                <rdf:type rdf:resource="&rdf;List"/>
                                                <rdf:first rdf:datatype="&xsd;string">Puntos de Control</rdf:first>
                                                <rdf:rest>
                                                    <rdf:Description>
                                                        <rdf:type rdf:resource="&rdf;List"/>
                                                        <rdf:first rdf:datatype="&xsd;string">Relieve</rdf:first>
                                                        <rdf:rest>
                                                            <rdf:Description>
                                                                <rdf:type rdf:resource="&rdf;List"/>
                                                                <rdf:first rdf:datatype="&xsd;string">Transportes</rdf:first>
                                                                <rdf:rest>
                                                                    <rdf:Description>
                                                                        <rdf:type rdf:resource="&rdf;List"/>
                                                                        <rdf:first rdf:datatype="&xsd;string">Unidades administrativas y zonas protegidas</rdf:first>
                                                                        <rdf:rest rdf:resource="&rdf;nil"/>
                                                                    </rdf:Description>
                                                                </rdf:rest>
                                                            </rdf:Description>
                                                        </rdf:rest>
                                                    </rdf:Description>
                                                </rdf:rest>
                                            </rdf:Description>
                                        </rdf:rest>
                                    </rdf:Description>
                                </rdf:rest>
                            </rdf:Description>
                        </rdf:rest>
                    </rdf:Description>
                </owl:oneOf>
            </rdfs:Datatype>
        </rdfs:range>
    </owl:DatatypeProperty>
    


    <!-- http://geo.linkeddata.es/def/feature#importanciaCartografica -->

    <owl:DatatypeProperty rdf:about="h&btn100;importanciaCartografica">
        <rdfs:label xml:lang="es">importanciaCartografica</rdfs:label>
        <rdfs:domain rdf:resource="h&btn100;Isla"/>
        <rdfs:range>
            <rdfs:Datatype>
                <owl:oneOf>
                    <rdf:Description>
                        <rdf:type rdf:resource="&rdf;List"/>
                        <rdf:first rdf:datatype="&xsd;string">importante</rdf:first>
                        <rdf:rest>
                            <rdf:Description>
                                <rdf:type rdf:resource="&rdf;List"/>
                                <rdf:first rdf:datatype="&xsd;string">no definida</rdf:first>
                                <rdf:rest rdf:resource="&rdf;nil"/>
                            </rdf:Description>
                        </rdf:rest>
                    </rdf:Description>
                </owl:oneOf>
            </rdfs:Datatype>
        </rdfs:range>
    </owl:DatatypeProperty>
    


    <!-- http://geo.linkeddata.es/def/feature#itinerarioEuropeo -->

    <owl:DatatypeProperty rdf:about="h&btn100;itinerarioEuropeo">
        <rdfs:label xml:lang="es">itinerarioEuropeo</rdfs:label>
        <rdfs:comment xml:lang="es">Indica si el tramo perteneciente a la Red de Carreteras Europeas</rdfs:comment>
        <rdfs:domain rdf:resource="h&btn100;Autovia"/>
        <rdfs:domain rdf:resource="&ontology;Autopista"/>
        <rdfs:domain rdf:resource="&ontology;Carretera"/>
        <rdfs:range>
            <rdfs:Datatype>
                <owl:oneOf>
                    <rdf:Description>
                        <rdf:type rdf:resource="&rdf;List"/>
                        <rdf:first rdf:datatype="&xsd;string">itinerario europeo</rdf:first>
                        <rdf:rest>
                            <rdf:Description>
                                <rdf:type rdf:resource="&rdf;List"/>
                                <rdf:first rdf:datatype="&xsd;string">itinerario no europeo</rdf:first>
                                <rdf:rest rdf:resource="&rdf;nil"/>
                            </rdf:Description>
                        </rdf:rest>
                    </rdf:Description>
                </owl:oneOf>
            </rdfs:Datatype>
        </rdfs:range>
    </owl:DatatypeProperty>
    


    <!-- http://geo.linkeddata.es/def/feature#numeroDeVias -->

    <owl:DatatypeProperty rdf:about="h&btn100;numeroDeVias">
        <rdfs:label xml:lang="es">numeroDeVias</rdfs:label>
        <rdfs:comment xml:lang="es">Se indicará si, según la base de datos de ferrocarriles, es de vía simple o doble. En caso de que sea triple se capturará como una doble y una simple. En caso de que sea cuádruple se capturará como dos dobles.</rdfs:comment>
        <rdfs:domain rdf:resource="h&btn100;ViaDeFerrocarrilConvencional"/>
        <rdfs:range>
            <rdfs:Datatype>
                <owl:oneOf>
                    <rdf:Description>
                        <rdf:type rdf:resource="&rdf;List"/>
                        <rdf:first rdf:datatype="&xsd;string">desconocido</rdf:first>
                        <rdf:rest>
                            <rdf:Description>
                                <rdf:type rdf:resource="&rdf;List"/>
                                <rdf:first rdf:datatype="&xsd;string">doble (una via para cada sentido)</rdf:first>
                                <rdf:rest>
                                    <rdf:Description>
                                        <rdf:type rdf:resource="&rdf;List"/>
                                        <rdf:first rdf:datatype="&xsd;string">única (via de doble sentido)</rdf:first>
                                        <rdf:rest rdf:resource="&rdf;nil"/>
                                    </rdf:Description>
                                </rdf:rest>
                            </rdf:Description>
                        </rdf:rest>
                    </rdf:Description>
                </owl:oneOf>
            </rdfs:Datatype>
        </rdfs:range>
    </owl:DatatypeProperty>
    


    <!-- http://geo.linkeddata.es/def/feature#ordenDeImportancia -->

    <owl:DatatypeProperty rdf:about="h&btn100;ordenDeImportancia">
        <rdfs:label xml:lang="es">ordenDeImportancia</rdfs:label>
        <rdfs:comment xml:lang="es">Se indicará la categoría de la carretera segun su importancia.</rdfs:comment>
        <rdfs:domain rdf:resource="h&btn100;CarreteraAutonomica"/>
        <rdfs:range>
            <rdfs:Datatype>
                <owl:oneOf>
                    <rdf:Description>
                        <rdf:type rdf:resource="&rdf;List"/>
                        <rdf:first rdf:datatype="&xsd;string">no definido</rdf:first>
                        <rdf:rest>
                            <rdf:Description>
                                <rdf:type rdf:resource="&rdf;List"/>
                                <rdf:first rdf:datatype="&xsd;string">primer orden</rdf:first>
                                <rdf:rest>
                                    <rdf:Description>
                                        <rdf:type rdf:resource="&rdf;List"/>
                                        <rdf:first rdf:datatype="&xsd;string">segundo orden</rdf:first>
                                        <rdf:rest>
                                            <rdf:Description>
                                                <rdf:type rdf:resource="&rdf;List"/>
                                                <rdf:first rdf:datatype="&xsd;string">tercer orden</rdf:first>
                                                <rdf:rest rdf:resource="&rdf;nil"/>
                                            </rdf:Description>
                                        </rdf:rest>
                                    </rdf:Description>
                                </rdf:rest>
                            </rdf:Description>
                        </rdf:rest>
                    </rdf:Description>
                </owl:oneOf>
            </rdfs:Datatype>
        </rdfs:range>
    </owl:DatatypeProperty>
    


    <!-- http://geo.linkeddata.es/def/feature#ordenDeInteres -->

    <owl:DatatypeProperty rdf:about="h&btn100;ordenDeInteres">
        <rdfs:label xml:lang="es">ordenDeInteres</rdfs:label>
        <rdfs:comment xml:lang="es">Define el orden de interes de un rio.</rdfs:comment>
        <rdfs:domain rdf:resource="h&btn100;Rio"/>
        <rdfs:range>
            <rdfs:Datatype>
                <owl:oneOf>
                    <rdf:Description>
                        <rdf:type rdf:resource="&rdf;List"/>
                        <rdf:first rdf:datatype="&xsd;string">río de interés no definido</rdf:first>
                        <rdf:rest>
                            <rdf:Description>
                                <rdf:type rdf:resource="&rdf;List"/>
                                <rdf:first rdf:datatype="&xsd;string">río de interés principal</rdf:first>
                                <rdf:rest>
                                    <rdf:Description>
                                        <rdf:type rdf:resource="&rdf;List"/>
                                        <rdf:first rdf:datatype="&xsd;string">río de interés secundario</rdf:first>
                                        <rdf:rest>
                                            <rdf:Description>
                                                <rdf:type rdf:resource="&rdf;List"/>
                                                <rdf:first rdf:datatype="&xsd;string">río de interés terciario</rdf:first>
                                                <rdf:rest>
                                                    <rdf:Description>
                                                        <rdf:type rdf:resource="&rdf;List"/>
                                                        <rdf:first rdf:datatype="&xsd;string">río de menor interés</rdf:first>
                                                        <rdf:rest rdf:resource="&rdf;nil"/>
                                                    </rdf:Description>
                                                </rdf:rest>
                                            </rdf:Description>
                                        </rdf:rest>
                                    </rdf:Description>
                                </rdf:rest>
                            </rdf:Description>
                        </rdf:rest>
                    </rdf:Description>
                </owl:oneOf>
            </rdfs:Datatype>
        </rdfs:range>
    </owl:DatatypeProperty>
    


    <!-- http://geo.linkeddata.es/def/feature#poblacion -->

    <owl:DatatypeProperty rdf:about="h&btn100;poblacion">
        <rdfs:label xml:lang="es">poblacion</rdfs:label>
        <rdfs:comment xml:lang="es">Número total de habitantes del núcleo según el nomenclátor del Instituto Nacional de Estadística (INE) del Ministerio de Economía y Hacienda. para el año que aparezca en los metadatos.</rdfs:comment>
        <rdfs:domain rdf:resource="h&btn100;NucleoPoblacional"/>
        <rdfs:range rdf:resource="&xsd;int"/>
    </owl:DatatypeProperty>
    


    <!-- http://geo.linkeddata.es/def/feature#producto -->

    <owl:DatatypeProperty rdf:about="h&btn100;producto">
        <rdfs:label xml:lang="es">producto</rdfs:label>
        <rdfs:comment xml:lang="es">Producto de origen o fuente de información</rdfs:comment>
        <rdfs:domain rdf:resource="h&btn100;AccidenteMaritimoLineal"/>
        <rdfs:domain rdf:resource="h&btn100;AccidenteMaritimoPuntual"/>
        <rdfs:domain rdf:resource="&ontology;Mar"/>
        <rdfs:domain rdf:resource="&ontology;Oceano"/>
        <rdfs:domain rdf:resource="&btn100;EntidadVirtualDeAccidenteOrografico"/>
        <rdfs:range>
            <rdfs:Datatype>
                <owl:oneOf>
                    <rdf:Description>
                        <rdf:type rdf:resource="&rdf;List"/>
                        <rdf:first rdf:datatype="&xsd;string">MP200</rdf:first>
                        <rdf:rest>
                            <rdf:Description>
                                <rdf:type rdf:resource="&rdf;List"/>
                                <rdf:first rdf:datatype="&xsd;string">MP200 y SERIE C</rdf:first>
                                <rdf:rest>
                                    <rdf:Description>
                                        <rdf:type rdf:resource="&rdf;List"/>
                                        <rdf:first rdf:datatype="&xsd;string">SERIE C</rdf:first>
                                        <rdf:rest rdf:resource="&rdf;nil"/>
                                    </rdf:Description>
                                </rdf:rest>
                            </rdf:Description>
                        </rdf:rest>
                    </rdf:Description>
                </owl:oneOf>
            </rdfs:Datatype>
        </rdfs:range>
    </owl:DatatypeProperty>
    


    <!-- http://geo.linkeddata.es/def/feature#regimen -->

    <owl:DatatypeProperty rdf:about="h&btn100;regimen">
        <rdfs:label xml:lang="es">regimen</rdfs:label>
        <rdfs:comment xml:lang="es">Estacionalidad de las aguas en cauce</rdfs:comment>
        <rdfs:domain rdf:resource="h&btn100;RioLineal"/>
        <rdfs:domain rdf:resource="&ontology;Laguna"/>
        <rdfs:range>
            <rdfs:Datatype>
                <owl:oneOf>
                    <rdf:Description>
                        <rdf:type rdf:resource="&rdf;List"/>
                        <rdf:first rdf:datatype="&xsd;string">no permanente (agua variable dependiendo de estacionalidad)</rdf:first>
                        <rdf:rest>
                            <rdf:Description>
                                <rdf:type rdf:resource="&rdf;List"/>
                                <rdf:first rdf:datatype="&xsd;string">permanente (discurre agua durante todo el año)</rdf:first>
                                <rdf:rest rdf:resource="&rdf;nil"/>
                            </rdf:Description>
                        </rdf:rest>
                    </rdf:Description>
                </owl:oneOf>
            </rdfs:Datatype>
        </rdfs:range>
    </owl:DatatypeProperty>
    


    <!-- http://geo.linkeddata.es/def/feature#rutaTEN-T -->

    <owl:DatatypeProperty rdf:about="h&btn100;rutaTEN-T">
        <rdfs:label xml:lang="es">rutaTEN-T</rdfs:label>
        <rdfs:comment xml:lang="es">Indica si la via pertenece a la Red Transeuropea de Transporte (TEN-T)</rdfs:comment>
        <rdfs:domain rdf:resource="h&btn100;Autovia"/>
        <rdfs:domain rdf:resource="h&btn100;ViaDeFerrocarrilConvencional"/>
        <rdfs:domain rdf:resource="h&btn100;ViaDeFerrocarrilDeAltaVelocidad"/>
        <rdfs:domain rdf:resource="&ontology;Aeropuerto"/>
        <rdfs:domain rdf:resource="&ontology;Autopista"/>
        <rdfs:domain rdf:resource="&ontology;Carretera"/>
        <rdfs:range>
            <rdfs:Datatype>
                <owl:oneOf>
                    <rdf:Description>
                        <rdf:type rdf:resource="&rdf;List"/>
                        <rdf:first rdf:datatype="&xsd;string">no pertenece a ruta TEN-T</rdf:first>
                        <rdf:rest>
                            <rdf:Description>
                                <rdf:type rdf:resource="&rdf;List"/>
                                <rdf:first rdf:datatype="&xsd;string">ruta TEN-T</rdf:first>
                                <rdf:rest rdf:resource="&rdf;nil"/>
                            </rdf:Description>
                        </rdf:rest>
                    </rdf:Description>
                </owl:oneOf>
            </rdfs:Datatype>
        </rdfs:range>
    </owl:DatatypeProperty>
    


    <!-- http://geo.linkeddata.es/def/feature#situadoEnLugarDeInteres -->

    <owl:DatatypeProperty rdf:about="h&btn100;situadoEnLugarDeInteres">
        <rdfs:label xml:lang="es">situadoEnLugarDeInteres</rdfs:label>
        <rdfs:domain rdf:resource="&btn100;EntidadVirtualDeAccidenteOrografico"/>
        <rdfs:range>
            <rdfs:Datatype>
                <owl:oneOf>
                    <rdf:Description>
                        <rdf:type rdf:resource="&rdf;List"/>
                        <rdf:first rdf:datatype="&xsd;string">Interés no definido</rdf:first>
                        <rdf:rest>
                            <rdf:Description>
                                <rdf:type rdf:resource="&rdf;List"/>
                                <rdf:first rdf:datatype="&xsd;string">Lugar de interés principal</rdf:first>
                                <rdf:rest>
                                    <rdf:Description>
                                        <rdf:type rdf:resource="&rdf;List"/>
                                        <rdf:first rdf:datatype="&xsd;string">Lugar de interés secundario</rdf:first>
                                        <rdf:rest>
                                            <rdf:Description>
                                                <rdf:type rdf:resource="&rdf;List"/>
                                                <rdf:first rdf:datatype="&xsd;string">Lugar de interés terciario</rdf:first>
                                                <rdf:rest>
                                                    <rdf:Description>
                                                        <rdf:type rdf:resource="&rdf;List"/>
                                                        <rdf:first rdf:datatype="&xsd;string">Lugar de menor interés</rdf:first>
                                                        <rdf:rest rdf:resource="&rdf;nil"/>
                                                    </rdf:Description>
                                                </rdf:rest>
                                            </rdf:Description>
                                        </rdf:rest>
                                    </rdf:Description>
                                </rdf:rest>
                            </rdf:Description>
                        </rdf:rest>
                    </rdf:Description>
                </owl:oneOf>
            </rdfs:Datatype>
        </rdfs:range>
    </owl:DatatypeProperty>
    


    <!-- http://geo.linkeddata.es/def/feature#tipoDeCalzada -->

    <owl:DatatypeProperty rdf:about="h&btn100;tipoDeCalzada">
        <rdfs:label xml:lang="es">tipoDeCalzada</rdfs:label>
        <rdfs:comment xml:lang="es">Indicará el número de calzadas y sentido de circulación para el tramo de carretera.</rdfs:comment>
        <rdfs:domain rdf:resource="h&btn100;Autovia"/>
        <rdfs:domain rdf:resource="&ontology;Autopista"/>
        <rdfs:domain rdf:resource="&ontology;Carretera"/>
        <rdfs:range>
            <rdfs:Datatype>
                <owl:oneOf>
                    <rdf:Description>
                        <rdf:type rdf:resource="&rdf;List"/>
                        <rdf:first rdf:datatype="&xsd;string">convencional</rdf:first>
                        <rdf:rest>
                            <rdf:Description>
                                <rdf:type rdf:resource="&rdf;List"/>
                                <rdf:first rdf:datatype="&xsd;string">doble</rdf:first>
                                <rdf:rest>
                                    <rdf:Description>
                                        <rdf:type rdf:resource="&rdf;List"/>
                                        <rdf:first rdf:datatype="&xsd;string">sentido único</rdf:first>
                                        <rdf:rest rdf:resource="&rdf;nil"/>
                                    </rdf:Description>
                                </rdf:rest>
                            </rdf:Description>
                        </rdf:rest>
                    </rdf:Description>
                </owl:oneOf>
            </rdfs:Datatype>
        </rdfs:range>
    </owl:DatatypeProperty>
    


    <!-- http://geo.linkeddata.es/def/feature#tipoDeCapital -->

    <owl:DatatypeProperty rdf:about="h&btn100;tipoDeCapital">
        <rdfs:label xml:lang="es">tipoDeCapital</rdfs:label>
        <rdfs:comment xml:lang="es">Especifica el tipo de capital que es el núcleo de población. Pudiendo ser capital de la nacion, capital de comunidad autónoma, capital de la CCAA pero no
de la provincia, capital de una provincia, capital de un municipio, o es capital.</rdfs:comment>
        <rdfs:domain rdf:resource="h&btn100;Diseminado"/>
        <rdfs:domain rdf:resource="h&btn100;NucleoPoblacional"/>
        <rdfs:range>
            <rdfs:Datatype>
                <owl:oneOf>
                    <rdf:Description>
                        <rdf:type rdf:resource="&rdf;List"/>
                        <rdf:first rdf:datatype="&xsd;string">capital de comunidad autónoma</rdf:first>
                        <rdf:rest>
                            <rdf:Description>
                                <rdf:type rdf:resource="&rdf;List"/>
                                <rdf:first rdf:datatype="&xsd;string">capital de comunidad autónoma pero no de provincia</rdf:first>
                                <rdf:rest>
                                    <rdf:Description>
                                        <rdf:type rdf:resource="&rdf;List"/>
                                        <rdf:first rdf:datatype="&xsd;string">capital de nacion</rdf:first>
                                        <rdf:rest>
                                            <rdf:Description>
                                                <rdf:type rdf:resource="&rdf;List"/>
                                                <rdf:first rdf:datatype="&xsd;string">capital de provincia</rdf:first>
                                                <rdf:rest>
                                                    <rdf:Description>
                                                        <rdf:type rdf:resource="&rdf;List"/>
                                                        <rdf:first rdf:datatype="&xsd;string">capital de un municipio</rdf:first>
                                                        <rdf:rest>
                                                            <rdf:Description>
                                                                <rdf:type rdf:resource="&rdf;List"/>
                                                                <rdf:first rdf:datatype="&xsd;string">no es capital</rdf:first>
                                                                <rdf:rest rdf:resource="&rdf;nil"/>
                                                            </rdf:Description>
                                                        </rdf:rest>
                                                    </rdf:Description>
                                                </rdf:rest>
                                            </rdf:Description>
                                        </rdf:rest>
                                    </rdf:Description>
                                </rdf:rest>
                            </rdf:Description>
                        </rdf:rest>
                    </rdf:Description>
                </owl:oneOf>
            </rdfs:Datatype>
        </rdfs:range>
    </owl:DatatypeProperty>
    


    <!-- http://geo.linkeddata.es/def/feature#tipoDeGeometria -->

    <owl:DatatypeProperty rdf:about="h&btn100;tipoDeGeometria">
        <rdfs:label xml:lang="es">tipoDeGeometria</rdfs:label>
        <rdfs:domain rdf:resource="h&btn100;UnidadAdministrativa"/>
        <rdfs:domain rdf:resource="h&btn100;ZonaProtegida"/>
        <rdfs:range>
            <rdfs:Datatype>
                <owl:oneOf>
                    <rdf:Description>
                        <rdf:type rdf:resource="&rdf;List"/>
                        <rdf:first rdf:datatype="&xsd;string">Lineal</rdf:first>
                        <rdf:rest>
                            <rdf:Description>
                                <rdf:type rdf:resource="&rdf;List"/>
                                <rdf:first rdf:datatype="&xsd;string">Puntual</rdf:first>
                                <rdf:rest>
                                    <rdf:Description>
                                        <rdf:type rdf:resource="&rdf;List"/>
                                        <rdf:first rdf:datatype="&xsd;string">Superficial</rdf:first>
                                        <rdf:rest rdf:resource="&rdf;nil"/>
                                    </rdf:Description>
                                </rdf:rest>
                            </rdf:Description>
                        </rdf:rest>
                    </rdf:Description>
                </owl:oneOf>
            </rdfs:Datatype>
        </rdfs:range>
    </owl:DatatypeProperty>
    


    <!-- http://geo.linkeddata.es/def/feature#tipoDeTramo -->

    <owl:DatatypeProperty rdf:about="h&btn100;tipoDeTramo">
        <rdfs:label xml:lang="es">tipoDeTramo</rdfs:label>
        <rdfs:comment xml:lang="es">Indica si el tramo de vía  se desarrolla por el interior o exterior de núcleos o diseminados superficiales</rdfs:comment>
        <rdfs:domain rdf:resource="h&btn100;Autovia"/>
        <rdfs:domain rdf:resource="&ontology;Autopista"/>
        <rdfs:domain rdf:resource="&ontology;Carretera"/>
        <rdfs:range>
            <rdfs:Datatype>
                <owl:oneOf>
                    <rdf:Description>
                        <rdf:type rdf:resource="&rdf;List"/>
                        <rdf:first rdf:datatype="&xsd;string">interna</rdf:first>
                        <rdf:rest>
                            <rdf:Description>
                                <rdf:type rdf:resource="&rdf;List"/>
                                <rdf:first rdf:datatype="&xsd;string">no interna</rdf:first>
                                <rdf:rest rdf:resource="&rdf;nil"/>
                            </rdf:Description>
                        </rdf:rest>
                    </rdf:Description>
                </owl:oneOf>
            </rdfs:Datatype>
        </rdfs:range>
    </owl:DatatypeProperty>
    


    <!-- http://geo.linkeddata.es/def/feature#tipoDeUso -->

    <owl:DatatypeProperty rdf:about="h&btn100;tipoDeUso">
        <rdfs:label xml:lang="es">tipoDeUso</rdfs:label>
        <rdfs:domain rdf:resource="h&btn100;InstalacionFerroviaria"/>
        <rdfs:range>
            <rdfs:Datatype>
                <owl:oneOf>
                    <rdf:Description>
                        <rdf:type rdf:resource="&rdf;List"/>
                        <rdf:first rdf:datatype="&xsd;string">apartadero</rdf:first>
                        <rdf:rest>
                            <rdf:Description>
                                <rdf:type rdf:resource="&rdf;List"/>
                                <rdf:first rdf:datatype="&xsd;string">apeadero</rdf:first>
                                <rdf:rest>
                                    <rdf:Description>
                                        <rdf:type rdf:resource="&rdf;List"/>
                                        <rdf:first rdf:datatype="&xsd;string">cargadero</rdf:first>
                                        <rdf:rest>
                                            <rdf:Description>
                                                <rdf:type rdf:resource="&rdf;List"/>
                                                <rdf:first rdf:datatype="&xsd;string">estación</rdf:first>
                                                <rdf:rest>
                                                    <rdf:Description>
                                                        <rdf:type rdf:resource="&rdf;List"/>
                                                        <rdf:first rdf:datatype="&xsd;string">suministro</rdf:first>
                                                        <rdf:rest rdf:resource="&rdf;nil"/>
                                                    </rdf:Description>
                                                </rdf:rest>
                                            </rdf:Description>
                                        </rdf:rest>
                                    </rdf:Description>
                                </rdf:rest>
                            </rdf:Description>
                        </rdf:rest>
                    </rdf:Description>
                </owl:oneOf>
            </rdfs:Datatype>
        </rdfs:range>
    </owl:DatatypeProperty>
    


    <!-- http://geo.linkeddata.es/def/feature#trafico -->

    <owl:DatatypeProperty rdf:about="h&btn100;trafico">
        <rdfs:label xml:lang="es">trafico</rdfs:label>
        <rdfs:domain rdf:resource="h&btn100;InstalacionFerroviaria"/>
        <rdfs:domain rdf:resource="h&btn100;ViaDeFerrocarrilConvencional"/>
        <rdfs:range>
            <rdfs:Datatype>
                <owl:oneOf>
                    <rdf:Description>
                        <rdf:type rdf:resource="&rdf;List"/>
                        <rdf:first rdf:datatype="&xsd;string">desconocido</rdf:first>
                        <rdf:rest>
                            <rdf:Description>
                                <rdf:type rdf:resource="&rdf;List"/>
                                <rdf:first rdf:datatype="&xsd;string">mercancías</rdf:first>
                                <rdf:rest>
                                    <rdf:Description>
                                        <rdf:type rdf:resource="&rdf;List"/>
                                        <rdf:first rdf:datatype="&xsd;string">viajeros</rdf:first>
                                        <rdf:rest>
                                            <rdf:Description>
                                                <rdf:type rdf:resource="&rdf;List"/>
                                                <rdf:first rdf:datatype="&xsd;string">viajeros y mercancías</rdf:first>
                                                <rdf:rest rdf:resource="&rdf;nil"/>
                                            </rdf:Description>
                                        </rdf:rest>
                                    </rdf:Description>
                                </rdf:rest>
                            </rdf:Description>
                        </rdf:rest>
                    </rdf:Description>
                </owl:oneOf>
            </rdfs:Datatype>
        </rdfs:range>
    </owl:DatatypeProperty>
    


    <!-- http://geo.linkeddata.es/def/feature#tramo -->

    <owl:DatatypeProperty rdf:about="h&btn100;tramo">
        <rdfs:label xml:lang="es">tramo</rdfs:label>
        <rdfs:comment xml:lang="es">Tipología de tramo de rio</rdfs:comment>
        <rdfs:domain rdf:resource="h&btn100;RioLineal"/>
        <rdfs:range>
            <rdfs:Datatype>
                <owl:oneOf>
                    <rdf:Description>
                        <rdf:type rdf:resource="&rdf;List"/>
                        <rdf:first rdf:datatype="&xsd;string">Tramo no definido</rdf:first>
                        <rdf:rest>
                            <rdf:Description>
                                <rdf:type rdf:resource="&rdf;List"/>
                                <rdf:first rdf:datatype="&xsd;string">tramo alto (Tramo de rio aguas arriba cercano a la cabecera)</rdf:first>
                                <rdf:rest>
                                    <rdf:Description>
                                        <rdf:type rdf:resource="&rdf;List"/>
                                        <rdf:first rdf:datatype="&xsd;string">tramo bajo (Tramo de rio aguas abajo cercano a desembocadura)</rdf:first>
                                        <rdf:rest>
                                            <rdf:Description>
                                                <rdf:type rdf:resource="&rdf;List"/>
                                                <rdf:first rdf:datatype="&xsd;string">tramo medio (Tramo de rio discurre por zona intermedia) </rdf:first>
                                                <rdf:rest rdf:resource="&rdf;nil"/>
                                            </rdf:Description>
                                        </rdf:rest>
                                    </rdf:Description>
                                </rdf:rest>
                            </rdf:Description>
                        </rdf:rest>
                    </rdf:Description>
                </owl:oneOf>
            </rdfs:Datatype>
        </rdfs:range>
    </owl:DatatypeProperty>
    


    <!-- http://geo.linkeddata.es/ontology/situacion -->

    <owl:DatatypeProperty rdf:about="&ontology;situacion">
        <rdfs:domain rdf:resource="h&btn100;Autovia"/>
        <rdfs:domain rdf:resource="h&btn100;CauceArtificial"/>
        <rdfs:domain rdf:resource="h&btn100;ConduccionDeCombustible"/>
        <rdfs:domain rdf:resource="h&btn100;Enlace"/>
        <rdfs:domain rdf:resource="h&btn100;ViaDeFerrocarrilConvencional"/>
        <rdfs:domain rdf:resource="h&btn100;ViaDeFerrocarrilDeAltaVelocidad"/>
        <rdfs:domain rdf:resource="&ontology;Autopista"/>
        <rdfs:domain rdf:resource="&ontology;Carretera"/>
        <rdfs:range>
            <rdfs:Datatype>
                <owl:oneOf>
                    <rdf:Description>
                        <rdf:type rdf:resource="&rdf;List"/>
                        <rdf:first rdf:datatype="&xsd;string">elevado</rdf:first>
                        <rdf:rest>
                            <rdf:Description>
                                <rdf:type rdf:resource="&rdf;List"/>
                                <rdf:first rdf:datatype="&xsd;string">en superficie</rdf:first>
                                <rdf:rest>
                                    <rdf:Description>
                                        <rdf:type rdf:resource="&rdf;List"/>
                                        <rdf:first rdf:datatype="&xsd;string">sin clasificar</rdf:first>
                                        <rdf:rest>
                                            <rdf:Description>
                                                <rdf:type rdf:resource="&rdf;List"/>
                                                <rdf:first rdf:datatype="&xsd;string">subterraneo</rdf:first>
                                                <rdf:rest rdf:resource="&rdf;nil"/>
                                            </rdf:Description>
                                        </rdf:rest>
                                    </rdf:Description>
                                </rdf:rest>
                            </rdf:Description>
                        </rdf:rest>
                    </rdf:Description>
                </owl:oneOf>
            </rdfs:Datatype>
        </rdfs:range>
    </owl:DatatypeProperty>
    


    <!-- http://purl.org/dc/terms/created -->

    <owl:DatatypeProperty rdf:about="&terms;created">
        <rdfs:label xml:lang="en">Date Created</rdfs:label>
        <terms:issued rdf:datatype="&xsd;date">2000-07-11</terms:issued>
        <terms:modified rdf:datatype="&xsd;date">2008-01-14</terms:modified>
        <rdfs:comment xml:lang="en">Date of creation of the resource.</rdfs:comment>
        <terms:hasVersion rdf:resource="http://dublincore.org/usage/terms/history/#created-003"/>
        <rdfs:isDefinedBy rdf:resource="http://purl.org/dc/terms/"/>
        <rdfs:range rdf:resource="&rdfs;Literal"/>
    </owl:DatatypeProperty>
    


    <!-- http://purl.org/dc/terms/identifier -->

    <owl:DatatypeProperty rdf:about="&terms;identifier">
        <rdfs:label xml:lang="en">Identifier</rdfs:label>
        <terms:issued rdf:datatype="&xsd;date">2008-01-14</terms:issued>
        <terms:modified rdf:datatype="&xsd;date">2008-01-14</terms:modified>
        <rdfs:comment xml:lang="en">An unambiguous reference to the resource within a given context.</rdfs:comment>
        <terms:description xml:lang="en">Recommended best practice is to identify the resource by means of a string conforming to a formal identification system. </terms:description>
        <terms:hasVersion rdf:resource="http://dublincore.org/usage/terms/history/#identifierT-001"/>
        <rdfs:isDefinedBy rdf:resource="http://purl.org/dc/terms/"/>
        <rdfs:range rdf:resource="&rdfs;Literal"/>
    </owl:DatatypeProperty>
    


    <!-- http://purl.org/dc/terms/replaces -->

    <owl:DatatypeProperty rdf:about="&terms;replaces">
        <rdfs:label xml:lang="en">Replaces</rdfs:label>
        <terms:issued rdf:datatype="&xsd;date">2000-07-11</terms:issued>
        <terms:modified rdf:datatype="&xsd;date">2008-01-14</terms:modified>
        <rdfs:comment xml:lang="en">A related resource that is supplanted, displaced, or superseded by the described resource.</rdfs:comment>
        <skos:note xml:lang="en">This term is intended to be used with non-literal values as defined in the DCMI Abstract Model (http://dublincore.org/documents/abstract-model/).  As of December 2007, the DCMI Usage Board is seeking a way to express this intention with a formal range declaration.</skos:note>
        <terms:hasVersion rdf:resource="http://dublincore.org/usage/terms/history/#replaces-003"/>
        <rdfs:isDefinedBy rdf:resource="http://purl.org/dc/terms/"/>
    </owl:DatatypeProperty>
    


    <!-- http://purl.org/dc/terms/title -->

    <owl:DatatypeProperty rdf:about="&terms;title">
        <rdfs:label xml:lang="en">Title</rdfs:label>
        <terms:issued rdf:datatype="&xsd;date">2008-01-14</terms:issued>
        <terms:modified rdf:datatype="&xsd;date">2010-10-11</terms:modified>
        <rdfs:comment xml:lang="en">A name given to the resource.</rdfs:comment>
        <terms:hasVersion rdf:resource="http://dublincore.org/usage/terms/history/#titleT-002"/>
        <rdfs:isDefinedBy rdf:resource="http://purl.org/dc/terms/"/>
        <rdfs:range rdf:resource="&rdfs;Literal"/>
    </owl:DatatypeProperty>
    


    <!-- http://www.opengis.net/ont/geosparql#asGML -->

    <owl:DatatypeProperty rdf:about="&geosparql;asGML">
        <rdfs:label xml:lang="en">asGML</rdfs:label>
        <dc:date rdf:datatype="&xsd;date">2011-06-16</dc:date>
        <dc:creator>OGC GeoSPARQL 1.0 Standard Working Group</dc:creator>
        <dc:description xml:lang="en">
      The GML serialization of a geometry
    </dc:description>
        <skos:definition xml:lang="en">
      The GML serialization of a geometry
    </skos:definition>
        <rdfs:comment xml:lang="en">
      The GML serialization of a geometry
    </rdfs:comment>
        <dc:contributor>Matthew Perry</dc:contributor>
        <skos:prefLabel xml:lang="en">asGML</skos:prefLabel>
        <rdfs:isDefinedBy rdf:resource="http://www.opengis.net/ont/geosparql"/>
        <rdfs:domain rdf:resource="&geosparql;Geometry"/>
        <rdfs:range rdf:resource="&geosparql;gmlLiteral"/>
        <rdfs:subPropertyOf rdf:resource="&geosparql;hasSerialization"/>
        <rdfs:isDefinedBy rdf:resource="http://www.opengis.net/spec/geosparql/1.0"/>
    </owl:DatatypeProperty>
    


    <!-- http://www.opengis.net/ont/geosparql#asWKT -->

    <owl:DatatypeProperty rdf:about="&geosparql;asWKT">
        <rdfs:label xml:lang="en">asWKT</rdfs:label>
        <dc:date rdf:datatype="&xsd;date">2011-06-16</dc:date>
        <dc:contributor>Matthew Perry</dc:contributor>
        <dc:description xml:lang="en">
      The WKT serialization of a geometry
    </dc:description>
        <rdfs:comment xml:lang="en">
      The WKT serialization of a geometry
    </rdfs:comment>
        <dc:creator>OGC GeoSPARQL 1.0 Standard Working Group</dc:creator>
        <skos:definition xml:lang="en">
      The WKT serialization of a geometry
    </skos:definition>
        <skos:prefLabel xml:lang="en">asWKT</skos:prefLabel>
        <rdfs:isDefinedBy rdf:resource="http://www.opengis.net/ont/geosparql"/>
        <rdfs:domain rdf:resource="&geosparql;Geometry"/>
        <rdfs:subPropertyOf rdf:resource="&geosparql;hasSerialization"/>
        <rdfs:range rdf:resource="&geosparql;wktLiteral"/>
        <rdfs:isDefinedBy rdf:resource="http://www.opengis.net/spec/geosparql/1.0"/>
    </owl:DatatypeProperty>
    


    <!-- http://www.opengis.net/ont/geosparql#hasSerialization -->

    <owl:DatatypeProperty rdf:about="&geosparql;hasSerialization">
        <rdfs:label xml:lang="en">has serialization</rdfs:label>
        <dc:date rdf:datatype="&xsd;date">2011-06-16</dc:date>
        <dc:creator>OGC GeoSPARQL 1.0 Standard Working Group</dc:creator>
        <dc:description xml:lang="en">
      Connects a geometry object with its text-based serialization.
    </dc:description>
        <rdfs:comment xml:lang="en">
      Connects a geometry object with its text-based serialization.
    </rdfs:comment>
        <dc:contributor>Matthew Perry</dc:contributor>
        <skos:definition xml:lang="en">
      Connects a geometry object with its text-based serialization.
    </skos:definition>
        <skos:prefLabel xml:lang="en">has serialization</skos:prefLabel>
        <rdfs:isDefinedBy rdf:resource="http://www.opengis.net/ont/geosparql"/>
        <rdfs:domain rdf:resource="&geosparql;Geometry"/>
        <rdfs:isDefinedBy rdf:resource="http://www.opengis.net/spec/geosparql/1.0"/>
        <rdfs:range rdf:resource="&rdfs;Literal"/>
    </owl:DatatypeProperty>
    


    <!-- ttp://geo.linkeddata.es/def/feature#categoria -->

    <owl:DatatypeProperty rdf:about="&btn100;categoria">
        <rdfs:label xml:lang="es">categoria</rdfs:label>
        <rdfs:domain rdf:resource="&btn100;CurvaDeNivel"/>
        <rdfs:range>
            <rdfs:Datatype>
                <owl:oneOf>
                    <rdf:Description>
                        <rdf:type rdf:resource="&rdf;List"/>
                        <rdf:first rdf:datatype="&xsd;string">depresion genérica (Curva que define una concavidad del terreno cada 20 m)</rdf:first>
                        <rdf:rest>
                            <rdf:Description>
                                <rdf:type rdf:resource="&rdf;List"/>
                                <rdf:first rdf:datatype="&xsd;string">depresion maestra (Curva que define una concavidad del terreno cada 100 m)</rdf:first>
                                <rdf:rest>
                                    <rdf:Description>
                                        <rdf:type rdf:resource="&rdf;List"/>
                                        <rdf:first rdf:datatype="&xsd;string">genérica (Curva de nivel con altitud cada 20 m)</rdf:first>
                                        <rdf:rest>
                                            <rdf:Description>
                                                <rdf:type rdf:resource="&rdf;List"/>
                                                <rdf:first rdf:datatype="&xsd;string">interpolada (Curva con altitud resultado de un algoritmo de cálculo y no de los
datos del terreno)</rdf:first>
                                                <rdf:rest>
                                                    <rdf:Description>
                                                        <rdf:type rdf:resource="&rdf;List"/>
                                                        <rdf:first rdf:datatype="&xsd;string">maestra (Curva de nivel con altitud múltiplo de 100 m)</rdf:first>
                                                        <rdf:rest rdf:resource="&rdf;nil"/>
                                                    </rdf:Description>
                                                </rdf:rest>
                                            </rdf:Description>
                                        </rdf:rest>
                                    </rdf:Description>
                                </rdf:rest>
                            </rdf:Description>
                        </rdf:rest>
                    </rdf:Description>
                </owl:oneOf>
            </rdfs:Datatype>
        </rdfs:range>
    </owl:DatatypeProperty>
    


    <!-- 
    ///////////////////////////////////////////////////////////////////////////////////////
    //
    // Classes
    //
    ///////////////////////////////////////////////////////////////////////////////////////
     -->

    


    <!-- http://geo.linkeddata.es/def/feature#AccidenteMaritimo -->

    <owl:Class rdf:about="h&btn100;AccidenteMaritimo">
        <rdfs:label xml:lang="es">AccidenteMaritimo</rdfs:label>
        <rdfs:subClassOf rdf:resource="&ontology;FenomenoHidrografico"/>
        <rdfs:comment xml:lang="es">Accidente geográfico  en zona costera</rdfs:comment>
    </owl:Class>
    


    <!-- http://geo.linkeddata.es/def/feature#AccidenteMaritimoLineal -->

    <owl:Class rdf:about="h&btn100;AccidenteMaritimoLineal">
        <rdfs:label xml:lang="es">AccidenteMaritimoLineal</rdfs:label>
        <rdfs:subClassOf rdf:resource="h&btn100;AccidenteMaritimo"/>
        <rdfs:subClassOf>
            <owl:Restriction>
                <owl:onProperty rdf:resource="h&btn100;tipoDeGeometria"/>
                <owl:hasValue rdf:datatype="&xsd;string">Lineal</owl:hasValue>
            </owl:Restriction>
        </rdfs:subClassOf>
    </owl:Class>
    


    <!-- http://geo.linkeddata.es/def/feature#AccidenteMaritimoPuntual -->

    <owl:Class rdf:about="h&btn100;AccidenteMaritimoPuntual">
        <rdfs:label xml:lang="es">AccidenteMaritimoPuntual</rdfs:label>
        <rdfs:subClassOf rdf:resource="h&btn100;AccidenteMaritimo"/>
        <rdfs:comment xml:lang="es">Accidente geográfico  en zona costera, como consecuencia de entrantes y saliente: Cabos, calas, peñones, playas y puntas.</rdfs:comment>
    </owl:Class>
    


    <!-- http://geo.linkeddata.es/def/feature#Albergue -->

    <owl:Class rdf:about="h&btn100;Albergue">
        <rdfs:label xml:lang="es">Albergue</rdfs:label>
        <rdfs:subClassOf rdf:resource="h&btn100;Alojamiento"/>
        <rdfs:subClassOf rdf:resource="h&btn100;LugarDeOcio"/>
        <rdfs:comment xml:lang="es">Lugar que renta alojamiento, particularmente alentando las actividades al aire libre y el intercambio cultural entre jóvenes de distintos países.</rdfs:comment>
    </owl:Class>
    


    <!-- http://geo.linkeddata.es/def/feature#Alojamiento -->

    <owl:Class rdf:about="h&btn100;Alojamiento">
        <rdfs:label xml:lang="es">Alojamiento</rdfs:label>
        <rdfs:subClassOf rdf:resource="&geosparql;Feature"/>
        <rdfs:subClassOf>
            <owl:Restriction>
                <owl:onProperty rdf:resource="h&btn100;grupoTematico"/>
                <owl:hasValue rdf:datatype="&xsd;string">Poblaciones y Construcciones</owl:hasValue>
            </owl:Restriction>
        </rdfs:subClassOf>
        <rdfs:subClassOf>
            <owl:Restriction>
                <owl:onProperty rdf:resource="h&btn100;tipoDeGeometria"/>
                <owl:hasValue rdf:datatype="&xsd;string">Puntual</owl:hasValue>
            </owl:Restriction>
        </rdfs:subClassOf>
    </owl:Class>
    


    <!-- http://geo.linkeddata.es/def/feature#ApartaderoCargadero -->

    <owl:Class rdf:about="h&btn100;ApartaderoCargadero">
        <rdfs:label xml:lang="es">ApartaderoCargadero</rdfs:label>
        <owl:equivalentClass>
            <owl:Class>
                <owl:intersectionOf rdf:parseType="Collection">
                    <rdf:Description rdf:about="h&btn100;InstalacionFerroviaria"/>
                    <owl:Class>
                        <owl:unionOf rdf:parseType="Collection">
                            <owl:Restriction>
                                <owl:onProperty rdf:resource="h&btn100;tipoDeUso"/>
                                <owl:hasValue rdf:datatype="&xsd;string">apartadero</owl:hasValue>
                            </owl:Restriction>
                            <owl:Restriction>
                                <owl:onProperty rdf:resource="h&btn100;tipoDeUso"/>
                                <owl:hasValue rdf:datatype="&xsd;string">cargadero</owl:hasValue>
                            </owl:Restriction>
                        </owl:unionOf>
                    </owl:Class>
                </owl:intersectionOf>
            </owl:Class>
        </owl:equivalentClass>
        <rdfs:subClassOf rdf:resource="&geosparql;Feature"/>
        <rdfs:comment xml:lang="es">Sitio donde se cargan y descargan las mercancías que se transportan.</rdfs:comment>
    </owl:Class>
    


    <!-- http://geo.linkeddata.es/def/feature#Apeadero -->

    <owl:Class rdf:about="h&btn100;Apeadero">
        <rdfs:label xml:lang="es">Apeadero</rdfs:label>
        <owl:equivalentClass>
            <owl:Class>
                <owl:intersectionOf rdf:parseType="Collection">
                    <rdf:Description rdf:about="h&btn100;InstalacionFerroviaria"/>
                    <owl:Restriction>
                        <owl:onProperty rdf:resource="h&btn100;tipoDeUso"/>
                        <owl:hasValue rdf:datatype="&xsd;string">apeadero</owl:hasValue>
                    </owl:Restriction>
                </owl:intersectionOf>
            </owl:Class>
        </owl:equivalentClass>
        <rdfs:subClassOf rdf:resource="&geosparql;Feature"/>
        <rdfs:comment xml:lang="es">En los ferrocarriles, sitio de la vía preparado para el servicio público, pero sin apartadero ni los demás accesorios de una estación.</rdfs:comment>
    </owl:Class>
    


    <!-- http://geo.linkeddata.es/def/feature#AreaDeServicio -->

    <owl:Class rdf:about="h&btn100;AreaDeServicio">
        <rdfs:label xml:lang="es">AreaDeServicio</rdfs:label>
        <rdfs:subClassOf rdf:resource="h&btn100;ZonaDeUsoCaracteristico"/>
        <rdfs:comment xml:lang="es">En una autopista o autovía, lugar habilitado para el estacionamiento de los vehículos, en el que suele haber una gasolinera, un restaurante y otros
servicios.</rdfs:comment>
    </owl:Class>
    


    <!-- http://geo.linkeddata.es/def/feature#Autovia -->

    <owl:Class rdf:about="h&btn100;Autovia">
        <rdfs:label xml:lang="es">Autovia</rdfs:label>
        <rdfs:subClassOf rdf:resource="h&btn100;RedDeTransportes"/>
        <rdfs:subClassOf>
            <owl:Restriction>
                <owl:onProperty rdf:resource="h&btn100;tipoDeGeometria"/>
                <owl:hasValue rdf:datatype="&xsd;string">Lineal</owl:hasValue>
            </owl:Restriction>
        </rdfs:subClassOf>
        <rdfs:subClassOf>
            <owl:Class>
                <owl:unionOf rdf:parseType="Collection">
                    <owl:Restriction>
                        <owl:onProperty rdf:resource="h&btn100;tipoDeCalzada"/>
                        <owl:hasValue rdf:datatype="&xsd;string">doble</owl:hasValue>
                    </owl:Restriction>
                    <owl:Restriction>
                        <owl:onProperty rdf:resource="h&btn100;tipoDeCalzada"/>
                        <owl:hasValue rdf:datatype="&xsd;string">sentido único</owl:hasValue>
                    </owl:Restriction>
                </owl:unionOf>
            </owl:Class>
        </rdfs:subClassOf>
        <rdfs:subClassOf>
            <owl:Class>
                <owl:unionOf rdf:parseType="Collection">
                    <owl:Restriction>
                        <owl:onProperty rdf:resource="h&btn100;estado"/>
                        <owl:hasValue>en construcción</owl:hasValue>
                    </owl:Restriction>
                    <owl:Restriction>
                        <owl:onProperty rdf:resource="h&btn100;estado"/>
                        <owl:hasValue rdf:datatype="&xsd;string">en uso</owl:hasValue>
                    </owl:Restriction>
                </owl:unionOf>
            </owl:Class>
        </rdfs:subClassOf>
        <rdfs:comment xml:lang="es">Carretera con calzadas separadas para los dos sentidos de la circulación, cuyas entradas y salidas no se someten a las exigencias de seguridad de las autopistas.</rdfs:comment>
        <dc:source xml:lang="es">Diccionario de la Real Academia Espannola.</dc:source>
    </owl:Class>
    


    <!-- http://geo.linkeddata.es/def/feature#Bahia -->

    <owl:Class rdf:about="h&btn100;Bahia">
        <rdfs:label xml:lang="es">Bahia</rdfs:label>
        <rdfs:subClassOf rdf:resource="h&btn100;AccidenteMaritimoLineal"/>
        <dc:source xml:lang="es">Diccionario de la Real Academia Española</dc:source>
        <rdfs:comment xml:lang="es">Entrada de mar en la costa, de extensión considerable, que puede servir de abrigo a las embarcaciones.</rdfs:comment>
    </owl:Class>
    


    <!-- http://geo.linkeddata.es/def/feature#Balneario -->

    <owl:Class rdf:about="h&btn100;Balneario">
        <rdfs:label xml:lang="es">Balneario</rdfs:label>
        <rdfs:subClassOf rdf:resource="h&btn100;Alojamiento"/>
        <rdfs:subClassOf rdf:resource="h&btn100;LugarDeOcio"/>
        <rdfs:comment xml:lang="es">Lugar dedicado al reposo y la curación a través de la utilización de las aguas, sobre todo termales minerales, con un edificio para el hospedaje.</rdfs:comment>
    </owl:Class>
    


    <!-- http://geo.linkeddata.es/def/feature#Cabo -->

    <owl:Class rdf:about="h&btn100;Cabo">
        <rdfs:label xml:lang="es">Cabo</rdfs:label>
        <rdfs:subClassOf rdf:resource="h&btn100;AccidenteMaritimoPuntual"/>
        <dc:source xml:lang="es">Diccionario de la Real Academia Espannola.</dc:source>
        <rdfs:comment xml:lang="es">Lengua de tierra que penetra en el mar.</rdfs:comment>
    </owl:Class>
    


    <!-- http://geo.linkeddata.es/def/feature#Cala -->

    <owl:Class rdf:about="h&btn100;Cala">
        <rdfs:label xml:lang="es">Cala</rdfs:label>
        <rdfs:subClassOf rdf:resource="h&btn100;AccidenteMaritimoPuntual"/>
        <dc:source xml:lang="es">Diccionario de la Real Academia Espannola.</dc:source>
        <rdfs:comment xml:lang="es">Ensenada pequeña.</rdfs:comment>
    </owl:Class>
    


    <!-- http://geo.linkeddata.es/def/feature#Calle -->

    <owl:Class rdf:about="h&btn100;Calle">
        <rdfs:label xml:lang="es">Calle</rdfs:label>
        <rdfs:subClassOf rdf:resource="h&btn100;RedDeTransportes"/>
        <rdfs:subClassOf>
            <owl:Restriction>
                <owl:onProperty rdf:resource="h&btn100;tipoDeGeometria"/>
                <owl:hasValue rdf:datatype="&xsd;string">Lineal</owl:hasValue>
            </owl:Restriction>
        </rdfs:subClassOf>
        <rdfs:comment xml:lang="es">Vía que se encuentra localizada dentro de un núcleo de población o Diseminado superficial, y que ayuda a identificar la estructura de manzanas de dicho núcleo/diseminado.</rdfs:comment>
    </owl:Class>
    


    <!-- http://geo.linkeddata.es/def/feature#Camping -->

    <owl:Class rdf:about="h&btn100;Camping">
        <rdfs:label xml:lang="es">Camping</rdfs:label>
        <rdfs:subClassOf rdf:resource="h&btn100;Alojamiento"/>
        <rdfs:subClassOf rdf:resource="h&btn100;LugarDeOcio"/>
        <rdfs:comment xml:lang="es">Lugar al aire libre, especialmente dispuesto para albergar viajeros, turistas, personas en vacaciones, etc.</rdfs:comment>
    </owl:Class>
    


    <!-- http://geo.linkeddata.es/def/feature#Cantera -->

    <owl:Class rdf:about="h&btn100;Cantera">
        <rdfs:label xml:lang="es">Cantera</rdfs:label>
        <rdfs:subClassOf rdf:resource="h&btn100;ExplotacionMinera"/>
        <rdfs:comment xml:lang="es">Sitio de donde se saca piedra, greda u otra sustancia análoga para obras varias.</rdfs:comment>
    </owl:Class>
    


    <!-- http://geo.linkeddata.es/def/feature#CarreteraAutonomica -->

    <owl:Class rdf:about="h&btn100;CarreteraAutonomica">
        <rdfs:label xml:lang="es">CarreteraAutonomica</rdfs:label>
        <rdfs:subClassOf rdf:resource="&ontology;Carretera"/>
        <rdfs:subClassOf>
            <owl:Class>
                <owl:unionOf rdf:parseType="Collection">
                    <owl:Restriction>
                        <owl:onProperty rdf:resource="h&btn100;tipoDeCalzada"/>
                        <owl:hasValue rdf:datatype="&xsd;string">convencional</owl:hasValue>
                    </owl:Restriction>
                    <owl:Restriction>
                        <owl:onProperty rdf:resource="h&btn100;tipoDeCalzada"/>
                        <owl:hasValue rdf:datatype="&xsd;string">sentido único</owl:hasValue>
                    </owl:Restriction>
                </owl:unionOf>
            </owl:Class>
        </rdfs:subClassOf>
        <rdfs:subClassOf>
            <owl:Class>
                <owl:unionOf rdf:parseType="Collection">
                    <owl:Restriction>
                        <owl:onProperty rdf:resource="h&btn100;competencia"/>
                        <owl:hasValue rdf:datatype="&xsd;string">autonómica</owl:hasValue>
                    </owl:Restriction>
                    <owl:Restriction>
                        <owl:onProperty rdf:resource="h&btn100;competencia"/>
                        <owl:hasValue rdf:datatype="&xsd;string">municipal</owl:hasValue>
                    </owl:Restriction>
                    <owl:Restriction>
                        <owl:onProperty rdf:resource="h&btn100;competencia"/>
                        <owl:hasValue rdf:datatype="&xsd;string">provincial</owl:hasValue>
                    </owl:Restriction>
                </owl:unionOf>
            </owl:Class>
        </rdfs:subClassOf>
        <rdfs:comment xml:lang="es">Tramo de carretera convencional de competencia autonómica o de cualquier otra administración inferior a ésta.</rdfs:comment>
    </owl:Class>
    


    <!-- http://geo.linkeddata.es/def/feature#CarreteraNacional -->

    <owl:Class rdf:about="h&btn100;CarreteraNacional">
        <rdfs:label xml:lang="es">CarreteraNacional</rdfs:label>
        <rdfs:subClassOf rdf:resource="&ontology;Carretera"/>
        <rdfs:subClassOf>
            <owl:Restriction>
                <owl:onProperty rdf:resource="h&btn100;tipoDeGeometria"/>
                <owl:hasValue rdf:datatype="&xsd;string">Lineal</owl:hasValue>
            </owl:Restriction>
        </rdfs:subClassOf>
        <rdfs:subClassOf>
            <owl:Class>
                <owl:unionOf rdf:parseType="Collection">
                    <owl:Restriction>
                        <owl:onProperty rdf:resource="h&btn100;tipoDeCalzada"/>
                        <owl:hasValue rdf:datatype="&xsd;string">convencional</owl:hasValue>
                    </owl:Restriction>
                    <owl:Restriction>
                        <owl:onProperty rdf:resource="h&btn100;tipoDeCalzada"/>
                        <owl:hasValue rdf:datatype="&xsd;string">sentido único</owl:hasValue>
                    </owl:Restriction>
                </owl:unionOf>
            </owl:Class>
        </rdfs:subClassOf>
        <rdfs:comment xml:lang="es">Vía de comunicación dedicada al tráfico rodado, cuya competencia corresponde a la Administración Central del Estado, clasificada como carretera de primer orden por el Ministerio de Fomento (Red de Interés General del Estado).</rdfs:comment>
    </owl:Class>
    


    <!-- http://geo.linkeddata.es/def/feature#Castillo -->

    <owl:Class rdf:about="h&btn100;Castillo">
        <rdfs:label xml:lang="es">Castillo</rdfs:label>
        <rdfs:subClassOf rdf:resource="h&btn100;LugarDeInteres"/>
        <rdfs:comment xml:lang="es">Lugar fuerte, cercado de murallas, baluartes, fosos y otras fortificaciones</rdfs:comment>
    </owl:Class>
    


    <!-- http://geo.linkeddata.es/def/feature#CauceArtificial -->

    <owl:Class rdf:about="h&btn100;CauceArtificial">
        <rdfs:label xml:lang="es">CauceArtificial</rdfs:label>
        <rdfs:subClassOf rdf:resource="&ontology;FenomenoHidrografico"/>
        <rdfs:comment>Canalización artificial diseñada para transvasar agua.</rdfs:comment>
    </owl:Class>
    


    <!-- http://geo.linkeddata.es/def/feature#CauceCanalMayor -->

    <owl:Class rdf:about="h&btn100;CauceCanalMayor">
        <rdfs:label xml:lang="es">CauceCanalMayor</rdfs:label>
        <rdfs:subClassOf rdf:resource="h&btn100;CauceArtificial"/>
        <rdfs:comment xml:lang="es">Cauce cuyo canal es de mayor importancia</rdfs:comment>
    </owl:Class>
    


    <!-- http://geo.linkeddata.es/def/feature#CauceCanalMenor -->

    <owl:Class rdf:about="h&btn100;CauceCanalMenor">
        <rdfs:label xml:lang="es">CauceCanalMenor</rdfs:label>
        <rdfs:subClassOf rdf:resource="h&btn100;CauceArtificial"/>
        <rdfs:comment xml:lang="es">Cause cuyo canal es de menor importancia (Acequias y drenajes)</rdfs:comment>
    </owl:Class>
    


    <!-- http://geo.linkeddata.es/def/feature#CauceCanalTrasvase -->

    <owl:Class rdf:about="h&btn100;CauceCanalTrasvase">
        <rdfs:label xml:lang="es">CauceCanalTrasvase</rdfs:label>
        <rdfs:subClassOf rdf:resource="h&btn100;CauceArtificial"/>
        <rdfs:comment>Trasvase o aporte fluvial entre diferentes objetos hidrográficos.</rdfs:comment>
    </owl:Class>
    


    <!-- http://geo.linkeddata.es/def/feature#Cementerio -->

    <owl:Class rdf:about="h&btn100;Cementerio">
        <rdfs:label xml:lang="es">Cementerio</rdfs:label>
        <rdfs:subClassOf rdf:resource="h&btn100;LugarDeInteres"/>
        <rdfs:subClassOf rdf:resource="h&btn100;ZonaDeUsoCaracteristico"/>
        <rdfs:comment xml:lang="es">Lugar, generalmente cercado, destinado a enterrar los restos mortales o cadáveres de los difuntos.</rdfs:comment>
    </owl:Class>
    


    <!-- http://geo.linkeddata.es/def/feature#CentralCicloCombinado -->

    <owl:Class rdf:about="h&btn100;CentralCicloCombinado">
        <rdfs:label xml:lang="es">CentralCicloCombinado</rdfs:label>
        <rdfs:subClassOf rdf:resource="h&btn100;CentralElectrica"/>
        <rdfs:comment xml:lang="es"> La central térmica de ciclo combinado es aquella donde se genera electricidad mediante la utilización conjunta de dos turbinas:

    Un turbogrupo de gas
    Un turbogrupo de vapor
</rdfs:comment>
    </owl:Class>
    


    <!-- http://geo.linkeddata.es/def/feature#CentralElectrica -->

    <owl:Class rdf:about="h&btn100;CentralElectrica">
        <rdfs:label xml:lang="es">CentralElectrica</rdfs:label>
        <rdfs:subClassOf rdf:resource="&geosparql;Feature"/>
        <rdfs:subClassOf>
            <owl:Restriction>
                <owl:onProperty rdf:resource="h&btn100;tipoDeGeometria"/>
                <owl:hasValue rdf:datatype="&xsd;string">Superficial</owl:hasValue>
            </owl:Restriction>
        </rdfs:subClassOf>
        <rdfs:subClassOf>
            <owl:Restriction>
                <owl:onProperty rdf:resource="h&btn100;grupoTematico"/>
                <owl:hasValue rdf:datatype="&xsd;string">Conducciones y energía</owl:hasValue>
            </owl:Restriction>
        </rdfs:subClassOf>
        <rdfs:comment xml:lang="es">Conjunto de instalaciones utilizadas directa e indirectamente para la producción de energía eléctrica. </rdfs:comment>
    </owl:Class>
    


    <!-- http://geo.linkeddata.es/def/feature#CentralEolica -->

    <owl:Class rdf:about="h&btn100;CentralEolica">
        <rdfs:label xml:lang="es">CentralEolica</rdfs:label>
        <rdfs:subClassOf rdf:resource="h&btn100;CentralElectrica"/>
        <rdfs:comment xml:lang="es">Instalacion industrial que constituye una agrupación de aerogeneradores que transforman la energía eólica en energía eléctrica.</rdfs:comment>
    </owl:Class>
    


    <!-- http://geo.linkeddata.es/def/feature#CentralHidraulica -->

    <owl:Class rdf:about="h&btn100;CentralHidraulica">
        <rdfs:label xml:lang="es">CentralHidraulica</rdfs:label>
        <rdfs:subClassOf rdf:resource="h&btn100;CentralElectrica"/>
        <rdfs:comment xml:lang="es">Instalación empleada en la generación de energía eléctrica como resultado de la energía potencial gravitatoria que posee la masa de agua de un cauce natural en virtud de un desnivel, también conocido como «salto geodésico»</rdfs:comment>
    </owl:Class>
    


    <!-- http://geo.linkeddata.es/def/feature#CentralNuclear -->

    <owl:Class rdf:about="h&btn100;CentralNuclear">
        <rdfs:label xml:lang="es">CentralNuclear</rdfs:label>
        <rdfs:subClassOf rdf:resource="h&btn100;CentralElectrica"/>
        <rdfs:comment xml:lang="es">instalación industrial empleada para la generación de energía eléctrica a partir de energía nuclear. </rdfs:comment>
    </owl:Class>
    


    <!-- http://geo.linkeddata.es/def/feature#CentralSolar -->

    <owl:Class rdf:about="h&btn100;CentralSolar">
        <rdfs:label xml:lang="es">CentralSolar</rdfs:label>
        <rdfs:subClassOf rdf:resource="h&btn100;CentralElectrica"/>
        <rdfs:comment xml:lang="es">Instalación industrial en la que, a partir del calentamiento de un fluido mediante radiación solar y su uso en un ciclo termodinámico convencional, se produce la potencia necesaria para mover un alternador para generación de energía eléctrica </rdfs:comment>
    </owl:Class>
    


    <!-- http://geo.linkeddata.es/def/feature#CentralTermica -->

    <owl:Class rdf:about="h&btn100;CentralTermica">
        <rdfs:label xml:lang="es">CentralTermica</rdfs:label>
        <rdfs:subClassOf rdf:resource="h&btn100;CentralElectrica"/>
        <rdfs:comment xml:lang="es"> instalación empleada en la generación de energía eléctrica a partir de la energía liberada en forma de calor, normalmente mediante la combustión de combustibles fósiles como petróleo, gas natural o carbón. Este calor es empleado por un ciclo termodinámico convencional para mover un alternador y producir energía eléctrica.</rdfs:comment>
    </owl:Class>
    


    <!-- http://geo.linkeddata.es/def/feature#ConduccionDeCombustible -->

    <owl:Class rdf:about="h&btn100;ConduccionDeCombustible">
        <rdfs:label xml:lang="es">ConduccionDeCombustible</rdfs:label>
        <rdfs:subClassOf rdf:resource="&geosparql;Feature"/>
        <rdfs:subClassOf>
            <owl:Restriction>
                <owl:onProperty rdf:resource="h&btn100;grupoTematico"/>
                <owl:hasValue rdf:datatype="&xsd;string">Conducciones y energía</owl:hasValue>
            </owl:Restriction>
        </rdfs:subClassOf>
        <rdfs:subClassOf>
            <owl:Restriction>
                <owl:onProperty rdf:resource="h&btn100;tipoDeGeometria"/>
                <owl:hasValue rdf:datatype="&xsd;string">Lineal</owl:hasValue>
            </owl:Restriction>
        </rdfs:subClassOf>
        <rdfs:comment xml:lang="es">Tubería e instalaciones conexas utilizadas para el transporte de combustibles.</rdfs:comment>
    </owl:Class>
    


    <!-- http://geo.linkeddata.es/def/feature#ConjuntoHistoricoArtistico -->

    <owl:Class rdf:about="h&btn100;ConjuntoHistoricoArtistico">
        <rdfs:label xml:lang="es">ConjuntoHistoricoArtistico</rdfs:label>
        <rdfs:subClassOf rdf:resource="h&btn100;LugarDeInteres"/>
        <scovo2:max xml:lang="es">Es la agrupación de inmuebles que forman una unidad de asentamiento, continua o dispersa, condicionada por una estructura física representativa de la evolución de una comunidad humana por ser testimonio de su cultura o constituir un valor de uso y disfrute para la colectividad.</scovo2:max>
    </owl:Class>
    


    <!-- http://geo.linkeddata.es/def/feature#Costa -->

    <owl:Class rdf:about="h&btn100;Costa">
        <rdfs:label xml:lang="es">Costa</rdfs:label>
        <rdfs:subClassOf rdf:resource="h&btn100;AccidenteMaritimoLineal"/>
        <dc:source xml:lang="es">Diccionario de la Real Academia Española</dc:source>
        <rdfs:comment xml:lang="es">Orilla del mar, de un río, de un lago, etc., y tierra que está cerca de ella.</rdfs:comment>
    </owl:Class>
    


    <!-- http://geo.linkeddata.es/def/feature#Cueva -->

    <owl:Class rdf:about="h&btn100;Cueva">
        <rdfs:label xml:lang="es">Cueva</rdfs:label>
        <rdfs:subClassOf rdf:resource="h&btn100;LugarDeInteres"/>
        <rdfs:comment xml:lang="es">Cavidad natural del terreno causada por algún tipo de erosión de corrientes de agua, hielo o lava, o una combinación de varios de estos factores.</rdfs:comment>
    </owl:Class>
    


    <!-- http://geo.linkeddata.es/def/feature#DepositoCombustible -->

    <owl:Class rdf:about="h&btn100;DepositoCombustible">
        <rdfs:label xml:lang="es">DepositoCombustible</rdfs:label>
        <rdfs:subClassOf rdf:resource="&geosparql;Feature"/>
        <rdfs:subClassOf>
            <owl:Restriction>
                <owl:onProperty rdf:resource="h&btn100;tipoDeGeometria"/>
                <owl:hasValue rdf:datatype="&xsd;string">Puntual</owl:hasValue>
            </owl:Restriction>
        </rdfs:subClassOf>
        <rdfs:subClassOf>
            <owl:Restriction>
                <owl:onProperty rdf:resource="h&btn100;grupoTematico"/>
                <owl:hasValue rdf:datatype="&xsd;string">Conducciones y energía</owl:hasValue>
            </owl:Restriction>
        </rdfs:subClassOf>
        <rdfs:comment xml:lang="es">Contenedor seguro destinado al almacenamiento de líquidos o gases inflamables para su posterior distribución en algunos casos por medio de oleoductos o gaseoductos.</rdfs:comment>
    </owl:Class>
    


    <!-- http://geo.linkeddata.es/def/feature#DepositoDeAgua -->

    <owl:Class rdf:about="h&btn100;DepositoDeAgua">
        <rdfs:label xml:lang="es">DepositoDeAgua</rdfs:label>
        <rdfs:subClassOf rdf:resource="&geosparql;Feature"/>
        <rdfs:subClassOf>
            <owl:Restriction>
                <owl:onProperty rdf:resource="h&btn100;tipoDeGeometria"/>
                <owl:hasValue rdf:datatype="&xsd;string">Puntual</owl:hasValue>
            </owl:Restriction>
        </rdfs:subClassOf>
        <rdfs:subClassOf>
            <owl:Restriction>
                <owl:onProperty rdf:resource="h&btn100;grupoTematico"/>
                <owl:hasValue rdf:datatype="&xsd;string">Conducciones y energía</owl:hasValue>
            </owl:Restriction>
        </rdfs:subClassOf>
    </owl:Class>
    


    <!-- http://geo.linkeddata.es/def/feature#Diseminado -->

    <owl:Class rdf:about="h&btn100;Diseminado">
        <rdfs:label xml:lang="es">Diseminado</rdfs:label>
        <rdfs:subClassOf rdf:resource="&geosparql;Feature"/>
        <rdfs:subClassOf>
            <owl:Restriction>
                <owl:onProperty rdf:resource="h&btn100;grupoTematico"/>
                <owl:hasValue rdf:datatype="&xsd;string">Poblaciones y Construcciones</owl:hasValue>
            </owl:Restriction>
        </rdfs:subClassOf>
        <rdfs:subClassOf>
            <owl:Class>
                <owl:unionOf rdf:parseType="Collection">
                    <owl:Restriction>
                        <owl:onProperty rdf:resource="h&btn100;tipoDeCapital"/>
                        <owl:hasValue rdf:datatype="&xsd;string">capital de un municipio</owl:hasValue>
                    </owl:Restriction>
                    <owl:Restriction>
                        <owl:onProperty rdf:resource="h&btn100;tipoDeCapital"/>
                        <owl:hasValue rdf:datatype="&xsd;string">no es capital</owl:hasValue>
                    </owl:Restriction>
                </owl:unionOf>
            </owl:Class>
        </rdfs:subClassOf>
        <rdfs:comment xml:lang="es">El Instituto Nacional de Estadística de España considera poblamiento diseminado al constituido por las edificaciones o viviendas de una entidad singular de población que no pueden ser incluidas en el concepto de núcleo de población.</rdfs:comment>
    </owl:Class>
    


    <!-- http://geo.linkeddata.es/def/feature#DiseminadoPuntual -->

    <owl:Class rdf:about="h&btn100;DiseminadoPuntual">
        <rdfs:label xml:lang="es">DiseminadoPuntual</rdfs:label>
        <rdfs:subClassOf rdf:resource="h&btn100;Diseminado"/>
        <rdfs:subClassOf>
            <owl:Restriction>
                <owl:onProperty rdf:resource="h&btn100;tipoDeGeometria"/>
                <owl:hasValue rdf:datatype="&xsd;string">Puntual</owl:hasValue>
            </owl:Restriction>
        </rdfs:subClassOf>
        <rdfs:comment xml:lang="es">Las edificaciones o viviendas de una entidad singular de población que no pueden ser incluidas en el concepto de núcleo de población se consideran pertenecientes al diseminado, entendiendo así por diseminado aquellas casas aisladas que no están recogidas como núcleo de población por el INE.
Existen dos tipos de elementos que se engloban en el concepto de Diseminado puntual:
Edificación aislada: caseríos, cortijos, etc. en los que o bien existe una única edificación, o siendo un pequeño conjunto de edificaciones (dos, tres o cuatro...) están dispuestas de tal forma que entre ellas no existe una distancia superior a 100m sobre la imagen.
Edificación dispersa: es el caso de los diseminados comúnmente conocidos. Esto es, aquel conjunto considerable de edificaciones (cinco o más) que sin conformar un núcleo de población presentan características propias de estas (habitabilidad, comunicaciones, etc.).En este caso el objeto se representará por su centroide</rdfs:comment>
    </owl:Class>
    


    <!-- http://geo.linkeddata.es/def/feature#DiseminadoSuperficial -->

    <owl:Class rdf:about="h&btn100;DiseminadoSuperficial">
        <rdfs:label xml:lang="es">DiseminadoSuperficial</rdfs:label>
        <rdfs:subClassOf rdf:resource="h&btn100;Diseminado"/>
        <rdfs:subClassOf>
            <owl:Restriction>
                <owl:onProperty rdf:resource="h&btn100;tipoDeGeometria"/>
                <owl:hasValue rdf:datatype="&xsd;string">Superficial</owl:hasValue>
            </owl:Restriction>
        </rdfs:subClassOf>
        <rdfs:comment xml:lang="es">Agrupación de edificaciones que se extienden por una superficie considerable con estructura similar a un núcleo pero que no aparecen en el INE clasificado como tal. Es el caso de urbanizaciones, zonas residenciales u otras estructuras de población similar.</rdfs:comment>
    </owl:Class>
    


    <!-- http://geo.linkeddata.es/def/feature#EdificioReligioso -->

    <owl:Class rdf:about="h&btn100;EdificioReligioso">
        <rdfs:label xml:lang="es">EdificioReligioso</rdfs:label>
        <rdfs:subClassOf rdf:resource="h&btn100;LugarDeInteres"/>
        <rdfs:comment xml:lang="es">Templo destinado al culto religioso</rdfs:comment>
    </owl:Class>
    


    <!-- http://geo.linkeddata.es/def/feature#EdificioSingular -->

    <owl:Class rdf:about="h&btn100;EdificioSingular">
        <rdfs:label xml:lang="es">EdificioSingular</rdfs:label>
        <rdfs:subClassOf rdf:resource="h&btn100;LugarDeInteres"/>
        <rdfs:comment xml:lang="es">Comprende los edificios que deberán ser conservados íntegramente por su carácter singular y monumental, y por razones histórico-artísticas,
preservando todas sus características arquitectónicas.</rdfs:comment>
    </owl:Class>
    


    <!-- http://geo.linkeddata.es/def/feature#Enlace -->

    <owl:Class rdf:about="h&btn100;Enlace">
        <rdfs:label xml:lang="es">Enlace</rdfs:label>
        <rdfs:subClassOf rdf:resource="h&btn100;RedDeTransportes"/>
        <rdfs:subClassOf>
            <owl:Class>
                <owl:unionOf rdf:parseType="Collection">
                    <owl:Restriction>
                        <owl:onProperty rdf:resource="h&btn100;estado"/>
                        <owl:hasValue rdf:datatype="&xsd;string">en construcción</owl:hasValue>
                    </owl:Restriction>
                    <owl:Restriction>
                        <owl:onProperty rdf:resource="h&btn100;estado"/>
                        <owl:hasValue rdf:datatype="&xsd;string">en uso</owl:hasValue>
                    </owl:Restriction>
                </owl:unionOf>
            </owl:Class>
        </rdfs:subClassOf>
        <rdfs:subClassOf>
            <owl:Restriction>
                <owl:onProperty rdf:resource="h&btn100;tipoDeGeometria"/>
                <owl:hasValue rdf:datatype="&xsd;string">Lineal</owl:hasValue>
            </owl:Restriction>
        </rdfs:subClassOf>
        <rdfs:comment xml:lang="es">Tramo que une dos vías de nombre distinto y permite el acceso de una a otra.</rdfs:comment>
    </owl:Class>
    


    <!-- http://geo.linkeddata.es/def/feature#Ensenada -->

    <owl:Class rdf:about="h&btn100;Ensenada">
        <rdfs:label xml:lang="es">Ensenada</rdfs:label>
        <rdfs:subClassOf rdf:resource="h&btn100;AccidenteMaritimoLineal"/>
        <dc:source xml:lang="es">Diccionario de la Real Academia Española</dc:source>
        <rdfs:comment xml:lang="es">Parte de mar que entra en la tierra.</rdfs:comment>
    </owl:Class>
    


    <!-- http://geo.linkeddata.es/def/feature#Esclusa -->

    <owl:Class rdf:about="h&btn100;Esclusa">
        <rdfs:label xml:lang="es">Esclusa</rdfs:label>
        <rdfs:subClassOf rdf:resource="&ontology;FenomenoHidrografico"/>
        <rdfs:subClassOf>
            <owl:Restriction>
                <owl:onProperty rdf:resource="h&btn100;tipoDeGeometria"/>
                <owl:hasValue rdf:datatype="&xsd;string">Puntual</owl:hasValue>
            </owl:Restriction>
        </rdfs:subClassOf>
        <rdfs:comment xml:lang="es">Compartimento, con puertas de entrada y salida, que se construye en un canal de navegación para que los barcos puedan pasar de un tramo a otro de diferente nivel, para lo cual se llena de agua o se vacía el espacio comprendido entre dichas puertas.</rdfs:comment>
        <dc:source xml:lang="es">Diccionario de la Real Academia Espannola.</dc:source>
    </owl:Class>
    


    <!-- http://geo.linkeddata.es/def/feature#EstacionDeRadio -->

    <owl:Class rdf:about="h&btn100;EstacionDeRadio">
        <rdfs:label xml:lang="es">EstacionDeRadio</rdfs:label>
        <rdfs:subClassOf rdf:resource="h&btn100;EstacionTelecomunicaciones"/>
    </owl:Class>
    


    <!-- http://geo.linkeddata.es/def/feature#EstacionDeSuministro -->

    <owl:Class rdf:about="h&btn100;EstacionDeSuministro">
        <rdfs:label xml:lang="es">EstacionDeSuministro</rdfs:label>
        <owl:equivalentClass>
            <owl:Class>
                <owl:intersectionOf rdf:parseType="Collection">
                    <rdf:Description rdf:about="h&btn100;InstalacionFerroviaria"/>
                    <owl:Restriction>
                        <owl:onProperty rdf:resource="h&btn100;tipoDeUso"/>
                        <owl:hasValue rdf:datatype="&xsd;string">suministro</owl:hasValue>
                    </owl:Restriction>
                </owl:intersectionOf>
            </owl:Class>
        </owl:equivalentClass>
        <rdfs:subClassOf rdf:resource="&geosparql;Feature"/>
        <rdfs:comment xml:lang="es">Instalacion ferroviaria utilizada para suministrar cosas tales como butano, etc.</rdfs:comment>
    </owl:Class>
    


    <!-- http://geo.linkeddata.es/def/feature#EstacionDeTV -->

    <owl:Class rdf:about="h&btn100;EstacionDeTV">
        <rdfs:label xml:lang="es">EstacionDeTV</rdfs:label>
        <rdfs:subClassOf rdf:resource="h&btn100;EstacionTelecomunicaciones"/>
    </owl:Class>
    


    <!-- http://geo.linkeddata.es/def/feature#EstacionDepuradora -->

    <owl:Class rdf:about="h&btn100;EstacionDepuradora">
        <rdfs:label xml:lang="es">EstacionDepuradora</rdfs:label>
        <rdfs:subClassOf rdf:resource="&geosparql;Feature"/>
        <rdfs:subClassOf>
            <owl:Restriction>
                <owl:onProperty rdf:resource="h&btn100;grupoTematico"/>
                <owl:hasValue rdf:datatype="&xsd;string">Conducciones y energía</owl:hasValue>
            </owl:Restriction>
        </rdfs:subClassOf>
        <rdfs:subClassOf>
            <owl:Restriction>
                <owl:onProperty rdf:resource="h&btn100;tipoDeGeometria"/>
                <owl:hasValue rdf:datatype="&xsd;string">Puntual</owl:hasValue>
            </owl:Restriction>
        </rdfs:subClassOf>
        <rdfs:comment xml:lang="es">Construcción creada con fines de depurar o limpiar las aguas.</rdfs:comment>
    </owl:Class>
    


    <!-- http://geo.linkeddata.es/def/feature#EstacionInvernal -->

    <owl:Class rdf:about="h&btn100;EstacionInvernal">
        <rdfs:label xml:lang="es">EstacionInvernal</rdfs:label>
        <rdfs:subClassOf rdf:resource="h&btn100;Alojamiento"/>
        <rdfs:subClassOf rdf:resource="h&btn100;LugarDeOcio"/>
        <rdfs:comment xml:lang="es">Área preparada para el disfrute de la nieve. Dispone de pistas de esquí balizadas preparadas por máquinas especiales así como pistas de fondo,
hoteles para el descanso de los usuarios, remontes para el transporte de los esquiadores a zonas altas y diferentes servicios que pueden ir desde zona para usar trineos hasta pistas de patinaje.</rdfs:comment>
    </owl:Class>
    


    <!-- http://geo.linkeddata.es/def/feature#EstacionTelecomunicaciones -->

    <owl:Class rdf:about="h&btn100;EstacionTelecomunicaciones">
        <rdfs:label xml:lang="es">EstacionTelecomunicaciones</rdfs:label>
        <rdfs:subClassOf rdf:resource="&geosparql;Feature"/>
        <rdfs:subClassOf>
            <owl:Restriction>
                <owl:onProperty rdf:resource="h&btn100;grupoTematico"/>
                <owl:hasValue rdf:datatype="&xsd;string">Conducciones y energía</owl:hasValue>
            </owl:Restriction>
        </rdfs:subClassOf>
        <rdfs:subClassOf>
            <owl:Restriction>
                <owl:onProperty rdf:resource="h&btn100;tipoDeGeometria"/>
                <owl:hasValue rdf:datatype="&xsd;string">Puntual</owl:hasValue>
            </owl:Restriction>
        </rdfs:subClassOf>
        <rdfs:comment xml:lang="es">Centro que consta de todas las instalaciones necesarias para transmitir y recibir señales que aseguren un servicio de radiotelecomunicación determinado.</rdfs:comment>
    </owl:Class>
    


    <!-- http://geo.linkeddata.es/def/feature#EstacionTelefonica -->

    <owl:Class rdf:about="h&btn100;EstacionTelefonica">
        <rdfs:label xml:lang="es">EstacionTelefonica</rdfs:label>
        <rdfs:subClassOf rdf:resource="h&btn100;EstacionTelecomunicaciones"/>
    </owl:Class>
    


    <!-- http://geo.linkeddata.es/def/feature#Estrecho -->

    <owl:Class rdf:about="h&btn100;Estrecho">
        <rdfs:label xml:lang="es">Estrecho</rdfs:label>
        <rdfs:subClassOf rdf:resource="h&btn100;AccidenteMaritimoLineal"/>
        <rdfs:comment xml:lang="es">Paso angosto comprendido entre dos tierras y por el cual se comunica un mar con otro.</rdfs:comment>
    </owl:Class>
    


    <!-- http://geo.linkeddata.es/def/feature#ExplotacionMinera -->

    <owl:Class rdf:about="h&btn100;ExplotacionMinera">
        <rdfs:label xml:lang="es">ExplotacionMinera</rdfs:label>
        <rdfs:subClassOf rdf:resource="&geosparql;Feature"/>
        <rdfs:subClassOf>
            <owl:Restriction>
                <owl:onProperty rdf:resource="h&btn100;tipoDeGeometria"/>
                <owl:hasValue rdf:datatype="&xsd;string">Puntual</owl:hasValue>
            </owl:Restriction>
        </rdfs:subClassOf>
        <rdfs:subClassOf>
            <owl:Class>
                <owl:unionOf rdf:parseType="Collection">
                    <owl:Restriction>
                        <owl:onProperty rdf:resource="h&btn100;estado"/>
                        <owl:hasValue>abandonado</owl:hasValue>
                    </owl:Restriction>
                    <owl:Restriction>
                        <owl:onProperty rdf:resource="h&btn100;estado"/>
                        <owl:hasValue>en uso</owl:hasValue>
                    </owl:Restriction>
                </owl:unionOf>
            </owl:Class>
        </rdfs:subClassOf>
        <rdfs:subClassOf>
            <owl:Restriction>
                <owl:onProperty rdf:resource="h&btn100;grupoTematico"/>
                <owl:hasValue rdf:datatype="&xsd;string">Poblaciones y Construcciones</owl:hasValue>
            </owl:Restriction>
        </rdfs:subClassOf>
        <rdfs:comment xml:lang="es">Terreno dedicado a la explotación de minerales o piedra.</rdfs:comment>
    </owl:Class>
    


    <!-- http://geo.linkeddata.es/def/feature#Gaseoducto -->

    <owl:Class rdf:about="h&btn100;Gaseoducto">
        <rdfs:label xml:lang="es">Gaseoducto</rdfs:label>
        <rdfs:subClassOf rdf:resource="h&btn100;ConduccionDeCombustible"/>
        <rdfs:comment xml:lang="es">Tubería de grueso calibre y gran longitud para conducir a distancia gas combustible, procedente por lo general de emanaciones naturales.</rdfs:comment>
    </owl:Class>
    


    <!-- http://geo.linkeddata.es/def/feature#Gasolinera -->

    <owl:Class rdf:about="h&btn100;Gasolinera">
        <rdfs:label xml:lang="es">Gasolinera</rdfs:label>
        <rdfs:subClassOf rdf:resource="h&btn100;LugarDeInteres"/>
        <rdfs:comment xml:lang="es">Punto de venta de combustible para vehículos de motor.</rdfs:comment>
    </owl:Class>
    


    <!-- http://geo.linkeddata.es/def/feature#Golfo -->

    <owl:Class rdf:about="h&btn100;Golfo">
        <rdfs:label xml:lang="es">Golfo</rdfs:label>
        <rdfs:subClassOf rdf:resource="h&btn100;AccidenteMaritimoLineal"/>
        <dc:source xml:lang="es">Diccionario de la Real Academia Española</dc:source>
        <rdfs:comment xml:lang="es">Gran porción de mar que se interna en la tierra entre dos cabos.</rdfs:comment>
    </owl:Class>
    


    <!-- http://geo.linkeddata.es/def/feature#Helipuerto -->

    <owl:Class rdf:about="h&btn100;Helipuerto">
        <rdfs:label xml:lang="es">Helipuerto</rdfs:label>
        <rdfs:subClassOf rdf:resource="&ontology;Aeropuerto"/>
        <rdfs:comment xml:lang="es">Pista destinada al aterrizaje y despegue de helicópteros.</rdfs:comment>
    </owl:Class>
    


    <!-- http://geo.linkeddata.es/def/feature#Hospital -->

    <owl:Class rdf:about="h&btn100;Hospital">
        <rdfs:label xml:lang="es">Hospital</rdfs:label>
        <rdfs:subClassOf rdf:resource="h&btn100;LugarDeInteres"/>
        <rdfs:comment xml:lang="es">Establecimiento sanitario donde se atiende a los enfermos para proporcionar el diagnóstico y tratamiento que necesitan.</rdfs:comment>
    </owl:Class>
    


    <!-- http://geo.linkeddata.es/def/feature#InstalacionDeportiva -->

    <owl:Class rdf:about="h&btn100;InstalacionDeportiva">
        <rdfs:label xml:lang="es">InstalacionDeportiva</rdfs:label>
        <rdfs:subClassOf rdf:resource="h&btn100;Alojamiento"/>
        <rdfs:subClassOf rdf:resource="h&btn100;LugarDeOcio"/>
        <rdfs:comment xml:lang="es">Recinto o construcción provista de los medios necesarios para el aprendizaje, la práctica y la competición de uno o más deportes.</rdfs:comment>
    </owl:Class>
    


    <!-- http://geo.linkeddata.es/def/feature#InstalacionFerroviaria -->

    <owl:Class rdf:about="h&btn100;InstalacionFerroviaria">
        <rdfs:label xml:lang="es">InstalacionFerroviaria</rdfs:label>
        <rdfs:subClassOf rdf:resource="&geosparql;Feature"/>
        <rdfs:subClassOf>
            <owl:Restriction>
                <owl:onProperty rdf:resource="h&btn100;tipoDeGeometria"/>
                <owl:hasValue rdf:datatype="&xsd;string">Puntual</owl:hasValue>
            </owl:Restriction>
        </rdfs:subClassOf>
        <rdfs:subClassOf>
            <owl:Restriction>
                <owl:onProperty rdf:resource="h&btn100;grupoTematico"/>
                <owl:hasValue rdf:datatype="&xsd;string">Transportes</owl:hasValue>
            </owl:Restriction>
        </rdfs:subClassOf>
        <rdfs:comment xml:lang="es">Lugar conectado a una vía de FFCC, donde alguno de los trenes que circula por dicha vía tiene establecida una parada, ya sea para descarga de mercancías o de viajeros.</rdfs:comment>
    </owl:Class>
    


    <!-- http://geo.linkeddata.es/def/feature#Invernadero -->

    <owl:Class rdf:about="h&btn100;Invernadero">
        <rdfs:label xml:lang="es">Invernadero</rdfs:label>
        <rdfs:subClassOf rdf:resource="h&btn100;ZonaDeUsoCaracteristico"/>
        <rdfs:comment xml:lang="es">Lugar preparado artificialmente para cultivar las plantas fuera de su ambiente y clima habituales.</rdfs:comment>
    </owl:Class>
    


    <!-- http://geo.linkeddata.es/def/feature#Isla -->

    <owl:Class rdf:about="h&btn100;Isla">
        <rdfs:label xml:lang="es">Isla</rdfs:label>
        <rdfs:subClassOf rdf:resource="&ontology;FenomenoHidrografico"/>
        <rdfs:subClassOf>
            <owl:Restriction>
                <owl:onProperty rdf:resource="h&btn100;tipoDeGeometria"/>
                <owl:hasValue rdf:datatype="&xsd;string">Superficial</owl:hasValue>
            </owl:Restriction>
        </rdfs:subClassOf>
        <rdfs:comment xml:lang="es">Masa de tierra firme, más o menos extensa, rodeada de agua por todas partes.</rdfs:comment>
    </owl:Class>
    


    <!-- http://geo.linkeddata.es/def/feature#IslaMaritima -->

    <owl:Class rdf:about="h&btn100;IslaMaritima">
        <rdfs:label xml:lang="es">Isla Maritima</rdfs:label>
        <rdfs:subClassOf rdf:resource="h&btn100;Isla"/>
        <rdfs:comment xml:lang="es">Porción de tierra rodeada de agua del mar</rdfs:comment>
    </owl:Class>
    


    <!-- http://geo.linkeddata.es/def/feature#Itinerario -->

    <owl:Class rdf:about="h&btn100;Itinerario">
        <rdfs:label xml:lang="es">Itinerario</rdfs:label>
        <rdfs:subClassOf rdf:resource="h&btn100;RedDeTransportes"/>
        <rdfs:subClassOf>
            <owl:Restriction>
                <owl:onProperty rdf:resource="h&btn100;tipoDeGeometria"/>
                <owl:hasValue rdf:datatype="&xsd;string">Lineal</owl:hasValue>
            </owl:Restriction>
        </rdfs:subClassOf>
        <rdfs:comment xml:lang="es">Tramo de vía perteneciente al Camino de Santiago o catalogada como Vía verde.</rdfs:comment>
    </owl:Class>
    


    <!-- http://geo.linkeddata.es/def/feature#ItinerarioCaminoDeSantiago -->

    <owl:Class rdf:about="h&btn100;ItinerarioCaminoDeSantiago">
        <rdfs:label xml:lang="es">ItinerarioCaminoDeSantiago</rdfs:label>
        <rdfs:subClassOf rdf:resource="h&btn100;Itinerario"/>
        <rdfs:subClassOf>
            <owl:Restriction>
                <owl:onProperty rdf:resource="&terms;title"/>
                <owl:maxQualifiedCardinality rdf:datatype="&xsd;nonNegativeInteger">0</owl:maxQualifiedCardinality>
                <owl:onDataRange rdf:resource="&xsd;string"/>
            </owl:Restriction>
        </rdfs:subClassOf>
    </owl:Class>
    


    <!-- http://geo.linkeddata.es/def/feature#ItinerarioZonaVerde -->

    <owl:Class rdf:about="h&btn100;ItinerarioZonaVerde">
        <rdfs:label xml:lang="es">ItinerarioZonaVerde</rdfs:label>
        <rdfs:subClassOf rdf:resource="h&btn100;Itinerario"/>
    </owl:Class>
    


    <!-- http://geo.linkeddata.es/def/feature#JardinHistorico -->

    <owl:Class rdf:about="h&btn100;JardinHistorico">
        <rdfs:label xml:lang="es">JardinHistorico</rdfs:label>
        <rdfs:subClassOf rdf:resource="h&btn100;LugarDeInteres"/>
        <rdfs:comment xml:lang="es">Es el espacio delimitado, producto de la ordenación por el hombre de elementos naturales, a veces complementado con estructuras de fábrica, y
estimado de interés en función de su origen o pasado histórico, o de sus valores estéticos, sensoriales o botánicos.</rdfs:comment>
    </owl:Class>
    


    <!-- http://geo.linkeddata.es/def/feature#LIC -->

    <owl:Class rdf:about="h&btn100;LIC">
        <rdfs:label xml:lang="es">LIC</rdfs:label>
        <rdfs:subClassOf rdf:resource="h&btn100;ZonaProtegida"/>
        <rdfs:comment xml:lang="es"> Lugar de importancia comunitaria garantiza la conservación de la biodiversidad (fauna y flora)</rdfs:comment>
    </owl:Class>
    


    <!-- http://geo.linkeddata.es/def/feature#LineaElectrica -->

    <owl:Class rdf:about="h&btn100;LineaElectrica">
        <rdfs:label xml:lang="es">LineaElectrica</rdfs:label>
        <rdfs:subClassOf rdf:resource="&geosparql;Feature"/>
        <rdfs:subClassOf>
            <owl:Restriction>
                <owl:onProperty rdf:resource="h&btn100;tipoDeGeometria"/>
                <owl:hasValue rdf:datatype="&xsd;string">Lineal</owl:hasValue>
            </owl:Restriction>
        </rdfs:subClassOf>
        <rdfs:subClassOf>
            <owl:Restriction>
                <owl:onProperty rdf:resource="h&btn100;grupoTematico"/>
                <owl:hasValue rdf:datatype="&xsd;string">Conducciones y energía</owl:hasValue>
            </owl:Restriction>
        </rdfs:subClassOf>
        <rdfs:comment xml:lang="es">Conjunto de hilos (o cables) y otras instalaciones con fines conducir energía eléctrica. Una Línea eléctrica está constituida tanto por el elemento conductor (usualmente cables de acero, cobre o aluminio) como por sus elementos de soporte (las torres de alta tensión).</rdfs:comment>
    </owl:Class>
    


    <!-- http://geo.linkeddata.es/def/feature#LineaElectricaAltaTension -->

    <owl:Class rdf:about="h&btn100;LineaElectricaAltaTension">
        <rdfs:label xml:lang="es">LineaElectricaAltaTension</rdfs:label>
        <rdfs:subClassOf rdf:resource="h&btn100;LineaElectrica"/>
        <rdfs:comment xml:lang="es">Se considera instalación de alta tensión eléctrica aquella que genere, transporte, transforme, distribuya o utilice energía eléctrica con tensiones superiores a los siguientes límites:

    Corriente alterna: Superior a 1000 voltios.
    Corriente continua: Superior a 1500 voltios.
</rdfs:comment>
    </owl:Class>
    


    <!-- http://geo.linkeddata.es/def/feature#LineaElectricaBajaTension -->

    <owl:Class rdf:about="h&btn100;LineaElectricaBajaTension">
        <rdfs:label xml:lang="es">LineaElectricaBajaTension</rdfs:label>
        <rdfs:subClassOf rdf:resource="h&btn100;LineaElectrica"/>
        <rdfs:comment xml:lang="es"> se considera instalación de baja tensión eléctrica a aquella que distribuya o genere energía eléctrica para consumo propio y a las receptoras en los siguientes límites de tensiones nominales:

    Tensión alterna: igual o inferior a 1000 voltios.
    Tensión continua: igual o inferior a 1500 voltios.
</rdfs:comment>
    </owl:Class>
    


    <!-- http://geo.linkeddata.es/def/feature#LugarDeInteres -->

    <owl:Class rdf:about="h&btn100;LugarDeInteres">
        <rdfs:label xml:lang="es">LugarDeInteres</rdfs:label>
        <rdfs:subClassOf rdf:resource="&geosparql;Feature"/>
        <rdfs:subClassOf>
            <owl:Restriction>
                <owl:onProperty rdf:resource="h&btn100;tipoDeGeometria"/>
                <owl:hasValue rdf:datatype="&xsd;string">Puntual</owl:hasValue>
            </owl:Restriction>
        </rdfs:subClassOf>
        <rdfs:subClassOf>
            <owl:Restriction>
                <owl:onProperty rdf:resource="h&btn100;grupoTematico"/>
                <owl:hasValue rdf:datatype="&xsd;string">Poblaciones y Construcciones</owl:hasValue>
            </owl:Restriction>
        </rdfs:subClassOf>
        <rdfs:comment xml:lang="es">Edificación o Lugar de interés por el uso que se le da o su relación con la cultura. Aquí se incluyen los Bienes de Interés Cultural (BIC)</rdfs:comment>
    </owl:Class>
    


    <!-- http://geo.linkeddata.es/def/feature#LugarDeOcio -->

    <owl:Class rdf:about="h&btn100;LugarDeOcio">
        <rdfs:label xml:lang="es">LugarDeOcio</rdfs:label>
        <rdfs:subClassOf rdf:resource="&geosparql;Feature"/>
        <rdfs:subClassOf>
            <owl:Restriction>
                <owl:onProperty rdf:resource="h&btn100;tipoDeGeometria"/>
                <owl:hasValue rdf:datatype="&xsd;string">Puntual</owl:hasValue>
            </owl:Restriction>
        </rdfs:subClassOf>
        <rdfs:subClassOf>
            <owl:Restriction>
                <owl:onProperty rdf:resource="h&btn100;grupoTematico"/>
                <owl:hasValue rdf:datatype="&xsd;string">Poblaciones y Construcciones</owl:hasValue>
            </owl:Restriction>
        </rdfs:subClassOf>
    </owl:Class>
    


    <!-- http://geo.linkeddata.es/def/feature#Mina -->

    <owl:Class rdf:about="h&btn100;Mina">
        <rdfs:label xml:lang="es">Mina</rdfs:label>
        <rdfs:subClassOf rdf:resource="h&btn100;ExplotacionMinera"/>
        <rdfs:comment>lugar de extracción de recursos minerales</rdfs:comment>
    </owl:Class>
    


    <!-- http://geo.linkeddata.es/def/feature#Muralla -->

    <owl:Class rdf:about="h&btn100;Muralla">
        <rdfs:label xml:lang="es">Muralla</rdfs:label>
        <rdfs:subClassOf rdf:resource="&geosparql;Feature"/>
        <rdfs:subClassOf>
            <owl:Restriction>
                <owl:onProperty rdf:resource="h&btn100;grupoTematico"/>
                <owl:hasValue rdf:datatype="&xsd;string">Poblaciones y Construcciones</owl:hasValue>
            </owl:Restriction>
        </rdfs:subClassOf>
        <rdfs:subClassOf>
            <owl:Restriction>
                <owl:onProperty rdf:resource="h&btn100;tipoDeGeometria"/>
                <owl:hasValue rdf:datatype="&xsd;string">Lineal</owl:hasValue>
            </owl:Restriction>
        </rdfs:subClassOf>
        <rdfs:comment xml:lang="es">Construcción realizada con fines defensivos.</rdfs:comment>
    </owl:Class>
    


    <!-- http://geo.linkeddata.es/def/feature#NucleoPoblacional -->

    <owl:Class rdf:about="h&btn100;NucleoPoblacional">
        <rdfs:label xml:lang="es">NucleoPoblacional</rdfs:label>
        <rdfs:subClassOf rdf:resource="&geosparql;Feature"/>
        <rdfs:subClassOf>
            <owl:Restriction>
                <owl:onProperty rdf:resource="h&btn100;grupoTematico"/>
                <owl:hasValue rdf:datatype="&xsd;string">Poblaciones y Construcciones</owl:hasValue>
            </owl:Restriction>
        </rdfs:subClassOf>
    </owl:Class>
    


    <!-- http://geo.linkeddata.es/def/feature#NucleoPoblacionalPuntual -->

    <owl:Class rdf:about="h&btn100;NucleoPoblacionalPuntual">
        <rdfs:label xml:lang="es">NucleoPoblacionalPuntual</rdfs:label>
        <rdfs:subClassOf rdf:resource="h&btn100;NucleoPoblacional"/>
        <rdfs:subClassOf>
            <owl:Restriction>
                <owl:onProperty rdf:resource="h&btn100;tipoDeGeometria"/>
                <owl:hasValue rdf:datatype="&xsd;string">Puntual</owl:hasValue>
            </owl:Restriction>
        </rdfs:subClassOf>
        <rdfs:subClassOf>
            <owl:Class>
                <owl:unionOf rdf:parseType="Collection">
                    <owl:Restriction>
                        <owl:onProperty rdf:resource="h&btn100;tipoDeCapital"/>
                        <owl:hasValue rdf:datatype="&xsd;string">capital de un municipio</owl:hasValue>
                    </owl:Restriction>
                    <owl:Restriction>
                        <owl:onProperty rdf:resource="h&btn100;tipoDeCapital"/>
                        <owl:hasValue rdf:datatype="&xsd;string">no es capital</owl:hasValue>
                    </owl:Restriction>
                </owl:unionOf>
            </owl:Class>
        </rdfs:subClassOf>
        <rdfs:comment xml:lang="es">Se considera Núcleo de población a un conjunto de al menos diez edificaciones, que están formando calles, plazas y otras vías urbanas. Por excepción el número de edificaciones podrá ser inferior
a 10, siempre que la población de derecho supere los 50 habitantes.
Pertenecerán a esta clase de entidad puntual sólo los núcleos de aquellas comunidades autónomas en las que la densidad de elementos impida su representación superficial a escala. Estas comunidades son
Asturias, Galicia e Islas Canarias.</rdfs:comment>
    </owl:Class>
    


    <!-- http://geo.linkeddata.es/def/feature#NucleoPoblacionalSuperficial -->

    <owl:Class rdf:about="h&btn100;NucleoPoblacionalSuperficial">
        <rdfs:subClassOf rdf:resource="h&btn100;NucleoPoblacional"/>
        <rdfs:subClassOf>
            <owl:Restriction>
                <owl:onProperty rdf:resource="h&btn100;tipoDeGeometria"/>
                <owl:hasValue rdf:datatype="&xsd;string">Superficial</owl:hasValue>
            </owl:Restriction>
        </rdfs:subClassOf>
        <wgs84_pos:long xml:lang="es">NucleoPoblacionalSuperficial</wgs84_pos:long>
        <rdfs:comment xml:lang="es">Se considera Núcleo de población a un conjunto de al menos diez edificaciones, que están formando calles, plazas y otras vías urbanas. Por excepción el número de edificaciones podrá ser inferior a 10, siempre que la población de derecho supere los 50 habitantes Pertenecerán a esta clase de entidad superficial todos los núcleos de población de España salvo
excepciones los de aquellas comunidades autónomas en las que la densidad de elementos impida su representación superficial a escala. Estas comunidades son Asturias, Galicia e Islas Canaria</rdfs:comment>
    </owl:Class>
    


    <!-- http://geo.linkeddata.es/def/feature#Oleoducto -->

    <owl:Class rdf:about="h&btn100;Oleoducto">
        <rdfs:label xml:lang="es">Oleoducto</rdfs:label>
        <rdfs:subClassOf rdf:resource="h&btn100;ConduccionDeCombustible"/>
        <rdfs:comment xml:lang="es">Tubería provista de bombas y otros aparatos para conducir el petróleo a larga distancia.</rdfs:comment>
    </owl:Class>
    


    <!-- http://geo.linkeddata.es/def/feature#ParadorNacional -->

    <owl:Class rdf:about="h&btn100;ParadorNacional">
        <rdfs:label xml:lang="es">ParadorNacional</rdfs:label>
        <rdfs:subClassOf rdf:resource="h&btn100;Alojamiento"/>
        <rdfs:subClassOf rdf:resource="h&btn100;LugarDeOcio"/>
        <rdfs:comment xml:lang="es">Conjunto de hoteles de alta categoría distribuidos por toda España, localizados en edificios emblemáticos o emplazamientos destacables que
han sido seleccionados por su interés histórico, artístico o cultural.</rdfs:comment>
    </owl:Class>
    


    <!-- http://geo.linkeddata.es/def/feature#ParqueNacional -->

    <owl:Class rdf:about="h&btn100;ParqueNacional">
        <rdfs:label xml:lang="es">ParqueNacional</rdfs:label>
        <rdfs:subClassOf rdf:resource="h&btn100;ZonaProtegida"/>
        <rdfs:comment xml:lang="es">Delimitación de protección legal por el estado</rdfs:comment>
    </owl:Class>
    


    <!-- http://geo.linkeddata.es/def/feature#ParqueNatural -->

    <owl:Class rdf:about="h&btn100;ParqueNatural">
        <rdfs:label xml:lang="es">ParqueNatural</rdfs:label>
        <rdfs:subClassOf rdf:resource="h&btn100;ZonaProtegida"/>
        <rdfs:comment xml:lang="es">Delimitación de protección legal por otros organismos</rdfs:comment>
    </owl:Class>
    


    <!-- http://geo.linkeddata.es/def/feature#PasoANivel -->

    <owl:Class rdf:about="h&btn100;PasoANivel">
        <rdfs:label xml:lang="es">PasoANivel</rdfs:label>
        <rdfs:subClassOf rdf:resource="&geosparql;Feature"/>
        <rdfs:subClassOf>
            <owl:Restriction>
                <owl:onProperty rdf:resource="h&btn100;grupoTematico"/>
                <owl:hasValue rdf:datatype="&xsd;string">Transportes</owl:hasValue>
            </owl:Restriction>
        </rdfs:subClassOf>
        <rdfs:subClassOf>
            <owl:Restriction>
                <owl:onProperty rdf:resource="h&btn100;tipoDeGeometria"/>
                <owl:hasValue rdf:datatype="&xsd;string">Puntual</owl:hasValue>
            </owl:Restriction>
        </rdfs:subClassOf>
        <rdfs:comment xml:lang="es">Cruce entre carretera y ferrocarril, que se produce al mismo nivel.</rdfs:comment>
    </owl:Class>
    


    <!-- http://geo.linkeddata.es/def/feature#PatrimonioDeLaHumanidad -->

    <owl:Class rdf:about="h&btn100;PatrimonioDeLaHumanidad">
        <rdfs:label xml:lang="es">PatrimonioDeLaHumanidad</rdfs:label>
        <rdfs:subClassOf rdf:resource="h&btn100;LugarDeInteres"/>
        <rdfs:comment xml:lang="es">Título conferido por la Unesco a sitios específicos del planeta (sean bosque, montaña, lago, cueva, desierto, edificación, complejo arquitectónico o
ciudad) que han sido nominados y confirmados para su inclusión en la lista mantenida por el Programa Patrimonio de la Humanidad.</rdfs:comment>
    </owl:Class>
    


    <!-- http://geo.linkeddata.es/def/feature#Pennon -->

    <owl:Class rdf:about="h&btn100;Pennon">
        <rdfs:label xml:lang="es">Pennon</rdfs:label>
        <rdfs:subClassOf rdf:resource="h&btn100;AccidenteMaritimoPuntual"/>
        <dc:source xml:lang="es">Diccionario de la Real Academia Espannola.</dc:source>
        <rdfs:comment xml:lang="es">Monte peñascoso rodeado de mar.</rdfs:comment>
    </owl:Class>
    


    <!-- http://geo.linkeddata.es/def/feature#PistaDeAterrizaje -->

    <owl:Class rdf:about="h&btn100;PistaDeAterrizaje">
        <rdfs:label xml:lang="es">PistaDeAterrizaje</rdfs:label>
        <rdfs:subClassOf rdf:resource="&geosparql;Feature"/>
        <rdfs:subClassOf>
            <owl:Restriction>
                <owl:onProperty rdf:resource="h&btn100;tipoDeGeometria"/>
                <owl:hasValue rdf:datatype="&xsd;string">Superficie</owl:hasValue>
            </owl:Restriction>
        </rdfs:subClassOf>
        <rdfs:subClassOf>
            <owl:Restriction>
                <owl:onProperty rdf:resource="h&btn100;grupoTematico"/>
                <owl:hasValue rdf:datatype="&xsd;string">Transportes</owl:hasValue>
            </owl:Restriction>
        </rdfs:subClassOf>
        <rdfs:comment xml:lang="es">Espacio dentro de las instalaciones de un aeropuerto, donde circulan los aviones y otros aparatos de navegación aérea, y desde donde se realiza el despegue/aterrizaje.</rdfs:comment>
    </owl:Class>
    


    <!-- http://geo.linkeddata.es/def/feature#Presa -->

    <owl:Class rdf:about="h&btn100;Presa">
        <rdfs:label xml:lang="es">Presa</rdfs:label>
        <rdfs:subClassOf rdf:resource="&geosparql;Feature"/>
        <rdfs:subClassOf>
            <owl:Restriction>
                <owl:onProperty rdf:resource="h&btn100;grupoTematico"/>
                <owl:hasValue rdf:datatype="&xsd;string">Poblaciones y Construcciones</owl:hasValue>
            </owl:Restriction>
        </rdfs:subClassOf>
        <rdfs:subClassOf>
            <owl:Restriction>
                <owl:onProperty rdf:resource="h&btn100;tipoDeGeometria"/>
                <owl:hasValue rdf:datatype="&xsd;string">Lineal</owl:hasValue>
            </owl:Restriction>
        </rdfs:subClassOf>
        <rdfs:comment xml:lang="es">Construcción que se realiza en los embalses o ríos para almacenar el agua.</rdfs:comment>
    </owl:Class>
    


    <!-- http://geo.linkeddata.es/def/feature#Puente -->

    <owl:Class rdf:about="h&btn100;Puente">
        <rdfs:label xml:lang="es">Puente</rdfs:label>
        <rdfs:subClassOf rdf:resource="&geosparql;Feature"/>
        <rdfs:subClassOf>
            <owl:Restriction>
                <owl:onProperty rdf:resource="h&btn100;tipoDeGeometria"/>
                <owl:hasValue rdf:datatype="&xsd;string">Puntual</owl:hasValue>
            </owl:Restriction>
        </rdfs:subClassOf>
        <rdfs:subClassOf>
            <owl:Restriction>
                <owl:onProperty rdf:resource="h&btn100;grupoTematico"/>
                <owl:hasValue rdf:datatype="&xsd;string">Poblaciones y Construcciones</owl:hasValue>
            </owl:Restriction>
        </rdfs:subClassOf>
        <rdfs:comment xml:lang="es">Construcción realizada para paso a distinto nivel entre vías de comunicación o hidrografía.</rdfs:comment>
    </owl:Class>
    


    <!-- http://geo.linkeddata.es/def/feature#Punta -->

    <owl:Class rdf:about="h&btn100;Punta">
        <rdfs:label xml:lang="es">Punta</rdfs:label>
        <rdfs:subClassOf rdf:resource="h&btn100;AccidenteMaritimoPuntual"/>
        <dc:source xml:lang="es">Diccionario de la Real Academia Espannola.</dc:source>
        <rdfs:comment xml:lang="es">engua de tierra, generalmente baja y de poca
extensión, que penetra en el mar.</rdfs:comment>
    </owl:Class>
    


    <!-- http://geo.linkeddata.es/def/feature#Rada -->

    <owl:Class rdf:about="h&btn100;Rada">
        <rdfs:label xml:lang="es">Rada</rdfs:label>
        <rdfs:subClassOf rdf:resource="h&btn100;AccidenteMaritimoLineal"/>
        <rdfs:comment xml:lang="es">Bahía, ensenada, donde las naves pueden estar ancladas al abrigo de algunos vientos.</rdfs:comment>
        <dc:source xml:lang="es">Diccionario de la Real Academia Española</dc:source>
    </owl:Class>
    


    <!-- http://geo.linkeddata.es/def/feature#RedDeTransportes -->

    <owl:Class rdf:about="h&btn100;RedDeTransportes">
        <rdfs:label xml:lang="es">RedDeTransportes</rdfs:label>
        <rdfs:subClassOf rdf:resource="&geosparql;Feature"/>
        <rdfs:subClassOf>
            <owl:Restriction>
                <owl:onProperty rdf:resource="h&btn100;grupoTematico"/>
                <owl:hasValue rdf:datatype="&xsd;string">Transportes</owl:hasValue>
            </owl:Restriction>
        </rdfs:subClassOf>
    </owl:Class>
    


    <!-- http://geo.linkeddata.es/def/feature#Rio -->

    <owl:Class rdf:about="h&btn100;Rio">
        <rdfs:label xml:lang="es">Rio</rdfs:label>
        <rdfs:subClassOf rdf:resource="&ontology;FenomenoHidrografico"/>
    </owl:Class>
    


    <!-- http://geo.linkeddata.es/def/feature#RioLineal -->

    <owl:Class rdf:about="h&btn100;RioLineal">
        <rdfs:label xml:lang="es">RioLineal</rdfs:label>
        <rdfs:subClassOf rdf:resource="h&btn100;Rio"/>
        <rdfs:subClassOf>
            <owl:Restriction>
                <owl:onProperty rdf:resource="h&btn100;tipoDeGeometria"/>
                <owl:hasValue rdf:datatype="&xsd;string">Lineal</owl:hasValue>
            </owl:Restriction>
        </rdfs:subClassOf>
        <rdfs:subClassOf>
            <owl:Class>
                <owl:unionOf rdf:parseType="Collection">
                    <owl:Class>
                        <owl:intersectionOf rdf:parseType="Collection">
                            <owl:Class>
                                <owl:unionOf rdf:parseType="Collection">
                                    <owl:Restriction>
                                        <owl:onProperty rdf:resource="h&btn100;ordenDeInteres"/>
                                        <owl:hasValue rdf:datatype="&xsd;string">río de interés no definido</owl:hasValue>
                                    </owl:Restriction>
                                    <owl:Restriction>
                                        <owl:onProperty rdf:resource="h&btn100;ordenDeInteres"/>
                                        <owl:hasValue rdf:datatype="&xsd;string">río de menor interes</owl:hasValue>
                                    </owl:Restriction>
                                </owl:unionOf>
                            </owl:Class>
                            <owl:Restriction>
                                <owl:onProperty rdf:resource="h&btn100;regimen"/>
                                <owl:hasValue rdf:datatype="&xsd;string">no permanente (agua variable dependiendo de estacionalidad)</owl:hasValue>
                            </owl:Restriction>
                        </owl:intersectionOf>
                    </owl:Class>
                    <owl:Restriction>
                        <owl:onProperty rdf:resource="h&btn100;regimen"/>
                        <owl:hasValue>permanente</owl:hasValue>
                    </owl:Restriction>
                </owl:unionOf>
            </owl:Class>
        </rdfs:subClassOf>
        <rdfs:comment xml:lang="es">Corriente de agua, permanente o no, más o menos caudalosa que desemboca en otra, en una laguna, o en el mar.</rdfs:comment>
    </owl:Class>
    


    <!-- http://geo.linkeddata.es/def/feature#RioSuperficial -->

    <owl:Class rdf:about="h&btn100;RioSuperficial">
        <rdfs:label xml:lang="es">RioSuperficial</rdfs:label>
        <rdfs:subClassOf rdf:resource="h&btn100;Rio"/>
        <rdfs:subClassOf>
            <owl:Restriction>
                <owl:onProperty rdf:resource="h&btn100;tipoDeGeometria"/>
                <owl:hasValue rdf:datatype="&xsd;string">Superficial</owl:hasValue>
            </owl:Restriction>
        </rdfs:subClassOf>
        <rdfs:comment xml:lang="es">Corriente de agua permanente, más o menos caudalosa que desemboca en otra, en laguna, o en el mar y que tiene un ancho mayor de 20m durante más de 500m.</rdfs:comment>
    </owl:Class>
    


    <!-- http://geo.linkeddata.es/def/feature#SitioHistorico -->

    <owl:Class rdf:about="h&btn100;SitioHistorico">
        <rdfs:label xml:lang="es">SitioHistorico</rdfs:label>
        <rdfs:subClassOf rdf:resource="h&btn100;LugarDeInteres"/>
        <rdfs:comment xml:lang="es">Es el lugar o paraje natural, vinculado a acontecimientos o recuerdos del pasado, a tradiciones populares, creaciones culturales o de la naturaleza, y a obras del hombre, que poseen valor histórico, etnológico, paleontológico o
antropológico.</rdfs:comment>
    </owl:Class>
    


    <!-- http://geo.linkeddata.es/def/feature#SubestacionElectrica -->

    <owl:Class rdf:about="h&btn100;SubestacionElectrica">
        <rdfs:label xml:lang="es">SubestacionElectrica</rdfs:label>
        <rdfs:subClassOf rdf:resource="&geosparql;Feature"/>
        <rdfs:subClassOf>
            <owl:Restriction>
                <owl:onProperty rdf:resource="h&btn100;grupoTematico"/>
                <owl:hasValue rdf:datatype="&xsd;string">Conducciones y energía</owl:hasValue>
            </owl:Restriction>
        </rdfs:subClassOf>
        <rdfs:subClassOf>
            <owl:Restriction>
                <owl:onProperty rdf:resource="h&btn100;tipoDeGeometria"/>
                <owl:hasValue rdf:datatype="&xsd;string">Puntual</owl:hasValue>
            </owl:Restriction>
        </rdfs:subClassOf>
        <rdfs:comment xml:lang="es">Conjunto de instalaciones utilizadas para la reducción de la tensión o el voltaje de las líneas eléctricas.</rdfs:comment>
    </owl:Class>
    


    <!-- http://geo.linkeddata.es/def/feature#Teleferico -->

    <owl:Class rdf:about="h&btn100;Teleferico">
        <rdfs:label xml:lang="es">Teleferico</rdfs:label>
        <rdfs:subClassOf rdf:resource="h&btn100;TransporteSuspendido"/>
        <rdfs:comment xml:lang="es">sistema de transporte aéreo constituido por cabinas colgadas de una serie de cables que se encargan de hacer avanzar a las unidades a través de las estaciones.</rdfs:comment>
    </owl:Class>
    


    <!-- http://geo.linkeddata.es/def/feature#Telesilla -->

    <owl:Class rdf:about="h&btn100;Telesilla">
        <rdfs:label xml:lang="es">Telesilla</rdfs:label>
        <rdfs:subClassOf rdf:resource="h&btn100;TransporteSuspendido"/>
        <rdfs:comment xml:lang="es">Asiento suspendido de un cable de tracción, para el transporte de personas a la cumbre de una montaña o a un lugar elevado.</rdfs:comment>
    </owl:Class>
    


    <!-- http://geo.linkeddata.es/def/feature#Telesqui -->

    <owl:Class rdf:about="h&btn100;Telesqui">
        <rdfs:label xml:lang="es">Telesqui</rdfs:label>
        <rdfs:subClassOf rdf:resource="h&btn100;TransporteSuspendido"/>
        <rdfs:comment xml:lang="es">sistema mecánico para transportar esquiadores montaña arriba, por la superficie de la pendiente. Por lo general es empleado en pendientes poco pronunciadas en grandes centros de esquí.</rdfs:comment>
    </owl:Class>
    


    <!-- http://geo.linkeddata.es/def/feature#TransporteSuspendido -->

    <owl:Class rdf:about="h&btn100;TransporteSuspendido">
        <rdfs:label xml:lang="es">TransporteSuspendido</rdfs:label>
        <rdfs:subClassOf rdf:resource="&geosparql;Feature"/>
        <rdfs:subClassOf>
            <owl:Restriction>
                <owl:onProperty rdf:resource="h&btn100;tipoDeGeometria"/>
                <owl:hasValue rdf:datatype="&xsd;string">Lineal</owl:hasValue>
            </owl:Restriction>
        </rdfs:subClassOf>
        <rdfs:subClassOf>
            <owl:Restriction>
                <owl:onProperty rdf:resource="h&btn100;grupoTematico"/>
                <owl:hasValue rdf:datatype="&xsd;string">Transportes</owl:hasValue>
            </owl:Restriction>
        </rdfs:subClassOf>
        <rdfs:comment xml:lang="es">Sistema de transporte en el que los vehículos van suspendidos de un cable de tracción. Se emplea principalmente para salvar grandes diferencias de altitud.</rdfs:comment>
    </owl:Class>
    


    <!-- http://geo.linkeddata.es/def/feature#UnidadAdministrativa -->

    <owl:Class rdf:about="h&btn100;UnidadAdministrativa">
        <rdfs:label xml:lang="es">Unidad Administrativa</rdfs:label>
        <rdfs:subClassOf rdf:resource="&geosparql;Feature"/>
        <rdfs:subClassOf>
            <owl:Restriction>
                <owl:onProperty rdf:resource="h&btn100;grupoTematico"/>
                <owl:hasValue>Unidades administrativas y zonas protegidas</owl:hasValue>
            </owl:Restriction>
        </rdfs:subClassOf>
        <rdfs:subClassOf>
            <owl:Restriction>
                <owl:onProperty rdf:resource="h&btn100;tipoDeGeometria"/>
                <owl:hasValue>Superficial</owl:hasValue>
            </owl:Restriction>
        </rdfs:subClassOf>
        <rdfs:comment xml:lang="es">Definen las áreas de cada municipio o condominio, provincia, comunidad autónoma y nación española.</rdfs:comment>
    </owl:Class>
    


    <!-- http://geo.linkeddata.es/def/feature#UnidadAdministrativaDeCiudadAutonoma -->

    <owl:Class rdf:about="h&btn100;UnidadAdministrativaDeCiudadAutonoma">
        <rdfs:label xml:lang="es">Unidad Administrativa de Ciudad Autonoma</rdfs:label>
        <rdfs:subClassOf rdf:resource="h&btn100;UnidadAdministrativa"/>
        <rdfs:comment xml:lang="es">Unidad administrativa de Ciudad Autónoma.</rdfs:comment>
    </owl:Class>
    


    <!-- http://geo.linkeddata.es/def/feature#UnidadAdministrativaDeComunidadAutonoma -->

    <owl:Class rdf:about="h&btn100;UnidadAdministrativaDeComunidadAutonoma">
        <rdfs:label xml:lang="es">Unidad Administrativa de Comunidad Autonoma</rdfs:label>
        <rdfs:subClassOf rdf:resource="h&btn100;UnidadAdministrativa"/>
        <rdfs:comment xml:lang="es">Unidad administrativa de Comunidad Autónoma</rdfs:comment>
    </owl:Class>
    


    <!-- http://geo.linkeddata.es/def/feature#UnidadAdministrativaDeComunidadJurisdiccional -->

    <owl:Class rdf:about="h&btn100;UnidadAdministrativaDeComunidadJurisdiccional">
        <rdfs:label xml:lang="es">Unidad Administrativa de Comunidad Jurisdiccional</rdfs:label>
        <rdfs:subClassOf rdf:resource="h&btn100;UnidadAdministrativa"/>
        <rdfs:comment xml:lang="es">Unidad administrativa de comunidad jurisdiccional</rdfs:comment>
    </owl:Class>
    


    <!-- http://geo.linkeddata.es/def/feature#UnidadAdministrativaDeMunicipio -->

    <owl:Class rdf:about="h&btn100;UnidadAdministrativaDeMunicipio">
        <rdfs:label xml:lang="es">Unidad Administrativa de Municipio</rdfs:label>
        <rdfs:subClassOf rdf:resource="h&btn100;UnidadAdministrativa"/>
        <rdfs:comment xml:lang="es">Unidad administrativa de Municipio</rdfs:comment>
    </owl:Class>
    


    <!-- http://geo.linkeddata.es/def/feature#UnidadAdministrativaDeNacion -->

    <owl:Class rdf:about="h&btn100;UnidadAdministrativaDeNacion">
        <rdfs:label xml:lang="es">Unidad Administrativa de Nacion</rdfs:label>
        <rdfs:subClassOf rdf:resource="h&btn100;UnidadAdministrativa"/>
        <rdfs:comment xml:lang="es">Unidad administrativa de Nación</rdfs:comment>
    </owl:Class>
    


    <!-- http://geo.linkeddata.es/def/feature#UnidadAdministrativaDeProvincia -->

    <owl:Class rdf:about="h&btn100;UnidadAdministrativaDeProvincia">
        <rdfs:label xml:lang="es">Unidad Administrativa de Provincia</rdfs:label>
        <rdfs:subClassOf rdf:resource="h&btn100;UnidadAdministrativa"/>
        <rdfs:comment xml:lang="es">Unidad administrativa de Provincia</rdfs:comment>
    </owl:Class>
    


    <!-- http://geo.linkeddata.es/def/feature#ViaDeFerrocarril -->

    <owl:Class rdf:about="h&btn100;ViaDeFerrocarril">
        <rdfs:label xml:lang="es">ViaDeFerrocarril</rdfs:label>
        <rdfs:subClassOf rdf:resource="h&btn100;RedDeTransportes"/>
        <rdfs:subClassOf>
            <owl:Restriction>
                <owl:onProperty rdf:resource="h&btn100;tipoDeGeometria"/>
                <owl:hasValue rdf:datatype="&xsd;string">Lineal</owl:hasValue>
            </owl:Restriction>
        </rdfs:subClassOf>
    </owl:Class>
    


    <!-- http://geo.linkeddata.es/def/feature#ViaDeFerrocarrilConvencional -->

    <owl:Class rdf:about="h&btn100;ViaDeFerrocarrilConvencional">
        <rdfs:label xml:lang="es">ViaDeFerrocarrilConvencional</rdfs:label>
        <rdfs:subClassOf rdf:resource="h&btn100;ViaDeFerrocarril"/>
        <rdfs:comment xml:lang="es">Vía por la que circulan los trenes de RENFE que no pertenecen a la red AVE.</rdfs:comment>
    </owl:Class>
    


    <!-- http://geo.linkeddata.es/def/feature#ViaDeFerrocarrilDeAltaVelocidad -->

    <owl:Class rdf:about="h&btn100;ViaDeFerrocarrilDeAltaVelocidad">
        <rdfs:label xml:lang="es">ViaDeFerrocarrilDeAltaVelocidad</rdfs:label>
        <rdfs:subClassOf rdf:resource="h&btn100;ViaDeFerrocarril"/>
        <rdfs:subClassOf>
            <owl:Restriction>
                <owl:onProperty rdf:resource="h&btn100;tipoDeGeometria"/>
                <owl:hasValue rdf:datatype="&xsd;string">Lineal</owl:hasValue>
            </owl:Restriction>
        </rdfs:subClassOf>
        <rdfs:subClassOf>
            <owl:Class>
                <owl:unionOf rdf:parseType="Collection">
                    <owl:Restriction>
                        <owl:onProperty rdf:resource="h&btn100;estado"/>
                        <owl:hasValue rdf:datatype="&xsd;string">en construcción</owl:hasValue>
                    </owl:Restriction>
                    <owl:Restriction>
                        <owl:onProperty rdf:resource="h&btn100;estado"/>
                        <owl:hasValue rdf:datatype="&xsd;string">en uso</owl:hasValue>
                    </owl:Restriction>
                </owl:unionOf>
            </owl:Class>
        </rdfs:subClassOf>
        <rdfs:comment xml:lang="es">Tramo de vía por la que circula el Tren de alta velocidad de España (AVE).</rdfs:comment>
    </owl:Class>
    


    <!-- http://geo.linkeddata.es/def/feature#VistaPanoramica -->

    <owl:Class rdf:about="h&btn100;VistaPanoramica">
        <rdfs:label xml:lang="es">VistaPanoramica</rdfs:label>
        <rdfs:subClassOf rdf:resource="h&btn100;LugarDeInteres"/>
        <rdfs:comment xml:lang="es">Es la que muestra un panorama usualmente paisajístico o arquitectónico, y que se distingue por el amplio horizonte visual que cubre.</rdfs:comment>
    </owl:Class>
    


    <!-- http://geo.linkeddata.es/def/feature#Zepa -->

    <owl:Class rdf:about="h&btn100;Zepa">
        <rdfs:label xml:lang="es">Zepa</rdfs:label>
        <rdfs:subClassOf rdf:resource="h&btn100;ZonaProtegida"/>
        <rdfs:comment xml:lang="es">Zona especial de protección de aves.</rdfs:comment>
    </owl:Class>
    


    <!-- http://geo.linkeddata.es/def/feature#ZonaArqueologica -->

    <owl:Class rdf:about="h&btn100;ZonaArqueologica">
        <rdfs:label xml:lang="es">ZonaArqueologica</rdfs:label>
        <rdfs:subClassOf rdf:resource="h&btn100;LugarDeInteres"/>
        <rdfs:comment xml:lang="es">Es el lugar o paraje natural donde existen bienes muebles o inmuebles susceptibles de ser estudiados con metodología arqueológica, hayan sido o no extraídos y tanto si se encuentran en la superficie, en el subsuelo o bajo las aguas españolas.</rdfs:comment>
    </owl:Class>
    


    <!-- http://geo.linkeddata.es/def/feature#ZonaDeUsoCaracteristico -->

    <owl:Class rdf:about="h&btn100;ZonaDeUsoCaracteristico">
        <rdfs:label xml:lang="es">ZonaDeUsoCaracteristico</rdfs:label>
        <rdfs:subClassOf rdf:resource="&geosparql;Feature"/>
        <rdfs:subClassOf>
            <owl:Restriction>
                <owl:onProperty rdf:resource="h&btn100;tipoDeGeometria"/>
                <owl:hasValue rdf:datatype="&xsd;string">Superficial</owl:hasValue>
            </owl:Restriction>
        </rdfs:subClassOf>
        <rdfs:subClassOf>
            <owl:Restriction>
                <owl:onProperty rdf:resource="h&btn100;grupoTematico"/>
                <owl:hasValue rdf:datatype="&xsd;string">Poblaciones y Construcciones</owl:hasValue>
            </owl:Restriction>
        </rdfs:subClassOf>
        <rdfs:comment xml:lang="es">Superficie delimitada, empleada para desarrollar una actividad específica.</rdfs:comment>
    </owl:Class>
    


    <!-- http://geo.linkeddata.es/def/feature#ZonaDeportiva -->

    <owl:Class rdf:about="h&btn100;ZonaDeportiva">
        <rdfs:label xml:lang="es">ZonaDeportiva</rdfs:label>
        <rdfs:subClassOf rdf:resource="h&btn100;ZonaDeUsoCaracteristico"/>
        <rdfs:comment xml:lang="es">Áreas donde se realizan las actividades deportivas, los diferentes espacios complementarios y los de servicios auxiliares.</rdfs:comment>
    </owl:Class>
    


    <!-- http://geo.linkeddata.es/def/feature#ZonaFerroviaria -->

    <owl:Class rdf:about="h&btn100;ZonaFerroviaria">
        <rdfs:label xml:lang="es">ZonaFerroviaria</rdfs:label>
        <rdfs:subClassOf rdf:resource="h&btn100;ZonaDeUsoCaracteristico"/>
        <rdfs:comment xml:lang="es">Instalaciones pertenecientes o destinadas para la explotación de la infraestructura del ferrocarril.</rdfs:comment>
    </owl:Class>
    


    <!-- http://geo.linkeddata.es/def/feature#ZonaIndustrial -->

    <owl:Class rdf:about="h&btn100;ZonaIndustrial">
        <rdfs:label xml:lang="es">ZonaIndustrial</rdfs:label>
        <rdfs:subClassOf rdf:resource="h&btn100;ZonaDeUsoCaracteristico"/>
        <rdfs:comment xml:lang="es">Espacio territorial en el cual se agrupan una serie de actividades industriales, que pueden o no estar relacionadas entre sí.</rdfs:comment>
    </owl:Class>
    


    <!-- http://geo.linkeddata.es/def/feature#ZonaMilitar -->

    <owl:Class rdf:about="h&btn100;ZonaMilitar">
        <rdfs:label xml:lang="es">ZonaMilitar</rdfs:label>
        <rdfs:subClassOf rdf:resource="h&btn100;ZonaDeUsoCaracteristico"/>
        <rdfs:comment xml:lang="es">Zona reservada para fines de la defensa nacional o de las bases ofensivas que en cada territorio se instalen.</rdfs:comment>
    </owl:Class>
    


    <!-- http://geo.linkeddata.es/def/feature#ZonaMonumental -->

    <owl:Class rdf:about="h&btn100;ZonaMonumental">
        <rdfs:label xml:lang="es">ZonaMonumental</rdfs:label>
        <rdfs:subClassOf rdf:resource="h&btn100;ZonaDeUsoCaracteristico"/>
        <rdfs:comment xml:lang="es">Espacio perteneciente o relativo a un monumento.</rdfs:comment>
    </owl:Class>
    


    <!-- http://geo.linkeddata.es/def/feature#ZonaPortuaria -->

    <owl:Class rdf:about="h&btn100;ZonaPortuaria">
        <rdfs:label xml:lang="es">ZonaPortuaria</rdfs:label>
        <rdfs:subClassOf rdf:resource="h&btn100;ZonaDeUsoCaracteristico"/>
        <rdfs:comment xml:lang="es">Espacio destinado y orientado especialmente al flujo de mercancías, personas, información o a dar abrigo y seguridad a aquellas embarcaciones o naves encargadas de llevar a cabo dichas tareas.</rdfs:comment>
    </owl:Class>
    


    <!-- http://geo.linkeddata.es/def/feature#ZonaProtegida -->

    <owl:Class rdf:about="h&btn100;ZonaProtegida">
        <rdfs:label xml:lang="es">Zona Protegida</rdfs:label>
        <rdfs:subClassOf rdf:resource="&geosparql;Feature"/>
        <rdfs:subClassOf>
            <owl:Restriction>
                <owl:onProperty rdf:resource="h&btn100;grupoTematico"/>
                <owl:hasValue>Unidades administrativas y zonas protegidas</owl:hasValue>
            </owl:Restriction>
        </rdfs:subClassOf>
        <rdfs:subClassOf>
            <owl:Restriction>
                <owl:onProperty rdf:resource="h&btn100;tipoDeGeometria"/>
                <owl:hasValue>Superficial</owl:hasValue>
            </owl:Restriction>
        </rdfs:subClassOf>
        <rdfs:comment xml:lang="es">Se capturan los espacios protegidos que según MAGRAMA se corresponden con las figuras de Parque Nacional, Parque Natural, Paisaje protegido, Parque Regional y Paraje Natural, así como los LICs y ZEPAs facilitados por la Red Natura 2000.</rdfs:comment>
    </owl:Class>
    


    <!-- http://geo.linkeddata.es/def/feature#ZonaRecreativa -->

    <owl:Class rdf:about="h&btn100;ZonaRecreativa">
        <rdfs:label xml:lang="es">ZonaRecreativa</rdfs:label>
        <rdfs:subClassOf rdf:resource="h&btn100;ZonaDeUsoCaracteristico"/>
        <rdfs:comment xml:lang="es">Espacio donde se encuentran lugares de ocio o entretenimiento de los ciudadanos.</rdfs:comment>
    </owl:Class>
    


    <!-- http://geo.linkeddata.es/def/feature#ZonaUniversitaria -->

    <owl:Class rdf:about="h&btn100;ZonaUniversitaria">
        <rdfs:label xml:lang="es">ZonaUniversitaria</rdfs:label>
        <rdfs:subClassOf rdf:resource="h&btn100;LugarDeInteres"/>
        <rdfs:subClassOf rdf:resource="h&btn100;ZonaDeUsoCaracteristico"/>
        <rdfs:comment xml:lang="es">Conjunto de edificios situados en terreno acotado al efecto, destinados a la enseñanza superior, y más especialmente la que es propia de las universidades.</rdfs:comment>
    </owl:Class>
    


    <!-- http://geo.linkeddata.es/def/feature#ZonaVerde -->

    <owl:Class rdf:about="h&btn100;ZonaVerde">
        <rdfs:label xml:lang="es">ZonaVerde</rdfs:label>
        <rdfs:subClassOf rdf:resource="h&btn100;ZonaDeUsoCaracteristico"/>
        <rdfs:comment xml:lang="es">Zona del terreno donde se cultivan especies vegetales, con posible añadidura de otros elemntos como fuentes o esculturas.</rdfs:comment>
    </owl:Class>
    


    <!-- http://geo.linkeddata.es/def/feature#zonaAeroportuaria -->

    <owl:Class rdf:about="h&btn100;zonaAeroportuaria">
        <rdfs:label xml:lang="es">zonaAeroportuaria</rdfs:label>
        <rdfs:subClassOf rdf:resource="h&btn100;ZonaDeUsoCaracteristico"/>
        <rdfs:comment xml:lang="es">Estación o terminal situada en un terreno llano que cuenta con pistas, instalaciones y servicios destinados al tráfico de aviones.</rdfs:comment>
    </owl:Class>
    


    <!-- http://geo.linkeddata.es/ontology/Aerodromo -->

    <owl:Class rdf:about="&ontology;Aerodromo">
        <rdfs:label xml:lang="en">Aerodrome</rdfs:label>
        <rdfs:label xml:lang="es">Aeródromo</rdfs:label>
        <rdfs:subClassOf rdf:resource="&ontology;Aeropuerto"/>
        <rdfs:comment xml:lang="es">Terreno llano provisto de pistas y demás instalaciones necesarias para el despegue y aterrizaje de aviones.</rdfs:comment>
    </owl:Class>
    


    <!-- http://geo.linkeddata.es/ontology/Aeropuerto -->

    <owl:Class rdf:about="&ontology;Aeropuerto">
        <rdfs:label xml:lang="en">Airport</rdfs:label>
        <rdfs:label xml:lang="es">Aeropuerto</rdfs:label>
        <rdfs:subClassOf rdf:resource="&geosparql;Feature"/>
        <rdfs:subClassOf>
            <owl:Restriction>
                <owl:onProperty rdf:resource="h&btn100;tipoDeGeometria"/>
                <owl:hasValue rdf:datatype="&xsd;string">Puntual</owl:hasValue>
            </owl:Restriction>
        </rdfs:subClassOf>
        <rdfs:subClassOf>
            <owl:Restriction>
                <owl:onProperty rdf:resource="h&btn100;grupoTematico"/>
                <owl:hasValue rdf:datatype="&xsd;string">Transportes</owl:hasValue>
            </owl:Restriction>
        </rdfs:subClassOf>
        <rdfs:comment xml:lang="es">Terreno llano provisto de un conjunto de pistas, instalaciones y servicios destinados al tráfico regular de aviones.</rdfs:comment>
    </owl:Class>
    


    <!-- http://geo.linkeddata.es/ontology/Alberca -->

    <owl:Class rdf:about="&ontology;Alberca">
        <rdfs:label xml:lang="es">Alberca</rdfs:label>
        <rdfs:subClassOf rdf:resource="&ontology;FenomenoHidrografico"/>
        <rdfs:subClassOf>
            <owl:Restriction>
                <owl:onProperty rdf:resource="h&btn100;tipoDeGeometria"/>
                <owl:hasValue rdf:datatype="&xsd;string">Superficial</owl:hasValue>
            </owl:Restriction>
        </rdfs:subClassOf>
        <rdfs:comment rdf:datatype="&xsd;string">Deposito artificial de agua, con muros de fabrica, destinado al riego</rdfs:comment>
        <dc:source rdf:datatype="&xsd;string">Seco, Manuel. Diccionario del espannol actual. Madrid: Editorial Aguilar. 1999</dc:source>
    </owl:Class>
    


    <!-- http://geo.linkeddata.es/ontology/Albufera -->

    <owl:Class rdf:about="&ontology;Albufera">
        <rdfs:label xml:lang="es">Albufera</rdfs:label>
        <rdfs:subClassOf rdf:resource="&ontology;Humedal"/>
        <dc:source xml:lang="es">Diccionario de la Real Academia Española</dc:source>
        <rdfs:comment xml:lang="es">Laguna litoral, en costa baja, de agua salina o ligeramente salobre, separada del mar por una lengua o cordon de arenas</rdfs:comment>
    </owl:Class>
    


    <!-- http://geo.linkeddata.es/ontology/Autopista -->

    <owl:Class rdf:about="&ontology;Autopista">
        <rdfs:label xml:lang="en">Highway</rdfs:label>
        <rdfs:label xml:lang="es">Autopista</rdfs:label>
        <rdfs:subClassOf rdf:resource="h&btn100;RedDeTransportes"/>
        <rdfs:subClassOf>
            <owl:Restriction>
                <owl:onProperty rdf:resource="h&btn100;tipoDeGeometria"/>
                <owl:hasValue rdf:datatype="&xsd;string">Lineal</owl:hasValue>
            </owl:Restriction>
        </rdfs:subClassOf>
        <rdfs:subClassOf>
            <owl:Class>
                <owl:unionOf rdf:parseType="Collection">
                    <owl:Restriction>
                        <owl:onProperty rdf:resource="h&btn100;tipoDeCalzada"/>
                        <owl:hasValue rdf:datatype="&xsd;string">doble</owl:hasValue>
                    </owl:Restriction>
                    <owl:Restriction>
                        <owl:onProperty rdf:resource="h&btn100;tipoDeCalzada"/>
                        <owl:hasValue rdf:datatype="&xsd;string">sentido único</owl:hasValue>
                    </owl:Restriction>
                </owl:unionOf>
            </owl:Class>
        </rdfs:subClassOf>
        <rdfs:comment xml:lang="es">Carretera con calzadas separadas para los dos sentidos de la circulación, cada una de ellas con dos o más carriles, sin cruces a nivel.</rdfs:comment>
    </owl:Class>
    


    <!-- http://geo.linkeddata.es/ontology/Carretera -->

    <owl:Class rdf:about="&ontology;Carretera">
        <rdfs:label xml:lang="en">Road</rdfs:label>
        <rdfs:label xml:lang="es">Carretera</rdfs:label>
        <rdfs:subClassOf rdf:resource="h&btn100;RedDeTransportes"/>
        <rdfs:comment xml:lang="es">Camino público, ancho y espacioso, pavimentado y dispuesto para el tránsito de vehículos.</rdfs:comment>
    </owl:Class>
    


    <!-- http://geo.linkeddata.es/ontology/Delta -->

    <owl:Class rdf:about="&ontology;Delta">
        <rdfs:label xml:lang="es">Delta</rdfs:label>
        <rdfs:subClassOf rdf:resource="h&btn100;AccidenteMaritimoLineal"/>
        <provenance xml:lang="en">Alexandria Digital Library (ADL) Feature Type Thesaurus</provenance>
        <dc:source xml:lang="es">Diccionario de la Real Academia Española</dc:source>
        <rdfs:comment xml:lang="es">Terreno comprendido entre los brazos de un rio en su desembocadura</rdfs:comment>
    </owl:Class>
    


    <!-- http://geo.linkeddata.es/ontology/Embalse -->

    <owl:Class rdf:about="&ontology;Embalse">
        <rdfs:label xml:lang="en">Reservoir</rdfs:label>
        <rdfs:label xml:lang="es">Embalse</rdfs:label>
        <rdfs:label xml:lang="es">Pantano</rdfs:label>
        <rdfs:subClassOf rdf:resource="&ontology;FenomenoHidrografico"/>
        <rdfs:subClassOf>
            <owl:Restriction>
                <owl:onProperty rdf:resource="h&btn100;tipoDeGeometria"/>
                <owl:hasValue rdf:datatype="&xsd;string">Superficial</owl:hasValue>
            </owl:Restriction>
        </rdfs:subClassOf>
        <rdfs:comment rdf:datatype="&xsd;string">Gran deposito que se forma artificialmente, por lo comun cerrando la boca de un valle mediante un dique o presa, y en el que se almacenan las aguas de un rio o arroyo, a fin de utilizarlas en el riego de terrenos, en el abastecimiento de poblaciones, en la produccion de energia electrica, etc.</rdfs:comment>
        <dc:source xml:lang="es">Diccionario de la Real Academia Española</dc:source>
    </owl:Class>
    


    <!-- http://geo.linkeddata.es/ontology/EstacionDeFerrocarril -->

    <owl:Class rdf:about="&ontology;EstacionDeFerrocarril">
        <rdfs:label xml:lang="en">Train station</rdfs:label>
        <rdfs:label xml:lang="es">Estación de ferrocarril</rdfs:label>
        <owl:equivalentClass>
            <owl:Class>
                <owl:intersectionOf rdf:parseType="Collection">
                    <rdf:Description rdf:about="h&btn100;InstalacionFerroviaria"/>
                    <owl:Restriction>
                        <owl:onProperty rdf:resource="h&btn100;tipoDeUso"/>
                        <owl:hasValue rdf:datatype="&xsd;string">estación</owl:hasValue>
                    </owl:Restriction>
                </owl:intersectionOf>
            </owl:Class>
        </owl:equivalentClass>
        <rdfs:subClassOf rdf:resource="&geosparql;Feature"/>
    </owl:Class>
    


    <!-- http://geo.linkeddata.es/ontology/Faro -->

    <owl:Class rdf:about="&ontology;Faro">
        <rdfs:label xml:lang="en">Lighthouse</rdfs:label>
        <rdfs:label xml:lang="es">Faro</rdfs:label>
        <rdfs:subClassOf rdf:resource="&geosparql;Feature"/>
        <rdfs:subClassOf>
            <owl:Restriction>
                <owl:onProperty rdf:resource="h&btn100;tipoDeGeometria"/>
                <owl:hasValue rdf:datatype="&xsd;string">Puntual</owl:hasValue>
            </owl:Restriction>
        </rdfs:subClassOf>
        <rdfs:subClassOf>
            <owl:Restriction>
                <owl:onProperty rdf:resource="h&btn100;grupoTematico"/>
                <owl:hasValue rdf:datatype="&xsd;string">Transportes</owl:hasValue>
            </owl:Restriction>
        </rdfs:subClassOf>
        <rdfs:comment xml:lang="es">Torre alta en las costas, con luz en su parte superior, para que durante la noche sirva de señal a los navegantes.</rdfs:comment>
    </owl:Class>
    


    <!-- http://geo.linkeddata.es/ontology/FenomenoHidrografico -->

    <owl:Class rdf:about="&ontology;FenomenoHidrografico">
        <rdfs:label xml:lang="en">Hydrographical feature</rdfs:label>
        <rdfs:label xml:lang="es">Accidente hidrografico</rdfs:label>
        <rdfs:label xml:lang="es">Elemento hidrografico</rdfs:label>
        <rdfs:label xml:lang="es">Fenomeno hidrográfico</rdfs:label>
        <rdfs:subClassOf rdf:resource="&geosparql;Feature"/>
        <rdfs:subClassOf>
            <owl:Restriction>
                <owl:onProperty rdf:resource="h&btn100;grupoTematico"/>
                <owl:hasValue rdf:datatype="&xsd;string">Hidrografía</owl:hasValue>
            </owl:Restriction>
        </rdfs:subClassOf>
        <rdfs:comment rdf:datatype="&xsd;string">Abstraccion de un ente que forma parte del conjunto de las aguas de un pais o region o que configura su estructura.</rdfs:comment>
        <dc:source rdf:datatype="&xsd;string">Diccionario de la Real Academia Espannola &amp; International Organization for Standardization. ISO 19101:2002 Geographic information - Reference model.</dc:source>
    </owl:Class>
    


    <!-- http://geo.linkeddata.es/ontology/Humedal -->

    <owl:Class rdf:about="&ontology;Humedal">
        <rdfs:label xml:lang="en">Wetland</rdfs:label>
        <rdfs:label xml:lang="es">Humedal</rdfs:label>
        <rdfs:subClassOf rdf:resource="&ontology;FenomenoHidrografico"/>
        <rdfs:subClassOf>
            <owl:Restriction>
                <owl:onProperty rdf:resource="h&btn100;tipoDeGeometria"/>
                <owl:hasValue rdf:datatype="&xsd;string">Superficial</owl:hasValue>
            </owl:Restriction>
        </rdfs:subClassOf>
        <dc:source rdf:datatype="&xsd;string">Gonzalez Bernaldez, Fernando. (1992) Los paisajes del agua. Terminologia popular de los humedales. Madrid: J.M. Reyero Editor. 257 p. ISBN: 84-604-3756-6.</dc:source>
        <rdfs:comment rdf:datatype="&xsd;string">Terreno sometido a una descarga difusa de agua subterranea sin que se manifieste forzosamente un flujo copioso de agua liquida, aunque suele ser inundable y estar generalmente cubierto de vegetacion freatofitica tipo soto o juncal</rdfs:comment>
    </owl:Class>
    


    <!-- http://geo.linkeddata.es/ontology/IslaFluvial -->

    <owl:Class rdf:about="&ontology;IslaFluvial">
        <rdfs:label xml:lang="en">River island</rdfs:label>
        <rdfs:label xml:lang="es">Isla fluvial</rdfs:label>
        <rdfs:subClassOf rdf:resource="h&btn100;Isla"/>
        <dc:source xml:lang="es">Diccionario de la Real Academia Española &amp; Elaboración propia</dc:source>
        <rdfs:comment xml:lang="es">Porcion de tierra rodeada por las aguas de un río, laguna o embalse</rdfs:comment>
    </owl:Class>
    


    <!-- http://geo.linkeddata.es/ontology/Lago -->

    <owl:Class rdf:about="&ontology;Lago">
        <rdfs:label xml:lang="en">Lake</rdfs:label>
        <rdfs:label xml:lang="es">Lago</rdfs:label>
        <rdfs:subClassOf rdf:resource="&ontology;FenomenoHidrografico"/>
        <dc:source rdf:datatype="&xsd;string">Fontanillo, E. (1986) Diccionario de Geografia. Ed. Anaya. Madrid &amp; Diccionario de la Real Academia Espannola</dc:source>
        <rdfs:comment rdf:datatype="&xsd;string">Gran masa permanente de agua depositada en una depresion del terreno, aunque puede haber casos en los que el lago dispone de un rio emisario que le conecta con otro lago o con el mar.</rdfs:comment>
    </owl:Class>
    


    <!-- http://geo.linkeddata.es/ontology/Laguna -->

    <owl:Class rdf:about="&ontology;Laguna">
        <rdfs:label xml:lang="en">Lagoon</rdfs:label>
        <rdfs:label xml:lang="es">Laguna</rdfs:label>
        <rdfs:subClassOf rdf:resource="&ontology;FenomenoHidrografico"/>
        <rdfs:subClassOf>
            <owl:Restriction>
                <owl:onProperty rdf:resource="h&btn100;tipoDeGeometria"/>
                <owl:hasValue rdf:datatype="&xsd;string">Superficial</owl:hasValue>
            </owl:Restriction>
        </rdfs:subClassOf>
        <rdfs:comment rdf:datatype="&xsd;string">Deposito natural de agua generalmente dulce, que hace referencia o a lagos de poca extension, o a otros que aunque de mayores dimensiones superficiales son de poca profundidad</rdfs:comment>
        <dc:source rdf:datatype="&xsd;string">Fontanillo, E. (1986) Diccionario de Geografia. Ed. Anaya. Madrid &amp; Diccionario de la Real Academia Espannola</dc:source>
    </owl:Class>
    


    <!-- http://geo.linkeddata.es/ontology/Mar -->

    <owl:Class rdf:about="&ontology;Mar">
        <rdfs:label xml:lang="en">Sea</rdfs:label>
        <rdfs:label xml:lang="es">Mar</rdfs:label>
        <rdfs:subClassOf rdf:resource="&ontology;FenomenoHidrografico"/>
        <rdfs:subClassOf>
            <owl:Restriction>
                <owl:onProperty rdf:resource="h&btn100;tipoDeGeometria"/>
                <owl:hasValue rdf:datatype="&xsd;string">Lineal</owl:hasValue>
            </owl:Restriction>
        </rdfs:subClassOf>
        <rdfs:comment rdf:datatype="&xsd;string">Masa de agua salada de gran extension, con denominacion propia y limites relativamente definidos</rdfs:comment>
        <dc:source rdf:datatype="&xsd;string">Vazquez Maure F.; Martin Lopez J. (1987) Vocabulario de terminos geograficos. Ed. Ministerio de Obras Publicas y Urbanismo. Instituto Geografico Nacional. Madrid. ISBN: 84-505-4929-9.</dc:source>
    </owl:Class>
    


    <!-- http://geo.linkeddata.es/ontology/Marisma -->

    <owl:Class rdf:about="&ontology;Marisma">
        <rdfs:label xml:lang="en">Marsh</rdfs:label>
        <rdfs:label xml:lang="es">Marisma</rdfs:label>
        <rdfs:subClassOf rdf:resource="&ontology;Humedal"/>
        <dc:source rdf:datatype="&xsd;string">Fontanillo, E. (1986) Diccionario de Geografia. Ed. Anaya. Madrid.</dc:source>
        <rdfs:comment rdf:datatype="&xsd;string">Terreno un poco por debajo del nivel del mar que se inunda con las aguas de la creciente marina y de los rios, o de ambas a la vez</rdfs:comment>
    </owl:Class>
    


    <!-- http://geo.linkeddata.es/ontology/Oceano -->

    <owl:Class rdf:about="&ontology;Oceano">
        <rdfs:label xml:lang="en">Ocean</rdfs:label>
        <rdfs:label xml:lang="es">Océano</rdfs:label>
        <rdfs:subClassOf rdf:resource="&ontology;FenomenoHidrografico"/>
        <rdfs:subClassOf>
            <owl:Restriction>
                <owl:onProperty rdf:resource="h&btn100;tipoDeGeometria"/>
                <owl:hasValue rdf:datatype="&xsd;string">Lineal</owl:hasValue>
            </owl:Restriction>
        </rdfs:subClassOf>
        <dc:source rdf:datatype="&xsd;string">Diccionario de la Real Academia Espannola</dc:source>
        <rdfs:comment rdf:datatype="&xsd;string">Grande y dilatado mar que cubre la mayor parte de la superficie terrestre</rdfs:comment>
        <provenance rdf:datatype="&xsd;string">Oceanographic geographical features - Data Specification of INSPIRE</provenance>
    </owl:Class>
    


    <!-- http://geo.linkeddata.es/ontology/Pista -->

    <owl:Class rdf:about="&ontology;Pista">
        <rdfs:label xml:lang="es">Pista</rdfs:label>
        <rdfs:subClassOf rdf:resource="h&btn100;RedDeTransportes"/>
        <rdfs:subClassOf>
            <owl:Restriction>
                <owl:onProperty rdf:resource="h&btn100;tipoDeGeometria"/>
                <owl:hasValue rdf:datatype="&xsd;string">Lineal</owl:hasValue>
            </owl:Restriction>
        </rdfs:subClassOf>
        <rdfs:comment xml:lang="es">Vía de comunicación dedicada al tráfico rodado sin recubrimiento asfáltico.</rdfs:comment>
    </owl:Class>
    


    <!-- http://geo.linkeddata.es/ontology/Playa -->

    <owl:Class rdf:about="&ontology;Playa">
        <rdfs:label xml:lang="en">Beach</rdfs:label>
        <rdfs:label xml:lang="es">Playa</rdfs:label>
        <rdfs:subClassOf rdf:resource="h&btn100;AccidenteMaritimoPuntual"/>
        <rdfs:comment xml:lang="es">Ribera del mar formada de arenales en superficie casi plana</rdfs:comment>
    </owl:Class>
    


    <!-- http://geo.linkeddata.es/ontology/Puerto -->

    <owl:Class rdf:about="&ontology;Puerto">
        <rdfs:label xml:lang="en">Port</rdfs:label>
        <rdfs:label xml:lang="es">Puerto</rdfs:label>
        <rdfs:subClassOf rdf:resource="&geosparql;Feature"/>
        <rdfs:subClassOf>
            <owl:Restriction>
                <owl:onProperty rdf:resource="h&btn100;grupoTematico"/>
                <owl:hasValue rdf:datatype="&xsd;string">Transportes</owl:hasValue>
            </owl:Restriction>
        </rdfs:subClassOf>
        <rdfs:subClassOf>
            <owl:Class>
                <owl:unionOf rdf:parseType="Collection">
                    <owl:Restriction>
                        <owl:onProperty rdf:resource="h&btn100;estado"/>
                        <owl:hasValue rdf:datatype="&xsd;string">en construcción</owl:hasValue>
                    </owl:Restriction>
                    <owl:Restriction>
                        <owl:onProperty rdf:resource="h&btn100;estado"/>
                        <owl:hasValue rdf:datatype="&xsd;string">en uso</owl:hasValue>
                    </owl:Restriction>
                </owl:unionOf>
            </owl:Class>
        </rdfs:subClassOf>
        <rdfs:subClassOf>
            <owl:Restriction>
                <owl:onProperty rdf:resource="h&btn100;tipoDeGeometria"/>
                <owl:hasValue rdf:datatype="&xsd;string">Puntual</owl:hasValue>
            </owl:Restriction>
        </rdfs:subClassOf>
        <rdfs:comment xml:lang="es">Lugar en la costa o en las orillas de un río que por sus características, naturales o artificiales, sirve para que las embarcaciones realicen operaciones de carga y descarga, embarque y desembarco, etc.</rdfs:comment>
    </owl:Class>
    


    <!-- http://geo.linkeddata.es/ontology/Rambla -->

    <owl:Class rdf:about="&ontology;Rambla">
        <rdfs:label xml:lang="es">Rambla</rdfs:label>
        <rdfs:subClassOf rdf:resource="&ontology;Humedal"/>
        <rdfs:comment rdf:datatype="&xsd;string">Rio de lecho muy ancho, pero casi permanentemente seco, por donde solo discurren aguas durante avenidas torrenciales</rdfs:comment>
        <dc:source rdf:datatype="&xsd;string">Vazquez Maure F.; Martin Lopez J. (1987) Vocabulario de terminos geograficos. Ed. Ministerio de Obras Publicas y Urbanismo. Instituto Geografico Nacional. Madrid. ISBN: 84-505-4929-9.</dc:source>
    </owl:Class>
    


    <!-- http://geo.linkeddata.es/ontology/Ria -->

    <owl:Class rdf:about="&ontology;Ria">
        <rdfs:label xml:lang="en">Ria</rdfs:label>
        <rdfs:label xml:lang="es">Ría</rdfs:label>
        <rdfs:subClassOf rdf:resource="&ontology;FenomenoHidrografico"/>
        <rdfs:comment rdf:datatype="&xsd;string">Parte del rio proxima a su desembocadura donde las aguas dulces se mezclan con las marinas durante la marea</rdfs:comment>
        <dc:source rdf:datatype="&xsd;string">Vazquez Maure F.; Martin Lopez J. (1987) Vocabulario de terminos geograficos. Ed. Ministerio de Obras Publicas y Urbanismo. Instituto Geografico Nacional. Madrid. ISBN: 84-505-4929-9.</dc:source>
    </owl:Class>
    


    <!-- http://geo.linkeddata.es/ontology/Salina -->

    <owl:Class rdf:about="&ontology;Salina">
        <rdfs:label xml:lang="es">Salina</rdfs:label>
        <rdfs:subClassOf rdf:resource="&ontology;Humedal"/>
        <dc:source rdf:datatype="&xsd;string">Fontanillo, E. (1986) Diccionario de Geografia. Ed. Anaya. Madrid.</dc:source>
        <rdfs:comment rdf:datatype="&xsd;string">Terreno susceptible de recibir agua salada a voluntad, donde mediante una serie de estanques de evaporacion y cristalizacion se extraen las sales contenidas en ella. Las mas usuales son las construidas en la proximidad del mar, pero podemos encontrarlas tambien en puntos del interior de los continentes, construidas junto a fuentes de aguas salinas</rdfs:comment>
    </owl:Class>
    


    <!-- http://www.opengis.net/ont/geosparql#Feature -->

    <owl:Class rdf:about="&geosparql;Feature">
        <rdfs:label xml:lang="en">Feature</rdfs:label>
        <rdfs:subClassOf rdf:resource="&geosparql;SpatialObject"/>
        <owl:disjointWith rdf:resource="&geosparql;Geometry"/>
        <dc:date rdf:datatype="&xsd;date">2011-06-16</dc:date>
        <dc:creator>OGC GeoSPARQL 1.0 Standard Working Group</dc:creator>
        <dc:contributor>Matthew Perry</dc:contributor>
        <rdfs:comment xml:lang="en">
      This class represents the top-level feature type. This class is 
      equivalent to GFI_Feature defined in ISO 19156:2011, and it is 
      superclass of all feature types.
    </rdfs:comment>
        <skos:definition xml:lang="en">
      This class represents the top-level feature type. This class is 
      equivalent to GFI_Feature defined in ISO 19156:2011, and it is 
      superclass of all feature types.
    </skos:definition>
        <dc:description xml:lang="en">
      This class represents the top-level feature type. This class is 
      equivalent to GFI_Feature defined in ISO 19156:2011, and it is 
      superclass of all feature types.
    </dc:description>
        <skos:prefLabel xml:lang="en">Feature</skos:prefLabel>
        <rdfs:isDefinedBy rdf:resource="http://www.opengis.net/ont/geosparql"/>
        <rdfs:isDefinedBy rdf:resource="http://www.opengis.net/ont/gml"/>
        <rdfs:isDefinedBy rdf:resource="http://www.opengis.net/spec/geosparql/1.0"/>
    </owl:Class>
    


    <!-- http://www.opengis.net/ont/geosparql#Geometry -->

    <owl:Class rdf:about="&geosparql;Geometry">
        <rdfs:label xml:lang="en">Geometry</rdfs:label>
        <rdfs:subClassOf rdf:resource="&geosparql;SpatialObject"/>
        <dc:date rdf:datatype="&xsd;date">2011-06-16</dc:date>
        <dc:contributor>Matthew Perry</dc:contributor>
        <dc:creator>OGC GeoSPARQL 1.0 Standard Working Group</dc:creator>
        <skos:definition xml:lang="en">
      The class represents the top-level geometry type. This class is 
      equivalent to the UML class GM_Object defined in ISO 19107, and 
      it is superclass of all geometry types.
    </skos:definition>
        <dc:description xml:lang="en">
      The class represents the top-level geometry type. This class is 
      equivalent to the UML class GM_Object defined in ISO 19107, and 
      it is superclass of all geometry types.
    </dc:description>
        <rdfs:comment xml:lang="en">
      The class represents the top-level geometry type. This class is 
      equivalent to the UML class GM_Object defined in ISO 19107, and 
      it is superclass of all geometry types.
    </rdfs:comment>
        <skos:prefLabel xml:lang="en">Geometry</skos:prefLabel>
        <rdfs:isDefinedBy rdf:resource="http://www.opengis.net/ont/geosparql"/>
        <rdfs:isDefinedBy rdf:resource="http://www.opengis.net/ont/gml"/>
        <rdfs:isDefinedBy rdf:resource="http://www.opengis.net/spec/geosparql/1.0"/>
    </owl:Class>
    


    <!-- http://www.opengis.net/ont/geosparql#SpatialObject -->

    <owl:Class rdf:about="&geosparql;SpatialObject">
        <rdfs:label xml:lang="en">SpatialObject</rdfs:label>
        <dc:date rdf:datatype="&xsd;date">2011-06-16</dc:date>
        <dc:creator>OGC GeoSPARQL 1.0 Standard Working Group</dc:creator>
        <dc:description xml:lang="en">
      The class spatial-object represents everything that can have 
      a spatial representation. It is superclass of feature and geometry.
    </dc:description>
        <skos:definition xml:lang="en">
      The class spatial-object represents everything that can have 
      a spatial representation. It is superclass of feature and geometry.
    </skos:definition>
        <dc:contributor>Matthew Perry</dc:contributor>
        <rdfs:comment xml:lang="en">
      The class spatial-object represents everything that can have 
      a spatial representation. It is superclass of feature and geometry.
    </rdfs:comment>
        <skos:prefLabel xml:lang="en">SpatialObject</skos:prefLabel>
        <rdfs:isDefinedBy rdf:resource="http://www.opengis.net/ont/geosparql"/>
        <rdfs:isDefinedBy rdf:resource="http://www.opengis.net/ont/gml"/>
        <rdfs:isDefinedBy rdf:resource="http://www.opengis.net/spec/geosparql/1.0"/>
    </owl:Class>
    


    <!-- http://www.opengis.net/ont/gml#AbstractCurveSegment -->

    <owl:Class rdf:about="&gml;AbstractCurveSegment">
        <rdfs:label xml:lang="en">Abstract Curve Segment</rdfs:label>
        <rdfs:subClassOf rdf:resource="&geosparql;Geometry"/>
        <rdfs:isDefinedBy rdf:resource="http://www.opengis.net/ont/gml"/>
    </owl:Class>
    


    <!-- http://www.opengis.net/ont/gml#AbstractGeometricPrimitive -->

    <owl:Class rdf:about="&gml;AbstractGeometricPrimitive">
        <rdfs:label xml:lang="en">Abstract Geometric Primitive</rdfs:label>
        <rdfs:subClassOf rdf:resource="&gml;AbstractGeometry"/>
        <rdfs:isDefinedBy rdf:resource="http://www.opengis.net/ont/gml"/>
    </owl:Class>
    


    <!-- http://www.opengis.net/ont/gml#AbstractGeometry -->

    <owl:Class rdf:about="&gml;AbstractGeometry">
        <rdfs:label xml:lang="en">Abstract Geometry</rdfs:label>
        <rdfs:subClassOf rdf:resource="&geosparql;Geometry"/>
        <rdfs:isDefinedBy rdf:resource="http://www.opengis.net/ont/gml"/>
    </owl:Class>
    


    <!-- http://www.opengis.net/ont/gml#AbstractGriddedSurface -->

    <owl:Class rdf:about="&gml;AbstractGriddedSurface">
        <rdfs:label xml:lang="en">Abstract Gridded Surface</rdfs:label>
        <rdfs:subClassOf rdf:resource="&gml;AbstractParametricCurveSurface"/>
        <rdfs:isDefinedBy rdf:resource="http://www.opengis.net/ont/gml"/>
    </owl:Class>
    


    <!-- http://www.opengis.net/ont/gml#AbstractParametricCurveSurface -->

    <owl:Class rdf:about="&gml;AbstractParametricCurveSurface">
        <rdfs:label xml:lang="en">Abstract Parametric Curve Surface</rdfs:label>
        <rdfs:subClassOf rdf:resource="&gml;AbstractSurfacePatch"/>
        <rdfs:isDefinedBy rdf:resource="http://www.opengis.net/ont/gml"/>
    </owl:Class>
    


    <!-- http://www.opengis.net/ont/gml#AbstractSurfacePatch -->

    <owl:Class rdf:about="&gml;AbstractSurfacePatch">
        <rdfs:label xml:lang="en">Abstract Surface Patch</rdfs:label>
        <rdfs:subClassOf rdf:resource="&geosparql;Geometry"/>
        <rdfs:isDefinedBy rdf:resource="http://www.opengis.net/ont/gml"/>
    </owl:Class>
    


    <!-- http://www.opengis.net/ont/gml#Arc -->

    <owl:Class rdf:about="&gml;Arc">
        <rdfs:label xml:lang="en">Arc</rdfs:label>
        <rdfs:subClassOf rdf:resource="&gml;ArcString"/>
        <rdfs:isDefinedBy rdf:resource="http://www.opengis.net/ont/gml"/>
    </owl:Class>
    


    <!-- http://www.opengis.net/ont/gml#ArcByBulge -->

    <owl:Class rdf:about="&gml;ArcByBulge">
        <rdfs:label xml:lang="en">Arc by Bulge</rdfs:label>
        <rdfs:subClassOf rdf:resource="&gml;ArcStringByBulge"/>
        <rdfs:isDefinedBy rdf:resource="http://www.opengis.net/ont/gml"/>
    </owl:Class>
    


    <!-- http://www.opengis.net/ont/gml#ArcByCenterPoint -->

    <owl:Class rdf:about="&gml;ArcByCenterPoint">
        <rdfs:label xml:lang="en">Arc by Center Point</rdfs:label>
        <rdfs:subClassOf rdf:resource="&gml;AbstractCurveSegment"/>
        <rdfs:isDefinedBy rdf:resource="http://www.opengis.net/ont/gml"/>
    </owl:Class>
    


    <!-- http://www.opengis.net/ont/gml#ArcString -->

    <owl:Class rdf:about="&gml;ArcString">
        <rdfs:label xml:lang="en">Arc String</rdfs:label>
        <rdfs:subClassOf rdf:resource="&gml;AbstractCurveSegment"/>
        <rdfs:isDefinedBy rdf:resource="http://www.opengis.net/ont/gml"/>
    </owl:Class>
    


    <!-- http://www.opengis.net/ont/gml#ArcStringByBulge -->

    <owl:Class rdf:about="&gml;ArcStringByBulge">
        <rdfs:label xml:lang="en">Arc String by Bulge</rdfs:label>
        <rdfs:subClassOf rdf:resource="&gml;AbstractCurveSegment"/>
        <rdfs:isDefinedBy rdf:resource="http://www.opengis.net/ont/gml"/>
    </owl:Class>
    


    <!-- http://www.opengis.net/ont/gml#BSpline -->

    <owl:Class rdf:about="&gml;BSpline">
        <rdfs:label xml:lang="en">BSpline</rdfs:label>
        <rdfs:subClassOf rdf:resource="&gml;SplineCurve"/>
        <rdfs:isDefinedBy rdf:resource="http://www.opengis.net/ont/gml"/>
    </owl:Class>
    


    <!-- http://www.opengis.net/ont/gml#Bezier -->

    <owl:Class rdf:about="&gml;Bezier">
        <rdfs:label xml:lang="en">Bezier</rdfs:label>
        <rdfs:subClassOf rdf:resource="&gml;BSpline"/>
        <rdfs:isDefinedBy rdf:resource="http://www.opengis.net/ont/gml"/>
    </owl:Class>
    


    <!-- http://www.opengis.net/ont/gml#Circle -->

    <owl:Class rdf:about="&gml;Circle">
        <rdfs:label xml:lang="en">Circle</rdfs:label>
        <rdfs:subClassOf rdf:resource="&gml;Arc"/>
        <rdfs:isDefinedBy rdf:resource="http://www.opengis.net/ont/gml"/>
    </owl:Class>
    


    <!-- http://www.opengis.net/ont/gml#CircleByCenterPoint -->

    <owl:Class rdf:about="&gml;CircleByCenterPoint">
        <rdfs:label xml:lang="en">CircleByCenterPoint</rdfs:label>
        <rdfs:subClassOf rdf:resource="&gml;ArcByCenterPoint"/>
        <rdfs:isDefinedBy rdf:resource="http://www.opengis.net/ont/gml"/>
    </owl:Class>
    


    <!-- http://www.opengis.net/ont/gml#Clothoid -->

    <owl:Class rdf:about="&gml;Clothoid">
        <rdfs:label xml:lang="en">Clothoid</rdfs:label>
        <rdfs:subClassOf rdf:resource="&gml;AbstractCurveSegment"/>
        <rdfs:isDefinedBy rdf:resource="http://www.opengis.net/ont/gml"/>
    </owl:Class>
    


    <!-- http://www.opengis.net/ont/gml#Composite -->

    <owl:Class rdf:about="&gml;Composite">
        <rdfs:label xml:lang="en">Composite</rdfs:label>
        <rdfs:subClassOf rdf:resource="&gml;GeometricComplex"/>
        <rdfs:isDefinedBy rdf:resource="http://www.opengis.net/ont/gml"/>
    </owl:Class>
    


    <!-- http://www.opengis.net/ont/gml#CompositeCurve -->

    <owl:Class rdf:about="&gml;CompositeCurve">
        <rdfs:label xml:lang="en">Composite Curve</rdfs:label>
        <rdfs:subClassOf rdf:resource="&gml;Composite"/>
        <rdfs:subClassOf rdf:resource="&gml;OrientableCurve"/>
        <rdfs:isDefinedBy rdf:resource="http://www.opengis.net/ont/gml"/>
    </owl:Class>
    


    <!-- http://www.opengis.net/ont/gml#CompositeSolid -->

    <owl:Class rdf:about="&gml;CompositeSolid">
        <rdfs:label xml:lang="en">Composite Solid</rdfs:label>
        <rdfs:subClassOf rdf:resource="&gml;Composite"/>
        <rdfs:subClassOf rdf:resource="&gml;Solid"/>
        <rdfs:isDefinedBy rdf:resource="http://www.opengis.net/ont/gml"/>
    </owl:Class>
    


    <!-- http://www.opengis.net/ont/gml#CompositeSurface -->

    <owl:Class rdf:about="&gml;CompositeSurface">
        <rdfs:label xml:lang="en">Composite Surface</rdfs:label>
        <rdfs:subClassOf rdf:resource="&gml;Composite"/>
        <rdfs:subClassOf rdf:resource="&gml;OrientableSurface"/>
        <rdfs:isDefinedBy rdf:resource="http://www.opengis.net/ont/gml"/>
    </owl:Class>
    


    <!-- http://www.opengis.net/ont/gml#Cone -->

    <owl:Class rdf:about="&gml;Cone">
        <rdfs:label xml:lang="en">Cone</rdfs:label>
        <rdfs:subClassOf rdf:resource="&gml;AbstractGriddedSurface"/>
        <rdfs:isDefinedBy rdf:resource="http://www.opengis.net/ont/gml"/>
    </owl:Class>
    


    <!-- http://www.opengis.net/ont/gml#CubicSpline -->

    <owl:Class rdf:about="&gml;CubicSpline">
        <rdfs:label xml:lang="en">Cubic Spline</rdfs:label>
        <rdfs:subClassOf rdf:resource="&gml;PolynomialSpline"/>
        <rdfs:isDefinedBy rdf:resource="http://www.opengis.net/ont/gml"/>
    </owl:Class>
    


    <!-- http://www.opengis.net/ont/gml#Curve -->

    <owl:Class rdf:about="&gml;Curve">
        <rdfs:label xml:lang="en">Curve</rdfs:label>
        <rdfs:subClassOf rdf:resource="&gml;AbstractGeometricPrimitive"/>
        <rdfs:subClassOf rdf:resource="&gml;OrientableCurve"/>
        <rdfs:isDefinedBy rdf:resource="http://www.opengis.net/ont/gml"/>
    </owl:Class>
    


    <!-- http://www.opengis.net/ont/gml#Cylinder -->

    <owl:Class rdf:about="&gml;Cylinder">
        <rdfs:label xml:lang="en">Cylinder</rdfs:label>
        <rdfs:subClassOf rdf:resource="&gml;AbstractGriddedSurface"/>
        <rdfs:isDefinedBy rdf:resource="http://www.opengis.net/ont/gml"/>
    </owl:Class>
    


    <!-- http://www.opengis.net/ont/gml#Geodesic -->

    <owl:Class rdf:about="&gml;Geodesic">
        <rdfs:label xml:lang="en">Geodesic</rdfs:label>
        <rdfs:subClassOf rdf:resource="&gml;GeodesicString"/>
        <rdfs:isDefinedBy rdf:resource="http://www.opengis.net/ont/gml"/>
    </owl:Class>
    


    <!-- http://www.opengis.net/ont/gml#GeodesicString -->

    <owl:Class rdf:about="&gml;GeodesicString">
        <rdfs:label xml:lang="en">Geodesic String</rdfs:label>
        <rdfs:subClassOf rdf:resource="&gml;AbstractCurveSegment"/>
        <rdfs:isDefinedBy rdf:resource="http://www.opengis.net/ont/gml"/>
    </owl:Class>
    


    <!-- http://www.opengis.net/ont/gml#GeometricComplex -->

    <owl:Class rdf:about="&gml;GeometricComplex">
        <rdfs:label xml:lang="en">Geometric Complex</rdfs:label>
        <rdfs:subClassOf rdf:resource="&gml;AbstractGeometry"/>
        <rdfs:isDefinedBy rdf:resource="http://www.opengis.net/ont/gml"/>
    </owl:Class>
    


    <!-- http://www.opengis.net/ont/gml#LineString -->

    <owl:Class rdf:about="&gml;LineString">
        <rdfs:label xml:lang="en">Line String</rdfs:label>
        <rdfs:subClassOf rdf:resource="&gml;LineStringSegment"/>
        <rdfs:isDefinedBy rdf:resource="http://www.opengis.net/ont/gml"/>
    </owl:Class>
    


    <!-- http://www.opengis.net/ont/gml#LineStringSegment -->

    <owl:Class rdf:about="&gml;LineStringSegment">
        <rdfs:label xml:lang="en">Line String Segment</rdfs:label>
        <rdfs:subClassOf rdf:resource="&gml;AbstractCurveSegment"/>
        <rdfs:isDefinedBy rdf:resource="http://www.opengis.net/ont/gml"/>
    </owl:Class>
    


    <!-- http://www.opengis.net/ont/gml#LinearRing -->

    <owl:Class rdf:about="&gml;LinearRing">
        <rdfs:label xml:lang="en">Linear Ring</rdfs:label>
        <rdfs:subClassOf rdf:resource="&gml;Ring"/>
        <rdfs:isDefinedBy rdf:resource="http://www.opengis.net/ont/gml"/>
    </owl:Class>
    


    <!-- http://www.opengis.net/ont/gml#MultiCurve -->

    <owl:Class rdf:about="&gml;MultiCurve">
        <rdfs:label xml:lang="en">Multi-Curve</rdfs:label>
        <rdfs:subClassOf rdf:resource="&gml;MultiGeometry"/>
        <rdfs:isDefinedBy rdf:resource="http://www.opengis.net/ont/gml"/>
    </owl:Class>
    


    <!-- http://www.opengis.net/ont/gml#MultiGeometry -->

    <owl:Class rdf:about="&gml;MultiGeometry">
        <rdfs:label xml:lang="en">Multi-Geometry</rdfs:label>
        <rdfs:subClassOf rdf:resource="&gml;AbstractGeometry"/>
        <rdfs:isDefinedBy rdf:resource="http://www.opengis.net/ont/gml"/>
    </owl:Class>
    


    <!-- http://www.opengis.net/ont/gml#MultiPoint -->

    <owl:Class rdf:about="&gml;MultiPoint">
        <rdfs:label xml:lang="en">Multi-Point</rdfs:label>
        <rdfs:subClassOf rdf:resource="&gml;MultiGeometry"/>
        <rdfs:isDefinedBy rdf:resource="http://www.opengis.net/ont/gml"/>
    </owl:Class>
    


    <!-- http://www.opengis.net/ont/gml#MultiSolid -->

    <owl:Class rdf:about="&gml;MultiSolid">
        <rdfs:label xml:lang="en">Multi-Solid</rdfs:label>
        <rdfs:subClassOf rdf:resource="&gml;MultiGeometry"/>
        <rdfs:isDefinedBy rdf:resource="http://www.opengis.net/ont/gml"/>
    </owl:Class>
    


    <!-- http://www.opengis.net/ont/gml#MultiSurface -->

    <owl:Class rdf:about="&gml;MultiSurface">
        <rdfs:label xml:lang="en">Multi-Surface</rdfs:label>
        <rdfs:subClassOf rdf:resource="&gml;MultiGeometry"/>
        <rdfs:isDefinedBy rdf:resource="http://www.opengis.net/ont/gml"/>
    </owl:Class>
    


    <!-- http://www.opengis.net/ont/gml#OffsetCurve -->

    <owl:Class rdf:about="&gml;OffsetCurve">
        <rdfs:label xml:lang="en">Offset Curve</rdfs:label>
        <rdfs:subClassOf rdf:resource="&gml;AbstractCurveSegment"/>
        <rdfs:isDefinedBy rdf:resource="http://www.opengis.net/ont/gml"/>
    </owl:Class>
    


    <!-- http://www.opengis.net/ont/gml#OrientableCurve -->

    <owl:Class rdf:about="&gml;OrientableCurve">
        <rdfs:label xml:lang="en">Orientable Curve</rdfs:label>
        <rdfs:subClassOf rdf:resource="&gml;AbstractGeometricPrimitive"/>
        <rdfs:isDefinedBy rdf:resource="http://www.opengis.net/ont/gml"/>
    </owl:Class>
    


    <!-- http://www.opengis.net/ont/gml#OrientableSurface -->

    <owl:Class rdf:about="&gml;OrientableSurface">
        <rdfs:label xml:lang="en">Orientable Surface</rdfs:label>
        <rdfs:subClassOf rdf:resource="&gml;AbstractGeometricPrimitive"/>
        <rdfs:isDefinedBy rdf:resource="http://www.opengis.net/ont/gml"/>
    </owl:Class>
    


    <!-- http://www.opengis.net/ont/gml#Point -->

    <owl:Class rdf:about="&gml;Point">
        <rdfs:label xml:lang="en">Point</rdfs:label>
        <rdfs:subClassOf rdf:resource="&gml;AbstractGeometricPrimitive"/>
        <rdfs:isDefinedBy rdf:resource="http://www.opengis.net/ont/gml"/>
    </owl:Class>
    


    <!-- http://www.opengis.net/ont/gml#Polygon -->

    <owl:Class rdf:about="&gml;Polygon">
        <rdfs:label xml:lang="en">Polygon</rdfs:label>
        <rdfs:subClassOf rdf:resource="&gml;Surface"/>
        <rdfs:isDefinedBy rdf:resource="http://www.opengis.net/ont/gml"/>
    </owl:Class>
    


    <!-- http://www.opengis.net/ont/gml#PolygonPatch -->

    <owl:Class rdf:about="&gml;PolygonPatch">
        <rdfs:label xml:lang="en">Polygon Patch</rdfs:label>
        <rdfs:subClassOf rdf:resource="&gml;AbstractSurfacePatch"/>
        <rdfs:isDefinedBy rdf:resource="http://www.opengis.net/ont/gml"/>
    </owl:Class>
    


    <!-- http://www.opengis.net/ont/gml#PolyhedralSurface -->

    <owl:Class rdf:about="&gml;PolyhedralSurface">
        <rdfs:label xml:lang="en">Polyhedral Surface</rdfs:label>
        <rdfs:subClassOf rdf:resource="&gml;Surface"/>
        <rdfs:isDefinedBy rdf:resource="http://www.opengis.net/ont/gml"/>
    </owl:Class>
    


    <!-- http://www.opengis.net/ont/gml#PolynomialSpline -->

    <owl:Class rdf:about="&gml;PolynomialSpline">
        <rdfs:label xml:lang="en">Polynomial Spline</rdfs:label>
        <rdfs:subClassOf rdf:resource="&gml;SplineCurve"/>
        <rdfs:isDefinedBy rdf:resource="http://www.opengis.net/ont/gml"/>
    </owl:Class>
    


    <!-- http://www.opengis.net/ont/gml#Rectangle -->

    <owl:Class rdf:about="&gml;Rectangle">
        <rdfs:label xml:lang="en">Rectangle</rdfs:label>
        <rdfs:subClassOf rdf:resource="&gml;PolygonPatch"/>
        <rdfs:isDefinedBy rdf:resource="http://www.opengis.net/ont/gml"/>
    </owl:Class>
    


    <!-- http://www.opengis.net/ont/gml#Ring -->

    <owl:Class rdf:about="&gml;Ring">
        <rdfs:label xml:lang="en">Ring</rdfs:label>
        <rdfs:subClassOf rdf:resource="&gml;CompositeCurve"/>
        <rdfs:isDefinedBy rdf:resource="http://www.opengis.net/ont/gml"/>
    </owl:Class>
    


    <!-- http://www.opengis.net/ont/gml#Shell -->

    <owl:Class rdf:about="&gml;Shell">
        <rdfs:label xml:lang="en">Shell</rdfs:label>
        <rdfs:subClassOf rdf:resource="&gml;CompositeSurface"/>
        <rdfs:isDefinedBy rdf:resource="http://www.opengis.net/ont/gml"/>
    </owl:Class>
    


    <!-- http://www.opengis.net/ont/gml#Solid -->

    <owl:Class rdf:about="&gml;Solid">
        <rdfs:label xml:lang="en">Solid</rdfs:label>
        <rdfs:subClassOf rdf:resource="&gml;AbstractGeometricPrimitive"/>
        <rdfs:isDefinedBy rdf:resource="http://www.opengis.net/ont/gml"/>
    </owl:Class>
    


    <!-- http://www.opengis.net/ont/gml#Sphere -->

    <owl:Class rdf:about="&gml;Sphere">
        <rdfs:label xml:lang="en">Sphere</rdfs:label>
        <rdfs:subClassOf rdf:resource="&gml;AbstractGriddedSurface"/>
        <rdfs:isDefinedBy rdf:resource="http://www.opengis.net/ont/gml"/>
    </owl:Class>
    


    <!-- http://www.opengis.net/ont/gml#SplineCurve -->

    <owl:Class rdf:about="&gml;SplineCurve">
        <rdfs:label xml:lang="en">Spline Curve</rdfs:label>
        <rdfs:subClassOf rdf:resource="&gml;AbstractCurveSegment"/>
        <rdfs:isDefinedBy rdf:resource="http://www.opengis.net/ont/gml"/>
    </owl:Class>
    


    <!-- http://www.opengis.net/ont/gml#Surface -->

    <owl:Class rdf:about="&gml;Surface">
        <rdfs:label xml:lang="en">Surface</rdfs:label>
        <rdfs:subClassOf rdf:resource="&gml;AbstractGeometricPrimitive"/>
        <rdfs:subClassOf rdf:resource="&gml;OrientableSurface"/>
        <rdfs:isDefinedBy rdf:resource="http://www.opengis.net/ont/gml"/>
    </owl:Class>
    


    <!-- http://www.opengis.net/ont/gml#Tin -->

    <owl:Class rdf:about="&gml;Tin">
        <rdfs:label xml:lang="en">Triangulated Irregular Network</rdfs:label>
        <rdfs:subClassOf rdf:resource="&gml;TriangulatedSurface"/>
        <rdfs:isDefinedBy rdf:resource="http://www.opengis.net/ont/gml"/>
    </owl:Class>
    


    <!-- http://www.opengis.net/ont/gml#Triangle -->

    <owl:Class rdf:about="&gml;Triangle">
        <rdfs:label xml:lang="en">Triangle</rdfs:label>
        <rdfs:subClassOf rdf:resource="&gml;PolygonPatch"/>
        <rdfs:isDefinedBy rdf:resource="http://www.opengis.net/ont/gml"/>
    </owl:Class>
    


    <!-- http://www.opengis.net/ont/gml#TriangulatedSurface -->

    <owl:Class rdf:about="&gml;TriangulatedSurface">
        <rdfs:label xml:lang="en">Triangulated Surface</rdfs:label>
        <rdfs:subClassOf rdf:resource="&gml;PolyhedralSurface"/>
        <rdfs:isDefinedBy rdf:resource="http://www.opengis.net/ont/gml"/>
    </owl:Class>
    


    <!-- http://www.opengis.net/ont/sf#Curve -->

    <owl:Class rdf:about="&sf;Curve">
        <rdfs:label xml:lang="en">Curve</rdfs:label>
        <rdfs:subClassOf rdf:resource="&sf;Geometry"/>
        <rdfs:comment xml:lang="en">
A Curve is a 1-dimensional geometric object usually stored as a sequence of Points, with the subtype of Curve specifying the form of the interpolation between Points. This specification defines only one subclass of Curve, LineString, which uses linear interpolation between Points.
A Curve is a 1-dimensional geometric object that is the homeomorphic image of a real, closed, interval.
A Curve is simple if it does not pass through the same Point twice with the possible exception of the two end
points.
A Curve is closed if its start Point is equal to its end Point.
The boundary of a closed Curve is empty.
A Curve that is simple and closed is a Ring.
The boundary of a non-closed Curve consists of its two end Points.
A Curve is defined as topologically closed, that is, it contains its endpoints f(a) and f(b).
    </rdfs:comment>
        <rdfs:isDefinedBy rdf:resource="http://www.opengis.net/ont/sf"/>
    </owl:Class>
    


    <!-- http://www.opengis.net/ont/sf#Geometry -->

    <owl:Class rdf:about="&sf;Geometry">
        <rdfs:label xml:lang="en">Geometry</rdfs:label>
        <rdfs:subClassOf rdf:resource="&geosparql;Geometry"/>
        <rdfs:comment xml:lang="en">
Geometry is the root class of the hierarchy.
The instantiable subclasses of Geometry are restricted to 0, 1 and 2-dimensional geometric objects that exist in 2, 3 or 4-dimensional coordinate space (R2, R3 or R4). Geometry values in R2 have points with coordinate values for x and y. Geometry values in R3 have points with coordinate values for x, y and z or for x, y and m. Geometry values in R4 have points with coordinate values for x, y, z and m.
The interpretation of the coordinates is subject to the coordinate reference systems associated to the point. All coordinates within a geometry object should be in the same coordinate reference systems. Each coordinate shall be unambiguously associated to a coordinate reference system either directly or through its containing geometry. The z coordinate of a point is typically, but not necessarily, represents altitude or elevation. The m coordinate represents a measurement.
All Geometry classes described in this specification are defined so that instances of Geometry are topologically closed, i.e. all represented geometries include their boundary as point sets. This does not affect their representation, and open version of the same classes may be used in other circumstances, such as topological representations.
    </rdfs:comment>
        <rdfs:isDefinedBy rdf:resource="http://www.opengis.net/ont/sf"/>
    </owl:Class>
    


    <!-- http://www.opengis.net/ont/sf#GeometryCollection -->

    <owl:Class rdf:about="&sf;GeometryCollection">
        <rdfs:label xml:lang="en">Geometry Collection</rdfs:label>
        <rdfs:subClassOf rdf:resource="&sf;Geometry"/>
        <rdfs:comment xml:lang="en">
A GeometryCollection is a geometric object that is a collection of some number of geometric objects.
All the elements in a GeometryCollection shall be in the same Spatial Reference System. This is also the Spatial Reference System for the GeometryCollection.
GeometryCollection places no other constraints on its elements. Subclasses of GeometryCollection may restrict membership based on dimension and may also place other constraints on the degree of spatial overlap between elements.
    </rdfs:comment>
        <rdfs:isDefinedBy rdf:resource="http://www.opengis.net/ont/sf"/>
    </owl:Class>
    


    <!-- http://www.opengis.net/ont/sf#Line -->

    <owl:Class rdf:about="&sf;Line">
        <rdfs:label xml:lang="en">Line</rdfs:label>
        <rdfs:subClassOf rdf:resource="&sf;LineString"/>
        <rdfs:comment xml:lang="en">
A Line is a LineString with exactly 2 Points.
    </rdfs:comment>
        <rdfs:isDefinedBy rdf:resource="http://www.opengis.net/ont/sf"/>
    </owl:Class>
    


    <!-- http://www.opengis.net/ont/sf#LineString -->

    <owl:Class rdf:about="&sf;LineString">
        <rdfs:label xml:lang="en">Line String</rdfs:label>
        <rdfs:subClassOf rdf:resource="&sf;Curve"/>
        <rdfs:comment xml:lang="en">
A LineString is a Curve with linear interpolation between Points. Each consecutive pair of Points defines a Line segment.
    </rdfs:comment>
        <rdfs:isDefinedBy rdf:resource="http://www.opengis.net/ont/sf"/>
    </owl:Class>
    


    <!-- http://www.opengis.net/ont/sf#LinearRing -->

    <owl:Class rdf:about="&sf;LinearRing">
        <rdfs:label xml:lang="en">Linear Ring</rdfs:label>
        <rdfs:subClassOf rdf:resource="&sf;LineString"/>
        <rdfs:comment xml:lang="en">
A LinearRing is a LineString that is both closed and simple.
    </rdfs:comment>
        <rdfs:isDefinedBy rdf:resource="http://www.opengis.net/ont/sf"/>
    </owl:Class>
    


    <!-- http://www.opengis.net/ont/sf#MultiCurve -->

    <owl:Class rdf:about="&sf;MultiCurve">
        <rdfs:label xml:lang="en">Multi Curve</rdfs:label>
        <rdfs:subClassOf rdf:resource="&sf;GeometryCollection"/>
        <rdfs:comment xml:lang="en">
A MultiCurve is a 1-dimensional GeometryCollection whose elements are Curves.
A MultiCurve defines a set of methods for its subclasses and is included for reasons of extensibility.
A MultiCurve is simple if and only if all of its elements are simple and the only intersections between any two elements occur at Points that are on the boundaries of both elements.
The boundary of a MultiCurve is obtained by applying the mod 2 union rule: A Point is in the boundary of a MultiCurve if it is in the boundaries of an odd number of elements of the MultiCurve.
A MultiCurve is closed if all of its elements are closed. The boundary of a closed MultiCurve is always empty.
A MultiCurve is defined as topologically closed.
    </rdfs:comment>
        <rdfs:isDefinedBy rdf:resource="http://www.opengis.net/ont/sf"/>
    </owl:Class>
    


    <!-- http://www.opengis.net/ont/sf#MultiLineString -->

    <owl:Class rdf:about="&sf;MultiLineString">
        <rdfs:label xml:lang="en">Multi Line String</rdfs:label>
        <rdfs:subClassOf rdf:resource="&sf;MultiCurve"/>
        <rdfs:comment xml:lang="en">
A MultiLineString is a MultiCurve whose elements are LineStrings.
    </rdfs:comment>
        <rdfs:isDefinedBy rdf:resource="http://www.opengis.net/ont/sf"/>
    </owl:Class>
    


    <!-- http://www.opengis.net/ont/sf#MultiPoint -->

    <owl:Class rdf:about="&sf;MultiPoint">
        <rdfs:label xml:lang="en">Multi Point</rdfs:label>
        <rdfs:subClassOf rdf:resource="&sf;GeometryCollection"/>
        <rdfs:comment xml:lang="en">
A MultiPoint is a 0-dimensional GeometryCollection. The elements of a MultiPoint are restricted to Points. ThePoints are not connected or ordered in any semantically important way.
A MultiPoint is simple if no two Points in the MultiPoint are equal (have identical coordinate values in X and Y).
Every MultiPoint is spatially equal to a simple Multipoint.
The boundary of a MultiPoint is the empty set.
    </rdfs:comment>
        <rdfs:isDefinedBy rdf:resource="http://www.opengis.net/ont/sf"/>
    </owl:Class>
    


    <!-- http://www.opengis.net/ont/sf#MultiPolygon -->

    <owl:Class rdf:about="&sf;MultiPolygon">
        <rdfs:label xml:lang="en">Multi Polygon</rdfs:label>
        <rdfs:subClassOf rdf:resource="&sf;MultiSurface"/>
        <rdfs:comment xml:lang="en">
A MultiPolygon is a MultiSurface whose elements are Polygons.
The assertions for MultiPolygons are as follows.
a) The interiors of 2 Polygons that are elements of a MultiPolygon may not intersect.
b) The boundaries of any 2 Polygons that are elements of a MultiPolygon may not cross and may touch at only a finite number of Points.
c) A MultiPolygon is defined as topologically closed.
d) A MultiPolygon may not have cut lines, spikes or punctures, a MultiPolygon is a regular closed Point set,
e) The interior of a MultiPolygon with more than 1 Polygon is not connected; the number of connected components of the interior of a MultiPolygon is equal to the number of Polygons in the MultiPolygon. 
The boundary of a MultiPolygon is a set of closed Curves (LineStrings) corresponding to the boundaries of its element Polygons. Each Curve in the boundary of the MultiPolygon is in the boundary of exactly 1 element Polygon, and every Curve in the boundary of an element Polygon is in the boundary of the MultiPolygon.
    </rdfs:comment>
        <rdfs:isDefinedBy rdf:resource="http://www.opengis.net/ont/sf"/>
    </owl:Class>
    


    <!-- http://www.opengis.net/ont/sf#MultiSurface -->

    <owl:Class rdf:about="&sf;MultiSurface">
        <rdfs:label xml:lang="en">Multi Surface</rdfs:label>
        <rdfs:subClassOf rdf:resource="&sf;GeometryCollection"/>
        <rdfs:comment xml:lang="en">
A MultiSurface is a 2-dimensional GeometryCollection whose elements are Surfaces, all using coordinates from the same coordinate reference system. The geometric interiors of any two Surfaces in a MultiSurface may not intersect in the full coordinate system. The boundaries of any two coplanar elements in a MultiSurface may intersect, at most, at a finite number of Points. If they were to meet along a curve, they could be merged into a single surface.
A MultiSurface may be used to represent heterogeneous surfaces collections of polygons and polyhedral surfaces. It defines a set of methods for its subclasses. The subclass of MultiSurface is MultiPolygon corresponding to a collection of Polygons only. Other collections shall use MultiSurface.
    </rdfs:comment>
        <rdfs:isDefinedBy rdf:resource="http://www.opengis.net/ont/sf"/>
    </owl:Class>
    


    <!-- http://www.opengis.net/ont/sf#Point -->

    <owl:Class rdf:about="&sf;Point">
        <rdfs:label xml:lang="en">Point</rdfs:label>
        <rdfs:subClassOf rdf:resource="&sf;Geometry"/>
        <rdfs:comment xml:lang="en">
A Point is a 0-dimensional geometric object and represents a single location in coordinate space. 
A Point has an x-coordinate value, a y-coordinate value. If called for by the associated Spatial Reference System, it may also have coordinate values for z and m.
The boundary of a Point is the empty set.
    </rdfs:comment>
        <rdfs:isDefinedBy rdf:resource="http://www.opengis.net/ont/sf"/>
    </owl:Class>
    


    <!-- http://www.opengis.net/ont/sf#Polygon -->

    <owl:Class rdf:about="&sf;Polygon">
        <rdfs:label xml:lang="en">Polygon</rdfs:label>
        <rdfs:subClassOf rdf:resource="&sf;Surface"/>
        <rdfs:comment xml:lang="en">
A Polygon is a planar Surface defined by 1 exterior boundary and 0 or more interior boundaries. Each interior boundary defines a hole in the Polygon.
The exterior boundary LinearRing defines the top of the surface which is the side of the surface from which the exterior boundary appears to traverse the boundary in a counter clockwise direction. The interior LinearRings will have the opposite orientation, and appear as clockwise when viewed from the top,
The assertions for Polygons (the rules that define valid Polygons) are as follows:
a) Polygons are topologically closed;
b) The boundary of a Polygon consists of a set of LinearRings that make up its exterior and interior boundaries;
c) No two Rings in the boundary cross and the Rings in the boundary of a Polygon may intersect at a Point but only as a tangent.
d) A Polygon may not have cut lines, spikes or punctures.
e) The interior of every Polygon is a connected point set;
f) The exterior of a Polygon with 1 or more holes is not connected. Each hole defines a connected component of the exterior.
    </rdfs:comment>
        <rdfs:isDefinedBy rdf:resource="http://www.opengis.net/ont/sf"/>
    </owl:Class>
    


    <!-- http://www.opengis.net/ont/sf#PolyhedralSurface -->

    <owl:Class rdf:about="&sf;PolyhedralSurface">
        <rdfs:label xml:lang="en">Polyhedral Surface</rdfs:label>
        <rdfs:subClassOf rdf:resource="&sf;Surface"/>
        <rdfs:comment xml:lang="en">
A PolyhedralSurface is a contiguous collection of polygons, which share common boundary segments. For each pair of polygons that touch, the common boundary shall be expressible as a finite collection of LineStrings. Each such LineString shall be part of the boundary of at most 2 Polygon patches. 
For any two polygons that share a common boundary, the top of the polygon shall be consistent. This means that when two LinearRings from these two Polygons traverse the common boundary segment, they do so in opposite directions. Since the Polyhedral surface is contiguous, all polygons will be thus consistently oriented. This means that a non-oriented surface (such as Mbius band) shall not have single surface representations. They may be represented by a MultiSurface.
If each such LineString is the boundary of exactly 2 Polygon patches, then the PolyhedralSurface is a simple, closed polyhedron and is topologically isomorphic to the surface of a sphere. By the Jordan Surface Theorem (Jordans Theorem for 2-spheres), such polyhedrons enclose a solid topologically isomorphic to the interior of a sphere; the ball. In this case, the top of the surface will either point inward or outward of the enclosed finite solid. If outward, the surface is the exterior boundary of the enclosed surface. If inward, the surface is the interior of the infinite complement of the enclosed solid. A Ball with some number of voids (holes) inside can thus be presented as one exterior boundary shell, and some number in interior boundary shells.
    </rdfs:comment>
        <rdfs:isDefinedBy rdf:resource="http://www.opengis.net/ont/sf"/>
    </owl:Class>
    


    <!-- http://www.opengis.net/ont/sf#Surface -->

    <owl:Class rdf:about="&sf;Surface">
        <rdfs:label xml:lang="en">Surface</rdfs:label>
        <rdfs:subClassOf rdf:resource="&sf;Geometry"/>
        <rdfs:comment xml:lang="en">
A Surface is a 2-dimensional geometric object.
A simple Surface may consists of a single patch that is associated with one exterior boundary and 0 or more interior boundaries. A single such Surface patch in 3-dimensional space is isometric to planar Surfaces, by a simple affine rotation matrix that rotates the patch onto the plane z = 0. If the patch is not vertical, the projection onto the same plane is an isomorphism, and can be represented as a linear transformation, i.e. an affine.
Polyhedral Surfaces are formed by stitching together such simple Surfaces patches along their common boundaries. Such polyhedral Surfaces in a 3-dimensional space may not be planar as a whole, depending on the orientation of their planar normals. If all the patches are in alignment (their normals are parallel), then the whole stitched polyhedral surface is co-planar and can be represented as a single patch if it is connected.
The boundary of a simple Surface is the set of closed Curves corresponding to its exterior and interior boundaries.
A Polygon is a simple Surface that is planar. A PolyhedralSurface is a simple surface, consisting of some number of Polygon patches or facets. If a PolyhedralSurface is closed, then it bounds a solid. A MultiSurface containing a set of closed PolyhedralSurfaces can be used to represent a Solid object with holes.
    </rdfs:comment>
        <rdfs:isDefinedBy rdf:resource="http://www.opengis.net/ont/sf"/>
    </owl:Class>
    


    <!-- http://www.opengis.net/ont/sf#TIN -->

    <owl:Class rdf:about="&sf;TIN">
        <rdfs:label xml:lang="en">Triangulated Irregular Network</rdfs:label>
        <rdfs:subClassOf rdf:resource="&sf;PolyhedralSurface"/>
        <rdfs:comment xml:lang="en">
A TIN (triangulated irregular network) is a PolyhedralSurface consisting only of Triangle patches.
    </rdfs:comment>
        <rdfs:isDefinedBy rdf:resource="http://www.opengis.net/ont/sf"/>
    </owl:Class>
    


    <!-- http://www.opengis.net/ont/sf#Triangle -->

    <owl:Class rdf:about="&sf;Triangle">
        <rdfs:label xml:lang="en">Triangle</rdfs:label>
        <rdfs:subClassOf rdf:resource="&sf;Polygon"/>
        <rdfs:comment xml:lang="en">
 A Triangle is a polygon with 3 distinct, non-collinear vertices and no interior boundary.
    </rdfs:comment>
        <rdfs:isDefinedBy rdf:resource="http://www.opengis.net/ont/sf"/>
    </owl:Class>
    


    <!-- http://www.w3.org/2002/07/owl#Thing -->

    <owl:Class rdf:about="&owl;Thing"/>
    


    <!-- http://www.w3.org/2004/02/skos/core#Collection -->

    <owl:Class rdf:about="&skos;Collection">
        <rdfs:label xml:lang="en">Collection</rdfs:label>
        <owl:disjointWith rdf:resource="&skos;Concept"/>
        <owl:disjointWith rdf:resource="&skos;ConceptScheme"/>
        <skos:definition xml:lang="en">A meaningful collection of concepts.</skos:definition>
        <skos:scopeNote xml:lang="en">Labelled collections can be used where you would like a set of concepts to be displayed under a &#39;node label&#39; in the hierarchy.</skos:scopeNote>
        <rdfs:isDefinedBy rdf:resource="http://www.w3.org/2004/02/skos/core"/>
    </owl:Class>
    


    <!-- http://www.w3.org/2004/02/skos/core#Concept -->

    <owl:Class rdf:about="&skos;Concept">
        <rdfs:label xml:lang="en">Concept</rdfs:label>
        <owl:disjointWith rdf:resource="&skos;ConceptScheme"/>
        <skos:definition xml:lang="en">An idea or notion; a unit of thought.</skos:definition>
        <rdfs:isDefinedBy rdf:resource="http://www.w3.org/2004/02/skos/core"/>
    </owl:Class>
    


    <!-- http://www.w3.org/2004/02/skos/core#ConceptScheme -->

    <owl:Class rdf:about="&skos;ConceptScheme">
        <rdfs:label xml:lang="en">Concept Scheme</rdfs:label>
        <skos:scopeNote xml:lang="en">A concept scheme may be defined to include concepts from different sources.</skos:scopeNote>
        <skos:definition xml:lang="en">A set of concepts, optionally including statements about semantic relationships between those concepts.</skos:definition>
        <skos:example xml:lang="en">Thesauri, classification schemes, subject heading lists, taxonomies, &#39;folksonomies&#39;, and other types of controlled vocabulary are all examples of concept schemes. Concept schemes are also embedded in glossaries and terminologies.</skos:example>
        <rdfs:isDefinedBy rdf:resource="http://www.w3.org/2004/02/skos/core"/>
    </owl:Class>
    


    <!-- http://www.w3.org/2004/02/skos/core#OrderedCollection -->

    <owl:Class rdf:about="&skos;OrderedCollection">
        <rdfs:label xml:lang="en">Ordered Collection</rdfs:label>
        <rdfs:subClassOf rdf:resource="&skos;Collection"/>
        <skos:definition xml:lang="en">An ordered collection of concepts, where both the grouping and the ordering are meaningful.</skos:definition>
        <skos:scopeNote xml:lang="en">Ordered collections can be used where you would like a set of concepts to be displayed in a specific order, and optionally under a &#39;node label&#39;.</skos:scopeNote>
        <rdfs:isDefinedBy rdf:resource="http://www.w3.org/2004/02/skos/core"/>
    </owl:Class>
    


    <!-- ttp://geo.linkeddata.es/def/feature#Cerro -->

    <owl:Class rdf:about="&btn100;Cerro">
        <rdfs:label xml:lang="es">Cerro</rdfs:label>
        <rdfs:subClassOf rdf:resource="&btn100;PuntoAcotado"/>
        <rdfs:comment xml:lang="es">Elevación de tierra aislada y de menor altura que el monte o la montaña.</rdfs:comment>
    </owl:Class>
    


    <!-- ttp://geo.linkeddata.es/def/feature#Collado -->

    <owl:Class rdf:about="&btn100;Collado">
        <rdfs:label xml:lang="es">Collado</rdfs:label>
        <rdfs:subClassOf rdf:resource="&btn100;PuntoAcotado"/>
        <rdfs:comment xml:lang="es">Paso o depresión suave por donde se puede atravesar con facilidad de un lado a otro una montaña o sierra.</rdfs:comment>
    </owl:Class>
    


    <!-- ttp://geo.linkeddata.es/def/feature#Comarca -->

    <owl:Class rdf:about="&btn100;Comarca">
        <rdfs:label xml:lang="es">Comarca</rdfs:label>
        <rdfs:subClassOf rdf:resource="&btn100;EntidadVirtualDeAccidenteOrografico"/>
        <rdfs:comment xml:lang="es">Delimitación que contiene conjunto de municipios oficiales</rdfs:comment>
    </owl:Class>
    


    <!-- ttp://geo.linkeddata.es/def/feature#Cordillera -->

    <owl:Class rdf:about="&btn100;Cordillera">
        <rdfs:label xml:lang="es">Cordillera</rdfs:label>
        <rdfs:subClassOf rdf:resource="&btn100;EntidadVirtualDeAccidenteOrografico"/>
        <rdfs:comment xml:lang="es">Serie de montañas enlazadas entre sí.</rdfs:comment>
    </owl:Class>
    


    <!-- ttp://geo.linkeddata.es/def/feature#CotaMunicipal -->

    <owl:Class rdf:about="&btn100;CotaMunicipal">
        <rdfs:label xml:lang="es">CotaMunicipal</rdfs:label>
        <rdfs:subClassOf rdf:resource="&btn100;PuntoAcotado"/>
    </owl:Class>
    


    <!-- ttp://geo.linkeddata.es/def/feature#CurvaDeNivel -->

    <owl:Class rdf:about="&btn100;CurvaDeNivel">
        <rdfs:label xml:lang="es">CurvaDeNivel</rdfs:label>
        <rdfs:subClassOf rdf:resource="&btn100;Relieve"/>
        <rdfs:subClassOf>
            <owl:Restriction>
                <owl:onProperty rdf:resource="h&btn100;tipoDeGeometria"/>
                <owl:hasValue>Lineal</owl:hasValue>
            </owl:Restriction>
        </rdfs:subClassOf>
        <rdfs:comment xml:lang="es">Se representan como curvas de nivel aquellas líneas que tienen la misma altitud sobre la superficie de referencia, siendo esta altitud un múltiplo de 40 o un múltiplo de 100 (para líneas interpoladas).</rdfs:comment>
    </owl:Class>
    


    <!-- ttp://geo.linkeddata.es/def/feature#CurvaDeNivelAltimetrica -->

    <owl:Class rdf:about="&btn100;CurvaDeNivelAltimetrica">
        <rdfs:label xml:lang="es">CurvaDeNivelAltimetrica</rdfs:label>
        <rdfs:subClassOf rdf:resource="&btn100;CurvaDeNivel"/>
    </owl:Class>
    


    <!-- ttp://geo.linkeddata.es/def/feature#CurvaDeNivelBatimetrica -->

    <owl:Class rdf:about="&btn100;CurvaDeNivelBatimetrica">
        <rdfs:label xml:lang="es">CurvaDeNivelBatimetrica</rdfs:label>
        <rdfs:subClassOf rdf:resource="&btn100;CurvaDeNivel"/>
        <rdfs:subClassOf>
            <owl:Class>
                <owl:unionOf rdf:parseType="Collection">
                    <owl:Restriction>
                        <owl:onProperty rdf:resource="&btn100;categoria"/>
                        <owl:hasValue rdf:datatype="&xsd;string">genérica (Curva de nivel con altitud cada 20 m)</owl:hasValue>
                    </owl:Restriction>
                    <owl:Restriction>
                        <owl:onProperty rdf:resource="&btn100;categoria"/>
                        <owl:hasValue rdf:datatype="&xsd;string">maestra (Curva de nivel con altitud múltiplo de 100 m)</owl:hasValue>
                    </owl:Restriction>
                </owl:unionOf>
            </owl:Class>
        </rdfs:subClassOf>
    </owl:Class>
    


    <!-- ttp://geo.linkeddata.es/def/feature#EntidadVirtualDeAccidenteOrografico -->

    <owl:Class rdf:about="&btn100;EntidadVirtualDeAccidenteOrografico">
        <rdfs:label xml:lang="es">EntidadVirtualDeAccidenteOrografico</rdfs:label>
        <rdfs:subClassOf rdf:resource="&btn100;Relieve"/>
        <rdfs:comment xml:lang="es">Línea sobre la que iría colocado el texto del accidente orográfico que representa.</rdfs:comment>
    </owl:Class>
    


    <!-- ttp://geo.linkeddata.es/def/feature#Montanna -->

    <owl:Class rdf:about="&btn100;Montanna">
        <rdfs:label xml:lang="es">Montanna</rdfs:label>
        <rdfs:subClassOf rdf:resource="&btn100;EntidadVirtualDeAccidenteOrografico"/>
        <rdfs:comment xml:lang="es">Gran elevación natural del terreno.</rdfs:comment>
    </owl:Class>
    


    <!-- ttp://geo.linkeddata.es/def/feature#Paraje -->

    <owl:Class rdf:about="&btn100;Paraje">
        <rdfs:label xml:lang="es">Paraje</rdfs:label>
        <rdfs:subClassOf rdf:resource="&btn100;EntidadVirtualDeAccidenteOrografico"/>
        <rdfs:comment xml:lang="es">Lugar, sitio con interés.</rdfs:comment>
    </owl:Class>
    


    <!-- ttp://geo.linkeddata.es/def/feature#Pico -->

    <owl:Class rdf:about="&btn100;Pico">
        <rdfs:label xml:lang="es">Pico</rdfs:label>
        <rdfs:subClassOf rdf:resource="&btn100;PuntoAcotado"/>
        <rdfs:comment xml:lang="es">Montaña de cumbre puntiaguda</rdfs:comment>
    </owl:Class>
    


    <!-- ttp://geo.linkeddata.es/def/feature#PuertoDeMontanna -->

    <owl:Class rdf:about="&btn100;PuertoDeMontanna">
        <rdfs:label xml:lang="es">PuertoDeMontanna</rdfs:label>
        <rdfs:subClassOf rdf:resource="&btn100;PuntoAcotado"/>
        <rdfs:comment xml:lang="es">Paso entre montañas.</rdfs:comment>
    </owl:Class>
    


    <!-- ttp://geo.linkeddata.es/def/feature#PuntoAcotado -->

    <owl:Class rdf:about="&btn100;PuntoAcotado">
        <rdfs:label xml:lang="es">PuntoAcotado</rdfs:label>
        <rdfs:subClassOf rdf:resource="&btn100;Relieve"/>
        <rdfs:subClassOf>
            <owl:Restriction>
                <owl:onProperty rdf:resource="h&btn100;tipoDeGeometria"/>
                <owl:hasValue>Puntual</owl:hasValue>
            </owl:Restriction>
        </rdfs:subClassOf>
        <rdfs:comment xml:lang="es">Se define como puntos acotados a aquellos puntos con cota que poseen una ubicación representativa del relieve y complementan la información facilitada por las curvas de nivel.</rdfs:comment>
    </owl:Class>
    


    <!-- ttp://geo.linkeddata.es/def/feature#Region -->

    <owl:Class rdf:about="&btn100;Region">
        <rdfs:label xml:lang="es">Region</rdfs:label>
        <rdfs:subClassOf rdf:resource="&btn100;EntidadVirtualDeAccidenteOrografico"/>
        <rdfs:comment xml:lang="es">Delimitación que contiene conjunto de municipios históricos</rdfs:comment>
    </owl:Class>
    


    <!-- ttp://geo.linkeddata.es/def/feature#Relieve -->

    <owl:Class rdf:about="&btn100;Relieve">
        <rdfs:label xml:lang="es">Relieve</rdfs:label>
        <rdfs:subClassOf rdf:resource="&geosparql;Feature"/>
        <rdfs:subClassOf>
            <owl:Restriction>
                <owl:onProperty rdf:resource="h&btn100;grupoTematico"/>
                <owl:hasValue>Relieve</owl:hasValue>
            </owl:Restriction>
        </rdfs:subClassOf>
        <rdfs:comment xml:lang="es">El relieve es el conjunto de formas de la superficie terrestre que resalta sobre una superficie horizontal</rdfs:comment>
    </owl:Class>
    


    <!-- ttp://geo.linkeddata.es/def/feature#Sierra -->

    <owl:Class rdf:about="&btn100;Sierra">
        <rdfs:label xml:lang="es">Sierra</rdfs:label>
        <rdfs:subClassOf rdf:resource="&btn100;EntidadVirtualDeAccidenteOrografico"/>
        <rdfs:comment xml:lang="es">Conjunto de montañas o Parte de una cordillera.</rdfs:comment>
    </owl:Class>
    


    <!-- 
    ///////////////////////////////////////////////////////////////////////////////////////
    //
    // Individuals
    //
    ///////////////////////////////////////////////////////////////////////////////////////
     -->

    


    <!-- http://aims.fao.org/aos/geopolitical.owl#AMU -->

    <owl:NamedIndividual rdf:about="&geopolitical;AMU">
        <geopolitical:sourceCreator rdf:datatype="&xsd;string">UMA</geopolitical:sourceCreator>
        <terms:source rdf:datatype="&xsd;string">UMA http://www.maghrebarabe.org/en/index.cfm</terms:source>
        <geopolitical:sourceIdentifier xml:lang="ar">http://www.maghrebarabe.org/ar/</geopolitical:sourceIdentifier>
        <geopolitical:sourceIdentifier xml:lang="en">http://www.maghrebarabe.org/en/index.cfm</geopolitical:sourceIdentifier>
        <geopolitical:sourceIdentifier xml:lang="fr">http://www.maghrebarabe.org/fr/</geopolitical:sourceIdentifier>
    </owl:NamedIndividual>
    


    <!-- http://aims.fao.org/aos/geopolitical.owl#Afghanistan -->

    <owl:NamedIndividual rdf:about="&geopolitical;Afghanistan"/>
    


    <!-- http://aims.fao.org/aos/geopolitical.owl#Africa -->

    <owl:NamedIndividual rdf:about="&geopolitical;Africa"/>
    


    <!-- http://aims.fao.org/aos/geopolitical.owl#Albania -->

    <owl:NamedIndividual rdf:about="&geopolitical;Albania"/>
    


    <!-- http://aims.fao.org/aos/geopolitical.owl#Algeria -->

    <owl:NamedIndividual rdf:about="&geopolitical;Algeria"/>
    


    <!-- http://aims.fao.org/aos/geopolitical.owl#American_Samoa -->

    <owl:NamedIndividual rdf:about="&geopolitical;American_Samoa"/>
    


    <!-- http://aims.fao.org/aos/geopolitical.owl#Americas -->

    <owl:NamedIndividual rdf:about="&geopolitical;Americas"/>
    


    <!-- http://aims.fao.org/aos/geopolitical.owl#Andorra -->

    <owl:NamedIndividual rdf:about="&geopolitical;Andorra"/>
    


    <!-- http://aims.fao.org/aos/geopolitical.owl#Angola -->

    <owl:NamedIndividual rdf:about="&geopolitical;Angola"/>
    


    <!-- http://aims.fao.org/aos/geopolitical.owl#Anguilla -->

    <owl:NamedIndividual rdf:about="&geopolitical;Anguilla"/>
    


    <!-- http://aims.fao.org/aos/geopolitical.owl#Antarctica -->

    <owl:NamedIndividual rdf:about="&geopolitical;Antarctica"/>
    


    <!-- http://aims.fao.org/aos/geopolitical.owl#Antigua_and_Barbuda -->

    <owl:NamedIndividual rdf:about="&geopolitical;Antigua_and_Barbuda"/>
    


    <!-- http://aims.fao.org/aos/geopolitical.owl#Argentina -->

    <owl:NamedIndividual rdf:about="&geopolitical;Argentina"/>
    


    <!-- http://aims.fao.org/aos/geopolitical.owl#Armenia -->

    <owl:NamedIndividual rdf:about="&geopolitical;Armenia"/>
    


    <!-- http://aims.fao.org/aos/geopolitical.owl#Aruba -->

    <owl:NamedIndividual rdf:about="&geopolitical;Aruba"/>
    


    <!-- http://aims.fao.org/aos/geopolitical.owl#Asia -->

    <owl:NamedIndividual rdf:about="&geopolitical;Asia"/>
    


    <!-- http://aims.fao.org/aos/geopolitical.owl#Australia -->

    <owl:NamedIndividual rdf:about="&geopolitical;Australia"/>
    


    <!-- http://aims.fao.org/aos/geopolitical.owl#Australia_and_New_Zealand -->

    <owl:NamedIndividual rdf:about="&geopolitical;Australia_and_New_Zealand"/>
    


    <!-- http://aims.fao.org/aos/geopolitical.owl#Austria -->

    <owl:NamedIndividual rdf:about="&geopolitical;Austria"/>
    


    <!-- http://aims.fao.org/aos/geopolitical.owl#Azerbaijan -->

    <owl:NamedIndividual rdf:about="&geopolitical;Azerbaijan"/>
    


    <!-- http://aims.fao.org/aos/geopolitical.owl#Bahamas_the -->

    <owl:NamedIndividual rdf:about="&geopolitical;Bahamas_the"/>
    


    <!-- http://aims.fao.org/aos/geopolitical.owl#Bahrain -->

    <owl:NamedIndividual rdf:about="&geopolitical;Bahrain"/>
    


    <!-- http://aims.fao.org/aos/geopolitical.owl#Bangladesh -->

    <owl:NamedIndividual rdf:about="&geopolitical;Bangladesh"/>
    


    <!-- http://aims.fao.org/aos/geopolitical.owl#Barbados -->

    <owl:NamedIndividual rdf:about="&geopolitical;Barbados"/>
    


    <!-- http://aims.fao.org/aos/geopolitical.owl#Belarus -->

    <owl:NamedIndividual rdf:about="&geopolitical;Belarus"/>
    


    <!-- http://aims.fao.org/aos/geopolitical.owl#Belgium -->

    <owl:NamedIndividual rdf:about="&geopolitical;Belgium"/>
    


    <!-- http://aims.fao.org/aos/geopolitical.owl#Belize -->

    <owl:NamedIndividual rdf:about="&geopolitical;Belize"/>
    


    <!-- http://aims.fao.org/aos/geopolitical.owl#Benin -->

    <owl:NamedIndividual rdf:about="&geopolitical;Benin"/>
    


    <!-- http://aims.fao.org/aos/geopolitical.owl#Bermuda -->

    <owl:NamedIndividual rdf:about="&geopolitical;Bermuda"/>
    


    <!-- http://aims.fao.org/aos/geopolitical.owl#Bhutan -->

    <owl:NamedIndividual rdf:about="&geopolitical;Bhutan"/>
    


    <!-- http://aims.fao.org/aos/geopolitical.owl#Bolivia -->

    <owl:NamedIndividual rdf:about="&geopolitical;Bolivia"/>
    


    <!-- http://aims.fao.org/aos/geopolitical.owl#Bonaire_Sint_Eustatius_and_Saba -->

    <owl:NamedIndividual rdf:about="&geopolitical;Bonaire_Sint_Eustatius_and_Saba"/>
    


    <!-- http://aims.fao.org/aos/geopolitical.owl#Bosnia_and_Herzegovina -->

    <owl:NamedIndividual rdf:about="&geopolitical;Bosnia_and_Herzegovina"/>
    


    <!-- http://aims.fao.org/aos/geopolitical.owl#Botswana -->

    <owl:NamedIndividual rdf:about="&geopolitical;Botswana"/>
    


    <!-- http://aims.fao.org/aos/geopolitical.owl#Brazil -->

    <owl:NamedIndividual rdf:about="&geopolitical;Brazil"/>
    


    <!-- http://aims.fao.org/aos/geopolitical.owl#British_Virgin_Islands -->

    <owl:NamedIndividual rdf:about="&geopolitical;British_Virgin_Islands"/>
    


    <!-- http://aims.fao.org/aos/geopolitical.owl#Brunei_Darussalam -->

    <owl:NamedIndividual rdf:about="&geopolitical;Brunei_Darussalam"/>
    


    <!-- http://aims.fao.org/aos/geopolitical.owl#Bulgaria -->

    <owl:NamedIndividual rdf:about="&geopolitical;Bulgaria"/>
    


    <!-- http://aims.fao.org/aos/geopolitical.owl#Burkina_Faso -->

    <owl:NamedIndividual rdf:about="&geopolitical;Burkina_Faso"/>
    


    <!-- http://aims.fao.org/aos/geopolitical.owl#Burundi -->

    <owl:NamedIndividual rdf:about="&geopolitical;Burundi"/>
    


    <!-- http://aims.fao.org/aos/geopolitical.owl#CAC -->

    <owl:NamedIndividual rdf:about="&geopolitical;CAC">
        <geopolitical:sourceModified rdf:datatype="&xsd;string">2010-08-31</geopolitical:sourceModified>
        <geopolitical:sourceCreator rdf:datatype="&xsd;string">CAC</geopolitical:sourceCreator>
        <terms:source rdf:datatype="&xsd;string">CAC http://www.sica.int/busqueda/busqueda_basica.aspx?IdCat=29&amp;IdMod=6&amp;IdEnt=695&amp;IdEntStyle=690&amp;Indv=2</terms:source>
        <geopolitical:sourceIdentifier xml:lang="es">http://www.sica.int/busqueda/busqueda_basica.aspx?IdCat=29&amp;IdMod=6&amp;IdEnt=695&amp;IdEntStyle=690&amp;Indv=2</geopolitical:sourceIdentifier>
    </owl:NamedIndividual>
    


    <!-- http://aims.fao.org/aos/geopolitical.owl#CAEU -->

    <owl:NamedIndividual rdf:about="&geopolitical;CAEU">
        <geopolitical:sourceModified rdf:datatype="&xsd;string">2010-08-16</geopolitical:sourceModified>
        <geopolitical:sourceCreator rdf:datatype="&xsd;string">Wikipedia</geopolitical:sourceCreator>
        <terms:source rdf:datatype="&xsd;string">Wikipedia http://en.wikipedia.org/wiki/Council_of_Arab_Economic_Unity</terms:source>
        <geopolitical:sourceIdentifier xml:lang="en">http://en.wikipedia.org/wiki/Council_of_Arab_Economic_Unity</geopolitical:sourceIdentifier>
    </owl:NamedIndividual>
    


    <!-- http://aims.fao.org/aos/geopolitical.owl#CAN -->

    <owl:NamedIndividual rdf:about="&geopolitical;CAN">
        <geopolitical:sourceCreator rdf:datatype="&xsd;string">CAN</geopolitical:sourceCreator>
        <terms:source rdf:datatype="&xsd;string">CAN http://www.comunidadandina.org/</terms:source>
        <geopolitical:sourceIdentifier rdf:datatype="&xsd;string">http://www.comunidadandina.org/index.htm</geopolitical:sourceIdentifier>
        <geopolitical:sourceIdentifier xml:lang="en">http://www.comunidadandina.org/endex.htm</geopolitical:sourceIdentifier>
    </owl:NamedIndividual>
    


    <!-- http://aims.fao.org/aos/geopolitical.owl#CARICOM -->

    <owl:NamedIndividual rdf:about="&geopolitical;CARICOM">
        <geopolitical:sourceCreator rdf:datatype="&xsd;string">CARICOM</geopolitical:sourceCreator>
        <terms:source rdf:datatype="&xsd;string">CARICOM http://www.caricom.org/</terms:source>
        <geopolitical:sourceIdentifier xml:lang="en">http://www.caricom.org/</geopolitical:sourceIdentifier>
    </owl:NamedIndividual>
    


    <!-- http://aims.fao.org/aos/geopolitical.owl#CARICOM_1985 -->

    <owl:NamedIndividual rdf:about="&geopolitical;CARICOM_1985"/>
    


    <!-- http://aims.fao.org/aos/geopolitical.owl#CARIFORUM -->

    <owl:NamedIndividual rdf:about="&geopolitical;CARIFORUM"/>
    


    <!-- http://aims.fao.org/aos/geopolitical.owl#CCASG -->

    <owl:NamedIndividual rdf:about="&geopolitical;CCASG">
        <geopolitical:sourceCreator rdf:datatype="&xsd;string">CCASG</geopolitical:sourceCreator>
        <terms:source rdf:datatype="&xsd;string">CCASG http://www.gcc-sg.org/eng/index.php</terms:source>
        <geopolitical:sourceIdentifier xml:lang="ar">http://www.gcc-sg.org/</geopolitical:sourceIdentifier>
        <geopolitical:sourceIdentifier xml:lang="en">http://www.gcc-sg.org/eng/index.php</geopolitical:sourceIdentifier>
    </owl:NamedIndividual>
    


    <!-- http://aims.fao.org/aos/geopolitical.owl#CEEAC -->

    <owl:NamedIndividual rdf:about="&geopolitical;CEEAC">
        <geopolitical:sourceCreator rdf:datatype="&xsd;string">CEEAC</geopolitical:sourceCreator>
        <terms:source rdf:datatype="&xsd;string">CEEAC http://www.ceeac-eccas.org/</terms:source>
        <geopolitical:sourceIdentifier xml:lang="fr">http://www.ceeac-eccas.org/</geopolitical:sourceIdentifier>
    </owl:NamedIndividual>
    


    <!-- http://aims.fao.org/aos/geopolitical.owl#CEMAC -->

    <owl:NamedIndividual rdf:about="&geopolitical;CEMAC">
        <geopolitical:sourceModified rdf:datatype="&xsd;string">2010-09-01</geopolitical:sourceModified>
        <geopolitical:sourceCreator rdf:datatype="&xsd;string">CEMAC</geopolitical:sourceCreator>
        <terms:source rdf:datatype="&xsd;string">CEMAC http://www.cemac.int/</terms:source>
        <geopolitical:sourceIdentifier xml:lang="fr">http://www.cemac.int/</geopolitical:sourceIdentifier>
    </owl:NamedIndividual>
    


    <!-- http://aims.fao.org/aos/geopolitical.owl#CEN_SAD -->

    <owl:NamedIndividual rdf:about="&geopolitical;CEN_SAD">
        <geopolitical:sourceCreator rdf:datatype="&xsd;string">CEN-SAD</geopolitical:sourceCreator>
        <terms:source rdf:datatype="&xsd;string">CEN-SAD http://www.cen-sad.org/new/?lang=english</terms:source>
        <geopolitical:sourceIdentifier xml:lang="en">http://www.cen-sad.org/new/?lang=english</geopolitical:sourceIdentifier>
    </owl:NamedIndividual>
    


    <!-- http://aims.fao.org/aos/geopolitical.owl#CEN_SAD_1998 -->

    <owl:NamedIndividual rdf:about="&geopolitical;CEN_SAD_1998"/>
    


    <!-- http://aims.fao.org/aos/geopolitical.owl#COMESA -->

    <owl:NamedIndividual rdf:about="&geopolitical;COMESA">
        <geopolitical:sourceModified rdf:datatype="&xsd;string">2010-08-31</geopolitical:sourceModified>
        <geopolitical:sourceCreator rdf:datatype="&xsd;string">COMEDA</geopolitical:sourceCreator>
        <terms:source rdf:datatype="&xsd;string">COMEDA http://www.comesa.int/</terms:source>
        <geopolitical:sourceIdentifier xml:lang="en">http://www.comesa.int/</geopolitical:sourceIdentifier>
    </owl:NamedIndividual>
    


    <!-- http://aims.fao.org/aos/geopolitical.owl#COMESA_1994 -->

    <owl:NamedIndividual rdf:about="&geopolitical;COMESA_1994"/>
    


    <!-- http://aims.fao.org/aos/geopolitical.owl#Cambodia -->

    <owl:NamedIndividual rdf:about="&geopolitical;Cambodia"/>
    


    <!-- http://aims.fao.org/aos/geopolitical.owl#Cameroon -->

    <owl:NamedIndividual rdf:about="&geopolitical;Cameroon"/>
    


    <!-- http://aims.fao.org/aos/geopolitical.owl#Canada -->

    <owl:NamedIndividual rdf:about="&geopolitical;Canada"/>
    


    <!-- http://aims.fao.org/aos/geopolitical.owl#Cape_Verde -->

    <owl:NamedIndividual rdf:about="&geopolitical;Cape_Verde"/>
    


    <!-- http://aims.fao.org/aos/geopolitical.owl#Caribbean -->

    <owl:NamedIndividual rdf:about="&geopolitical;Caribbean"/>
    


    <!-- http://aims.fao.org/aos/geopolitical.owl#Cayman_Islands -->

    <owl:NamedIndividual rdf:about="&geopolitical;Cayman_Islands"/>
    


    <!-- http://aims.fao.org/aos/geopolitical.owl#Central_African_Republic_the -->

    <owl:NamedIndividual rdf:about="&geopolitical;Central_African_Republic_the"/>
    


    <!-- http://aims.fao.org/aos/geopolitical.owl#Chad -->

    <owl:NamedIndividual rdf:about="&geopolitical;Chad"/>
    


    <!-- http://aims.fao.org/aos/geopolitical.owl#Chile -->

    <owl:NamedIndividual rdf:about="&geopolitical;Chile"/>
    


    <!-- http://aims.fao.org/aos/geopolitical.owl#China -->

    <owl:NamedIndividual rdf:about="&geopolitical;China"/>
    


    <!-- http://aims.fao.org/aos/geopolitical.owl#Colombia -->

    <owl:NamedIndividual rdf:about="&geopolitical;Colombia"/>
    


    <!-- http://aims.fao.org/aos/geopolitical.owl#Comoros_the -->

    <owl:NamedIndividual rdf:about="&geopolitical;Comoros_the"/>
    


    <!-- http://aims.fao.org/aos/geopolitical.owl#Congo_the -->

    <owl:NamedIndividual rdf:about="&geopolitical;Congo_the"/>
    


    <!-- http://aims.fao.org/aos/geopolitical.owl#Cook_Islands_the -->

    <owl:NamedIndividual rdf:about="&geopolitical;Cook_Islands_the"/>
    


    <!-- http://aims.fao.org/aos/geopolitical.owl#Costa_Rica -->

    <owl:NamedIndividual rdf:about="&geopolitical;Costa_Rica"/>
    


    <!-- http://aims.fao.org/aos/geopolitical.owl#Cote_d_Ivoire -->

    <owl:NamedIndividual rdf:about="&geopolitical;Cote_d_Ivoire"/>
    


    <!-- http://aims.fao.org/aos/geopolitical.owl#Croatia -->

    <owl:NamedIndividual rdf:about="&geopolitical;Croatia"/>
    


    <!-- http://aims.fao.org/aos/geopolitical.owl#Cuba -->

    <owl:NamedIndividual rdf:about="&geopolitical;Cuba"/>
    


    <!-- http://aims.fao.org/aos/geopolitical.owl#Curacao -->

    <owl:NamedIndividual rdf:about="&geopolitical;Curacao"/>
    


    <!-- http://aims.fao.org/aos/geopolitical.owl#Cyprus -->

    <owl:NamedIndividual rdf:about="&geopolitical;Cyprus"/>
    


    <!-- http://aims.fao.org/aos/geopolitical.owl#Czech_Republic_the -->

    <owl:NamedIndividual rdf:about="&geopolitical;Czech_Republic_the"/>
    


    <!-- http://aims.fao.org/aos/geopolitical.owl#Czechoslovakia -->

    <owl:NamedIndividual rdf:about="&geopolitical;Czechoslovakia"/>
    


    <!-- http://aims.fao.org/aos/geopolitical.owl#Democratic_People_s_Republic_of_Korea_the -->

    <owl:NamedIndividual rdf:about="&geopolitical;Democratic_People_s_Republic_of_Korea_the"/>
    


    <!-- http://aims.fao.org/aos/geopolitical.owl#Democratic_Republic_of_the_Congo -->

    <owl:NamedIndividual rdf:about="&geopolitical;Democratic_Republic_of_the_Congo"/>
    


    <!-- http://aims.fao.org/aos/geopolitical.owl#Democratic_Yemen -->

    <owl:NamedIndividual rdf:about="&geopolitical;Democratic_Yemen"/>
    


    <!-- http://aims.fao.org/aos/geopolitical.owl#Denmark -->

    <owl:NamedIndividual rdf:about="&geopolitical;Denmark"/>
    


    <!-- http://aims.fao.org/aos/geopolitical.owl#Djibouti -->

    <owl:NamedIndividual rdf:about="&geopolitical;Djibouti"/>
    


    <!-- http://aims.fao.org/aos/geopolitical.owl#Dominica -->

    <owl:NamedIndividual rdf:about="&geopolitical;Dominica"/>
    


    <!-- http://aims.fao.org/aos/geopolitical.owl#Dominican_Republic_the -->

    <owl:NamedIndividual rdf:about="&geopolitical;Dominican_Republic_the"/>
    


    <!-- http://aims.fao.org/aos/geopolitical.owl#ECO -->

    <owl:NamedIndividual rdf:about="&geopolitical;ECO">
        <geopolitical:sourceModified rdf:datatype="&xsd;string">2010-08-30</geopolitical:sourceModified>
        <geopolitical:sourceCreator rdf:datatype="&xsd;string">ECO</geopolitical:sourceCreator>
        <terms:source rdf:datatype="&xsd;string">ECO http://www.ecosecretariat.org/</terms:source>
        <geopolitical:sourceIdentifier xml:lang="en">http://www.ecosecretariat.org/</geopolitical:sourceIdentifier>
    </owl:NamedIndividual>
    


    <!-- http://aims.fao.org/aos/geopolitical.owl#ECOWAS -->

    <owl:NamedIndividual rdf:about="&geopolitical;ECOWAS">
        <geopolitical:sourceModified rdf:datatype="&xsd;string">2010-04-21</geopolitical:sourceModified>
        <geopolitical:sourceCreator rdf:datatype="&xsd;string">ECOWAS</geopolitical:sourceCreator>
        <terms:source rdf:datatype="&xsd;string">ECOWAS http://www.ecowas.int/</terms:source>
        <geopolitical:sourceIdentifier xml:lang="en">http://www.ecowas.int/</geopolitical:sourceIdentifier>
        <geopolitical:sourceIdentifier xml:lang="fr">http://www.ecowas.int/?lang=fr</geopolitical:sourceIdentifier>
    </owl:NamedIndividual>
    


    <!-- http://aims.fao.org/aos/geopolitical.owl#ECOWAS_1985 -->

    <owl:NamedIndividual rdf:about="&geopolitical;ECOWAS_1985"/>
    


    <!-- http://aims.fao.org/aos/geopolitical.owl#EU -->

    <owl:NamedIndividual rdf:about="&geopolitical;EU">
        <geopolitical:sourceCreator rdf:datatype="&xsd;string">EU</geopolitical:sourceCreator>
        <terms:source rdf:datatype="&xsd;string">EU http://europa.eu/index_en.htm</terms:source>
        <geopolitical:sourceIdentifier xml:lang="en">http://europa.eu/index_en.htm</geopolitical:sourceIdentifier>
        <geopolitical:sourceIdentifier xml:lang="es">http://europa.eu/index_es.htm</geopolitical:sourceIdentifier>
        <geopolitical:sourceIdentifier xml:lang="fr">http://europa.eu/index_fr.htm</geopolitical:sourceIdentifier>
    </owl:NamedIndividual>
    


    <!-- http://aims.fao.org/aos/geopolitical.owl#Ecuador -->

    <owl:NamedIndividual rdf:about="&geopolitical;Ecuador"/>
    


    <!-- http://aims.fao.org/aos/geopolitical.owl#Egypt -->

    <owl:NamedIndividual rdf:about="&geopolitical;Egypt"/>
    


    <!-- http://aims.fao.org/aos/geopolitical.owl#El_Salvador -->

    <owl:NamedIndividual rdf:about="&geopolitical;El_Salvador"/>
    


    <!-- http://aims.fao.org/aos/geopolitical.owl#Equatorial_Guinea -->

    <owl:NamedIndividual rdf:about="&geopolitical;Equatorial_Guinea"/>
    


    <!-- http://aims.fao.org/aos/geopolitical.owl#Eritrea -->

    <owl:NamedIndividual rdf:about="&geopolitical;Eritrea"/>
    


    <!-- http://aims.fao.org/aos/geopolitical.owl#Estonia -->

    <owl:NamedIndividual rdf:about="&geopolitical;Estonia"/>
    


    <!-- http://aims.fao.org/aos/geopolitical.owl#Ethiopia -->

    <owl:NamedIndividual rdf:about="&geopolitical;Ethiopia"/>
    


    <!-- http://aims.fao.org/aos/geopolitical.owl#Ethiopia_1993 -->

    <owl:NamedIndividual rdf:about="&geopolitical;Ethiopia_1993"/>
    


    <!-- http://aims.fao.org/aos/geopolitical.owl#Europe -->

    <owl:NamedIndividual rdf:about="&geopolitical;Europe"/>
    


    <!-- http://aims.fao.org/aos/geopolitical.owl#FAO -->

    <owl:NamedIndividual rdf:about="&geopolitical;FAO">
        <geopolitical:sourceCreator rdf:datatype="&xsd;string">FAO Terminology</geopolitical:sourceCreator>
        <terms:source rdf:datatype="&xsd;string">FAO Terminology http://termportal.fao.org/faonocs/main/start.do?lang=en&amp;lang2=en</terms:source>
        <geopolitical:sourceIdentifier xml:lang="en">http://termportal.fao.org/faonocs/main/start.do?lang=en&amp;lang2=en</geopolitical:sourceIdentifier>
    </owl:NamedIndividual>
    


    <!-- http://aims.fao.org/aos/geopolitical.owl#FAO_2006 -->

    <owl:NamedIndividual rdf:about="&geopolitical;FAO_2006"/>
    


    <!-- http://aims.fao.org/aos/geopolitical.owl#FAO_2007 -->

    <owl:NamedIndividual rdf:about="&geopolitical;FAO_2007">
        <geopolitical:sourceCreator rdf:datatype="&xsd;string">FAO Terminology</geopolitical:sourceCreator>
        <terms:source rdf:datatype="&xsd;string">FAO Terminology http://termportal.fao.org/faonocs/main/start.do?lang=en&amp;lang2=en</terms:source>
        <geopolitical:sourceIdentifier xml:lang="en">http://termportal.fao.org/faonocs/main/start.do?lang=en&amp;lang2=en</geopolitical:sourceIdentifier>
    </owl:NamedIndividual>
    


    <!-- http://aims.fao.org/aos/geopolitical.owl#Falkland_Is -->

    <owl:NamedIndividual rdf:about="&geopolitical;Falkland_Is"/>
    


    <!-- http://aims.fao.org/aos/geopolitical.owl#Faroe_Islands -->

    <owl:NamedIndividual rdf:about="&geopolitical;Faroe_Islands">
        <rdfs:comment rdf:datatype="&xsd;string">associate member of FAO</rdfs:comment>
    </owl:NamedIndividual>
    


    <!-- http://aims.fao.org/aos/geopolitical.owl#Federal_Republic_of_Germany_the -->

    <owl:NamedIndividual rdf:about="&geopolitical;Federal_Republic_of_Germany_the"/>
    


    <!-- http://aims.fao.org/aos/geopolitical.owl#Fiji -->

    <owl:NamedIndividual rdf:about="&geopolitical;Fiji"/>
    


    <!-- http://aims.fao.org/aos/geopolitical.owl#Finland -->

    <owl:NamedIndividual rdf:about="&geopolitical;Finland"/>
    


    <!-- http://aims.fao.org/aos/geopolitical.owl#France -->

    <owl:NamedIndividual rdf:about="&geopolitical;France"/>
    


    <!-- http://aims.fao.org/aos/geopolitical.owl#French_Guiana -->

    <owl:NamedIndividual rdf:about="&geopolitical;French_Guiana"/>
    


    <!-- http://aims.fao.org/aos/geopolitical.owl#French_Polynesia -->

    <owl:NamedIndividual rdf:about="&geopolitical;French_Polynesia"/>
    


    <!-- http://aims.fao.org/aos/geopolitical.owl#Gabon -->

    <owl:NamedIndividual rdf:about="&geopolitical;Gabon"/>
    


    <!-- http://aims.fao.org/aos/geopolitical.owl#Gambia__the -->

    <owl:NamedIndividual rdf:about="&geopolitical;Gambia__the"/>
    


    <!-- http://aims.fao.org/aos/geopolitical.owl#Georgia -->

    <owl:NamedIndividual rdf:about="&geopolitical;Georgia"/>
    


    <!-- http://aims.fao.org/aos/geopolitical.owl#German_Democratic_Republic_the -->

    <owl:NamedIndividual rdf:about="&geopolitical;German_Democratic_Republic_the"/>
    


    <!-- http://aims.fao.org/aos/geopolitical.owl#Germany -->

    <owl:NamedIndividual rdf:about="&geopolitical;Germany"/>
    


    <!-- http://aims.fao.org/aos/geopolitical.owl#Ghana -->

    <owl:NamedIndividual rdf:about="&geopolitical;Ghana"/>
    


    <!-- http://aims.fao.org/aos/geopolitical.owl#Gibraltar -->

    <owl:NamedIndividual rdf:about="&geopolitical;Gibraltar"/>
    


    <!-- http://aims.fao.org/aos/geopolitical.owl#Greece -->

    <owl:NamedIndividual rdf:about="&geopolitical;Greece"/>
    


    <!-- http://aims.fao.org/aos/geopolitical.owl#Grenada -->

    <owl:NamedIndividual rdf:about="&geopolitical;Grenada"/>
    


    <!-- http://aims.fao.org/aos/geopolitical.owl#Guadeloupe -->

    <owl:NamedIndividual rdf:about="&geopolitical;Guadeloupe"/>
    


    <!-- http://aims.fao.org/aos/geopolitical.owl#Guam -->

    <owl:NamedIndividual rdf:about="&geopolitical;Guam"/>
    


    <!-- http://aims.fao.org/aos/geopolitical.owl#Guatemala -->

    <owl:NamedIndividual rdf:about="&geopolitical;Guatemala"/>
    


    <!-- http://aims.fao.org/aos/geopolitical.owl#Guinea -->

    <owl:NamedIndividual rdf:about="&geopolitical;Guinea"/>
    


    <!-- http://aims.fao.org/aos/geopolitical.owl#Guinea-Bissau -->

    <owl:NamedIndividual rdf:about="&geopolitical;Guinea-Bissau"/>
    


    <!-- http://aims.fao.org/aos/geopolitical.owl#Guyana -->

    <owl:NamedIndividual rdf:about="&geopolitical;Guyana"/>
    


    <!-- http://aims.fao.org/aos/geopolitical.owl#Haiti -->

    <owl:NamedIndividual rdf:about="&geopolitical;Haiti"/>
    


    <!-- http://aims.fao.org/aos/geopolitical.owl#Holy_See -->

    <owl:NamedIndividual rdf:about="&geopolitical;Holy_See"/>
    


    <!-- http://aims.fao.org/aos/geopolitical.owl#Honduras -->

    <owl:NamedIndividual rdf:about="&geopolitical;Honduras"/>
    


    <!-- http://aims.fao.org/aos/geopolitical.owl#Hungary -->

    <owl:NamedIndividual rdf:about="&geopolitical;Hungary"/>
    


    <!-- http://aims.fao.org/aos/geopolitical.owl#IGAD -->

    <owl:NamedIndividual rdf:about="&geopolitical;IGAD">
        <geopolitical:sourceCreator rdf:datatype="&xsd;string">IGAD</geopolitical:sourceCreator>
        <terms:source rdf:datatype="&xsd;string">IGAD http://igad.int/</terms:source>
        <geopolitical:sourceIdentifier xml:lang="en">http://igad.int/</geopolitical:sourceIdentifier>
    </owl:NamedIndividual>
    


    <!-- http://aims.fao.org/aos/geopolitical.owl#IGADD -->

    <owl:NamedIndividual rdf:about="&geopolitical;IGADD"/>
    


    <!-- http://aims.fao.org/aos/geopolitical.owl#Iceland -->

    <owl:NamedIndividual rdf:about="&geopolitical;Iceland"/>
    


    <!-- http://aims.fao.org/aos/geopolitical.owl#India -->

    <owl:NamedIndividual rdf:about="&geopolitical;India"/>
    


    <!-- http://aims.fao.org/aos/geopolitical.owl#Indonesia -->

    <owl:NamedIndividual rdf:about="&geopolitical;Indonesia"/>
    


    <!-- http://aims.fao.org/aos/geopolitical.owl#Iran_Islamic_Rep_of_ -->

    <owl:NamedIndividual rdf:about="&geopolitical;Iran_Islamic_Rep_of_"/>
    


    <!-- http://aims.fao.org/aos/geopolitical.owl#Iraq -->

    <owl:NamedIndividual rdf:about="&geopolitical;Iraq"/>
    


    <!-- http://aims.fao.org/aos/geopolitical.owl#Ireland -->

    <owl:NamedIndividual rdf:about="&geopolitical;Ireland"/>
    


    <!-- http://aims.fao.org/aos/geopolitical.owl#Israel -->

    <owl:NamedIndividual rdf:about="&geopolitical;Israel"/>
    


    <!-- http://aims.fao.org/aos/geopolitical.owl#Italy -->

    <owl:NamedIndividual rdf:about="&geopolitical;Italy"/>
    


    <!-- http://aims.fao.org/aos/geopolitical.owl#Jamaica -->

    <owl:NamedIndividual rdf:about="&geopolitical;Jamaica"/>
    


    <!-- http://aims.fao.org/aos/geopolitical.owl#Japan -->

    <owl:NamedIndividual rdf:about="&geopolitical;Japan"/>
    


    <!-- http://aims.fao.org/aos/geopolitical.owl#Jordan -->

    <owl:NamedIndividual rdf:about="&geopolitical;Jordan"/>
    


    <!-- http://aims.fao.org/aos/geopolitical.owl#Kazakhstan -->

    <owl:NamedIndividual rdf:about="&geopolitical;Kazakhstan"/>
    


    <!-- http://aims.fao.org/aos/geopolitical.owl#Kenya -->

    <owl:NamedIndividual rdf:about="&geopolitical;Kenya"/>
    


    <!-- http://aims.fao.org/aos/geopolitical.owl#Kiribati -->

    <owl:NamedIndividual rdf:about="&geopolitical;Kiribati"/>
    


    <!-- http://aims.fao.org/aos/geopolitical.owl#Kuwait -->

    <owl:NamedIndividual rdf:about="&geopolitical;Kuwait"/>
    


    <!-- http://aims.fao.org/aos/geopolitical.owl#Kyrgyzstan -->

    <owl:NamedIndividual rdf:about="&geopolitical;Kyrgyzstan"/>
    


    <!-- http://aims.fao.org/aos/geopolitical.owl#LDC -->

    <owl:NamedIndividual rdf:about="&geopolitical;LDC">
        <geopolitical:sourceCreator rdf:datatype="&xsd;string">WTO</geopolitical:sourceCreator>
        <terms:source rdf:datatype="&xsd;string">WTO http://www.wto.org/english/thewto_e/whatis_e/tif_e/org7_e.htm</terms:source>
        <geopolitical:sourceIdentifier xml:lang="en">http://www.wto.org/english/thewto_e/whatis_e/tif_e/org7_e.htm</geopolitical:sourceIdentifier>
        <geopolitical:sourceIdentifier xml:lang="es">http://www.wto.org/spanish/thewto_s/whatis_s/tif_s/org7_s.htm</geopolitical:sourceIdentifier>
        <geopolitical:sourceIdentifier xml:lang="fr">http://www.wto.org/french/thewto_f/whatis_f/tif_f/org7_f.htm</geopolitical:sourceIdentifier>
    </owl:NamedIndividual>
    


    <!-- http://aims.fao.org/aos/geopolitical.owl#LDC_1993 -->

    <owl:NamedIndividual rdf:about="&geopolitical;LDC_1993">
        <geopolitical:sourceCreator rdf:datatype="&xsd;string">WTO</geopolitical:sourceCreator>
        <terms:source rdf:datatype="&xsd;string">WTO http://www.wto.org/english/thewto_e/whatis_e/tif_e/org7_e.htm</terms:source>
        <geopolitical:sourceIdentifier xml:lang="en">http://www.wto.org/english/thewto_e/whatis_e/tif_e/org7_e.htm</geopolitical:sourceIdentifier>
        <geopolitical:sourceIdentifier xml:lang="es">http://www.wto.org/spanish/thewto_s/whatis_s/tif_s/org7_s.htm</geopolitical:sourceIdentifier>
        <geopolitical:sourceIdentifier xml:lang="fr">http://www.wto.org/french/thewto_f/whatis_f/tif_f/org7_f.htm</geopolitical:sourceIdentifier>
    </owl:NamedIndividual>
    


    <!-- http://aims.fao.org/aos/geopolitical.owl#LDC_2010 -->

    <owl:NamedIndividual rdf:about="&geopolitical;LDC_2010">
        <geopolitical:sourceCreator rdf:datatype="&xsd;string">WTO</geopolitical:sourceCreator>
        <terms:source rdf:datatype="&xsd;string">WTO http://www.wto.org/english/thewto_e/whatis_e/tif_e/org7_e.htm</terms:source>
        <geopolitical:sourceIdentifier xml:lang="en">http://www.wto.org/english/thewto_e/whatis_e/tif_e/org7_e.htm</geopolitical:sourceIdentifier>
        <geopolitical:sourceIdentifier xml:lang="es">http://www.wto.org/spanish/thewto_s/whatis_s/tif_s/org7_s.htm</geopolitical:sourceIdentifier>
        <geopolitical:sourceIdentifier xml:lang="fr">http://www.wto.org/french/thewto_f/whatis_f/tif_f/org7_f.htm</geopolitical:sourceIdentifier>
    </owl:NamedIndividual>
    


    <!-- http://aims.fao.org/aos/geopolitical.owl#LIFDC -->

    <owl:NamedIndividual rdf:about="&geopolitical;LIFDC">
        <geopolitical:sourceCreator rdf:datatype="&xsd;string">FAO Country profiles</geopolitical:sourceCreator>
        <terms:source rdf:datatype="&xsd;string">FAO Country profiles http://www.fao.org/countryprofiles/lifdc.asp?lang=en</terms:source>
        <geopolitical:sourceIdentifier xml:lang="ar">http://www.fao.org/countryprofiles/lifdc.asp?lang=ar</geopolitical:sourceIdentifier>
        <geopolitical:sourceIdentifier xml:lang="en">http://www.fao.org/countryprofiles/lifdc.asp?lang=en</geopolitical:sourceIdentifier>
        <geopolitical:sourceIdentifier xml:lang="es">http://www.fao.org/countryprofiles/lifdc.asp?lang=es</geopolitical:sourceIdentifier>
        <geopolitical:sourceIdentifier xml:lang="fr">http://www.fao.org/countryprofiles/lifdc.asp?lang=fr</geopolitical:sourceIdentifier>
        <geopolitical:sourceIdentifier xml:lang="zh">http://www.fao.org/countryprofiles/lifdc.asp?lang=zh</geopolitical:sourceIdentifier>
    </owl:NamedIndividual>
    


    <!-- http://aims.fao.org/aos/geopolitical.owl#LIFDC_2005 -->

    <owl:NamedIndividual rdf:about="&geopolitical;LIFDC_2005"/>
    


    <!-- http://aims.fao.org/aos/geopolitical.owl#LIFDC_2008 -->

    <owl:NamedIndividual rdf:about="&geopolitical;LIFDC_2008"/>
    


    <!-- http://aims.fao.org/aos/geopolitical.owl#LIFDC_2009 -->

    <owl:NamedIndividual rdf:about="&geopolitical;LIFDC_2009">
        <geopolitical:sourceCreator rdf:datatype="&xsd;string">FAO Country profiles</geopolitical:sourceCreator>
        <terms:source rdf:datatype="&xsd;string">FAO Country profiles http://www.fao.org/countryprofiles/lifdc.asp?lang=en</terms:source>
        <geopolitical:sourceIdentifier rdf:datatype="&xsd;string">http://www.fao.org/countryprofiles/lifdc.asp?lang=en</geopolitical:sourceIdentifier>
        <geopolitical:sourceIdentifier xml:lang="ar">http://www.fao.org/countryprofiles/lifdc.asp?lang=ar</geopolitical:sourceIdentifier>
        <geopolitical:sourceIdentifier xml:lang="es">http://www.fao.org/countryprofiles/lifdc.asp?lang=es</geopolitical:sourceIdentifier>
        <geopolitical:sourceIdentifier xml:lang="fr">http://www.fao.org/countryprofiles/lifdc.asp?lang=fr</geopolitical:sourceIdentifier>
        <geopolitical:sourceIdentifier xml:lang="zh">http://www.fao.org/countryprofiles/lifdc.asp?lang=zh</geopolitical:sourceIdentifier>
    </owl:NamedIndividual>
    


    <!-- http://aims.fao.org/aos/geopolitical.owl#LIFDC_2010 -->

    <owl:NamedIndividual rdf:about="&geopolitical;LIFDC_2010">
        <geopolitical:sourceCreator rdf:datatype="&xsd;string">FAO Country profiles</geopolitical:sourceCreator>
        <terms:source rdf:datatype="&xsd;string">FAO Country profiles http://www.fao.org/countryprofiles/lifdc.asp?lang=en</terms:source>
        <geopolitical:sourceIdentifier xml:lang="ar">http://www.fao.org/countryprofiles/lifdc.asp?lang=ar</geopolitical:sourceIdentifier>
        <geopolitical:sourceIdentifier xml:lang="en">http://www.fao.org/countryprofiles/lifdc.asp?lang=en</geopolitical:sourceIdentifier>
        <geopolitical:sourceIdentifier xml:lang="es">http://www.fao.org/countryprofiles/lifdc.asp?lang=es</geopolitical:sourceIdentifier>
        <geopolitical:sourceIdentifier xml:lang="fr">http://www.fao.org/countryprofiles/lifdc.asp?lang=fr</geopolitical:sourceIdentifier>
        <geopolitical:sourceIdentifier xml:lang="zh">http://www.fao.org/countryprofiles/lifdc.asp?lang=zh</geopolitical:sourceIdentifier>
    </owl:NamedIndividual>
    


    <!-- http://aims.fao.org/aos/geopolitical.owl#LLDC -->

    <owl:NamedIndividual rdf:about="&geopolitical;LLDC">
        <geopolitical:sourceModified rdf:datatype="&xsd;string">2010-08-06</geopolitical:sourceModified>
        <geopolitical:sourceCreator rdf:datatype="&xsd;string">UN -OHRLLS</geopolitical:sourceCreator>
        <terms:source rdf:datatype="&xsd;string">UN -OHRLLS http://www.un.org/special-rep/ohrlls/lldc/default.htm</terms:source>
        <geopolitical:sourceIdentifier xml:lang="en">http://www.un.org/special-rep/ohrlls/lldc/default.htm</geopolitical:sourceIdentifier>
    </owl:NamedIndividual>
    


    <!-- http://aims.fao.org/aos/geopolitical.owl#Lao_People_s_Democratic_Republic__the -->

    <owl:NamedIndividual rdf:about="&geopolitical;Lao_People_s_Democratic_Republic__the"/>
    


    <!-- http://aims.fao.org/aos/geopolitical.owl#Latvia -->

    <owl:NamedIndividual rdf:about="&geopolitical;Latvia"/>
    


    <!-- http://aims.fao.org/aos/geopolitical.owl#Lebanon -->

    <owl:NamedIndividual rdf:about="&geopolitical;Lebanon"/>
    


    <!-- http://aims.fao.org/aos/geopolitical.owl#Lesotho -->

    <owl:NamedIndividual rdf:about="&geopolitical;Lesotho"/>
    


    <!-- http://aims.fao.org/aos/geopolitical.owl#Liberia -->

    <owl:NamedIndividual rdf:about="&geopolitical;Liberia"/>
    


    <!-- http://aims.fao.org/aos/geopolitical.owl#Libya -->

    <owl:NamedIndividual rdf:about="&geopolitical;Libya"/>
    


    <!-- http://aims.fao.org/aos/geopolitical.owl#Libyan_Arab_Jamahiriya__the -->

    <owl:NamedIndividual rdf:about="&geopolitical;Libyan_Arab_Jamahiriya__the"/>
    


    <!-- http://aims.fao.org/aos/geopolitical.owl#Liechtenstein -->

    <owl:NamedIndividual rdf:about="&geopolitical;Liechtenstein"/>
    


    <!-- http://aims.fao.org/aos/geopolitical.owl#Lithuania -->

    <owl:NamedIndividual rdf:about="&geopolitical;Lithuania"/>
    


    <!-- http://aims.fao.org/aos/geopolitical.owl#Luxembourg -->

    <owl:NamedIndividual rdf:about="&geopolitical;Luxembourg"/>
    


    <!-- http://aims.fao.org/aos/geopolitical.owl#MERCOSUR -->

    <owl:NamedIndividual rdf:about="&geopolitical;MERCOSUR">
        <geopolitical:sourceModified rdf:datatype="&xsd;string">2010-08-29</geopolitical:sourceModified>
        <geopolitical:sourceCreator rdf:datatype="&xsd;string">MERCOSUR</geopolitical:sourceCreator>
        <terms:source rdf:datatype="&xsd;string">MERCOSUR http://www.mercosur.int/</terms:source>
        <geopolitical:sourceIdentifier xml:lang="es">http://www.mercosur.int/</geopolitical:sourceIdentifier>
        <geopolitical:sourceIdentifier xml:lang="pt">http://www.mercosur.int/show?contentid=10&amp;channel=secretaria</geopolitical:sourceIdentifier>
    </owl:NamedIndividual>
    


    <!-- http://aims.fao.org/aos/geopolitical.owl#MERCOSUR_1991 -->

    <owl:NamedIndividual rdf:about="&geopolitical;MERCOSUR_1991"/>
    


    <!-- http://aims.fao.org/aos/geopolitical.owl#Madagascar -->

    <owl:NamedIndividual rdf:about="&geopolitical;Madagascar"/>
    


    <!-- http://aims.fao.org/aos/geopolitical.owl#Malawi -->

    <owl:NamedIndividual rdf:about="&geopolitical;Malawi"/>
    


    <!-- http://aims.fao.org/aos/geopolitical.owl#Malaysia -->

    <owl:NamedIndividual rdf:about="&geopolitical;Malaysia"/>
    


    <!-- http://aims.fao.org/aos/geopolitical.owl#Maldives -->

    <owl:NamedIndividual rdf:about="&geopolitical;Maldives"/>
    


    <!-- http://aims.fao.org/aos/geopolitical.owl#Mali -->

    <owl:NamedIndividual rdf:about="&geopolitical;Mali"/>
    


    <!-- http://aims.fao.org/aos/geopolitical.owl#Malta -->

    <owl:NamedIndividual rdf:about="&geopolitical;Malta"/>
    


    <!-- http://aims.fao.org/aos/geopolitical.owl#Marshall_Islands__the -->

    <owl:NamedIndividual rdf:about="&geopolitical;Marshall_Islands__the"/>
    


    <!-- http://aims.fao.org/aos/geopolitical.owl#Martinique -->

    <owl:NamedIndividual rdf:about="&geopolitical;Martinique"/>
    


    <!-- http://aims.fao.org/aos/geopolitical.owl#Mauritania -->

    <owl:NamedIndividual rdf:about="&geopolitical;Mauritania"/>
    


    <!-- http://aims.fao.org/aos/geopolitical.owl#Mauritius -->

    <owl:NamedIndividual rdf:about="&geopolitical;Mauritius"/>
    


    <!-- http://aims.fao.org/aos/geopolitical.owl#Melanesia -->

    <owl:NamedIndividual rdf:about="&geopolitical;Melanesia"/>
    


    <!-- http://aims.fao.org/aos/geopolitical.owl#Mexico -->

    <owl:NamedIndividual rdf:about="&geopolitical;Mexico"/>
    


    <!-- http://aims.fao.org/aos/geopolitical.owl#Micronesia -->

    <owl:NamedIndividual rdf:about="&geopolitical;Micronesia"/>
    


    <!-- http://aims.fao.org/aos/geopolitical.owl#Micronesia__Fed_States_of_ -->

    <owl:NamedIndividual rdf:about="&geopolitical;Micronesia__Fed_States_of_"/>
    


    <!-- http://aims.fao.org/aos/geopolitical.owl#Monaco -->

    <owl:NamedIndividual rdf:about="&geopolitical;Monaco"/>
    


    <!-- http://aims.fao.org/aos/geopolitical.owl#Mongolia -->

    <owl:NamedIndividual rdf:about="&geopolitical;Mongolia"/>
    


    <!-- http://aims.fao.org/aos/geopolitical.owl#Montenegro -->

    <owl:NamedIndividual rdf:about="&geopolitical;Montenegro"/>
    


    <!-- http://aims.fao.org/aos/geopolitical.owl#Montserrat -->

    <owl:NamedIndividual rdf:about="&geopolitical;Montserrat"/>
    


    <!-- http://aims.fao.org/aos/geopolitical.owl#Morocco -->

    <owl:NamedIndividual rdf:about="&geopolitical;Morocco"/>
    


    <!-- http://aims.fao.org/aos/geopolitical.owl#Mozambique -->

    <owl:NamedIndividual rdf:about="&geopolitical;Mozambique"/>
    


    <!-- http://aims.fao.org/aos/geopolitical.owl#Myanmar -->

    <owl:NamedIndividual rdf:about="&geopolitical;Myanmar"/>
    


    <!-- http://aims.fao.org/aos/geopolitical.owl#NFIDC -->

    <owl:NamedIndividual rdf:about="&geopolitical;NFIDC">
        <geopolitical:sourceCreator rdf:datatype="&xsd;string">WTO Committe on Agriculture</geopolitical:sourceCreator>
        <terms:source rdf:datatype="&xsd;string">WTO Committe on Agriculture</terms:source>
    </owl:NamedIndividual>
    


    <!-- http://aims.fao.org/aos/geopolitical.owl#NFIDC_2010 -->

    <owl:NamedIndividual rdf:about="&geopolitical;NFIDC_2010"/>
    


    <!-- http://aims.fao.org/aos/geopolitical.owl#Namibia -->

    <owl:NamedIndividual rdf:about="&geopolitical;Namibia"/>
    


    <!-- http://aims.fao.org/aos/geopolitical.owl#Nauru -->

    <owl:NamedIndividual rdf:about="&geopolitical;Nauru"/>
    


    <!-- http://aims.fao.org/aos/geopolitical.owl#Nepal -->

    <owl:NamedIndividual rdf:about="&geopolitical;Nepal"/>
    


    <!-- http://aims.fao.org/aos/geopolitical.owl#Netherlands_Antilles -->

    <owl:NamedIndividual rdf:about="&geopolitical;Netherlands_Antilles"/>
    


    <!-- http://aims.fao.org/aos/geopolitical.owl#Netherlands_the -->

    <owl:NamedIndividual rdf:about="&geopolitical;Netherlands_the"/>
    


    <!-- http://aims.fao.org/aos/geopolitical.owl#New_Caledonia -->

    <owl:NamedIndividual rdf:about="&geopolitical;New_Caledonia"/>
    


    <!-- http://aims.fao.org/aos/geopolitical.owl#New_Zealand -->

    <owl:NamedIndividual rdf:about="&geopolitical;New_Zealand"/>
    


    <!-- http://aims.fao.org/aos/geopolitical.owl#Nicaragua -->

    <owl:NamedIndividual rdf:about="&geopolitical;Nicaragua"/>
    


    <!-- http://aims.fao.org/aos/geopolitical.owl#Niger_the -->

    <owl:NamedIndividual rdf:about="&geopolitical;Niger_the"/>
    


    <!-- http://aims.fao.org/aos/geopolitical.owl#Nigeria -->

    <owl:NamedIndividual rdf:about="&geopolitical;Nigeria"/>
    


    <!-- http://aims.fao.org/aos/geopolitical.owl#Niue -->

    <owl:NamedIndividual rdf:about="&geopolitical;Niue"/>
    


    <!-- http://aims.fao.org/aos/geopolitical.owl#Norway -->

    <owl:NamedIndividual rdf:about="&geopolitical;Norway"/>
    


    <!-- http://aims.fao.org/aos/geopolitical.owl#Oceania -->

    <owl:NamedIndividual rdf:about="&geopolitical;Oceania"/>
    


    <!-- http://aims.fao.org/aos/geopolitical.owl#Oman -->

    <owl:NamedIndividual rdf:about="&geopolitical;Oman"/>
    


    <!-- http://aims.fao.org/aos/geopolitical.owl#PIF -->

    <owl:NamedIndividual rdf:about="&geopolitical;PIF">
        <geopolitical:sourceCreator rdf:datatype="&xsd;string">PIF</geopolitical:sourceCreator>
        <terms:source rdf:datatype="&xsd;string">PIF http://www.forumsec.org/</terms:source>
        <geopolitical:sourceIdentifier xml:lang="en">http://www.forumsec.org/</geopolitical:sourceIdentifier>
    </owl:NamedIndividual>
    


    <!-- http://aims.fao.org/aos/geopolitical.owl#PIF_1985 -->

    <owl:NamedIndividual rdf:about="&geopolitical;PIF_1985"/>
    


    <!-- http://aims.fao.org/aos/geopolitical.owl#PTA -->

    <owl:NamedIndividual rdf:about="&geopolitical;PTA"/>
    


    <!-- http://aims.fao.org/aos/geopolitical.owl#Pakistan -->

    <owl:NamedIndividual rdf:about="&geopolitical;Pakistan"/>
    


    <!-- http://aims.fao.org/aos/geopolitical.owl#Palau -->

    <owl:NamedIndividual rdf:about="&geopolitical;Palau"/>
    


    <!-- http://aims.fao.org/aos/geopolitical.owl#Panama -->

    <owl:NamedIndividual rdf:about="&geopolitical;Panama"/>
    


    <!-- http://aims.fao.org/aos/geopolitical.owl#Papua_New_Guinea -->

    <owl:NamedIndividual rdf:about="&geopolitical;Papua_New_Guinea"/>
    


    <!-- http://aims.fao.org/aos/geopolitical.owl#Paraguay -->

    <owl:NamedIndividual rdf:about="&geopolitical;Paraguay"/>
    


    <!-- http://aims.fao.org/aos/geopolitical.owl#Peru -->

    <owl:NamedIndividual rdf:about="&geopolitical;Peru"/>
    


    <!-- http://aims.fao.org/aos/geopolitical.owl#Philippines__the -->

    <owl:NamedIndividual rdf:about="&geopolitical;Philippines__the"/>
    


    <!-- http://aims.fao.org/aos/geopolitical.owl#Poland -->

    <owl:NamedIndividual rdf:about="&geopolitical;Poland"/>
    


    <!-- http://aims.fao.org/aos/geopolitical.owl#Polynesia -->

    <owl:NamedIndividual rdf:about="&geopolitical;Polynesia"/>
    


    <!-- http://aims.fao.org/aos/geopolitical.owl#Portugal -->

    <owl:NamedIndividual rdf:about="&geopolitical;Portugal"/>
    


    <!-- http://aims.fao.org/aos/geopolitical.owl#Puerto_Rico -->

    <owl:NamedIndividual rdf:about="&geopolitical;Puerto_Rico"/>
    


    <!-- http://aims.fao.org/aos/geopolitical.owl#Qatar -->

    <owl:NamedIndividual rdf:about="&geopolitical;Qatar"/>
    


    <!-- http://aims.fao.org/aos/geopolitical.owl#Republic_of_Korea__the -->

    <owl:NamedIndividual rdf:about="&geopolitical;Republic_of_Korea__the"/>
    


    <!-- http://aims.fao.org/aos/geopolitical.owl#Republic_of_Moldova -->

    <owl:NamedIndividual rdf:about="&geopolitical;Republic_of_Moldova"/>
    


    <!-- http://aims.fao.org/aos/geopolitical.owl#Reunion -->

    <owl:NamedIndividual rdf:about="&geopolitical;Reunion"/>
    


    <!-- http://aims.fao.org/aos/geopolitical.owl#Romania -->

    <owl:NamedIndividual rdf:about="&geopolitical;Romania"/>
    


    <!-- http://aims.fao.org/aos/geopolitical.owl#Russian_Federation__the -->

    <owl:NamedIndividual rdf:about="&geopolitical;Russian_Federation__the"/>
    


    <!-- http://aims.fao.org/aos/geopolitical.owl#Rwanda -->

    <owl:NamedIndividual rdf:about="&geopolitical;Rwanda"/>
    


    <!-- http://aims.fao.org/aos/geopolitical.owl#SAARC -->

    <owl:NamedIndividual rdf:about="&geopolitical;SAARC">
        <geopolitical:sourceModified rdf:datatype="&xsd;string">2010-08-31</geopolitical:sourceModified>
        <geopolitical:sourceCreator rdf:datatype="&xsd;string">SAARC</geopolitical:sourceCreator>
        <terms:source rdf:datatype="&xsd;string">SAARC http://www.saarc-sec.org/</terms:source>
        <geopolitical:sourceIdentifier xml:lang="en">http://www.saarc-sec.org/</geopolitical:sourceIdentifier>
    </owl:NamedIndividual>
    


    <!-- http://aims.fao.org/aos/geopolitical.owl#SAARC_1985 -->

    <owl:NamedIndividual rdf:about="&geopolitical;SAARC_1985"/>
    


    <!-- http://aims.fao.org/aos/geopolitical.owl#SADC -->

    <owl:NamedIndividual rdf:about="&geopolitical;SADC">
        <geopolitical:sourceModified rdf:datatype="&xsd;string">2010-08-31</geopolitical:sourceModified>
        <geopolitical:sourceCreator rdf:datatype="&xsd;string">SADC</geopolitical:sourceCreator>
        <terms:source rdf:datatype="&xsd;string">SADC http://www.sadc.int/</terms:source>
        <geopolitical:sourceIdentifier xml:lang="en">http://www.sadc.int/</geopolitical:sourceIdentifier>
    </owl:NamedIndividual>
    


    <!-- http://aims.fao.org/aos/geopolitical.owl#SIDS -->

    <owl:NamedIndividual rdf:about="&geopolitical;SIDS">
        <geopolitical:sourceModified rdf:datatype="&xsd;string">2010-08-31</geopolitical:sourceModified>
        <geopolitical:sourceCreator rdf:datatype="&xsd;string">UN -OHRLLS</geopolitical:sourceCreator>
        <terms:source rdf:datatype="&xsd;string">UN -OHRLLS http://www.un.org/special-rep/ohrlls/sid/default.htm</terms:source>
        <geopolitical:sourceIdentifier xml:lang="en">http://www.un.org/special-rep/ohrlls/sid/default.htm</geopolitical:sourceIdentifier>
    </owl:NamedIndividual>
    


    <!-- http://aims.fao.org/aos/geopolitical.owl#Saint-Martin -->

    <owl:NamedIndividual rdf:about="&geopolitical;Saint-Martin"/>
    


    <!-- http://aims.fao.org/aos/geopolitical.owl#Saint_Barthelemy -->

    <owl:NamedIndividual rdf:about="&geopolitical;Saint_Barthelemy"/>
    


    <!-- http://aims.fao.org/aos/geopolitical.owl#Saint_Helena -->

    <owl:NamedIndividual rdf:about="&geopolitical;Saint_Helena"/>
    


    <!-- http://aims.fao.org/aos/geopolitical.owl#Saint_Kitts_and_Nevis -->

    <owl:NamedIndividual rdf:about="&geopolitical;Saint_Kitts_and_Nevis"/>
    


    <!-- http://aims.fao.org/aos/geopolitical.owl#Saint_Lucia -->

    <owl:NamedIndividual rdf:about="&geopolitical;Saint_Lucia"/>
    


    <!-- http://aims.fao.org/aos/geopolitical.owl#Saint_Pierre_and_Miquelon -->

    <owl:NamedIndividual rdf:about="&geopolitical;Saint_Pierre_and_Miquelon"/>
    


    <!-- http://aims.fao.org/aos/geopolitical.owl#Saint_Vincent_and_the_Grenadines -->

    <owl:NamedIndividual rdf:about="&geopolitical;Saint_Vincent_and_the_Grenadines"/>
    


    <!-- http://aims.fao.org/aos/geopolitical.owl#Samoa -->

    <owl:NamedIndividual rdf:about="&geopolitical;Samoa"/>
    


    <!-- http://aims.fao.org/aos/geopolitical.owl#San_Marino -->

    <owl:NamedIndividual rdf:about="&geopolitical;San_Marino"/>
    


    <!-- http://aims.fao.org/aos/geopolitical.owl#Sao_Tome_and_Principe -->

    <owl:NamedIndividual rdf:about="&geopolitical;Sao_Tome_and_Principe"/>
    


    <!-- http://aims.fao.org/aos/geopolitical.owl#Saudi_Arabia -->

    <owl:NamedIndividual rdf:about="&geopolitical;Saudi_Arabia"/>
    


    <!-- http://aims.fao.org/aos/geopolitical.owl#Senegal -->

    <owl:NamedIndividual rdf:about="&geopolitical;Senegal"/>
    


    <!-- http://aims.fao.org/aos/geopolitical.owl#Serbia -->

    <owl:NamedIndividual rdf:about="&geopolitical;Serbia"/>
    


    <!-- http://aims.fao.org/aos/geopolitical.owl#Serbia_and_Montenegro -->

    <owl:NamedIndividual rdf:about="&geopolitical;Serbia_and_Montenegro"/>
    


    <!-- http://aims.fao.org/aos/geopolitical.owl#Seychelles -->

    <owl:NamedIndividual rdf:about="&geopolitical;Seychelles"/>
    


    <!-- http://aims.fao.org/aos/geopolitical.owl#Sierra_Leone -->

    <owl:NamedIndividual rdf:about="&geopolitical;Sierra_Leone"/>
    


    <!-- http://aims.fao.org/aos/geopolitical.owl#Singapore -->

    <owl:NamedIndividual rdf:about="&geopolitical;Singapore"/>
    


    <!-- http://aims.fao.org/aos/geopolitical.owl#Sint_Maarten -->

    <owl:NamedIndividual rdf:about="&geopolitical;Sint_Maarten"/>
    


    <!-- http://aims.fao.org/aos/geopolitical.owl#Slovakia -->

    <owl:NamedIndividual rdf:about="&geopolitical;Slovakia"/>
    


    <!-- http://aims.fao.org/aos/geopolitical.owl#Slovenia -->

    <owl:NamedIndividual rdf:about="&geopolitical;Slovenia"/>
    


    <!-- http://aims.fao.org/aos/geopolitical.owl#Socialist_Federal_Republic_of_Yugoslavia_the -->

    <owl:NamedIndividual rdf:about="&geopolitical;Socialist_Federal_Republic_of_Yugoslavia_the"/>
    


    <!-- http://aims.fao.org/aos/geopolitical.owl#Solomon_Islands -->

    <owl:NamedIndividual rdf:about="&geopolitical;Solomon_Islands"/>
    


    <!-- http://aims.fao.org/aos/geopolitical.owl#Somalia -->

    <owl:NamedIndividual rdf:about="&geopolitical;Somalia"/>
    


    <!-- http://aims.fao.org/aos/geopolitical.owl#South_Africa -->

    <owl:NamedIndividual rdf:about="&geopolitical;South_Africa"/>
    


    <!-- http://aims.fao.org/aos/geopolitical.owl#South_America -->

    <owl:NamedIndividual rdf:about="&geopolitical;South_America"/>
    


    <!-- http://aims.fao.org/aos/geopolitical.owl#South_Sudan -->

    <owl:NamedIndividual rdf:about="&geopolitical;South_Sudan"/>
    


    <!-- http://aims.fao.org/aos/geopolitical.owl#Spain -->

    <owl:NamedIndividual rdf:about="&geopolitical;Spain"/>
    


    <!-- http://aims.fao.org/aos/geopolitical.owl#Sri_Lanka -->

    <owl:NamedIndividual rdf:about="&geopolitical;Sri_Lanka"/>
    


    <!-- http://aims.fao.org/aos/geopolitical.owl#Sudan_the -->

    <owl:NamedIndividual rdf:about="&geopolitical;Sudan_the"/>
    


    <!-- http://aims.fao.org/aos/geopolitical.owl#Sudan_the_1956 -->

    <owl:NamedIndividual rdf:about="&geopolitical;Sudan_the_1956"/>
    


    <!-- http://aims.fao.org/aos/geopolitical.owl#Suriname -->

    <owl:NamedIndividual rdf:about="&geopolitical;Suriname"/>
    


    <!-- http://aims.fao.org/aos/geopolitical.owl#Swaziland -->

    <owl:NamedIndividual rdf:about="&geopolitical;Swaziland"/>
    


    <!-- http://aims.fao.org/aos/geopolitical.owl#Sweden -->

    <owl:NamedIndividual rdf:about="&geopolitical;Sweden"/>
    


    <!-- http://aims.fao.org/aos/geopolitical.owl#Switzerland -->

    <owl:NamedIndividual rdf:about="&geopolitical;Switzerland"/>
    


    <!-- http://aims.fao.org/aos/geopolitical.owl#Syrian_Arab_Republic_the -->

    <owl:NamedIndividual rdf:about="&geopolitical;Syrian_Arab_Republic_the"/>
    


    <!-- http://aims.fao.org/aos/geopolitical.owl#Tajikistan -->

    <owl:NamedIndividual rdf:about="&geopolitical;Tajikistan"/>
    


    <!-- http://aims.fao.org/aos/geopolitical.owl#Thailand -->

    <owl:NamedIndividual rdf:about="&geopolitical;Thailand"/>
    


    <!-- http://aims.fao.org/aos/geopolitical.owl#The_former_Yugoslav_Republic_of_Macedonia -->

    <owl:NamedIndividual rdf:about="&geopolitical;The_former_Yugoslav_Republic_of_Macedonia"/>
    


    <!-- http://aims.fao.org/aos/geopolitical.owl#Timor-Leste -->

    <owl:NamedIndividual rdf:about="&geopolitical;Timor-Leste"/>
    


    <!-- http://aims.fao.org/aos/geopolitical.owl#Togo -->

    <owl:NamedIndividual rdf:about="&geopolitical;Togo"/>
    


    <!-- http://aims.fao.org/aos/geopolitical.owl#Tokelau -->

    <owl:NamedIndividual rdf:about="&geopolitical;Tokelau">
        <rdfs:comment rdf:datatype="&xsd;string">associate member of FAO</rdfs:comment>
    </owl:NamedIndividual>
    


    <!-- http://aims.fao.org/aos/geopolitical.owl#Tonga -->

    <owl:NamedIndividual rdf:about="&geopolitical;Tonga"/>
    


    <!-- http://aims.fao.org/aos/geopolitical.owl#Trinidad_and_Tobago -->

    <owl:NamedIndividual rdf:about="&geopolitical;Trinidad_and_Tobago"/>
    


    <!-- http://aims.fao.org/aos/geopolitical.owl#Tunisia -->

    <owl:NamedIndividual rdf:about="&geopolitical;Tunisia"/>
    


    <!-- http://aims.fao.org/aos/geopolitical.owl#Turkey -->

    <owl:NamedIndividual rdf:about="&geopolitical;Turkey"/>
    


    <!-- http://aims.fao.org/aos/geopolitical.owl#Turkmenistan -->

    <owl:NamedIndividual rdf:about="&geopolitical;Turkmenistan"/>
    


    <!-- http://aims.fao.org/aos/geopolitical.owl#Turks_and_Caicos_Islands -->

    <owl:NamedIndividual rdf:about="&geopolitical;Turks_and_Caicos_Islands"/>
    


    <!-- http://aims.fao.org/aos/geopolitical.owl#Tuvalu -->

    <owl:NamedIndividual rdf:about="&geopolitical;Tuvalu"/>
    


    <!-- http://aims.fao.org/aos/geopolitical.owl#UEMOA -->

    <owl:NamedIndividual rdf:about="&geopolitical;UEMOA">
        <geopolitical:sourceCreator rdf:datatype="&xsd;string">UEMOA</geopolitical:sourceCreator>
        <terms:source rdf:datatype="&xsd;string">UEMOA http://www.uemoa.int/index.htm</terms:source>
        <geopolitical:sourceIdentifier xml:lang="fr">http://www.uemoa.int/index.htm</geopolitical:sourceIdentifier>
    </owl:NamedIndividual>
    


    <!-- http://aims.fao.org/aos/geopolitical.owl#Uganda -->

    <owl:NamedIndividual rdf:about="&geopolitical;Uganda"/>
    


    <!-- http://aims.fao.org/aos/geopolitical.owl#Ukraine -->

    <owl:NamedIndividual rdf:about="&geopolitical;Ukraine"/>
    


    <!-- http://aims.fao.org/aos/geopolitical.owl#Union_of_Soviet_Socialist_Republic_the -->

    <owl:NamedIndividual rdf:about="&geopolitical;Union_of_Soviet_Socialist_Republic_the"/>
    


    <!-- http://aims.fao.org/aos/geopolitical.owl#United_Arab_Emirates__the -->

    <owl:NamedIndividual rdf:about="&geopolitical;United_Arab_Emirates__the"/>
    


    <!-- http://aims.fao.org/aos/geopolitical.owl#United_Kingdom_of_Great_Britain_and_Northern_Ireland__the -->

    <owl:NamedIndividual rdf:about="&geopolitical;United_Kingdom_of_Great_Britain_and_Northern_Ireland__the"/>
    


    <!-- http://aims.fao.org/aos/geopolitical.owl#United_Republic_of_Tanzania__the -->

    <owl:NamedIndividual rdf:about="&geopolitical;United_Republic_of_Tanzania__the"/>
    


    <!-- http://aims.fao.org/aos/geopolitical.owl#United_States_Virgin_Islands -->

    <owl:NamedIndividual rdf:about="&geopolitical;United_States_Virgin_Islands"/>
    


    <!-- http://aims.fao.org/aos/geopolitical.owl#United_States_of_America -->

    <owl:NamedIndividual rdf:about="&geopolitical;United_States_of_America"/>
    


    <!-- http://aims.fao.org/aos/geopolitical.owl#Uruguay -->

    <owl:NamedIndividual rdf:about="&geopolitical;Uruguay"/>
    


    <!-- http://aims.fao.org/aos/geopolitical.owl#Uzbekistan -->

    <owl:NamedIndividual rdf:about="&geopolitical;Uzbekistan"/>
    


    <!-- http://aims.fao.org/aos/geopolitical.owl#Vanuatu -->

    <owl:NamedIndividual rdf:about="&geopolitical;Vanuatu"/>
    


    <!-- http://aims.fao.org/aos/geopolitical.owl#Venezuela -->

    <owl:NamedIndividual rdf:about="&geopolitical;Venezuela"/>
    


    <!-- http://aims.fao.org/aos/geopolitical.owl#Viet_Nam -->

    <owl:NamedIndividual rdf:about="&geopolitical;Viet_Nam"/>
    


    <!-- http://aims.fao.org/aos/geopolitical.owl#Wallis_and_Futuna_Is -->

    <owl:NamedIndividual rdf:about="&geopolitical;Wallis_and_Futuna_Is"/>
    


    <!-- http://aims.fao.org/aos/geopolitical.owl#World -->

    <owl:NamedIndividual rdf:about="&geopolitical;World">
        <geopolitical:sourceModified rdf:datatype="&xsd;string">2010-04-01</geopolitical:sourceModified>
        <geopolitical:sourceCreator rdf:datatype="&xsd;string">United Nations Statistics Department</geopolitical:sourceCreator>
        <terms:source rdf:datatype="&xsd;string">United Nations Statistics Department http://unstats.un.org/unsd/methods/m49/m49regin.htm</terms:source>
        <geopolitical:sourceIdentifier xml:lang="en">http://unstats.un.org/unsd/methods/m49/m49regin.htm</geopolitical:sourceIdentifier>
        <geopolitical:sourceIdentifier xml:lang="fr">http://unstats.un.org/unsd/methods/m49/m49regnf.htm</geopolitical:sourceIdentifier>
    </owl:NamedIndividual>
    


    <!-- http://aims.fao.org/aos/geopolitical.owl#Yemen -->

    <owl:NamedIndividual rdf:about="&geopolitical;Yemen"/>
    


    <!-- http://aims.fao.org/aos/geopolitical.owl#Yemen_1990 -->

    <owl:NamedIndividual rdf:about="&geopolitical;Yemen_1990"/>
    


    <!-- http://aims.fao.org/aos/geopolitical.owl#Yugoslavia -->

    <owl:NamedIndividual rdf:about="&geopolitical;Yugoslavia"/>
    


    <!-- http://aims.fao.org/aos/geopolitical.owl#Zaire -->

    <owl:NamedIndividual rdf:about="&geopolitical;Zaire"/>
    


    <!-- http://aims.fao.org/aos/geopolitical.owl#Zambia -->

    <owl:NamedIndividual rdf:about="&geopolitical;Zambia"/>
    


    <!-- http://aims.fao.org/aos/geopolitical.owl#Zimbabwe -->

    <owl:NamedIndividual rdf:about="&geopolitical;Zimbabwe"/>
    


    <!-- http://aims.fao.org/aos/geopolitical.owl#central_America -->

    <owl:NamedIndividual rdf:about="&geopolitical;central_America"/>
    


    <!-- http://aims.fao.org/aos/geopolitical.owl#central_Asia -->

    <owl:NamedIndividual rdf:about="&geopolitical;central_Asia"/>
    


    <!-- http://aims.fao.org/aos/geopolitical.owl#eastern_Africa -->

    <owl:NamedIndividual rdf:about="&geopolitical;eastern_Africa"/>
    


    <!-- http://aims.fao.org/aos/geopolitical.owl#eastern_Asia -->

    <owl:NamedIndividual rdf:about="&geopolitical;eastern_Asia"/>
    


    <!-- http://aims.fao.org/aos/geopolitical.owl#eastern_Europe -->

    <owl:NamedIndividual rdf:about="&geopolitical;eastern_Europe"/>
    


    <!-- http://aims.fao.org/aos/geopolitical.owl#middle_Africa -->

    <owl:NamedIndividual rdf:about="&geopolitical;middle_Africa"/>
    


    <!-- http://aims.fao.org/aos/geopolitical.owl#northern_Africa -->

    <owl:NamedIndividual rdf:about="&geopolitical;northern_Africa"/>
    


    <!-- http://aims.fao.org/aos/geopolitical.owl#northern_America -->

    <owl:NamedIndividual rdf:about="&geopolitical;northern_America"/>
    


    <!-- http://aims.fao.org/aos/geopolitical.owl#northern_Europe -->

    <owl:NamedIndividual rdf:about="&geopolitical;northern_Europe"/>
    


    <!-- http://aims.fao.org/aos/geopolitical.owl#south-eastern_Asia -->

    <owl:NamedIndividual rdf:about="&geopolitical;south-eastern_Asia"/>
    


    <!-- http://aims.fao.org/aos/geopolitical.owl#southern_Africa -->

    <owl:NamedIndividual rdf:about="&geopolitical;southern_Africa"/>
    


    <!-- http://aims.fao.org/aos/geopolitical.owl#southern_Asia -->

    <owl:NamedIndividual rdf:about="&geopolitical;southern_Asia"/>
    


    <!-- http://aims.fao.org/aos/geopolitical.owl#southern_Europe -->

    <owl:NamedIndividual rdf:about="&geopolitical;southern_Europe"/>
    


    <!-- http://aims.fao.org/aos/geopolitical.owl#western_Africa -->

    <owl:NamedIndividual rdf:about="&geopolitical;western_Africa"/>
    


    <!-- http://aims.fao.org/aos/geopolitical.owl#western_Asia -->

    <owl:NamedIndividual rdf:about="&geopolitical;western_Asia"/>
    


    <!-- http://aims.fao.org/aos/geopolitical.owl#western_Europe -->

    <owl:NamedIndividual rdf:about="&geopolitical;western_Europe"/>
    


    <!-- http://vocab.deri.ie/scovo -->

    <owl:NamedIndividual rdf:about="&vocab;scovo"/>
    


    <!-- http://vocab.deri.ie/scovo#JOANNEUM%20RESEARCH -->

    <owl:NamedIndividual rdf:about="&vocab;scovo#JOANNEUM%20RESEARCH">
        <foaf:name>JOANNEUM RESEARCH</foaf:name>
        <foaf:member rdf:resource="&vocab;scovo#whalb"/>
        <foaf:homepage rdf:resource="http://www.joanneum.at/en/digital/iis.html"/>
    </owl:NamedIndividual>
    


    <!-- http://vocab.deri.ie/scovo#LiDRC -->

    <owl:NamedIndividual rdf:about="&vocab;scovo#LiDRC">
        <foaf:name>LiDRC</foaf:name>
        <foaf:homepage rdf:resource="http://linkeddata.deri.ie/"/>
        <foaf:member rdf:resource="&vocab;scovo#Michael%20Hausenblas"/>
    </owl:NamedIndividual>
    


    <!-- http://vocab.deri.ie/scovo#Michael%20Hausenblas -->

    <owl:NamedIndividual rdf:about="&vocab;scovo#Michael%20Hausenblas">
        <foaf:name>Michael Hausenblas</foaf:name>
        <foaf:homepage rdf:resource="http://sw-app.org/about.html"/>
        <foaf:mbox rdf:resource="mailto:michael.hausenblas@deri.org"/>
    </owl:NamedIndividual>
    


    <!-- http://vocab.deri.ie/scovo#dayers -->

    <owl:NamedIndividual rdf:about="&vocab;scovo#dayers">
        <foaf:homepage></foaf:homepage>
        <foaf:name>Danny Ayers</foaf:name>
    </owl:NamedIndividual>
    


    <!-- http://vocab.deri.ie/scovo#lfeigenbaum -->

    <owl:NamedIndividual rdf:about="&vocab;scovo#lfeigenbaum">
        <foaf:homepage></foaf:homepage>
        <foaf:name>Lee Feigenbaum</foaf:name>
    </owl:NamedIndividual>
    


    <!-- http://vocab.deri.ie/scovo#rdf -->

    <owl:NamedIndividual rdf:about="&vocab;scovo#rdf">
        <adms:accessURL>http://vocab.deri.ie/scovo.rdf</adms:accessURL>
        <terms:FileFormat></terms:FileFormat>
        <adms:status rdf:resource="http://purl.org/adms/status/Completed"/>
    </owl:NamedIndividual>
    


    <!-- http://vocab.deri.ie/scovo#theath -->

    <owl:NamedIndividual rdf:about="&vocab;scovo#theath">
        <foaf:homepage></foaf:homepage>
        <foaf:name>Tom Heath</foaf:name>
    </owl:NamedIndividual>
    


    <!-- http://vocab.deri.ie/scovo#ttl -->

    <owl:NamedIndividual rdf:about="&vocab;scovo#ttl">
        <terms:FileFormat></terms:FileFormat>
        <adms:accessURL>http://vocab.deri.ie/scovo.ttl</adms:accessURL>
        <adms:status rdf:resource="http://purl.org/adms/status/Completed"/>
    </owl:NamedIndividual>
    


    <!-- http://vocab.deri.ie/scovo#whalb -->

    <owl:NamedIndividual rdf:about="&vocab;scovo#whalb">
        <foaf:homepage></foaf:homepage>
        <foaf:name>Wolfgang Halb</foaf:name>
    </owl:NamedIndividual>
    


    <!-- http://vocab.deri.ie/scovo#yraimond -->

    <owl:NamedIndividual rdf:about="&vocab;scovo#yraimond">
        <foaf:homepage></foaf:homepage>
        <foaf:name>Yves Raimond</foaf:name>
    </owl:NamedIndividual>
    


    <!-- http://www.w3.org/2006/time#Friday -->

    <owl:NamedIndividual rdf:about="&time;Friday"/>
    


    <!-- http://www.w3.org/2006/time#Monday -->

    <owl:NamedIndividual rdf:about="&time;Monday"/>
    


    <!-- http://www.w3.org/2006/time#Saturday -->

    <owl:NamedIndividual rdf:about="&time;Saturday"/>
    


    <!-- http://www.w3.org/2006/time#Sunday -->

    <owl:NamedIndividual rdf:about="&time;Sunday"/>
    


    <!-- http://www.w3.org/2006/time#Thursday -->

    <owl:NamedIndividual rdf:about="&time;Thursday"/>
    


    <!-- http://www.w3.org/2006/time#Tuesday -->

    <owl:NamedIndividual rdf:about="&time;Tuesday"/>
    


    <!-- http://www.w3.org/2006/time#Wednesday -->

    <owl:NamedIndividual rdf:about="&time;Wednesday"/>
    


    <!-- http://www.w3.org/2006/time#unitDay -->

    <owl:NamedIndividual rdf:about="&time;unitDay"/>
    


    <!-- http://www.w3.org/2006/time#unitHour -->

    <owl:NamedIndividual rdf:about="&time;unitHour"/>
    


    <!-- http://www.w3.org/2006/time#unitMinute -->

    <owl:NamedIndividual rdf:about="&time;unitMinute"/>
    


    <!-- http://www.w3.org/2006/time#unitMonth -->

    <owl:NamedIndividual rdf:about="&time;unitMonth"/>
    


    <!-- http://www.w3.org/2006/time#unitSecond -->

    <owl:NamedIndividual rdf:about="&time;unitSecond"/>
    


    <!-- http://www.w3.org/2006/time#unitWeek -->

    <owl:NamedIndividual rdf:about="&time;unitWeek"/>
    


    <!-- http://www.w3.org/2006/time#unitYear -->

    <owl:NamedIndividual rdf:about="&time;unitYear"/>
    


    <!-- 
    ///////////////////////////////////////////////////////////////////////////////////////
    //
    // Annotations
    //
    ///////////////////////////////////////////////////////////////////////////////////////
     -->

    <rdf:Description rdf:about="&terms;IMT">
        <rdfs:label xml:lang="en">IMT</rdfs:label>
        <terms:issued rdf:datatype="&xsd;date">2000-07-11</terms:issued>
        <terms:modified rdf:datatype="&xsd;date">2008-01-14</terms:modified>
        <rdfs:comment xml:lang="en">The set of media types specified by the Internet Assigned Numbers Authority.</rdfs:comment>
        <terms:hasVersion rdf:resource="http://dublincore.org/usage/terms/history/#IMT-004"/>
        <rdfs:isDefinedBy rdf:resource="http://purl.org/dc/terms/"/>
        <rdfs:seeAlso rdf:resource="http://www.iana.org/assignments/media-types/"/>
    </rdf:Description>
    <rdf:Description rdf:about="&terms;DCMIType">
        <rdfs:label xml:lang="en">DCMI Type Vocabulary</rdfs:label>
        <terms:issued rdf:datatype="&xsd;date">2000-07-11</terms:issued>
        <terms:modified rdf:datatype="&xsd;date">2012-06-14</terms:modified>
        <rdfs:comment xml:lang="en">The set of classes specified by the DCMI Type Vocabulary, used to categorize the nature or genre of the resource.</rdfs:comment>
        <terms:hasVersion rdf:resource="http://dublincore.org/usage/terms/history/#DCMIType-005"/>
        <rdfs:seeAlso rdf:resource="http://purl.org/dc/dcmitype/"/>
        <rdfs:isDefinedBy rdf:resource="http://purl.org/dc/terms/"/>
    </rdf:Description>
    <rdf:Description rdf:about="&terms;LCC">
        <rdfs:label xml:lang="en">LCC</rdfs:label>
        <terms:issued rdf:datatype="&xsd;date">2000-07-11</terms:issued>
        <terms:modified rdf:datatype="&xsd;date">2008-01-14</terms:modified>
        <rdfs:comment xml:lang="en">The set of conceptual resources specified by the Library of Congress Classification.</rdfs:comment>
        <terms:hasVersion rdf:resource="http://dublincore.org/usage/terms/history/#LCC-003"/>
        <rdfs:seeAlso rdf:resource="http://lcweb.loc.gov/catdir/cpso/lcco/lcco.html"/>
        <rdfs:isDefinedBy rdf:resource="http://purl.org/dc/terms/"/>
    </rdf:Description>
    <rdf:Description rdf:about="http://purl.org/dc/elements/1.1/">
        <terms:modified rdf:datatype="&xsd;date">2012-06-14</terms:modified>
        <terms:title xml:lang="en">Dublin Core Metadata Element Set, Version 1.1</terms:title>
        <terms:publisher rdf:resource="http://purl.org/dc/aboutdcmi#DCMI"/>
    </rdf:Description>
    <rdf:Description rdf:about="&terms;LCSH">
        <rdfs:label xml:lang="en">LCSH</rdfs:label>
        <terms:issued rdf:datatype="&xsd;date">2000-07-11</terms:issued>
        <terms:modified rdf:datatype="&xsd;date">2008-01-14</terms:modified>
        <rdfs:comment xml:lang="en">The set of labeled concepts specified by the Library of Congress Subject Headings.</rdfs:comment>
        <terms:hasVersion rdf:resource="http://dublincore.org/usage/terms/history/#LCSH-003"/>
        <rdfs:isDefinedBy rdf:resource="http://purl.org/dc/terms/"/>
    </rdf:Description>
    <rdf:Description rdf:about="&terms;instructionalMethod">
        <rdfs:label xml:lang="en">Instructional Method</rdfs:label>
        <terms:issued rdf:datatype="&xsd;date">2005-06-13</terms:issued>
        <terms:modified rdf:datatype="&xsd;date">2008-01-14</terms:modified>
        <rdfs:comment xml:lang="en">A process, used to engender knowledge, attitudes and skills, that the described resource is designed to support.</rdfs:comment>
        <terms:description xml:lang="en">Instructional Method will typically include ways of presenting instructional materials or conducting instructional activities, patterns of learner-to-learner and learner-to-instructor interactions, and mechanisms by which group and individual levels of learning are measured.  Instructional methods include all aspects of the instruction and learning processes from planning and implementation through evaluation and feedback.</terms:description>
        <terms:hasVersion rdf:resource="http://dublincore.org/usage/terms/history/#instructionalMethod-002"/>
        <rdfs:isDefinedBy rdf:resource="http://purl.org/dc/terms/"/>
    </rdf:Description>
    <rdf:Description rdf:about="&terms;provenance">
        <rdfs:label xml:lang="en">Provenance</rdfs:label>
        <terms:issued rdf:datatype="&xsd;date">2004-09-20</terms:issued>
        <terms:modified rdf:datatype="&xsd;date">2008-01-14</terms:modified>
        <rdfs:comment xml:lang="en">A statement of any changes in ownership and custody of the resource since its creation that are significant for its authenticity, integrity, and interpretation.</rdfs:comment>
        <terms:description xml:lang="en">The statement may include a description of any changes successive custodians made to the resource.</terms:description>
        <terms:hasVersion rdf:resource="http://dublincore.org/usage/terms/history/#provenance-002"/>
        <rdfs:isDefinedBy rdf:resource="http://purl.org/dc/terms/"/>
    </rdf:Description>
    <rdf:Description rdf:about="&terms;TGN">
        <rdfs:label xml:lang="en">TGN</rdfs:label>
        <terms:issued rdf:datatype="&xsd;date">2000-07-11</terms:issued>
        <terms:modified rdf:datatype="&xsd;date">2008-01-14</terms:modified>
        <rdfs:comment xml:lang="en">The set of places specified by the Getty Thesaurus of Geographic Names.</rdfs:comment>
        <terms:hasVersion rdf:resource="http://dublincore.org/usage/terms/history/#TGN-003"/>
        <rdfs:isDefinedBy rdf:resource="http://purl.org/dc/terms/"/>
        <rdfs:seeAlso rdf:resource="http://www.getty.edu/research/tools/vocabulary/tgn/index.html"/>
    </rdf:Description>
    <rdf:Description rdf:about="&wgs84_pos;lat_long">
        <rdfs:label>lat/long</rdfs:label>
        <rdfs:comment>A comma-separated representation of a latitude, longitude coordinate.</rdfs:comment>
    </rdf:Description>
    <rdf:Description rdf:about="&terms;rightsHolder">
        <rdfs:label xml:lang="en">Rights Holder</rdfs:label>
        <terms:issued rdf:datatype="&xsd;date">2004-06-14</terms:issued>
        <terms:modified rdf:datatype="&xsd;date">2008-01-14</terms:modified>
        <rdfs:comment xml:lang="en">A person or organization owning or managing rights over the resource.</rdfs:comment>
        <terms:hasVersion rdf:resource="http://dublincore.org/usage/terms/history/#rightsHolder-002"/>
        <rdfs:isDefinedBy rdf:resource="http://purl.org/dc/terms/"/>
    </rdf:Description>
    <rdf:Description rdf:about="&terms;DDC">
        <rdfs:label xml:lang="en">DDC</rdfs:label>
        <terms:issued rdf:datatype="&xsd;date">2000-07-11</terms:issued>
        <terms:modified rdf:datatype="&xsd;date">2008-01-14</terms:modified>
        <rdfs:comment xml:lang="en">The set of conceptual resources specified by the Dewey Decimal Classification.</rdfs:comment>
        <terms:hasVersion rdf:resource="http://dublincore.org/usage/terms/history/#DDC-003"/>
        <rdfs:isDefinedBy rdf:resource="http://purl.org/dc/terms/"/>
        <rdfs:seeAlso rdf:resource="http://www.oclc.org/dewey/"/>
    </rdf:Description>
    <rdf:Description rdf:about="http://purl.org/dc/terms/">
        <terms:modified rdf:datatype="&xsd;date">2012-06-14</terms:modified>
        <terms:title xml:lang="en">DCMI Metadata Terms - other</terms:title>
        <terms:publisher rdf:resource="http://purl.org/dc/aboutdcmi#DCMI"/>
    </rdf:Description>
    <rdf:Description rdf:about="&terms;UDC">
        <rdfs:label xml:lang="en">UDC</rdfs:label>
        <terms:issued rdf:datatype="&xsd;date">2000-07-11</terms:issued>
        <terms:modified rdf:datatype="&xsd;date">2008-01-14</terms:modified>
        <rdfs:comment xml:lang="en">The set of conceptual resources specified by the Universal Decimal Classification.</rdfs:comment>
        <terms:hasVersion rdf:resource="http://dublincore.org/usage/terms/history/#UDC-003"/>
        <rdfs:isDefinedBy rdf:resource="http://purl.org/dc/terms/"/>
        <rdfs:seeAlso rdf:resource="http://www.udcc.org/"/>
    </rdf:Description>
    <rdf:Description rdf:about="&terms;NLM">
        <rdfs:label xml:lang="en">NLM</rdfs:label>
        <terms:issued rdf:datatype="&xsd;date">2005-06-13</terms:issued>
        <terms:modified rdf:datatype="&xsd;date">2008-01-14</terms:modified>
        <rdfs:comment xml:lang="en">The set of conceptual resources specified by the National Library of Medicine Classification.</rdfs:comment>
        <terms:hasVersion rdf:resource="http://dublincore.org/usage/terms/history/#NLM-002"/>
        <rdfs:isDefinedBy rdf:resource="http://purl.org/dc/terms/"/>
        <rdfs:seeAlso rdf:resource="http://wwwcf.nlm.nih.gov/class/"/>
    </rdf:Description>
    <rdf:Description rdf:about="&terms;MESH">
        <rdfs:label xml:lang="en">MeSH</rdfs:label>
        <terms:issued rdf:datatype="&xsd;date">2000-07-11</terms:issued>
        <terms:modified rdf:datatype="&xsd;date">2008-01-14</terms:modified>
        <rdfs:comment xml:lang="en">The set of labeled concepts specified by the Medical Subject Headings.</rdfs:comment>
        <terms:hasVersion rdf:resource="http://dublincore.org/usage/terms/history/#MESH-003"/>
        <rdfs:isDefinedBy rdf:resource="http://purl.org/dc/terms/"/>
        <rdfs:seeAlso rdf:resource="http://www.nlm.nih.gov/mesh/meshhome.html"/>
    </rdf:Description>
    <rdf:Description rdf:about="http://www.w3.org/2003/01/geo/wgs84_pos#">
        <rdfs:label>geo</rdfs:label>
        <dc:description>A vocabulary for representing latitude, longitude and 
 altitude information in the WGS84 geodetic reference datum. 
 Version $Id: wgs84_pos.rdf,v 1.22 2009/04/20 15:00:30 timbl Exp $. See http://www.w3.org/2003/01/geo/ for more details.</dc:description>
        <rdfs:comment>
Recent changes to this namespace:
$Log: wgs84_pos.rdf,v $
Revision 1.22  2009/04/20 15:00:30  timbl
Remove the time bits which have been deal with elsewhere eg in iCal.

Revision 1.21  2009/04/20 12:52:47  timbl
try again

Revision 1.20  2009/04/20 12:42:11  timbl
Add Event (edited ages ago and never checked in), and location (following discussion http://chatlogs.planetrdf.com/swig/2009-04-20#T12-36-09)

Revision 1.19  2009/04/20 12:36:31  timbl
Add Event (edited ages ago and never checked in), and location (following discussion http://chatlogs.planetrdf.com/swig/2009-04-20#T12-36-09)

Revision 1.18  2006/02/01 22:01:04  danbri
Clarified that lat and long are decimal degrees, and that alt is decimal metres about local reference ellipsoid

Revision 1.17  2004/02/06 17:38:12  danbri
Fixed a bad commit screwup

Revision 1.15  2003/04/19 11:24:08  danbri
Fixed the typo even more.

Revision 1.14  2003/04/19 11:16:56  danbri
fixed a typo

Revision 1.13  2003/02/19 22:27:27  connolly
relaxed domain constraints on lat/long/alt from Point to SpatialThing

Revision 1.12  2003/01/12 01:41:41  danbri
Trying local copy of XSLT doc.

Revision 1.11  2003/01/12 01:20:18  danbri
added a link to morten&#39;s xslt rdfs viewer.

Revision 1.10  2003/01/11 18:56:49  danbri
Removed datatype range from lat and long properties, since they would
have required each occurance of the property to mention the datatype.

Revision 1.9  2003/01/11 11:41:31  danbri
Another typo; repaired rdfs:Property to rdf:Property x4

Revision 1.8  2003/01/11 11:05:02  danbri
Added an rdfs:range for each lat/long/alt property,
http://www.w3.org/2001/XMLSchema#float

Revision 1.7  2003/01/10 20:25:16  danbri
Longer rdfs:comment for Point, trying to be Earth-centric and neutral about
coordinate system(s) at the same time. Feedback welcomed.

Revision 1.6  2003/01/10 20:18:30  danbri
Added CVS log comments into the RDF/XML as an rdfs:comment property of the
vocabulary. Note that this is not common practice (but seems both harmless
and potentially useful).


revision 1.5
date: 2003/01/10 20:14:31;  author: danbri;  state: Exp;  lines: +16 -5
Updated schema:
Added a dc:date, added url for more info. Changed the rdfs:label of the
namespace from gp to geo. Added a class Point, set as the rdfs:domain of
each property. Added XML comment on the lat_long property suggesting that
we might not need it (based on #rdfig commentary from implementors).

revision 1.4
date: 2003/01/10 20:01:07;  author: danbri;  state: Exp;  lines: +6 -5
Fixed typo; several rdfs:about attributes are now rdf:about. Thanks to MortenF in
#rdfig for catching this error.

revision 1.3
date: 2003/01/10 11:59:03;  author: danbri;  state: Exp;  lines: +4 -3
fixed buglet in vocab, added more wgs links

revision 1.2
date: 2003/01/10 11:01:11;  author: danbri;  state: Exp;  lines: +4 -4
Removed alt from the as-a-flat-string property, and switched from
space separated to comma separated.

revision 1.1
date: 2003/01/10 10:53:23;  author: danbri;  state: Exp;
basic geo vocab

</rdfs:comment>
        <dc:date>$Date: 2009/04/20 15:00:30 $</dc:date>
        <dc:title>WGS84 Geo Positioning: an RDF vocabulary</dc:title>
    </rdf:Description>
</rdf:RDF>



<!-- Generated by the OWL API (version 3.2.3.1824) http://owlapi.sourceforge.net -->

